@prefix dc: <http://purl.org/dc/elements/1.1/> .
@prefix dcterms: <http://purl.org/dc/terms/> .
@prefix default1: <https://nfdi.fiz-karlsruhe.de/ontology/> .
@prefix emmo: <http://emmo.info/emmo#> .
@prefix foaf: <http://xmlns.com/foaf/0.1/> .
@prefix modsci: <https://w3id.org/skgo/modsci#> .
@prefix mwo: <http://purls.helmholtz-metadaten.de/mwo/> .
@prefix nfdicore: <http://nfdi.fiz-karlsruhe.de/ontology/> .
@prefix ns1: <https://w3id.org/scholarlydata/ontology/conference-ontology.owl#> .
@prefix ns2: <http://purl.obolibrary.org/obo/> .
@prefix ns3: <http://www.ebi.ac.uk/swo/> .
@prefix ns4: <http://www.geneontology.org/formats/oboInOwl#> .
@prefix owl: <http://www.w3.org/2002/07/owl#> .
@prefix rdf: <http://www.w3.org/1999/02/22-rdf-syntax-ns#> .
@prefix rdfs: <http://www.w3.org/2000/01/rdf-schema#> .
@prefix schema: <https://schema.org/> .
@prefix skos: <http://www.w3.org/2004/02/skos/core#> .
@prefix void: <http://rdfs.org/ns/void#> .
@prefix xsd: <http://www.w3.org/2001/XMLSchema#> .

<http://demo.fiz-karlsruhe.de/matwerk/E1004237> a nfdicore:DataPortal ;
    rdfs:label "Github" ;
    mwo:description "GitHub, Inc., is an Internet hosting service for software development and version control using Git. It provides the distributed version control of Git plus access control, bug tracking, software feature requests, task management, continuous integration, and wikis for every project." ;
    mwo:hasWebsite <http://demo.fiz-karlsruhe.de/matwerk/E335154> .

<http://demo.fiz-karlsruhe.de/matwerk/E1005654> a nfdicore:DataPortal ;
    rdfs:label "Zenodo" ;
    mwo:description "Zenodo is a general-purpose open repository developed under the European OpenAIRE program and operated by CERN. It allows researchers to deposit research papers, data sets, research software, reports, and any other research related digital artefacts." ;
    mwo:hasWebsite <http://demo.fiz-karlsruhe.de/matwerk/E335972> ;
    owl:sameAs <http://www.wikidata.org/entity/Q22661177> .

<http://demo.fiz-karlsruhe.de/matwerk/E1007072> a nfdicore:DataPortal ;
    rdfs:label "Dryad" ;
    mwo:description "Dryad is an international open-access repository of research data, especially data underlying scientific and medical publications. Dryad is a curated general-purpose repository that makes data discoverable, freely reusable, and citable." ;
    mwo:hasWebsite <http://demo.fiz-karlsruhe.de/matwerk/E336791> ;
    owl:sameAs <http://www.wikidata.org/entity/Q5309616> .

<http://demo.fiz-karlsruhe.de/matwerk/E1008491> a nfdicore:DataPortal ;
    rdfs:label "OSF" ;
    mwo:description "OSF is a free, open platform to support research data and enable collaboration." ;
    mwo:hasContactPoint <http://demo.fiz-karlsruhe.de/matwerk/E715611> ;
    mwo:hasRepository <http://demo.fiz-karlsruhe.de/matwerk/E387761> ;
    mwo:hasWebsite <http://demo.fiz-karlsruhe.de/matwerk/E337611> ;
    owl:sameAs <http://www.wikidata.org/entity/Q18691678> .

<http://demo.fiz-karlsruhe.de/matwerk/E1009911> a nfdicore:DataPortal ;
    rdfs:label "figshare" ;
    mwo:description "figshare is a repository where users can make all of their research outputs available in a citable, shareable and discoverable manner" ;
    mwo:hasContactPoint <http://demo.fiz-karlsruhe.de/matwerk/E716807> ;
    mwo:hasWebsite <http://demo.fiz-karlsruhe.de/matwerk/E338432> .

<http://demo.fiz-karlsruhe.de/matwerk/E1011332> a nfdicore:DataPortal ;
    rdfs:label "Zentrales Gitlab der Christian-Albrechts-Universität zu Kiel" ;
    mwo:hasWebsite <http://demo.fiz-karlsruhe.de/matwerk/E339254> .

<http://demo.fiz-karlsruhe.de/matwerk/E1012754> a nfdicore:DataPortal ;
    rdfs:label "opendata@uni-kiel" ;
    mwo:hasWebsite <http://demo.fiz-karlsruhe.de/matwerk/E340077> ;
    rdfs:comment "Currently in pilot stage, expected to start in Q3/2022" .

<http://demo.fiz-karlsruhe.de/matwerk/E1014177> a nfdicore:DataPortal ;
    rdfs:label "Interatomic potentials repository (NIST)" ;
    mwo:description "This repository provides a source for interatomic potentials (force fields), related files, and evaluation tools to help researchers obtain interatomic models and judge their quality and applicability. " ;
    mwo:hasContactPoint <http://demo.fiz-karlsruhe.de/matwerk/E718004> ;
    mwo:hasWebsite <http://demo.fiz-karlsruhe.de/matwerk/E340901> ;
    schema:citation <http://demo.fiz-karlsruhe.de/matwerk/E969137> .

<http://demo.fiz-karlsruhe.de/matwerk/E1015601> a nfdicore:DataPortal ;
    rdfs:label "OpenKIM" ;
    mwo:description "OpenKIM is a curated repository of interatomic potentials and analytics for making classical molecular simulations of materials reliable, reproducible, and accessible. Content on OpenKIM is open source and freely available." ;
    mwo:hasFormat <http://demo.fiz-karlsruhe.de/matwerk/E1220142> ;
    mwo:hasWebsite <http://demo.fiz-karlsruhe.de/matwerk/E341726> ;
    schema:citation <http://demo.fiz-karlsruhe.de/matwerk/E970529> .

<http://demo.fiz-karlsruhe.de/matwerk/E1017026> a nfdicore:DataPortal ;
    rdfs:label "Atomistica" ;
    mwo:description "Atomistica is a library of interatomic potentials. It is designed to be plugged into different simulation environments." ;
    mwo:hasContactPoint <http://demo.fiz-karlsruhe.de/matwerk/E20111> ;
    mwo:hasContributor <http://demo.fiz-karlsruhe.de/matwerk/E6152> ;
    mwo:hasRelatedResource <http://demo.fiz-karlsruhe.de/matwerk/E649092>,
        <http://demo.fiz-karlsruhe.de/matwerk/E650231> ;
    mwo:hasRepository <http://demo.fiz-karlsruhe.de/matwerk/E388641> ;
    mwo:hasVersion "v1.0.4" ;
    mwo:hasWebsite <http://demo.fiz-karlsruhe.de/matwerk/E342552> ;
    ns3:has_license <http://demo.fiz-karlsruhe.de/matwerk/E804279> .

<http://demo.fiz-karlsruhe.de/matwerk/E1018452> a nfdicore:DataPortal ;
    rdfs:label "CCP-NC database of calculated NMR data" ;
    mwo:conformsToSpecification <http://demo.fiz-karlsruhe.de/matwerk/E1125251> ;
    mwo:description "This is the prototype interface for the CCP-NC database of calculated NMR data." ;
    mwo:hasFormat <http://demo.fiz-karlsruhe.de/matwerk/E1221704>,
        <http://demo.fiz-karlsruhe.de/matwerk/E1223267> ;
    mwo:hasWebsite <http://demo.fiz-karlsruhe.de/matwerk/E343379> .

<http://demo.fiz-karlsruhe.de/matwerk/E1019879> a nfdicore:DataPortal ;
    rdfs:label "CASTEP Pseudopotentials" ;
    mwo:description "CASTEP pseudopotential strings and data for the elements" ;
    mwo:hasWebsite <http://demo.fiz-karlsruhe.de/matwerk/E344207> .

<http://demo.fiz-karlsruhe.de/matwerk/E1021307> a nfdicore:DataPortal ;
    rdfs:label "PubChem" ;
    mwo:description "PubChem is the world's largest collection of freely accessible chemical information. Search chemicals by name, molecular formula, structure, and other identifiers. Find chemical and physical properties, biological activities, safety and toxicity information, patents, literature citations and more." ;
    mwo:hasContactPoint <http://demo.fiz-karlsruhe.de/matwerk/E720401> ;
    mwo:hasFormat <http://demo.fiz-karlsruhe.de/matwerk/E1221704>,
        <http://demo.fiz-karlsruhe.de/matwerk/E1224831>,
        <http://demo.fiz-karlsruhe.de/matwerk/E1226396> ;
    mwo:hasWebsite <http://demo.fiz-karlsruhe.de/matwerk/E345036> ;
    owl:sameAs <http://www.wikidata.org/entity/Q278487> ;
    schema:citation <http://demo.fiz-karlsruhe.de/matwerk/E971922> .

<http://demo.fiz-karlsruhe.de/matwerk/E1022736> a nfdicore:DataPortal ;
    rdfs:label "Bilbao Crystallographic Server" ;
    mwo:description "Bilbao Crystallographic Server is an open access website offering online crystallographic database and programs aimed at analyzing, calculating and visualizing problems of structural and mathematical crystallography, solid state physics and structural chemistry." ;
    mwo:hasContactPoint <http://demo.fiz-karlsruhe.de/matwerk/E721601> ;
    mwo:hasContributor <http://demo.fiz-karlsruhe.de/matwerk/E6254> ;
    mwo:hasWebsite <http://demo.fiz-karlsruhe.de/matwerk/E345866> ;
    schema:citation <http://demo.fiz-karlsruhe.de/matwerk/E973316> .

<http://demo.fiz-karlsruhe.de/matwerk/E1024166> a nfdicore:DataPortal ;
    rdfs:label "Crystallography Open Database (COD)" ;
    mwo:conformsToSpecification <http://demo.fiz-karlsruhe.de/matwerk/E1125251> ;
    mwo:description "Open-access collection of crystal structures of organic, inorganic, metal-organic compounds and minerals, excluding biopolymers." ;
    mwo:hasContactPoint <http://demo.fiz-karlsruhe.de/matwerk/E722802> ;
    mwo:hasContributor <http://demo.fiz-karlsruhe.de/matwerk/E6357> ;
    mwo:hasFormat <http://demo.fiz-karlsruhe.de/matwerk/E1221704>,
        <http://demo.fiz-karlsruhe.de/matwerk/E1227962> ;
    mwo:hasWebsite <http://demo.fiz-karlsruhe.de/matwerk/E346697> ;
    ns3:has_license <http://demo.fiz-karlsruhe.de/matwerk/E805547> ;
    schema:citation <http://demo.fiz-karlsruhe.de/matwerk/E974711> .

<http://demo.fiz-karlsruhe.de/matwerk/E1025597> a nfdicore:DataPortal ;
    rdfs:label "MaterialsProject" ;
    mwo:conformsToSpecification <http://demo.fiz-karlsruhe.de/matwerk/E1125251> ;
    mwo:description "By computing properties of all known materials, the Materials Project aims to remove guesswork from materials design in a variety of applications. Experimental research can be targeted to the most promising compounds from computational data sets. Researchers will be able to data-mine scientific trends in materials properties. By providing materials researchers with the information they need to design better, the Materials Project aims to accelerate innovation in materials research." ;
    mwo:hasRelatedResource <http://demo.fiz-karlsruhe.de/matwerk/E651371>,
        <http://demo.fiz-karlsruhe.de/matwerk/E652512>,
        <http://demo.fiz-karlsruhe.de/matwerk/E653654>,
        <http://demo.fiz-karlsruhe.de/matwerk/E654797>,
        <http://demo.fiz-karlsruhe.de/matwerk/E655941> ;
    mwo:hasRepository <http://demo.fiz-karlsruhe.de/matwerk/E389522> ;
    mwo:hasWebsite <http://demo.fiz-karlsruhe.de/matwerk/E347529> ;
    ns3:has_license <http://demo.fiz-karlsruhe.de/matwerk/E811902> ;
    schema:citation <http://demo.fiz-karlsruhe.de/matwerk/E976107> .

<http://demo.fiz-karlsruhe.de/matwerk/E1028462> a nfdicore:DataPortal ;
    rdfs:label "Novel Materials Discovery (NOMAD)" ;
    mwo:conformsToSpecification <http://demo.fiz-karlsruhe.de/matwerk/E1125251> ;
    mwo:description "The Novel Materials Discovery (NOMAD) Laboratory maintains the largest worldwide repository for input and output files of all important computational materials science computer programs." ;
    mwo:hasContactPoint <http://demo.fiz-karlsruhe.de/matwerk/E725207> ;
    mwo:hasContributor <http://demo.fiz-karlsruhe.de/matwerk/E6566> ;
    mwo:hasRepository <http://demo.fiz-karlsruhe.de/matwerk/E391287> ;
    mwo:hasWebsite <http://demo.fiz-karlsruhe.de/matwerk/E349196> ;
    schema:citation <http://demo.fiz-karlsruhe.de/matwerk/E978902> .

<http://demo.fiz-karlsruhe.de/matwerk/E1029896> a nfdicore:DataPortal ;
    rdfs:label "MatPortal" ;
    mwo:description "Ontology repository for materials science." ;
    mwo:hasContributor <http://demo.fiz-karlsruhe.de/matwerk/E6672> ;
    mwo:hasWebsite <http://demo.fiz-karlsruhe.de/matwerk/E350031> .

<http://demo.fiz-karlsruhe.de/matwerk/E1031331> a nfdicore:DataPortal ;
    rdfs:label "Atomistictools" ;
    mwo:description "This website provides an interactive interface for the assessment of interatomic potentials presented in OpenKIM, NIST IPR and elsewhere with respect to DFT reference data. The calculations were carried out using the pyiron workflow management tool." ;
    mwo:hasContactPoint <http://demo.fiz-karlsruhe.de/matwerk/E726411> ;
    mwo:hasContributor <http://demo.fiz-karlsruhe.de/matwerk/E1037> ;
    mwo:hasRelatedResource <http://demo.fiz-karlsruhe.de/matwerk/E457491> ;
    mwo:hasWebsite <http://demo.fiz-karlsruhe.de/matwerk/E350867> .

<http://demo.fiz-karlsruhe.de/matwerk/E10317> a nfdicore:Person ;
    rdfs:label "PD Dr. habil.  Thomas Hammerschmidt" ;
    mwo:emailAddress "thomas.hammerschmidt@rub.de"^^xsd:string ;
    mwo:hasAffiliation <http://demo.fiz-karlsruhe.de/matwerk/E1037> ;
    mwo:hasExpertiseIn <http://demo.fiz-karlsruhe.de/matwerk/E39782>,
        <http://demo.fiz-karlsruhe.de/matwerk/E40061>,
        <http://demo.fiz-karlsruhe.de/matwerk/E40341>,
        <http://demo.fiz-karlsruhe.de/matwerk/E63482>,
        <http://demo.fiz-karlsruhe.de/matwerk/E63836>,
        <http://demo.fiz-karlsruhe.de/matwerk/E64191>,
        <http://demo.fiz-karlsruhe.de/matwerk/E67431> ;
    mwo:hasORCID <https://orcid.org/0000-0002-2270-4469> ;
    owl:sameAs <http://www.wikidata.org/entity/Q58818678> ;
    foaf:firstName "Thomas"^^xsd:string ;
    foaf:surname "Hammerschmidt"^^xsd:string ;
    foaf:title "PD Dr. habil. "^^xsd:string .

<http://demo.fiz-karlsruhe.de/matwerk/E1032767> a nfdicore:DataPortal ;
    rdfs:label "Aflow" ;
    mwo:conformsToSpecification <http://demo.fiz-karlsruhe.de/matwerk/E1125251> ;
    mwo:description "Automatic FLOW (AFLOW) database for computational materials science. Globally available database of 3,528,653 material compounds with over 733,959,824 calculated properties, and growing." ;
    mwo:hasWebsite <http://demo.fiz-karlsruhe.de/matwerk/E351704> .

<http://demo.fiz-karlsruhe.de/matwerk/E1034204> a nfdicore:DataPortal ;
    rdfs:label "Jarvis" ;
    mwo:description "JARVIS (Joint Automated Repository for Various Integrated Simulations) is a repository designed to automate materials discovery and optimization using classical force-field, density functional theory, machine learning calculations and experiments." ;
    mwo:hasWebsite <http://demo.fiz-karlsruhe.de/matwerk/E352542> ;
    schema:citation <http://demo.fiz-karlsruhe.de/matwerk/E980301> .

<http://demo.fiz-karlsruhe.de/matwerk/E1035642> a nfdicore:DataPortal ;
    rdfs:label "Materials Platform for Data Science" ;
    mwo:conformsToSpecification <http://demo.fiz-karlsruhe.de/matwerk/E1125251> ;
    mwo:description "Online materials database (known as PAULING FILE project) with nearly 2 million entries: physical properties, crystal structures, phase diagrams, available via API, ready for modern data-intensive applications. The source of these entries are about 300,000 peer-reviewed publications in materials science, processed during the last 16 years by an international team of PhD editors. The results are presented online with a quick search interface. The basic access is provided for free." ;
    mwo:hasWebsite <http://demo.fiz-karlsruhe.de/matwerk/E353381> .

<http://demo.fiz-karlsruhe.de/matwerk/E1037081> a nfdicore:DataPortal ;
    rdfs:label "The Open Quantum Materials Database" ;
    mwo:conformsToSpecification <http://demo.fiz-karlsruhe.de/matwerk/E1125251> ;
    mwo:description "The OQMD is a database of DFT calculated thermodynamic and structural properties of 1,022,603 materials, created in Chris Wolverton's group at Northwestern University." ;
    mwo:hasContactPoint <http://demo.fiz-karlsruhe.de/matwerk/E728822> ;
    mwo:hasRelatedResource <http://demo.fiz-karlsruhe.de/matwerk/E546491> ;
    mwo:hasVersion "CC-BY 4.0" ;
    mwo:hasWebsite <http://demo.fiz-karlsruhe.de/matwerk/E355062> ;
    schema:citation <http://demo.fiz-karlsruhe.de/matwerk/E981701> .

<http://demo.fiz-karlsruhe.de/matwerk/E1038521> a nfdicore:DataPortal ;
    rdfs:label "Citrination" ;
    mwo:description "Citrination is the premier open database and analytics platform for the world's material and chemical information. Developed by Citrine Informatics." ;
    mwo:hasWebsite <http://demo.fiz-karlsruhe.de/matwerk/E355904> ;
    ns3:has_license <http://demo.fiz-karlsruhe.de/matwerk/E808086> .

<http://demo.fiz-karlsruhe.de/matwerk/E1039962> a nfdicore:DataPortal ;
    rdfs:label "MatDB" ;
    mwo:description "MatDB is a database application for experimentally measured engineering materials data. It supports open, registered, and restricted access. It presently hosts more than 20.000 unique data sets coming mainly from European and Member State research programmes. It supports web interfaces for entering, browsing, and retrieving data. MatDB is also enabled for innovative services, including data citation and interoperability standards. The data citation service relies on DataCite DOIs. " ;
    mwo:hasWebsite <http://demo.fiz-karlsruhe.de/matwerk/E356747> .

<http://demo.fiz-karlsruhe.de/matwerk/E1041404> a nfdicore:DataPortal ;
    rdfs:label "MatDat" ;
    mwo:description "Over 1000 detailed, fully referenced and verified datasets for steels, aluminium and titanium alloys, cast irons/steels, weld metals. Materials can be searched according to a number of different criteria. Initial search results are presented in the form of a table from which they can be selected for presentation in form of detailed report or for comparison overview (up to 5 materials). In addition to material information and values of properties/parameters, images of microstructure, specimens and those of stress-strain, stress- and strain-life curves (if available) can be reviewed as well." ;
    mwo:hasContactPoint <http://demo.fiz-karlsruhe.de/matwerk/E730029> ;
    mwo:hasWebsite <http://demo.fiz-karlsruhe.de/matwerk/E357591> .

<http://demo.fiz-karlsruhe.de/matwerk/E1042847> a nfdicore:DataPortal ;
    rdfs:label "Materials Data Repository" ;
    mwo:description "MDR is a data repository to collect and store papers, presentation materials, and related materials data to accumulate and release them in a form suitable for the promotion of materials research and materials informatics. Users can search the documents and the data from information (metadata) such as sample, instrument, method, and from the full text of the deposited data, to browse and download them freely. " ;
    mwo:hasContributor <http://demo.fiz-karlsruhe.de/matwerk/E6779> ;
    mwo:hasWebsite <http://demo.fiz-karlsruhe.de/matwerk/E358436> .

<http://demo.fiz-karlsruhe.de/matwerk/E1044291> a nfdicore:DataPortal ;
    rdfs:label "MatNavi: NIMS Materials Database" ;
    mwo:description "The NIMS Materials Database (MatNavi) aims to contribute to the development of new materials and the selection of materials. MatNavi includes Polymer DB (chemical structures, polymerization, processing, physical properties, NMR spectra, etc.), Inorganic MaterialDB (crystal structures, phase diagrams, physical properties, etc.), Metallic Material DB (density, elastic constants, creep characteristics, etc.) and Computational Electronic Structure DB (band structures obtained by first-principles calculations, etc). It also offers applications such as the Composite Design & Property Prediction System. If you register, you can search and browse various databases for free." ;
    mwo:hasContributor <http://demo.fiz-karlsruhe.de/matwerk/E6779> ;
    mwo:hasWebsite <http://demo.fiz-karlsruhe.de/matwerk/E359282> .

<http://demo.fiz-karlsruhe.de/matwerk/E1045736> a nfdicore:DataPortal ;
    rdfs:label "Polymer Database (PoLyInfo)" ;
    mwo:description "Polymer Database \"PoLyInfo\" systematically provides various data required for polymeric material design. The main data source is academic literature on polymers. Information on polymers including properties, chemical structures, IUPAC names, processing methods of measured samples, measurement conditions, used monomers and polymerization methods are stored in a object database. About 100 types of properties including thermal, electrical and mechanical properties are covered. Homopolymers, copolymers, furthermore polymer blends, composites and compounds that consist of homopolymers and copolymers are open to the public." ;
    mwo:hasContributor <http://demo.fiz-karlsruhe.de/matwerk/E6779> ;
    mwo:hasWebsite <http://demo.fiz-karlsruhe.de/matwerk/E360129> .

<http://demo.fiz-karlsruhe.de/matwerk/E1047182> a nfdicore:DataPortal ;
    rdfs:label "Inorganic Material Database (AtomWork)" ;
    mwo:description "The Inorganic Material Database aims to cover all basic crystal structure, x-ray diffraction, property and phase diagram data of inorganic and metallic materials from main literature sources." ;
    mwo:hasContributor <http://demo.fiz-karlsruhe.de/matwerk/E6779> ;
    mwo:hasWebsite <http://demo.fiz-karlsruhe.de/matwerk/E360977> ;
    schema:citation <http://demo.fiz-karlsruhe.de/matwerk/E983102> .

<http://demo.fiz-karlsruhe.de/matwerk/E1048629> a nfdicore:DataPortal ;
    rdfs:label "Computational Electronic Structure Database (CompES-X)" ;
    mwo:description "CompES-X is a database of electronic structures predicted by the first-principles calculations for mono-element and multi-element crystalline inorganic compounds that are based on the experimental data of crystal structures (CIF file) of a broad range of materials collected in Inorganic Materials Database (AtomWork). The calculations are carried out mainly by using the first-principles plane wave pseudopotential method as implemented in VASP code. The entry of calculated electronic structure data is in one-to-one association with that of experimental data of crystal structures of inorganic compounds contained in AtomWork." ;
    mwo:hasContributor <http://demo.fiz-karlsruhe.de/matwerk/E6779> ;
    mwo:hasRelatedResource <http://demo.fiz-karlsruhe.de/matwerk/E661676>,
        <http://demo.fiz-karlsruhe.de/matwerk/E662826> ;
    mwo:hasWebsite <http://demo.fiz-karlsruhe.de/matwerk/E361826> .

<http://demo.fiz-karlsruhe.de/matwerk/E1050077> a nfdicore:DataPortal ;
    rdfs:label "Diffusion Database (Kakusan)" ;
    mwo:description "The Diffusion Database aims to cover all the basic diffusion data of metallic and inorganic materials mainly from the literature sources. The database consists of \"diffusion data\" and \"reference data\". Currently the system primarily contains information of pure metals, alloys, semiconductors, ceramics and intermetallics." ;
    mwo:hasContributor <http://demo.fiz-karlsruhe.de/matwerk/E6779> ;
    mwo:hasWebsite <http://demo.fiz-karlsruhe.de/matwerk/E362676> .

<http://demo.fiz-karlsruhe.de/matwerk/E1051526> a nfdicore:DataPortal ;
    rdfs:label "Thermophysical Property Database" ;
    mwo:description "This database contains data on density, surface tension and viscosity coefficient of metals, alloys and ceramics obtained by floating experiments using an electrostatic levitation furnace." ;
    mwo:hasContributor <http://demo.fiz-karlsruhe.de/matwerk/E6779> ;
    mwo:hasWebsite <http://demo.fiz-karlsruhe.de/matwerk/E363527> .

<http://demo.fiz-karlsruhe.de/matwerk/E1052976> a nfdicore:DataPortal ;
    rdfs:label "Metallic Material Database (Kinzoku)" ;
    mwo:description "The Metallic Materials Database (Kinzoku) includes the density, elastic modulus, poisson ratio, hardness, toughness, tensile, creep, creep rupture properties, and various fatigue properties of structural metallic materials. It can be searched by JIS standard number, ASTM standard number, material name, material form, etc." ;
    mwo:hasContributor <http://demo.fiz-karlsruhe.de/matwerk/E6779> ;
    mwo:hasWebsite <http://demo.fiz-karlsruhe.de/matwerk/E364379> .

<http://demo.fiz-karlsruhe.de/matwerk/E1054427> a nfdicore:DataPortal ;
    rdfs:label "CCT Diagram Database (CCTD)" ;
    mwo:description "The welding database system to predict hardness and microstructural constituents in the heat affected zone and to determine optimum welding conditions has been developed by using an estimated thermal cycle and the database of CCT diagram for welding." ;
    mwo:hasContributor <http://demo.fiz-karlsruhe.de/matwerk/E6779> ;
    mwo:hasWebsite <http://demo.fiz-karlsruhe.de/matwerk/E365232> .

<http://demo.fiz-karlsruhe.de/matwerk/E1055879> a nfdicore:DataPortal ;
    rdfs:label "Cambridge Structural Database (CSD)" ;
    mwo:description """The comprehensive repository of validated and curated small-molecule organic and metal-organic crystal structures. \r
""" ;
    mwo:hasContributor <http://demo.fiz-karlsruhe.de/matwerk/E6887> ;
    mwo:hasWebsite <http://demo.fiz-karlsruhe.de/matwerk/E366086> ;
    ns3:has_license <http://demo.fiz-karlsruhe.de/matwerk/E808086> .

<http://demo.fiz-karlsruhe.de/matwerk/E1057332> a nfdicore:DataPortal ;
    rdfs:label "Inorganic Crystal Structure Database (ICSD)" ;
    mwo:description "ICSD is an information service in crystallography and comprises the world’s largest database for fully identified inorganic crystal structures." ;
    mwo:hasContributor <http://demo.fiz-karlsruhe.de/matwerk/E6996> ;
    mwo:hasWebsite <http://demo.fiz-karlsruhe.de/matwerk/E366941> ;
    ns3:has_license <http://demo.fiz-karlsruhe.de/matwerk/E808086> .

<http://demo.fiz-karlsruhe.de/matwerk/E1058786> a nfdicore:DataPortal ;
    rdfs:label "ioChem-BD" ;
    mwo:hasWebsite <http://demo.fiz-karlsruhe.de/matwerk/E367797> .

<http://demo.fiz-karlsruhe.de/matwerk/E1060241> a nfdicore:DataPortal ;
    rdfs:label "Computational Materials Repository (CMR)" ;
    mwo:description "Each CMR project consists of an ASE-database and a project page describing the data and showing examples of how to work with the data using Python and ASE." ;
    mwo:hasRelatedResource <http://demo.fiz-karlsruhe.de/matwerk/E641147> ;
    mwo:hasWebsite <http://demo.fiz-karlsruhe.de/matwerk/E368654> ;
    ns3:has_license <http://demo.fiz-karlsruhe.de/matwerk/E809357> .

<http://demo.fiz-karlsruhe.de/matwerk/E1061697> a nfdicore:DataPortal ;
    rdfs:label "Electronic Structure Project (ESP)" ;
    mwo:description """The electronic structure project (ESP) is a collection\r
of some 60,000 electronic structure calculations. A\r
full-potential linear muffin-tin orbital (FP-LMTO)\r
implementation of density functional theory (DFT) within\r
the local density approximation (LDA) was used to solve\r
the electronic structures.""" ;
    mwo:hasWebsite <http://demo.fiz-karlsruhe.de/matwerk/E369512> ;
    schema:citation <http://demo.fiz-karlsruhe.de/matwerk/E984504> .

<http://demo.fiz-karlsruhe.de/matwerk/E1063154> a nfdicore:DataPortal ;
    rdfs:label "HybriD³ materials database" ;
    mwo:description "The HybriD³ materials database provides a comprehensive collection of experimental and computational materials data for crystalline organic-inorganic compounds, predominantly based on the perovskite paradigm." ;
    mwo:hasContactPoint <http://demo.fiz-karlsruhe.de/matwerk/E731237> ;
    mwo:hasRelatedResource <http://demo.fiz-karlsruhe.de/matwerk/E592329> ;
    mwo:hasWebsite <http://demo.fiz-karlsruhe.de/matwerk/E370371> ;
    ns3:has_license <http://demo.fiz-karlsruhe.de/matwerk/E810629> .

<http://demo.fiz-karlsruhe.de/matwerk/E1064612> a nfdicore:DataPortal ;
    rdfs:label "Khazana" ;
    mwo:description "A platform to store structure and property data created by atomistic simulations, and toold to design materials by learning from the data" ;
    mwo:hasWebsite <http://demo.fiz-karlsruhe.de/matwerk/E371231> .

<http://demo.fiz-karlsruhe.de/matwerk/E1066071> a nfdicore:DataPortal ;
    rdfs:label "Polymer Genome" ;
    mwo:description "An informatics platform for polymer property prediction and design using machine learning" ;
    mwo:hasWebsite <http://demo.fiz-karlsruhe.de/matwerk/E372092> ;
    schema:citation <http://demo.fiz-karlsruhe.de/matwerk/E985907> .

<http://demo.fiz-karlsruhe.de/matwerk/E1067531> a nfdicore:DataPortal ;
    rdfs:label "The Materials Data Facility (MDF)" ;
    mwo:description "A simple way to publish, discover, and access materials datasets" ;
    mwo:hasContactPoint <http://demo.fiz-karlsruhe.de/matwerk/E732446> ;
    mwo:hasWebsite <http://demo.fiz-karlsruhe.de/matwerk/E372954> ;
    schema:citation <http://demo.fiz-karlsruhe.de/matwerk/E987311> .

<http://demo.fiz-karlsruhe.de/matwerk/E1068992> a nfdicore:DataPortal ;
    rdfs:label "Material Properties Open Database (MPOD)" ;
    mwo:description """The Material Properties Open Database (MPOD) is a web-based, open access repository of quantitative information about the physical properties of crystalline materials.\r
\r
MPOD is oriented to design engineers, scientists, science teachers and students. Properties are generally treated as tensor magnitudes. In MPOD the compact matrix notation is applied. To bring an intuitive view of tensor properties, so-called longitudinal properties surfaces are displayed.""" ;
    mwo:hasWebsite <http://demo.fiz-karlsruhe.de/matwerk/E373817> ;
    schema:citation <http://demo.fiz-karlsruhe.de/matwerk/E988716> .

<http://demo.fiz-karlsruhe.de/matwerk/E1070454> a nfdicore:DataPortal ;
    rdfs:label "nanoHUB" ;
    mwo:description "nanoHUB.org is the premier place for computational nanotechnology research, education, and collaboration. Our site hosts a rapidly growing collection of Simulation Programs for nanoscale phenomena that run in the cloud and are accessible through a web browser." ;
    mwo:hasWebsite <http://demo.fiz-karlsruhe.de/matwerk/E374681> .

<http://demo.fiz-karlsruhe.de/matwerk/E1071917> a nfdicore:DataPortal ;
    rdfs:label "NRELMatDB" ;
    mwo:description """NRELMatDB is a computational materials database with the specific focus on materials for renewable energy applications including, but not limited to, photovoltaic materials, materials for photo-electrochemical water splitting, thermoelectrics, etc. The main goal of NRELMatDB is to enable and facilitate the access and exchange of computational data between different research groups following the guidelines outlined in the Presidential Materials Genome Initiative (http://www.mgi.gov).\r
\r
""" ;
    mwo:hasWebsite <http://demo.fiz-karlsruhe.de/matwerk/E375546> .

<http://demo.fiz-karlsruhe.de/matwerk/E10731> a nfdicore:Person ;
    rdfs:label "Prof. Dr.-Ing. Gerson Meschut" ;
    mwo:emailAddress "meschut@lwf.upb.de"^^xsd:string ;
    mwo:hasAffiliation <http://demo.fiz-karlsruhe.de/matwerk/E1056> ;
    mwo:hasExpertiseIn <http://demo.fiz-karlsruhe.de/matwerk/E42329>,
        <http://demo.fiz-karlsruhe.de/matwerk/E49206> ;
    mwo:hasORCID <https://orcid.org/0000-0002-2763-1246> ;
    owl:sameAs <http://www.wikidata.org/entity/Q111358951> ;
    foaf:firstName "Gerson"^^xsd:string ;
    foaf:surname "Meschut"^^xsd:string ;
    foaf:title "Prof. Dr.-Ing."^^xsd:string .

<http://demo.fiz-karlsruhe.de/matwerk/E1073381> a nfdicore:DataPortal ;
    rdfs:label "Organic Materials Database (OMDB)" ;
    mwo:description """The organic materials database is an open access electronic structure database for 3-dimensional organic crystals, developed and hosted at the Nordic Institute for Theoretical Physics – Nordita.\r
\r
It provides tools for search queries based on data-mining and machine learning techniques. The universal features provided on our web interface facilitate the design of novel functional organic materials with a wide-range of applications.""" ;
    mwo:hasWebsite <http://demo.fiz-karlsruhe.de/matwerk/E376412> .

<http://demo.fiz-karlsruhe.de/matwerk/E1074846> a nfdicore:DataPortal ;
    rdfs:label "Phonon database at Kyoto university" ;
    mwo:description "It’s getting to be a mainstream idea collecting a big set of ab-initio calculations and analyzing them by informatics approach. For scientific purpose, we plan to do it for phonon properties. As an attempt, we have run a set of ab-initio phonon calculations and left the raw data on this static web site. The aim of this web site is just leaving the data to distribute." ;
    mwo:hasContactPoint <http://demo.fiz-karlsruhe.de/matwerk/E20307> ;
    mwo:hasWebsite <http://demo.fiz-karlsruhe.de/matwerk/E377279> ;
    ns3:has_license <http://demo.fiz-karlsruhe.de/matwerk/E811902> .

<http://demo.fiz-karlsruhe.de/matwerk/E1076312> a nfdicore:DataPortal ;
    rdfs:label "Raman Open Database (ROD)" ;
    mwo:description "Open-access collection of Raman spectra used for the SOLSA H2020 project." ;
    mwo:hasContactPoint <http://demo.fiz-karlsruhe.de/matwerk/E722802> ;
    mwo:hasWebsite <http://demo.fiz-karlsruhe.de/matwerk/E378147> .

<http://demo.fiz-karlsruhe.de/matwerk/E1077779> a nfdicore:DataPortal ;
    rdfs:label "Topological Material Database" ;
    mwo:description "Using a recently developed formalism called topological quantum chemistry, we perform a high-throughput search of ‘high-quality’ materials (for which the atomic positions and structure have been measured very accurately) in the Inorganic Crystal Structure Database in order to identify new topological phases. We develop codes to compute all characters of all symmetries of 26,938 stoichiometric materials, and find 3,307 topological insulators, 4,078 topological semimetals and no fragile phases. For these 7,385 materials we provide the electronic band structure, including some electronic properties (bandgap and number of electrons), symmetry indicators, and other topological information. Our results show that more than 27 per cent of all materials in nature are topological. We provide an open-source code that checks the topology of any material and allows other researchers to reproduce our results." ;
    mwo:hasContactPoint <http://demo.fiz-karlsruhe.de/matwerk/E734867> ;
    mwo:hasRelatedResource <http://demo.fiz-karlsruhe.de/matwerk/E663977> ;
    mwo:hasWebsite <http://demo.fiz-karlsruhe.de/matwerk/E379016> ;
    schema:citation <http://demo.fiz-karlsruhe.de/matwerk/E990122> .

<http://demo.fiz-karlsruhe.de/matwerk/E1079247> a nfdicore:DataPortal ;
    rdfs:label "Carolina Materials Database" ;
    mwo:description "Welcome to Carolina Materials Database created in Jianjun Hu's and Ming Hu's groups at University of South Carolina. A freely, globally accessible database of 38,716 inorganic material compounds with over 80,000 calculated properties, and growing." ;
    mwo:hasWebsite <http://demo.fiz-karlsruhe.de/matwerk/E379886> .

<http://demo.fiz-karlsruhe.de/matwerk/E1080716> a nfdicore:DataPortal ;
    rdfs:label "CascadesDB" ;
    mwo:description "CascadesDB is a database of molecular dynamics simulations of collision cascades, developed by the International Atomic Energy Agency. The project was initiated by the 5th meeting of the IAEA's Code Centres Network in November 2017 to enhance the usage and long-term curation of collisional cascade simulations for the analysis and prediction of radiation damage in materials for fusion and fission applications." ;
    mwo:hasWebsite <http://demo.fiz-karlsruhe.de/matwerk/E380757> ;
    ns3:has_license <http://demo.fiz-karlsruhe.de/matwerk/E813176> .

<http://demo.fiz-karlsruhe.de/matwerk/E1082186> a nfdicore:DataPortal ;
    rdfs:label "Surface Reactions Database" ;
    mwo:description "The Surface Reactions database contains thousands of reaction energies and barriers from density functional theory (DFT) calculations on surface systems." ;
    mwo:hasWebsite <http://demo.fiz-karlsruhe.de/matwerk/E381629> .

<http://demo.fiz-karlsruhe.de/matwerk/E1083657> a nfdicore:DataPortal ;
    rdfs:label "Information Resources on Inorganic Chemistry (IRIC)" ;
    mwo:description "IRIC database (Information Resources on Inorganic Chemistry) contains brief information on information systems on inorganic chemistry and material science. All data are taken from publications." ;
    mwo:hasWebsite <http://demo.fiz-karlsruhe.de/matwerk/E382502> .

<http://demo.fiz-karlsruhe.de/matwerk/E1085129> a nfdicore:DataPortal ;
    rdfs:label "NFDI4Ing Data Collections Explorer" ;
    mwo:description "Information system to facilitate research of domain specific repositories and databases, as well as datasets published individually by research groups" ;
    mwo:hasRepository <http://demo.fiz-karlsruhe.de/matwerk/E392171> ;
    mwo:hasWebsite <http://demo.fiz-karlsruhe.de/matwerk/E383376> .

<http://demo.fiz-karlsruhe.de/matwerk/E1086602> a nfdicore:DataPortal ;
    rdfs:label "Materials Commons" ;
    mwo:description "A site for Materials Scientists to collaborate, store and publish research. The Materials Commons is supported by the U.S. Department of Energy, Office of Basic Energy Sciences, Division of Materials Sciences and Engineering." ;
    mwo:hasRepository <http://demo.fiz-karlsruhe.de/matwerk/E393056> ;
    mwo:hasWebsite <http://demo.fiz-karlsruhe.de/matwerk/E384251> .

<http://demo.fiz-karlsruhe.de/matwerk/E10871> a nfdicore:Person ;
    rdfs:label "Dr.-Ing. Mathias Bobbert" ;
    mwo:emailAddress "mathias.bobbert@lwf.upb.de"^^xsd:string ;
    mwo:hasAffiliation <http://demo.fiz-karlsruhe.de/matwerk/E1056> ;
    foaf:firstName "Mathias"^^xsd:string ;
    foaf:surname "Bobbert"^^xsd:string ;
    foaf:title "Dr.-Ing."^^xsd:string .

<http://demo.fiz-karlsruhe.de/matwerk/E1088076> a nfdicore:DataPortal ;
    rdfs:label "ThermoML" ;
    mwo:description "ThermoML is an XML-based IUPAC Standard for storage and exchange of thermophysical and thermochemical property data. " ;
    mwo:hasWebsite <http://demo.fiz-karlsruhe.de/matwerk/E385127> ;
    schema:citation <http://demo.fiz-karlsruhe.de/matwerk/E991529> .

<http://demo.fiz-karlsruhe.de/matwerk/E1089551> a nfdicore:DataPortal ;
    rdfs:label "GBRV pseudopotentials" ;
    mwo:description "This site hosts the GBRV pseudopotential library, a highly accurate and computationally inexpensive open-source pseudopotential library which has been designed and optimized for use in high-throughput DFT calculations and released under the gnu public license.  We provide potential files for direct use with the Quantum Espresso, Abinit, and JDFTx plane-wave pseudopotential codes, as well as input files for the Vanderbilt Ultrasoft pseudopotential generator. " ;
    mwo:hasWebsite <http://demo.fiz-karlsruhe.de/matwerk/E386004> ;
    ns3:has_license <http://demo.fiz-karlsruhe.de/matwerk/E814451> ;
    schema:citation <http://demo.fiz-karlsruhe.de/matwerk/E992937> .

<http://demo.fiz-karlsruhe.de/matwerk/E11012> a nfdicore:Person ;
    rdfs:label "Thilo Paul-Stüve" ;
    mwo:emailAddress "paul-stueve@rz.uni-kiel.de"^^xsd:string ;
    mwo:hasAffiliation <http://demo.fiz-karlsruhe.de/matwerk/E1067> ;
    foaf:firstName "Thilo"^^xsd:string ;
    foaf:surname "Paul-Stüve"^^xsd:string .

<http://demo.fiz-karlsruhe.de/matwerk/E1108817> a modsci:Instrument ;
    rdfs:label "Procon CT-alpha" ;
    nfdicore:location <http://demo.fiz-karlsruhe.de/matwerk/E80004> ;
    mwo:description "X-ray micro computed tomography (micro-CT)" ;
    mwo:hasContactPoint <http://demo.fiz-karlsruhe.de/matwerk/E9647> ;
    mwo:hasOwner <http://demo.fiz-karlsruhe.de/matwerk/E3212> ;
    mwo:hasWebsite <http://demo.fiz-karlsruhe.de/matwerk/E287147> ;
    mwo:instrumentModel "CT-alpha" ;
    mwo:usesTechnology <http://demo.fiz-karlsruhe.de/matwerk/E62426> ;
    modsci:hasManufacturer <http://demo.fiz-karlsruhe.de/matwerk/E1114779> .

<http://demo.fiz-karlsruhe.de/matwerk/E1110306> a modsci:Instrument ;
    rdfs:label "Procon XRM-II" ;
    nfdicore:location <http://demo.fiz-karlsruhe.de/matwerk/E80004> ;
    mwo:description "XRM-II is a correlative microsope based on an JEOL scanning electron microscope (SEM) combining electron imaging, electron dispersive X-ray spectroscopy (EDX) and nano X-ray computed tomography (nano-CT)" ;
    mwo:hasContactPoint <http://demo.fiz-karlsruhe.de/matwerk/E9647> ;
    mwo:hasOwner <http://demo.fiz-karlsruhe.de/matwerk/E3212> ;
    mwo:hasWebsite <http://demo.fiz-karlsruhe.de/matwerk/E287904> ;
    mwo:instrumentModel "XRM-II" ;
    mwo:usesTechnology <http://demo.fiz-karlsruhe.de/matwerk/E1116272> ;
    modsci:hasManufacturer <http://demo.fiz-karlsruhe.de/matwerk/E1114779> .

<http://demo.fiz-karlsruhe.de/matwerk/E1111796> a modsci:Instrument ;
    rdfs:label "https://www.fz-juelich.de/en/jcns/jcns-2/expertise/in-house-x-ray/powder-x-ray" .

<http://demo.fiz-karlsruhe.de/matwerk/E1113287> a modsci:Instrument ;
    rdfs:label "https://er-c.org/index.php/facilities-2/tfs-spectra-300/" .

<http://demo.fiz-karlsruhe.de/matwerk/E11154> a nfdicore:Person ;
    rdfs:label "Prof. Dr. Karsten  Durst" ;
    mwo:emailAddress "k.durst@phm.tu-darmstadt.de"^^xsd:string ;
    mwo:hasAffiliation <http://demo.fiz-karlsruhe.de/matwerk/E1011> ;
    mwo:hasExpertiseIn <http://demo.fiz-karlsruhe.de/matwerk/E42042>,
        <http://demo.fiz-karlsruhe.de/matwerk/E42906>,
        <http://demo.fiz-karlsruhe.de/matwerk/E43196>,
        <http://demo.fiz-karlsruhe.de/matwerk/E43487>,
        <http://demo.fiz-karlsruhe.de/matwerk/E43779>,
        <http://demo.fiz-karlsruhe.de/matwerk/E44072>,
        <http://demo.fiz-karlsruhe.de/matwerk/E44366>,
        <http://demo.fiz-karlsruhe.de/matwerk/E44661>,
        <http://demo.fiz-karlsruhe.de/matwerk/E44957>,
        <http://demo.fiz-karlsruhe.de/matwerk/E64547>,
        <http://demo.fiz-karlsruhe.de/matwerk/E65981> ;
    mwo:hasORCID <https://orcid.org/0000-0002-9246-6398> ;
    owl:sameAs <http://www.wikidata.org/entity/Q55762246> ;
    foaf:depiction <https://ams3.digitaloceanspaces.com/externalpublic/57/68ff2098-0363-4bf8-983d-a08ba11df83d/conversions/ce8c36f0-a8ab-4a9d-9f15-d25357eb1c47-md.jpg?X-Amz-Content-Sha256=UNSIGNED-PAYLOAD&X-Amz-Algorithm=AWS4-HMAC-SHA256&X-Amz-Credential=KVC4ZMO47JLTBHVHEFZ4%2F20230512%2Fams3%2Fs3%2Faws4_request&X-Amz-Date=20230512T150442Z&X-Amz-SignedHeaders=host&X-Amz-Expires=7200&X-Amz-Signature=144d6d5bbbb94f4cebe7a56beff4d6ba143d832cb1f808f26d37c2731952151c> ;
    foaf:firstName "Karsten "^^xsd:string ;
    foaf:surname "Durst"^^xsd:string ;
    foaf:title "Prof. Dr."^^xsd:string .

<http://demo.fiz-karlsruhe.de/matwerk/E1117766> a mwo:LargeScaleFacility ;
    rdfs:label "Deutsches Elektronen-Synchrotron" ;
    nfdicore:location <http://demo.fiz-karlsruhe.de/matwerk/E79607>,
        <http://demo.fiz-karlsruhe.de/matwerk/E80004> ;
    mwo:description "It conducts a broad spectrum of inter-disciplinary scientific research in three main areas: particle and high energy physics; photon science; and the development, construction and operation of particle accelerators. Its name refers to its first project, an electron synchrotron. DESY is publicly financed by the Federal Republic of Germany, the States of Germany, and the German Research Foundation (DFG). DESY is a member of the Helmholtz Association and operates at sites in Hamburg and Zeuthen." ;
    mwo:hasAcronym "DESY"^^xsd:string ;
    mwo:hasWebsite <http://demo.fiz-karlsruhe.de/matwerk/E297836> .

<http://demo.fiz-karlsruhe.de/matwerk/E1119261> a mwo:LargeScaleFacility ;
    rdfs:label "Jülich Supercomputing Centre" ;
    nfdicore:location <http://demo.fiz-karlsruhe.de/matwerk/E78422>,
        <http://demo.fiz-karlsruhe.de/matwerk/E80004> ;
    mwo:belongsTo <http://demo.fiz-karlsruhe.de/matwerk/E1022> ;
    mwo:description "The Jülich Supercomputing Centre at Forschungszentrum Jülich has been operating the first German supercomputing centre since 1987, and with the Jülich Institute for Advanced Simulation it is continuing the long tradition of scientific computing at Jülich. At the time being, JSC operates one of the most powerful supercomputers in Europe, JUWELS, and with JUNIQ the first European infrastructure for quantum computing." ;
    mwo:hasAcronym "JSC"^^xsd:string ;
    mwo:hasWebsite <http://demo.fiz-karlsruhe.de/matwerk/E299379> .

<http://demo.fiz-karlsruhe.de/matwerk/E1120757> a mwo:LargeScaleFacility ;
    rdfs:label "Steinbuch Centre for Computing" ;
    nfdicore:location <http://demo.fiz-karlsruhe.de/matwerk/E76467>,
        <http://demo.fiz-karlsruhe.de/matwerk/E80004> ;
    mwo:belongsTo <http://demo.fiz-karlsruhe.de/matwerk/E1121> ;
    mwo:description """SCC is a central scientific institution of the KIT in connection with tasks in research, teaching and innovation and provides comprehensive services within KIT and for external partners. These tasks are concrete:\r
Research and development in the fields of scientific computing and data analysis, management of large-scale research data and data-intensive computing as well as security in IT federations\r
Operation of the ICT infrastructure and provision of the basic IT equipment of KIT in conjunction with other service providers and system operators in the organisational units of KIT as part of a cooperative provider systemDevelopment and deployment of IT application systems, management of application software, training of users and administrators as well as end device support\r
Operation of large-scale facilities for scientific high-performance computing and data-intensive sciences within the framework of secure IT federations""" ;
    mwo:hasAcronym "SCC"^^xsd:string ;
    mwo:hasWebsite <http://demo.fiz-karlsruhe.de/matwerk/E300152> .

<http://demo.fiz-karlsruhe.de/matwerk/E1122254> a mwo:LargeScaleFacility ;
    rdfs:label "Ion Beam Center" ;
    nfdicore:location <http://demo.fiz-karlsruhe.de/matwerk/E79211>,
        <http://demo.fiz-karlsruhe.de/matwerk/E80004> ;
    mwo:description "Amongst the services offered at the IBC are ion beam modification of materials by ion implantation and irradiation, surface processing by low-energy / highly-charged ions (LEI/HCI) or focused ion beams (FIB), ion beam analysis (IBA), and accelerator mass spectrometry (AMS). " ;
    mwo:hasAcronym "IBC"^^xsd:string ;
    mwo:hasContactPoint <http://demo.fiz-karlsruhe.de/matwerk/E710837> ;
    mwo:hasWebsite <http://demo.fiz-karlsruhe.de/matwerk/E300926> .

<http://demo.fiz-karlsruhe.de/matwerk/E1123752> a mwo:MetadataSchema ;
    rdfs:label "Metadata schemes for materials science data" ;
    nfdicore:relatedProject <http://demo.fiz-karlsruhe.de/matwerk/E861017>,
        <http://demo.fiz-karlsruhe.de/matwerk/E862329> ;
    mwo:description "Metadata schemes for materials science data in JSON representation as implemented in TTL representation in the application profiles in the version from 01.05.2022 of the research data management platform CoScInE. The schema are actively developed in the SFB1394 with the aim to construct defect phase diagrams in an automated fashion using all data from advanced experimental characterization and computer simulations produced in this project." ;
    mwo:hasAuthor <http://demo.fiz-karlsruhe.de/matwerk/E20504>,
        <http://demo.fiz-karlsruhe.de/matwerk/E20702>,
        <http://demo.fiz-karlsruhe.de/matwerk/E20901>,
        <http://demo.fiz-karlsruhe.de/matwerk/E21101> ;
    mwo:hasDOI """https://doi.org/10.5281/zenodo.6513745\r
"""^^xsd:anyURI ;
    mwo:hasRepository <http://demo.fiz-karlsruhe.de/matwerk/E304032> ;
    ns3:has_license <http://demo.fiz-karlsruhe.de/matwerk/E817004> ;
    schema:datePublished "5/5/2022" .

<http://demo.fiz-karlsruhe.de/matwerk/E1126751> a mwo:SemanticResource ;
    rdfs:label "Elemental Multiperspective Material Ontology (EMMO)" ;
    nfdicore:relatedProject <http://demo.fiz-karlsruhe.de/matwerk/E863642>,
        <http://demo.fiz-karlsruhe.de/matwerk/E864956>,
        <http://demo.fiz-karlsruhe.de/matwerk/E866271>,
        <http://demo.fiz-karlsruhe.de/matwerk/E867587>,
        <http://demo.fiz-karlsruhe.de/matwerk/E868904>,
        <http://demo.fiz-karlsruhe.de/matwerk/E870222>,
        <http://demo.fiz-karlsruhe.de/matwerk/E871541>,
        <http://demo.fiz-karlsruhe.de/matwerk/E872861>,
        <http://demo.fiz-karlsruhe.de/matwerk/E874182>,
        <http://demo.fiz-karlsruhe.de/matwerk/E875504> ;
    nfdicore:semanticExpressivity nfdicore:Ontology ;
    mwo:description "The Elemental Multiperspective Material Ontology (EMMO) is the result of a multidisciplinary effort within the EMMC, aimed at the development of a standard representational ontology framework based on current materials modelling and characterization knowledge." ;
    mwo:hasContactPoint <http://demo.fiz-karlsruhe.de/matwerk/E712029> ;
    mwo:hasRepository <http://demo.fiz-karlsruhe.de/matwerk/E305591> ;
    ns3:has_license <http://demo.fiz-karlsruhe.de/matwerk/E819561> .

<http://demo.fiz-karlsruhe.de/matwerk/E1128252> a mwo:SemanticResource ;
    rdfs:label "MaterialsMine (MM)" ;
    nfdicore:semanticExpressivity nfdicore:Ontology ;
    mwo:description "A materials ontology to support data publication involving nanomaterials and metamaterials." ;
    mwo:hasRepository <http://demo.fiz-karlsruhe.de/matwerk/E306372> ;
    mwo:hasVersion "1" ;
    ns3:has_license <http://demo.fiz-karlsruhe.de/matwerk/E820841> ;
    schema:datePublished "2/19/2022" .

<http://demo.fiz-karlsruhe.de/matwerk/E11297> a nfdicore:Person ;
    rdfs:label "Jun. Prof. Dr.  Nina Merkert" ;
    mwo:emailAddress "nina.merkert@tu-clausthal.de"^^xsd:string ;
    mwo:hasAffiliation <http://demo.fiz-karlsruhe.de/matwerk/E1002> ;
    mwo:hasExpertiseIn <http://demo.fiz-karlsruhe.de/matwerk/E45254>,
        <http://demo.fiz-karlsruhe.de/matwerk/E45552>,
        <http://demo.fiz-karlsruhe.de/matwerk/E45851>,
        <http://demo.fiz-karlsruhe.de/matwerk/E61379> ;
    mwo:hasORCID <https://orcid.org/0000-0002-2909-5109> ;
    owl:sameAs <http://www.wikidata.org/entity/Q85888918> ;
    foaf:depiction <https://ams3.digitaloceanspaces.com/externalpublic/57/1fdf0c38-26d5-4cd9-92aa-f78b9a74a810/conversions/7aea4c5d-38d1-4055-ba68-93e979d2c6af-md.jpg?X-Amz-Content-Sha256=UNSIGNED-PAYLOAD&X-Amz-Algorithm=AWS4-HMAC-SHA256&X-Amz-Credential=KVC4ZMO47JLTBHVHEFZ4%2F20230512%2Fams3%2Fs3%2Faws4_request&X-Amz-Date=20230512T150442Z&X-Amz-SignedHeaders=host&X-Amz-Expires=7200&X-Amz-Signature=45c089b88ca5878da45241ef2e77fd755d16b0711c973674bc5e2be8747e139f> ;
    foaf:firstName "Nina"^^xsd:string ;
    foaf:surname "Merkert"^^xsd:string ;
    foaf:title "Jun. Prof. Dr. "^^xsd:string .

<http://demo.fiz-karlsruhe.de/matwerk/E1129754> a mwo:SemanticResource ;
    rdfs:label "Dislocation Ontology (DISO)" ;
    nfdicore:relatedProject <http://demo.fiz-karlsruhe.de/matwerk/E876827> ;
    nfdicore:semanticExpressivity nfdicore:Ontology ;
    mwo:description "DISO is a domain ontology that defines the linear defect, in particular dislocation concepts and relations between them in crystalline materials. Moreover, Crystal Structure Ontology (CSO) and Crystallographic Defect Ontology (CDO), which ontologies define the concepts of crystal structureand crystalline defect, respectively, are also introduced in this repository." ;
    mwo:hasAuthor <http://demo.fiz-karlsruhe.de/matwerk/E10181>,
        <http://demo.fiz-karlsruhe.de/matwerk/E29681>,
        <http://demo.fiz-karlsruhe.de/matwerk/E29921> ;
    mwo:hasContactPoint <http://demo.fiz-karlsruhe.de/matwerk/E10181> ;
    mwo:hasDocumentation <http://demo.fiz-karlsruhe.de/matwerk/E321401> ;
    mwo:hasRepository <http://demo.fiz-karlsruhe.de/matwerk/E307154> ;
    mwo:hasVersion "1" ;
    ns3:has_license <http://demo.fiz-karlsruhe.de/matwerk/E820841> ;
    schema:datePublished "5/29/2022" .

<http://demo.fiz-karlsruhe.de/matwerk/E1131257> a mwo:SemanticResource ;
    rdfs:label "Materials Design Ontology (MDO)" ;
    nfdicore:relatedProject <http://demo.fiz-karlsruhe.de/matwerk/E878151> ;
    nfdicore:semanticExpressivity nfdicore:Ontology ;
    mwo:description "MDO is an ontology for materials design field, representing the domain knowledge specifically related to solid-state physics and computational materials science." ;
    mwo:hasAuthor <http://demo.fiz-karlsruhe.de/matwerk/E30162>,
        <http://demo.fiz-karlsruhe.de/matwerk/E30404>,
        <http://demo.fiz-karlsruhe.de/matwerk/E30647> ;
    mwo:hasDocumentation <http://demo.fiz-karlsruhe.de/matwerk/E322202> ;
    mwo:hasRepository <http://demo.fiz-karlsruhe.de/matwerk/E307937> ;
    ns3:has_license <http://demo.fiz-karlsruhe.de/matwerk/E820841> ;
    schema:datePublished "11/7/2019" .

<http://demo.fiz-karlsruhe.de/matwerk/E1132761> a mwo:SemanticResource ;
    rdfs:label "Aditive Manufacturing Ontology (AMONTOLOGY)" ;
    nfdicore:semanticExpressivity nfdicore:Ontology ;
    mwo:description "The AM ontology has been developed following two major milestones. The ontology developed within the first milestone includes AMProcessOntology, ModelOntology and AMOntology files. AMProcessOntology contains the set of entities used to capture knowledge about additive manufacturing processes. ModelOntology contains the set of entities used to capture knowledge about modeling concepts that represent (possibly) multi-physics multi-scale processes. AMOntology uses AMProcessOntology and ModelOntology files to describe entities that capture knowledge about characteristics of computational models for AM processes." ;
    mwo:hasRepository <http://demo.fiz-karlsruhe.de/matwerk/E308721> .

<http://demo.fiz-karlsruhe.de/matwerk/E1134266> a mwo:SemanticResource ;
    rdfs:label "MatOnto Ontology (MATONTO)" ;
    nfdicore:semanticExpressivity nfdicore:Ontology ;
    mwo:description "Domain ontology for the MatOnto Project" ;
    mwo:hasRepository <http://demo.fiz-karlsruhe.de/matwerk/E309506> ;
    mwo:hasVersion "2" ;
    ns3:has_license <http://demo.fiz-karlsruhe.de/matwerk/E820841> .

<http://demo.fiz-karlsruhe.de/matwerk/E1135772> a mwo:SemanticResource ;
    rdfs:label "Virtual Materials Marketplace (VIMMP) Ontologies" ;
    nfdicore:semanticExpressivity nfdicore:Ontology ;
    mwo:description "The Virtual Materials Marketplace (VIMMP) project, which develops an open platform for providing and accessing services related to materials modelling, is presented with a focus on its ontology development and data technology aspects. Within VIMMP, a system of marketplace-level ontologies is developed to characterize services, models, and interactions between users; the European Materials and Modelling Ontology is employed as a top-level ontology. The ontologies are used to annotate data that are stored in the ZONTAL Space component of VIMMP and to support the ingest and retrieval of data and metadata at the VIMMP marketplace frontend." ;
    mwo:hasRepository <http://demo.fiz-karlsruhe.de/matwerk/E310292> ;
    schema:citation <http://demo.fiz-karlsruhe.de/matwerk/E995756> ;
    schema:datePublished "1/2/2021" .

<http://demo.fiz-karlsruhe.de/matwerk/E1137279> a mwo:SemanticResource ;
    rdfs:label "eNanoMapper ontology" ;
    nfdicore:semanticExpressivity nfdicore:Ontology ;
    mwo:description "The eNanoMapper ontologies aim to provide a comprehensive suite of ontologies for the nanomaterial safety assessment domain" ;
    mwo:hasDOI """Version 7: https://doi.org/10.5281/zenodo.4600986\r
Version 6: https://doi.org/10.5281/zenodo.3382100\r
Version 5: https://doi.org/10.5281/zenodo.3237535\r
Version 4: https://doi.org/10.5281/zenodo.260098\r
Version 3: https://doi.org/10.5281/zenodo.47119"""^^xsd:anyURI ;
    mwo:hasRepository <http://demo.fiz-karlsruhe.de/matwerk/E311079> ;
    mwo:hasVersion "8" ;
    ns3:has_license <http://demo.fiz-karlsruhe.de/matwerk/E822122> ;
    schema:citation <http://demo.fiz-karlsruhe.de/matwerk/E997167> .

<http://demo.fiz-karlsruhe.de/matwerk/E1138787> a mwo:SemanticResource ;
    rdfs:label "Material Science and Engineering Ontology (MSEO)" ;
    nfdicore:semanticExpressivity nfdicore:Ontology ;
    mwo:description "MSEO utilizes the Common Core Ontology stack giving materials scientists and engineers the ability to represent their experiments and resulting data. The goal is to create machine and human readable sematic data which can be easily digested by other science domains. It is a product of the joint venture Materials Open Lab Project between the Bundesanstalt für Materialforschung und -prüfung (BAM) and the Fraunhofer Group MATERIALS and used the BWMD ontology created by Fraunhofer IWM as a starting point." ;
    mwo:hasContactPoint <http://demo.fiz-karlsruhe.de/matwerk/E11879> ;
    mwo:hasRepository <http://demo.fiz-karlsruhe.de/matwerk/E311867> ;
    mwo:hasVersion "0.3" .

<http://demo.fiz-karlsruhe.de/matwerk/E1140296> a mwo:SemanticResource ;
    rdfs:label "PMD Core Ontology" ;
    nfdicore:relatedProject <http://demo.fiz-karlsruhe.de/matwerk/E879476> ;
    nfdicore:semanticExpressivity nfdicore:Ontology ;
    mwo:description "Ontology used in Platform Material Digital (PMD)" ;
    mwo:hasRepository <http://demo.fiz-karlsruhe.de/matwerk/E312656> .

<http://demo.fiz-karlsruhe.de/matwerk/E1141806> a mwo:SemanticResource ;
    rdfs:label "NanoParticle Ontology for Cancer Nanotechnology Research (NPO)" ;
    nfdicore:semanticExpressivity nfdicore:Ontology ;
    mwo:description "The NPO is developed to represent the knowledge underlying the description, preparation, and characterization of nanomaterials in cancer nanotechnology research." ;
    mwo:hasRepository <http://demo.fiz-karlsruhe.de/matwerk/E313446> ;
    ns3:has_license <http://demo.fiz-karlsruhe.de/matwerk/E1246803> ;
    schema:citation <http://demo.fiz-karlsruhe.de/matwerk/E998579> .

<http://demo.fiz-karlsruhe.de/matwerk/E1143317> a mwo:SemanticResource ;
    rdfs:label "Materials And Molecules Basic Ontology (MAMBO)" ;
    nfdicore:semanticExpressivity nfdicore:Ontology ;
    mwo:description "MAMBO (Materials And Molecules Basic Ontology) is a domain ontology for molecular materials. " ;
    mwo:hasRepository <http://demo.fiz-karlsruhe.de/matwerk/E314237> .

<http://demo.fiz-karlsruhe.de/matwerk/E11441> a nfdicore:Person ;
    rdfs:label "Prof. Dr.  Thomas Speck" ;
    mwo:emailAddress "thomas.speck@biologie.uni-freiburg.de"^^xsd:string ;
    mwo:hasAffiliation <http://demo.fiz-karlsruhe.de/matwerk/E1079> ;
    mwo:hasExpertiseIn <http://demo.fiz-karlsruhe.de/matwerk/E46151>,
        <http://demo.fiz-karlsruhe.de/matwerk/E46452>,
        <http://demo.fiz-karlsruhe.de/matwerk/E46754> ;
    foaf:depiction <https://ams3.digitaloceanspaces.com/externalpublic/57/feb1c404-6287-47c6-9fd9-87daa895653b/conversions/305b1666-bbaf-4570-825d-07d38a1e06de-md.jpg?X-Amz-Content-Sha256=UNSIGNED-PAYLOAD&X-Amz-Algorithm=AWS4-HMAC-SHA256&X-Amz-Credential=KVC4ZMO47JLTBHVHEFZ4%2F20230512%2Fams3%2Fs3%2Faws4_request&X-Amz-Date=20230512T150442Z&X-Amz-SignedHeaders=host&X-Amz-Expires=7200&X-Amz-Signature=fd068387480414caf7e6d5508031b2b160d404187b393ae5f96d50df768a84b8> ;
    foaf:firstName "Thomas"^^xsd:string ;
    foaf:surname "Speck"^^xsd:string ;
    foaf:title "Prof. Dr. "^^xsd:string .

<http://demo.fiz-karlsruhe.de/matwerk/E1144829> a mwo:MetadataSchema ;
    rdfs:label "Web Standards and Reference Data for First-Principles Simulations" ;
    mwo:description "The quantum-simulation.org web site aims at providing reference simulation data and promoting the use of XML standards for interchange of simulation data in the area of electronic structure calculations and first-principles molecular dynamics simulations. " ;
    mwo:hasDocumentation <http://demo.fiz-karlsruhe.de/matwerk/E323004> ;
    mwo:hasRelatedResource <http://demo.fiz-karlsruhe.de/matwerk/E647954> .

<http://demo.fiz-karlsruhe.de/matwerk/E1146342> a mwo:MetadataSchema ;
    rdfs:label "MatDB Online" ;
    mwo:description "MatDB Online facility is a Standards-based system for preserving, managing, and exchanging engineering materials test data." ;
    mwo:hasDOI "http://dx.doi.org/10.2481/dsj.AMDS-003"^^xsd:anyURI ;
    mwo:hasDocumentation <http://demo.fiz-karlsruhe.de/matwerk/E323807> ;
    schema:citation <http://demo.fiz-karlsruhe.de/matwerk/E999992> .

<http://demo.fiz-karlsruhe.de/matwerk/E1147856> a mwo:MetadataSchema ;
    rdfs:label "MatML" ;
    mwo:description "This specification describes a standard XML format for the exchange of materials information. Information such as product form, heat treatment, mechanical properties and chemistry can be transmitted.  " ;
    mwo:hasDocumentation <http://demo.fiz-karlsruhe.de/matwerk/E324611> ;
    schema:datePublished "6/6/2006" .

<http://demo.fiz-karlsruhe.de/matwerk/E1149371> a nfdicore:Specification ;
    rdfs:label "Crystallographic Information Framework (CIF2)" ;
    mwo:description "the Crystallographic Information Framework, a broader system of exchange protocols based on data dictionaries and relational rules expressible in different machine-readable manifestations, including, but not restricted to, Crystallographic Information File and XML." ;
    mwo:hasDocumentation <http://demo.fiz-karlsruhe.de/matwerk/E325416> ;
    schema:citation <http://demo.fiz-karlsruhe.de/matwerk/E1001406> .

<http://demo.fiz-karlsruhe.de/matwerk/E1150887> a nfdicore:Specification ;
    rdfs:label "ColabFit" ;
    mwo:description """The ColabFit project aims to create a framework to facilitate the training and use of machine learning (ML) models in materials science including interatomic potentials. This includes an online exchange for datasets used to train ML models and a portable format for deploying ML models to simulation platforms using the OpenKIM system.\r
\r
""" ;
    mwo:hasDocumentation <http://demo.fiz-karlsruhe.de/matwerk/E326222> ;
    mwo:hasRelatedResource <http://demo.fiz-karlsruhe.de/matwerk/E543362> .

<http://demo.fiz-karlsruhe.de/matwerk/E1152404> a nfdicore:Specification ;
    rdfs:label "Essential Source of Schemas and Examples (ESSE)" ;
    mwo:description "JSON schemas and examples representing structural data, characteristic properties, modeling workflows and related data about materials standardizing the diverse landscape of information" ;
    mwo:hasRepository <http://demo.fiz-karlsruhe.de/matwerk/E315029> .

<http://demo.fiz-karlsruhe.de/matwerk/E1153922> a nfdicore:Specification ;
    rdfs:label "Electronic Structure Common Data Format (ESCDF)" ;
    mwo:description """This project gathers the working documents used to design the specifications\r
of the Electronic Structure Common Data Format (ESCDF), an initiative of the\r
Electronic Structure Library (ESL) Contributors.\r
""" ;
    mwo:hasRepository <http://demo.fiz-karlsruhe.de/matwerk/E315822> .

<http://demo.fiz-karlsruhe.de/matwerk/E1155441> a nfdicore:Specification ;
    rdfs:label "Graphical Expression of Materials Data (GEMD)" ;
    mwo:description """GEMD stands for Graphical Expression of Materials Data. It's an open-source format initially developed by Citrine Informatics. A version of it is used in their AI platform for materials and chemicals, but as described here it can be used independently.\r
\r
""" ;
    mwo:hasDocumentation <http://demo.fiz-karlsruhe.de/matwerk/E327029> .

<http://demo.fiz-karlsruhe.de/matwerk/E1156961> a nfdicore:Specification ;
    rdfs:label "NOMAD Metainfo" ;
    mwo:description "The NOMAD Metainfo stores descriptive and structured information about materials-science data contained in the NOMAD Archive" ;
    mwo:hasDocumentation <http://demo.fiz-karlsruhe.de/matwerk/E327837> .

<http://demo.fiz-karlsruhe.de/matwerk/E1158482> a mwo:MetadataSchema ;
    rdfs:label "Physical Information File (PIF)" ;
    mwo:description "The Physical Information File (PIF) is a schema that is designed to impose structure on information about physical systems. Schema design, as well as tools for working with PIF-formatted files using the python (pypif) and java (jpif) programming languages are maintained by Citrine Informatics." ;
    mwo:hasDocumentation <http://demo.fiz-karlsruhe.de/matwerk/E328646> .

<http://demo.fiz-karlsruhe.de/matwerk/E11586> a nfdicore:Person ;
    rdfs:label "Prof. Dr.  Jürgen Rühe" ;
    mwo:emailAddress "ruehe@imtek.uni-freiburg.de"^^xsd:string ;
    mwo:hasAffiliation <http://demo.fiz-karlsruhe.de/matwerk/E1092> ;
    mwo:hasExpertiseIn <http://demo.fiz-karlsruhe.de/matwerk/E47057> ;
    foaf:firstName "Jürgen"^^xsd:string ;
    foaf:surname "Rühe"^^xsd:string ;
    foaf:title "Prof. Dr. "^^xsd:string .

<http://demo.fiz-karlsruhe.de/matwerk/E1161527> a mwo:MetadataSchema ;
    rdfs:label "MGI JSON Schema" ;
    mwo:description "The purpose of this repository is to enable community development of JSON schema within materials science and engineering." ;
    mwo:hasRepository <http://demo.fiz-karlsruhe.de/matwerk/E317411> .

<http://demo.fiz-karlsruhe.de/matwerk/E1163051> a mwo:SemanticResource ;
    rdfs:label "Chemical Methods Ontology (CHMO)" ;
    nfdicore:semanticExpressivity nfdicore:Ontology ;
    mwo:description """The Chemical Methods Ontology contains more than 3000 classes and describes methods used to: collect data in chemical experiments, such as mass spectrometry and electron microscopy\r
prepare and separate material for further analysis, such as sample ionisation, chromatography, and electrophoresis\r
synthesise materials, such as epitaxy and continuous vapour deposition It also describes the instruments used in these experiments, such as mass spectrometers and chromatography columns and their outputs.""" ;
    mwo:hasRepository <http://demo.fiz-karlsruhe.de/matwerk/E318207> ;
    ns3:has_license <http://demo.fiz-karlsruhe.de/matwerk/E823404> .

<http://demo.fiz-karlsruhe.de/matwerk/E1164576> a nfdicore:Specification ;
    rdfs:label "Standardised documentation of Simulations (MODA)" ;
    mwo:description "The MODA comprises a text template and a graphical workflow template which should be used to document materials modelling workflows for EU projects, but they may also find use in organisations' documentations or in supplementary documents of scientific publications." ;
    mwo:hasDocumentation <http://demo.fiz-karlsruhe.de/matwerk/E330267> .

<http://demo.fiz-karlsruhe.de/matwerk/E1166102> a mwo:SemanticResource ;
    rdfs:label "Characterisation Methodology Domain Ontology (CHAMEO)" ;
    nfdicore:semanticExpressivity nfdicore:Ontology ;
    mwo:description """An ontology for materials characterization based on the CHADA template.\r
This ontology development is supported by an EMMC Task Group. """ ;
    mwo:hasRepository <http://demo.fiz-karlsruhe.de/matwerk/E319004> .

<http://demo.fiz-karlsruhe.de/matwerk/E1167629> a nfdicore:Specification ;
    rdfs:label "Core Scientific Metadata Model (CSMD)" ;
    mwo:description """The CSMD is developed to support data collected within a facility's scientific workflow. However the model is also designed to be generic across scientific disciplines and has application beyond facilities science, particularly in the "structural sciences" (such as chemistry, material science, earth science, and biochemistry) which are concerned with analysing the structure of substances, and perform systematic experimental analyses on samples of those materials.\r
\r
""" ;
    mwo:hasDocumentation <http://demo.fiz-karlsruhe.de/matwerk/E331079> .

<http://demo.fiz-karlsruhe.de/matwerk/E1169157> a mwo:MetadataSchema ;
    rdfs:label "EngMeta" ;
    mwo:description "EngMeta ist ein Metadatenschema zur Beschreibung von ingenieurwissenschaftlichen Forschungsdaten" ;
    mwo:hasDocumentation <http://demo.fiz-karlsruhe.de/matwerk/E331892> .

<http://demo.fiz-karlsruhe.de/matwerk/E1170686> a nfdicore:Dataset ;
    rdfs:label "Datasets for the analysis of dislocations at grain boundaries and during vein formation in cyclically deformed Ni micropillars" ;
    nfdicore:fileExtension "png",
        "txt" ;
    nfdicore:objectType <http://demo.fiz-karlsruhe.de/matwerk/E1196832>,
        <http://demo.fiz-karlsruhe.de/matwerk/E1198379>,
        <http://demo.fiz-karlsruhe.de/matwerk/E1199927> ;
    mwo:aboutMaterial <http://demo.fiz-karlsruhe.de/matwerk/E1178346> ;
    mwo:description "The data consists of two parts: the simulation data that was used to analyze the effect of a particular grain boundary on curved dislocations and the precession electron diffraction (PED) strain maps together with post-processed data for analyzing details of the observed dislocation vein structures. " ;
    mwo:hasCreator <http://demo.fiz-karlsruhe.de/matwerk/E13721>,
        <http://demo.fiz-karlsruhe.de/matwerk/E29921>,
        <http://demo.fiz-karlsruhe.de/matwerk/E31136>,
        <http://demo.fiz-karlsruhe.de/matwerk/E31382>,
        <http://demo.fiz-karlsruhe.de/matwerk/E31629>,
        <http://demo.fiz-karlsruhe.de/matwerk/E31877>,
        <http://demo.fiz-karlsruhe.de/matwerk/E32126> ;
    mwo:hasDiscipline <http://demo.fiz-karlsruhe.de/matwerk/E1184492> ;
    mwo:hasDocumentation <http://demo.fiz-karlsruhe.de/matwerk/E293996> ;
    mwo:hasRepository <http://demo.fiz-karlsruhe.de/matwerk/E288662> ;
    mwo:usesMethod <http://demo.fiz-karlsruhe.de/matwerk/E625404> ;
    ns3:has_license <http://demo.fiz-karlsruhe.de/matwerk/E815727> ;
    rdfs:comment "-" ;
    schema:datePublished "10/30/2019" .

<http://demo.fiz-karlsruhe.de/matwerk/E1172216> a nfdicore:Dataset ;
    rdfs:label "datasets" ;
    nfdicore:fileExtension "",
        "dat",
        "h5",
        "hdf5",
        "ipynb",
        "py",
        "txt" ;
    nfdicore:objectType <http://demo.fiz-karlsruhe.de/matwerk/E1201476>,
        <http://demo.fiz-karlsruhe.de/matwerk/E1203026>,
        <http://demo.fiz-karlsruhe.de/matwerk/E1204577> ;
    mwo:description "This dataset was used in the work \"Material modeling for parametric, anisotropic finite hyperelasticity based on machine learning with application in optimization of metamaterials\" by M. Fernández, F. Fritzen and O. Weeger",
        "This dataset was used in the work \"On-the-Fly Adaptivity for Nonlinear Twoscale Simulations Using Artificial Neural Networks and Reduced Order Modeling\" by F. Fritzen, M. Fernández,  and F. Larsson" ;
    mwo:hasContributor <http://demo.fiz-karlsruhe.de/matwerk/E16226>,
        <http://demo.fiz-karlsruhe.de/matwerk/E16577>,
        <http://demo.fiz-karlsruhe.de/matwerk/E32376>,
        <http://demo.fiz-karlsruhe.de/matwerk/E32627> ;
    mwo:hasCreator <http://demo.fiz-karlsruhe.de/matwerk/E16226>,
        <http://demo.fiz-karlsruhe.de/matwerk/E16577>,
        <http://demo.fiz-karlsruhe.de/matwerk/E32376>,
        <http://demo.fiz-karlsruhe.de/matwerk/E32627> ;
    mwo:hasDiscipline <http://demo.fiz-karlsruhe.de/matwerk/E1186031>,
        <http://demo.fiz-karlsruhe.de/matwerk/E1187571>,
        <http://demo.fiz-karlsruhe.de/matwerk/E1189112> ;
    mwo:hasDocumentation <http://demo.fiz-karlsruhe.de/matwerk/E294762>,
        <http://demo.fiz-karlsruhe.de/matwerk/E295529>,
        <http://demo.fiz-karlsruhe.de/matwerk/E296297> ;
    mwo:hasRepository <http://demo.fiz-karlsruhe.de/matwerk/E289421>,
        <http://demo.fiz-karlsruhe.de/matwerk/E290181>,
        <http://demo.fiz-karlsruhe.de/matwerk/E290942> ;
    schema:datePublished "11/26/2021",
        "5/3/2019",
        "7/17/2020" .

<http://demo.fiz-karlsruhe.de/matwerk/E11732> a nfdicore:Person ;
    rdfs:label "Prof. Dr. Manfred Füting" ;
    foaf:firstName "Manfred"^^xsd:string ;
    foaf:surname "Füting"^^xsd:string ;
    foaf:title "Prof. Dr."^^xsd:string .

<http://demo.fiz-karlsruhe.de/matwerk/E1173747> a nfdicore:Dataset ;
    rdfs:label "BAM reference data: results of ASTM E139 -11 creep tests on a reference material of Nimonic 75 nickel-base alloy" ;
    nfdicore:fileExtension "csv",
        "pdf" ;
    nfdicore:objectType <http://demo.fiz-karlsruhe.de/matwerk/E1206129>,
        <http://demo.fiz-karlsruhe.de/matwerk/E1207682>,
        <http://demo.fiz-karlsruhe.de/matwerk/E1209236>,
        <http://demo.fiz-karlsruhe.de/matwerk/E1210791>,
        <http://demo.fiz-karlsruhe.de/matwerk/E1212347> ;
    nfdicore:standard <http://demo.fiz-karlsruhe.de/matwerk/E1195286> ;
    mwo:aboutMaterial <http://demo.fiz-karlsruhe.de/matwerk/E1179881> ;
    mwo:description "The creep behavior of a certified reference material was determined according to ASTM E139-11 using calibrated equipment of an accredited testing laboratory" ;
    mwo:hasCreator <http://demo.fiz-karlsruhe.de/matwerk/E32879>,
        <http://demo.fiz-karlsruhe.de/matwerk/E9002> ;
    mwo:hasDiscipline <http://demo.fiz-karlsruhe.de/matwerk/E1190654> ;
    mwo:hasRepository <http://demo.fiz-karlsruhe.de/matwerk/E291704> ;
    ns3:has_license <http://demo.fiz-karlsruhe.de/matwerk/E817004> ;
    schema:datePublished "7/15/2021" .

<http://demo.fiz-karlsruhe.de/matwerk/E1175279> a nfdicore:Dataset ;
    rdfs:label "Brinell-Hardness (HBW 2.5/62.5) of Al-alloy EN AW-2618A after different aging times and temperatures" ;
    nfdicore:fileExtension "pdf",
        "xlsx" ;
    nfdicore:objectType <http://demo.fiz-karlsruhe.de/matwerk/E1210791>,
        <http://demo.fiz-karlsruhe.de/matwerk/E1212347>,
        <http://demo.fiz-karlsruhe.de/matwerk/E1213904>,
        <http://demo.fiz-karlsruhe.de/matwerk/E1215462>,
        <http://demo.fiz-karlsruhe.de/matwerk/E1217021> ;
    mwo:aboutMaterial <http://demo.fiz-karlsruhe.de/matwerk/E1181417>,
        <http://demo.fiz-karlsruhe.de/matwerk/E1181418> ;
    mwo:description "The aging behavior of a technical Al alloy (EN AW-2618A) under long-term tempering (load -free and under tensile load) was characterized by hardness measurements" ;
    mwo:hasCreator <http://demo.fiz-karlsruhe.de/matwerk/E33132>,
        <http://demo.fiz-karlsruhe.de/matwerk/E33386>,
        <http://demo.fiz-karlsruhe.de/matwerk/E9002> ;
    mwo:hasDiscipline <http://demo.fiz-karlsruhe.de/matwerk/E1192197> ;
    mwo:hasDocumentation <http://demo.fiz-karlsruhe.de/matwerk/E297066>,
        <http://demo.fiz-karlsruhe.de/matwerk/E297067> ;
    mwo:hasRepository <http://demo.fiz-karlsruhe.de/matwerk/E292467> ;
    ns3:has_license <http://demo.fiz-karlsruhe.de/matwerk/E817004> ;
    schema:datePublished "7/1/2022" .

<http://demo.fiz-karlsruhe.de/matwerk/E1176812> a nfdicore:Dataset ;
    rdfs:label "Full dataset of several mechanical tests on an S355 steel sheet as reference data for digital representations" ;
    nfdicore:fileExtension "pdf",
        "xlsx" ;
    mwo:aboutMaterial <http://demo.fiz-karlsruhe.de/matwerk/E1182954> ;
    mwo:description "Well-documented characterizations (tensile test, charpy, sonic resonance) were performed on S355 to provide example/reference datasets" ;
    mwo:hasCreator <http://demo.fiz-karlsruhe.de/matwerk/E33641>,
        <http://demo.fiz-karlsruhe.de/matwerk/E33897>,
        <http://demo.fiz-karlsruhe.de/matwerk/E34154>,
        <http://demo.fiz-karlsruhe.de/matwerk/E34412>,
        <http://demo.fiz-karlsruhe.de/matwerk/E9002> ;
    mwo:hasDiscipline <http://demo.fiz-karlsruhe.de/matwerk/E1193741> ;
    mwo:hasRepository <http://demo.fiz-karlsruhe.de/matwerk/E293231> ;
    ns3:has_license <http://demo.fiz-karlsruhe.de/matwerk/E817004> ;
    schema:datePublished "6/29/2022" .

<http://demo.fiz-karlsruhe.de/matwerk/E12027> a nfdicore:Person ;
    rdfs:label "Prof. Dr.-Ing. Thomas Böhlke" ;
    mwo:emailAddress "thomas.boehlke@kit.edu"^^xsd:string ;
    mwo:hasAffiliation <http://demo.fiz-karlsruhe.de/matwerk/E1121> ;
    mwo:hasExpertiseIn <http://demo.fiz-karlsruhe.de/matwerk/E47361>,
        <http://demo.fiz-karlsruhe.de/matwerk/E47666>,
        <http://demo.fiz-karlsruhe.de/matwerk/E47972>,
        <http://demo.fiz-karlsruhe.de/matwerk/E48279>,
        <http://demo.fiz-karlsruhe.de/matwerk/E65262>,
        <http://demo.fiz-karlsruhe.de/matwerk/E65981> ;
    mwo:hasORCID <https://orcid.org/0000-0001-6884-0530> ;
    owl:sameAs <http://www.wikidata.org/entity/Q109087> ;
    foaf:firstName "Thomas"^^xsd:string ;
    foaf:surname "Böhlke"^^xsd:string ;
    foaf:title "Prof. Dr.-Ing."^^xsd:string .

<http://demo.fiz-karlsruhe.de/matwerk/E12326> a nfdicore:Person ;
    rdfs:label "Prof. Stefan Diebels" ;
    mwo:emailAddress "s.diebels@mx.uni-saarland.de"^^xsd:string ;
    mwo:hasAffiliation <http://demo.fiz-karlsruhe.de/matwerk/E1154> ;
    mwo:hasExpertiseIn <http://demo.fiz-karlsruhe.de/matwerk/E48587>,
        <http://demo.fiz-karlsruhe.de/matwerk/E49517>,
        <http://demo.fiz-karlsruhe.de/matwerk/E65262> ;
    mwo:hasORCID <https://orcid.org/0000-0002-1642-9018> ;
    owl:sameAs <http://www.wikidata.org/entity/Q111358858> ;
    foaf:depiction <https://nfdi.inventum.de/storage/defaultImages/avatar.svg> ;
    foaf:firstName "Stefan"^^xsd:string ;
    foaf:surname "Diebels"^^xsd:string ;
    foaf:title "Prof."^^xsd:string .

<http://demo.fiz-karlsruhe.de/matwerk/E1245255> a mwo:EducationalResource ;
    rdfs:label "Data Processing for Engineers and Scientists" ;
    dcterms:format "Training courses for international students" ;
    mwo:description "basic statistics; python programming; image processing; basic machine learning" ;
    mwo:hasLecturer <http://demo.fiz-karlsruhe.de/matwerk/E16577> ;
    mwo:hasWebsite <http://demo.fiz-karlsruhe.de/matwerk/E393942>,
        <http://demo.fiz-karlsruhe.de/matwerk/E406451> ;
    mwo:isOnline false ;
    mwo:requiredTool <http://demo.fiz-karlsruhe.de/matwerk/E1231097>,
        <http://demo.fiz-karlsruhe.de/matwerk/E836279> ;
    rdfs:comment "winter semester" ;
    ns1:duration "2x90 min/week"^^xsd:time .

<http://demo.fiz-karlsruhe.de/matwerk/E1245256> a mwo:EducationalResource ;
    rdfs:label "Selected Chapters in Data Processing: Microstructure Analysis and Synthesis" ;
    dcterms:format "Training courses for international students" ;
    mwo:description "2D and 3D image analysis; image processing; paraview and python" ;
    mwo:hasLecturer <http://demo.fiz-karlsruhe.de/matwerk/E16577> ;
    mwo:hasWebsite <http://demo.fiz-karlsruhe.de/matwerk/E394829>,
        <http://demo.fiz-karlsruhe.de/matwerk/E406451> ;
    mwo:isOnline false ;
    mwo:requiredTool <http://demo.fiz-karlsruhe.de/matwerk/E1231097>,
        <http://demo.fiz-karlsruhe.de/matwerk/E1232666>,
        <http://demo.fiz-karlsruhe.de/matwerk/E836279> ;
    rdfs:comment "winter semester" ;
    ns1:duration "1,5x90 min/week"^^xsd:time .

<http://demo.fiz-karlsruhe.de/matwerk/E1245261> a mwo:EducationalResource ;
    rdfs:label "Knowledge Graphs (openHPI Massive Open Online Course (MOOC))" ;
    dcterms:format "Academic teaching materials" ;
    mwo:description "In this course you will learn what is necessary to design, implement, and use knowledge graphs. The focus of this course will be on basic semantic technologies including the principles of knowledge representation and symbolic AI. This includes information encoding via RDF triples, knowledge representation via ontologies with OWL, efficiently querying knowledge graphs via SPARQL, latent representation of knowledge in vector space, as well as knowledge graph applications in innovative information systems, as e.g., semantic and exploratory search." ;
    mwo:hasLecturer <http://demo.fiz-karlsruhe.de/matwerk/E14862> ;
    mwo:hasWebsite <http://demo.fiz-karlsruhe.de/matwerk/E396606> ;
    mwo:isOnline true ;
    rdfs:comment "2020" ;
    ns1:duration "6 weeks"^^xsd:time .

<http://demo.fiz-karlsruhe.de/matwerk/E1245265> a mwo:EducationalResource ;
    rdfs:label "Information Service Engineering (openHPI Massive Open Online Course (MOOC))" ;
    dcterms:format "Academic teaching materials" ;
    mwo:description "The information available today exceeds all limits. Access to this abundance of data is only possible via search engines and sophisticated information processing applications. To enable the transition from raw data to well-structured knowledge, technologies such as natural language processing, information retrieval, data and knowledge mining must be applied. In the course of this transition, unstructured data such as natural language text, is analyzed based on statistical language models and machine learning, to represent the contained information with the help of formal knowledge representations. In general, “Information Service Engineering” covers the conceptualization, development, and maintenance of long-term operation of services for the exploitation, processing, and dissemination of information. In this lecture, students will learn the fundamentals of natural language processing, knowledge mining, machine learning, linked data engineering, as well as information retrieval required for the development of information services." ;
    mwo:hasLecturer <http://demo.fiz-karlsruhe.de/matwerk/E14862> ;
    mwo:hasWebsite <http://demo.fiz-karlsruhe.de/matwerk/E397496> ;
    mwo:isOnline true ;
    rdfs:comment "2017" ;
    ns1:duration "6 weeks"^^xsd:time .

<http://demo.fiz-karlsruhe.de/matwerk/E1245270> a mwo:EducationalResource ;
    rdfs:label "Linked Data Engineering (openHPI Massive Open Online Course (MOOC))" ;
    dcterms:format "Academic teaching materials" ;
    mwo:description "We are surrounded by data everywhere. By helping us to make better decisions, data plays a central role in our daily lives. An ever increasing number of data sources, driven by individuals and organizations, contribute to this data deluge by sharing their data with others. However, data is locked up behind proprietary, unreliable, and even unstable programming interfaces that prevent us from optimally making use of it. Linked Data has the potential to revolutionize the way we discover, access, integrate, and use data; just in the way the World Wide Web has revolutionized the way we consume and connect documents. This course will introduce you to the basic principles and technologies of Linked Data to enable data sharing and reuse on a massive scale. Held together by ontologies, i.e. knowledge representations based on Semantic Web technologies, Linked Data serves as the central building block of the emerging Web of Data." ;
    mwo:hasLecturer <http://demo.fiz-karlsruhe.de/matwerk/E14862> ;
    mwo:hasWebsite <http://demo.fiz-karlsruhe.de/matwerk/E398387> ;
    mwo:isOnline true ;
    rdfs:comment "2016" ;
    ns1:duration "6 weeks"^^xsd:time .

<http://demo.fiz-karlsruhe.de/matwerk/E1245276> a mwo:EducationalResource ;
    rdfs:label "Semantic Web Technologies (open HPI Massive Open Online Course (MOOC))" ;
    dcterms:format "Academic teaching materials" ;
    mwo:description "In this course, you will learn the fundamentals of Semantic Web technologies and how they are applied for knowledge representation in the World Wide Web. You will learn how to represent knowledge with ontologies and how to access and benefit from semantic data on the Web. Furthermore, you will also learn how to make use of Linked Data and the Web of Data, currently the most popular applications based on Semantic Web technologies.",
        "In this course, you will learn the fundamentals of Semantic Web technologies. You will learn how to represent knowledge and how to access and benefit from semantic data on the Web." ;
    mwo:hasLecturer <http://demo.fiz-karlsruhe.de/matwerk/E14862> ;
    mwo:hasWebsite <http://demo.fiz-karlsruhe.de/matwerk/E399279>,
        <http://demo.fiz-karlsruhe.de/matwerk/E400172> ;
    mwo:isOnline true ;
    rdfs:comment "2013",
        "2014" ;
    ns1:duration "6 weeks"^^xsd:time .

<http://demo.fiz-karlsruhe.de/matwerk/E1245283> a mwo:EducationalResource ;
    rdfs:label "Pyiron YouTube channel" ;
    dcterms:format "Academic teaching materials" ;
    mwo:description "Welcome to our youtube channel where we present pyiron - an integrated development environment for computational materials science. " ;
    mwo:hasContributor <http://demo.fiz-karlsruhe.de/matwerk/E3416> ;
    mwo:hasWebsite <http://demo.fiz-karlsruhe.de/matwerk/E401066> ;
    mwo:isOnline true ;
    mwo:requiredTool <http://demo.fiz-karlsruhe.de/matwerk/E457491> .

<http://demo.fiz-karlsruhe.de/matwerk/E1245291> a mwo:EducationalResource ;
    rdfs:label "Materials Cloud Youtube channel" ;
    dcterms:format "Academic teaching materials" ;
    mwo:description "Tutorials and lectures on Materials Science, with focus on the AiiDA workflow manager (www.aiida.net) and the Materials Cloud open science platform (materialscloud.org)." ;
    mwo:hasContributor <http://demo.fiz-karlsruhe.de/matwerk/E7106>,
        <http://demo.fiz-karlsruhe.de/matwerk/E7107> ;
    mwo:hasWebsite <http://demo.fiz-karlsruhe.de/matwerk/E401961> ;
    mwo:requiredTool <http://demo.fiz-karlsruhe.de/matwerk/E1027029>,
        <http://demo.fiz-karlsruhe.de/matwerk/E1234236> .

<http://demo.fiz-karlsruhe.de/matwerk/E1245300> a mwo:EducationalResource ;
    rdfs:label "Workshop: From Electrons to Phase Diagrams" ;
    dcterms:format "Workshop" ;
    mwo:description "Jupyter notebooks and video recordings of the workshop. The three-day workshop focussed hands-on classes that cover the complete chain from high-throughput electronic structure calculations to the computation of phase diagrams. " ;
    mwo:hasContributor <http://demo.fiz-karlsruhe.de/matwerk/E1037>,
        <http://demo.fiz-karlsruhe.de/matwerk/E3416> ;
    mwo:hasLecturer <http://demo.fiz-karlsruhe.de/matwerk/E34671>,
        <http://demo.fiz-karlsruhe.de/matwerk/E34931>,
        <http://demo.fiz-karlsruhe.de/matwerk/E35192>,
        <http://demo.fiz-karlsruhe.de/matwerk/E35454>,
        <http://demo.fiz-karlsruhe.de/matwerk/E8627> ;
    mwo:hasWebsite <http://demo.fiz-karlsruhe.de/matwerk/E402857>,
        <http://demo.fiz-karlsruhe.de/matwerk/E408254> ;
    mwo:isOnline true ;
    mwo:requiredTool <http://demo.fiz-karlsruhe.de/matwerk/E1235807>,
        <http://demo.fiz-karlsruhe.de/matwerk/E1237379>,
        <http://demo.fiz-karlsruhe.de/matwerk/E1238952>,
        <http://demo.fiz-karlsruhe.de/matwerk/E1240526>,
        <http://demo.fiz-karlsruhe.de/matwerk/E457491>,
        <http://demo.fiz-karlsruhe.de/matwerk/E511556> ;
    rdfs:comment "2022" ;
    ns1:duration "13:00:00"^^xsd:time .

<http://demo.fiz-karlsruhe.de/matwerk/E1245310> a mwo:EducationalResource ;
    rdfs:label "Workshop: Software tools from Atomistics to Phase diagrams" ;
    dcterms:format "Workshop" ;
    mwo:description "Series of interactive tutorials explaining how to calculate thermodynamic properties with atomistic simulation using pyiron, an integrated development environment for complex simulation protocols." ;
    mwo:hasContributor <http://demo.fiz-karlsruhe.de/matwerk/E3416> ;
    mwo:hasLecturer <http://demo.fiz-karlsruhe.de/matwerk/E35717> ;
    mwo:hasWebsite <http://demo.fiz-karlsruhe.de/matwerk/E403754>,
        <http://demo.fiz-karlsruhe.de/matwerk/E409157> ;
    mwo:isOnline true ;
    mwo:requiredTool <http://demo.fiz-karlsruhe.de/matwerk/E1240526>,
        <http://demo.fiz-karlsruhe.de/matwerk/E1242101>,
        <http://demo.fiz-karlsruhe.de/matwerk/E457491> ;
    rdfs:comment "2020" ;
    ns1:duration "3 hrs plus exercises"^^xsd:time .

<http://demo.fiz-karlsruhe.de/matwerk/E1245321> a mwo:EducationalResource ;
    rdfs:label "Workshop: Workflows for atomistic simulations" ;
    dcterms:format "Workshop" ;
    mwo:description "Workshop lectures and videos from fitting of interatomic potentials to validating them." ;
    mwo:hasContributor <http://demo.fiz-karlsruhe.de/matwerk/E1037>,
        <http://demo.fiz-karlsruhe.de/matwerk/E3416> ;
    mwo:hasLecturer <http://demo.fiz-karlsruhe.de/matwerk/E35717> ;
    mwo:hasWebsite <http://demo.fiz-karlsruhe.de/matwerk/E404652>,
        <http://demo.fiz-karlsruhe.de/matwerk/E410061> ;
    mwo:isOnline true ;
    mwo:requiredTool <http://demo.fiz-karlsruhe.de/matwerk/E1240526>,
        <http://demo.fiz-karlsruhe.de/matwerk/E1242101>,
        <http://demo.fiz-karlsruhe.de/matwerk/E1243677>,
        <http://demo.fiz-karlsruhe.de/matwerk/E1245254>,
        <http://demo.fiz-karlsruhe.de/matwerk/E457491> ;
    rdfs:comment "2021" ;
    ns1:duration "Exercises"^^xsd:time .

<http://demo.fiz-karlsruhe.de/matwerk/E1245333> a mwo:EducationalResource ;
    rdfs:label "Workshop: Simulation workflows in materials modelling" ;
    dcterms:format "Workshop" ;
    mwo:description "As part of the workshop for Simulation Workflows in Materials Modelling we present a series of pyiron tutorials, starting from a basic introduction to Pyiron, followed by a focus session on up-scaling existing workflows and finally the implementation of new simulation codes and general open science activities of the pyiron project." ;
    mwo:hasContributor <http://demo.fiz-karlsruhe.de/matwerk/E3416> ;
    mwo:hasLecturer <http://demo.fiz-karlsruhe.de/matwerk/E35717> ;
    mwo:hasWebsite <http://demo.fiz-karlsruhe.de/matwerk/E405551>,
        <http://demo.fiz-karlsruhe.de/matwerk/E410966> ;
    mwo:isOnline true ;
    mwo:requiredTool <http://demo.fiz-karlsruhe.de/matwerk/E1240526>,
        <http://demo.fiz-karlsruhe.de/matwerk/E457491> ;
    rdfs:comment "2021" ;
    ns1:duration "Exercises"^^xsd:time .

<http://demo.fiz-karlsruhe.de/matwerk/E1245566> a nfdicore:Person ;
    rdfs:label "Mirza Mohtashim Alam" ;
    mwo:emailAddress "Mirza-Mohtashim.Alam@fiz-Karlsruhe.de"^^xsd:string ;
    mwo:hasAffiliation <http://demo.fiz-karlsruhe.de/matwerk/E1016> ;
    mwo:hasExpertiseIn <http://demo.fiz-karlsruhe.de/matwerk/E1245567>,
        <http://demo.fiz-karlsruhe.de/matwerk/E1245569>,
        <http://demo.fiz-karlsruhe.de/matwerk/E1245572>,
        <http://demo.fiz-karlsruhe.de/matwerk/E59654> ;
    mwo:hasORCID <https://orcid.org/0000-0002-7047-0791> ;
    foaf:firstName "Mirza Mohtashim"^^xsd:string ;
    foaf:surname "Alam"^^xsd:string .

<http://demo.fiz-karlsruhe.de/matwerk/E1245574> a nfdicore:Person ;
    rdfs:label "Msc Fei Chen" ;
    mwo:emailAddress "fei.chen@dfki.de"^^xsd:string ;
    mwo:hasAffiliation <http://demo.fiz-karlsruhe.de/matwerk/E1352> ;
    mwo:hasExpertiseIn <http://demo.fiz-karlsruhe.de/matwerk/E59654> ;
    mwo:hasORCID <https://orcid.org/0000-0001-7890-0330> ;
    foaf:firstName "Fei"^^xsd:string ;
    foaf:surname "Chen"^^xsd:string ;
    foaf:title "Msc"^^xsd:string .

<http://demo.fiz-karlsruhe.de/matwerk/E1246620> a nfdicore:Software,
        mwo:ComputationalWorkflow ;
    rdfs:label "Imprint Physical Size Estimation of Aluminum Elastic Modulus Images" ;
    nfdicore:fundingProject <http://demo.fiz-karlsruhe.de/matwerk/E1247022> ;
    nfdicore:programmingLanguage <http://demo.fiz-karlsruhe.de/matwerk/E1247517> ;
    dcterms:description "Workflow to measure the physical size of imprints in aluminum elastic modulus images"^^xsd:string ;
    mwo:hasContributor <http://demo.fiz-karlsruhe.de/matwerk/E1246243> ;
    mwo:hasDiscipline <http://demo.fiz-karlsruhe.de/matwerk/E1245665> ;
    mwo:hasFormat <http://demo.fiz-karlsruhe.de/matwerk/E1246252> ;
    mwo:hasRelatedResource <http://demo.fiz-karlsruhe.de/matwerk/E1247370> ;
    mwo:hasRepository <http://demo.fiz-karlsruhe.de/matwerk/E1246452> ;
    mwo:keyword "Aluminium",
        "Elastic Constants",
        "imprint estimation" ;
    mwo:usesMethod <http://demo.fiz-karlsruhe.de/matwerk/E1246945> ;
    ns3:SWO_0000082 <http://demo.fiz-karlsruhe.de/matwerk/E1246263>,
        <http://demo.fiz-karlsruhe.de/matwerk/E1246270>,
        <http://demo.fiz-karlsruhe.de/matwerk/E1246278>,
        <http://demo.fiz-karlsruhe.de/matwerk/E1246287>,
        <http://demo.fiz-karlsruhe.de/matwerk/E1246297>,
        <http://demo.fiz-karlsruhe.de/matwerk/E1246362> ;
    ns3:has_license <http://demo.fiz-karlsruhe.de/matwerk/E740937> ;
    schema:dateCreated "5/9/2023"^^xsd:time ;
    schema:datePublished "5/9/2023"^^xsd:time ;
    schema:operatingSystem ns3:SWO_0000022,
        ns3:SWO_0000149,
        ns3:SWO_9000072 .

<http://demo.fiz-karlsruhe.de/matwerk/E1246677> a nfdicore:Software,
        mwo:ComputationalWorkflow ;
    rdfs:label "APT analysis using CompositionSpace and pyiron" ;
    nfdicore:fundingProject <http://demo.fiz-karlsruhe.de/matwerk/E1247022> ;
    nfdicore:programmingLanguage <http://demo.fiz-karlsruhe.de/matwerk/E1247517> ;
    dcterms:description "Workflow to analyse APT data using CompositionSpace jobs implemented in pyiron"^^xsd:string ;
    mwo:hasContactPoint <http://demo.fiz-karlsruhe.de/matwerk/E1246245>,
        <http://demo.fiz-karlsruhe.de/matwerk/E8627> ;
    mwo:hasDiscipline <http://demo.fiz-karlsruhe.de/matwerk/E1245665> ;
    mwo:hasFormat <http://demo.fiz-karlsruhe.de/matwerk/E1246252> ;
    mwo:hasRelatedResource <http://demo.fiz-karlsruhe.de/matwerk/E1247467> ;
    mwo:hasRepository <http://demo.fiz-karlsruhe.de/matwerk/E1246495> ;
    mwo:keyword "Atom Probe Tomography",
        "Experiment",
        "Workflows" ;
    mwo:usesMethod <http://demo.fiz-karlsruhe.de/matwerk/E1246872> ;
    ns3:SWO_0000082 <http://demo.fiz-karlsruhe.de/matwerk/E1246362>,
        <http://demo.fiz-karlsruhe.de/matwerk/E1246567>,
        <http://demo.fiz-karlsruhe.de/matwerk/E457491> ;
    ns3:has_license <http://demo.fiz-karlsruhe.de/matwerk/E1246837> ;
    schema:dateCreated "6/16/2023"^^xsd:time ;
    schema:datePublished "6/16/2023"^^xsd:time ;
    schema:operatingSystem ns3:SWO_0000020,
        ns3:SWO_0000022,
        ns3:SWO_0000149 .

<http://demo.fiz-karlsruhe.de/matwerk/E1246707> a nfdicore:Software,
        mwo:ComputationalWorkflow ;
    rdfs:label "APT analysis using Paraprobe-toolbox and pyiron" ;
    nfdicore:fundingProject <http://demo.fiz-karlsruhe.de/matwerk/E1247022>,
        <http://demo.fiz-karlsruhe.de/matwerk/E1247062> ;
    nfdicore:programmingLanguage <http://demo.fiz-karlsruhe.de/matwerk/E1247517> ;
    dcterms:description "Workflow to analyse APT data using Paraprobe-toolbox jobs implemented in pyiron"^^xsd:string ;
    mwo:hasContactPoint <http://demo.fiz-karlsruhe.de/matwerk/E1246248>,
        <http://demo.fiz-karlsruhe.de/matwerk/E8627> ;
    mwo:hasDiscipline <http://demo.fiz-karlsruhe.de/matwerk/E1245665> ;
    mwo:hasFormat <http://demo.fiz-karlsruhe.de/matwerk/E1246252> ;
    mwo:hasRelatedResource <http://demo.fiz-karlsruhe.de/matwerk/E1247467> ;
    mwo:hasRepository <http://demo.fiz-karlsruhe.de/matwerk/E1246495> ;
    mwo:keyword "Atom Probe Tomography",
        "Experiment",
        "Workflows" ;
    mwo:usesMethod <http://demo.fiz-karlsruhe.de/matwerk/E1246872> ;
    ns3:SWO_0000082 <http://demo.fiz-karlsruhe.de/matwerk/E1246362>,
        <http://demo.fiz-karlsruhe.de/matwerk/E1246395>,
        <http://demo.fiz-karlsruhe.de/matwerk/E457491> ;
    ns3:has_license <http://demo.fiz-karlsruhe.de/matwerk/E1246837> ;
    schema:dateCreated "6/16/2023"^^xsd:time ;
    schema:datePublished "6/16/2023"^^xsd:time ;
    schema:operatingSystem ns3:SWO_0000020,
        ns3:SWO_0000022,
        ns3:SWO_0000149 .

<http://demo.fiz-karlsruhe.de/matwerk/E1247519> a modsci:Instrument ;
    rdfs:label "Fischerscope H100C" ;
    nfdicore:location <http://demo.fiz-karlsruhe.de/matwerk/E1247671> ;
    mwo:hasOwner <http://demo.fiz-karlsruhe.de/matwerk/E1247518> ;
    mwo:instrumentModel "H100C" ;
    mwo:usesTechnology <http://demo.fiz-karlsruhe.de/matwerk/E1247584> ;
    modsci:hasManufacturer <http://demo.fiz-karlsruhe.de/matwerk/E1247533> .

<http://demo.fiz-karlsruhe.de/matwerk/E1247521> a modsci:Instrument ;
    rdfs:label "LEXT 3D measuring laser microscope OLS4000" ;
    nfdicore:location <http://demo.fiz-karlsruhe.de/matwerk/E1247671> ;
    mwo:hasOwner <http://demo.fiz-karlsruhe.de/matwerk/E1247518> ;
    mwo:instrumentModel "OLS4000" ;
    mwo:usesTechnology <http://demo.fiz-karlsruhe.de/matwerk/E1247596> ;
    modsci:hasManufacturer <http://demo.fiz-karlsruhe.de/matwerk/E1247539> .

<http://demo.fiz-karlsruhe.de/matwerk/E1247524> a modsci:Instrument ;
    rdfs:label "Extensometer" ;
    nfdicore:location <http://demo.fiz-karlsruhe.de/matwerk/E4571> ;
    mwo:description "Displacement measurement during tensile testing" ;
    mwo:hasSerialNumber "8273P01,  8273P07,  964540049/-52, 964540043/-50" ;
    mwo:instrumentModel "two-sided LVDTs" ;
    mwo:usesTechnology <http://demo.fiz-karlsruhe.de/matwerk/E1247638> ;
    modsci:hasManufacturer <http://demo.fiz-karlsruhe.de/matwerk/E1247563> .

<http://demo.fiz-karlsruhe.de/matwerk/E1247528> a modsci:Instrument ;
    rdfs:label "Thermocouples" ;
    nfdicore:location <http://demo.fiz-karlsruhe.de/matwerk/E4571> ;
    mwo:description "Temperature calibration " ;
    mwo:hasSerialNumber "52-PM102-0063, 52-PM102-0064, 52-PM102-0065" ;
    mwo:instrumentModel "Typ S" ;
    mwo:usesTechnology <http://demo.fiz-karlsruhe.de/matwerk/E1247654> ;
    modsci:hasManufacturer <http://demo.fiz-karlsruhe.de/matwerk/E1247573> .

<http://demo.fiz-karlsruhe.de/matwerk/E12477> a nfdicore:Person ;
    rdfs:label "Prof. Hans-Georg  Herrmann" ;
    mwo:emailAddress "hans-georg.herrmann@izfp.fraunhofer.de"^^xsd:string ;
    mwo:hasAffiliation <http://demo.fiz-karlsruhe.de/matwerk/E1154> ;
    mwo:hasExpertiseIn <http://demo.fiz-karlsruhe.de/matwerk/E49206> ;
    mwo:hasORCID <https://orcid.org/0000-0003-3471-1516> ;
    owl:sameAs <http://www.wikidata.org/entity/Q111358897> ;
    foaf:firstName "Hans-Georg "^^xsd:string ;
    foaf:surname "Herrmann"^^xsd:string ;
    foaf:title "Prof."^^xsd:string .

<http://demo.fiz-karlsruhe.de/matwerk/E1247717> a nfdicore:Specification ;
    rdfs:label "NeXus-FAIRmat" ;
    nfdicore:relatedProject <http://demo.fiz-karlsruhe.de/matwerk/E1247062> ;
    mwo:description "NeXus expansion for FAIRmat data." ;
    mwo:hasDocumentation <http://demo.fiz-karlsruhe.de/matwerk/E1247678> ;
    mwo:hasRelatedResource <http://demo.fiz-karlsruhe.de/matwerk/E1160004> .

<http://demo.fiz-karlsruhe.de/matwerk/E1247738> a nfdicore:Specification ;
    rdfs:label "BAM Dataset: Creating FDO for MatWerk" ;
    nfdicore:relatedProject <http://demo.fiz-karlsruhe.de/matwerk/E1247022> ;
    mwo:description "JSON Schema description for BAM MatWerk project" ;
    mwo:hasAuthor <http://demo.fiz-karlsruhe.de/matwerk/E1247763> ;
    mwo:hasContactPoint <http://demo.fiz-karlsruhe.de/matwerk/E1247763> ;
    mwo:hasDiscipline <http://demo.fiz-karlsruhe.de/matwerk/E1245665> ;
    mwo:hasFormat <http://demo.fiz-karlsruhe.de/matwerk/E1247825> ;
    mwo:hasRepository <http://demo.fiz-karlsruhe.de/matwerk/E1247675> ;
    mwo:keyword "FAIR DO",
        "Metadata",
        "Schema" ;
    schema:dateCreated "7/15/2021"^^xsd:time .

<http://demo.fiz-karlsruhe.de/matwerk/E1247847> a nfdicore:Dataset ;
    rdfs:label "Radii of S-phase Al2CuMg in Al-alloy EN AW-2618A after different aging times at 190°C" ;
    nfdicore:fileExtension "pdf",
        "xlsx" ;
    nfdicore:objectType <http://demo.fiz-karlsruhe.de/matwerk/E1196832> ;
    mwo:aboutMaterial <http://demo.fiz-karlsruhe.de/matwerk/E1181417>,
        <http://demo.fiz-karlsruhe.de/matwerk/E1247845> ;
    mwo:description "The dataset contains data from quantitative microstructural analysis of transmission electron microscopy (TEM) studies of the S-phase (Al2CuMg) radii in Al-alloy EN AW 2618A. The investigated material and the applied methods were described in detail in two publications. Further information is provided in the file content.pdf." ;
    mwo:hasCreator <http://demo.fiz-karlsruhe.de/matwerk/E33132>,
        <http://demo.fiz-karlsruhe.de/matwerk/E9002> ;
    mwo:hasDiscipline <http://demo.fiz-karlsruhe.de/matwerk/E1247850> ;
    mwo:hasDocumentation <http://demo.fiz-karlsruhe.de/matwerk/E1247844> ;
    mwo:hasRepository <http://demo.fiz-karlsruhe.de/matwerk/E1247844> ;
    mwo:usesMethod <http://demo.fiz-karlsruhe.de/matwerk/E625404> ;
    ns3:has_license <http://demo.fiz-karlsruhe.de/matwerk/E817004> ;
    schema:datePublished "9/2/2023" .

<http://demo.fiz-karlsruhe.de/matwerk/E1248353> rdfs:label "Web-based demonstration and teaching framework for MSE research data infrastructure" ;
    mwo:mainTaskArea <http://demo.fiz-karlsruhe.de/matwerk/E1247886> ;
    mwo:relatedParticipantProject <http://demo.fiz-karlsruhe.de/matwerk/E1247947>,
        <http://demo.fiz-karlsruhe.de/matwerk/E1248100>,
        <http://demo.fiz-karlsruhe.de/matwerk/E1248118>,
        <http://demo.fiz-karlsruhe.de/matwerk/E1248157>,
        <http://demo.fiz-karlsruhe.de/matwerk/E1248325> ;
    mwo:relatedTaskArea <http://demo.fiz-karlsruhe.de/matwerk/E1247881>,
        <http://demo.fiz-karlsruhe.de/matwerk/E1247890> .

<http://demo.fiz-karlsruhe.de/matwerk/E1248382> rdfs:label "Framework for curation and distribution of reference datasets" ;
    mwo:mainTaskArea <http://demo.fiz-karlsruhe.de/matwerk/E1247881> ;
    mwo:relatedParticipantProject <http://demo.fiz-karlsruhe.de/matwerk/E1247962>,
        <http://demo.fiz-karlsruhe.de/matwerk/E1247968>,
        <http://demo.fiz-karlsruhe.de/matwerk/E1247975> ;
    mwo:relatedTaskArea <http://demo.fiz-karlsruhe.de/matwerk/E1247883>,
        <http://demo.fiz-karlsruhe.de/matwerk/E1247886>,
        <http://demo.fiz-karlsruhe.de/matwerk/E1247890> .

<http://demo.fiz-karlsruhe.de/matwerk/E1248412> rdfs:label "Storage concepts for large hierarchical datasets" ;
    mwo:mainTaskArea <http://demo.fiz-karlsruhe.de/matwerk/E1247881> ;
    mwo:relatedParticipantProject <http://demo.fiz-karlsruhe.de/matwerk/E1247983>,
        <http://demo.fiz-karlsruhe.de/matwerk/E1248178> ;
    mwo:relatedTaskArea <http://demo.fiz-karlsruhe.de/matwerk/E1247880>,
        <http://demo.fiz-karlsruhe.de/matwerk/E1247890> .

<http://demo.fiz-karlsruhe.de/matwerk/E1248443> rdfs:label "Model driven data space exploration" ;
    mwo:mainTaskArea <http://demo.fiz-karlsruhe.de/matwerk/E1247890> ;
    mwo:relatedParticipantProject <http://demo.fiz-karlsruhe.de/matwerk/E1248002>,
        <http://demo.fiz-karlsruhe.de/matwerk/E1248013> ;
    mwo:relatedTaskArea <http://demo.fiz-karlsruhe.de/matwerk/E1247883> .

<http://demo.fiz-karlsruhe.de/matwerk/E1248475> rdfs:label "Digital infrastructure and workflows for labs" ;
    mwo:mainTaskArea <http://demo.fiz-karlsruhe.de/matwerk/E1247890> ;
    mwo:relatedParticipantProject <http://demo.fiz-karlsruhe.de/matwerk/E1247947>,
        <http://demo.fiz-karlsruhe.de/matwerk/E1248002>,
        <http://demo.fiz-karlsruhe.de/matwerk/E1248100>,
        <http://demo.fiz-karlsruhe.de/matwerk/E1248178>,
        <http://demo.fiz-karlsruhe.de/matwerk/E1248247>,
        <http://demo.fiz-karlsruhe.de/matwerk/E1248272> ;
    mwo:relatedTaskArea <http://demo.fiz-karlsruhe.de/matwerk/E1247881> .

<http://demo.fiz-karlsruhe.de/matwerk/E1248508> rdfs:label "Integrating materials data from experiments and computation (ICME) into Industry 4.0 manufacturing paradigms" ;
    mwo:mainTaskArea <http://demo.fiz-karlsruhe.de/matwerk/E1247890> ;
    mwo:relatedParticipantProject <http://demo.fiz-karlsruhe.de/matwerk/E1247983>,
        <http://demo.fiz-karlsruhe.de/matwerk/E1248013>,
        <http://demo.fiz-karlsruhe.de/matwerk/E1248067>,
        <http://demo.fiz-karlsruhe.de/matwerk/E1248083>,
        <http://demo.fiz-karlsruhe.de/matwerk/E1248100>,
        <http://demo.fiz-karlsruhe.de/matwerk/E1248118> ;
    mwo:relatedTaskArea <http://demo.fiz-karlsruhe.de/matwerk/E1247881>,
        <http://demo.fiz-karlsruhe.de/matwerk/E1247883> .

<http://demo.fiz-karlsruhe.de/matwerk/E1248542> rdfs:label "Beyond 3D: Tools for tracking spatiotemporal microstructure evolution" ;
    mwo:mainTaskArea <http://demo.fiz-karlsruhe.de/matwerk/E1247890> ;
    mwo:relatedParticipantProject <http://demo.fiz-karlsruhe.de/matwerk/E1248137>,
        <http://demo.fiz-karlsruhe.de/matwerk/E1248157>,
        <http://demo.fiz-karlsruhe.de/matwerk/E1248178>,
        <http://demo.fiz-karlsruhe.de/matwerk/E1248200>,
        <http://demo.fiz-karlsruhe.de/matwerk/E1248223> ;
    mwo:relatedTaskArea <http://demo.fiz-karlsruhe.de/matwerk/E1247883>,
        <http://demo.fiz-karlsruhe.de/matwerk/E1247886> .

<http://demo.fiz-karlsruhe.de/matwerk/E1248577> rdfs:label "Interactive visual exploration for analyzing correlations in high dimensional materials data spaces" ;
    mwo:mainTaskArea <http://demo.fiz-karlsruhe.de/matwerk/E1247890> ;
    mwo:relatedParticipantProject <http://demo.fiz-karlsruhe.de/matwerk/E1247983>,
        <http://demo.fiz-karlsruhe.de/matwerk/E1248013>,
        <http://demo.fiz-karlsruhe.de/matwerk/E1248067>,
        <http://demo.fiz-karlsruhe.de/matwerk/E1248118>,
        <http://demo.fiz-karlsruhe.de/matwerk/E1248200>,
        <http://demo.fiz-karlsruhe.de/matwerk/E1248247>,
        <http://demo.fiz-karlsruhe.de/matwerk/E1248272> ;
    mwo:relatedTaskArea <http://demo.fiz-karlsruhe.de/matwerk/E1247883> .

<http://demo.fiz-karlsruhe.de/matwerk/E1248613> rdfs:label "Infrastructure interfaces with condensed matter physics (collaboration with FAIRmat)" ;
    mwo:mainTaskArea <http://demo.fiz-karlsruhe.de/matwerk/E1247890> ;
    mwo:relatedParticipantProject <http://demo.fiz-karlsruhe.de/matwerk/E1247962>,
        <http://demo.fiz-karlsruhe.de/matwerk/E1248002> ;
    mwo:relatedTaskArea <http://demo.fiz-karlsruhe.de/matwerk/E1247883> .

<http://demo.fiz-karlsruhe.de/matwerk/E1248650> rdfs:label "Interoperability of workflow systems (collaboration with NFDI4Ing)" ;
    mwo:mainTaskArea <http://demo.fiz-karlsruhe.de/matwerk/E1247890> ;
    mwo:relatedParticipantProject <http://demo.fiz-karlsruhe.de/matwerk/E1248137>,
        <http://demo.fiz-karlsruhe.de/matwerk/E1248200>,
        <http://demo.fiz-karlsruhe.de/matwerk/E1248223> ;
    mwo:relatedTaskArea <http://demo.fiz-karlsruhe.de/matwerk/E1247883>,
        <http://demo.fiz-karlsruhe.de/matwerk/E1247886> .

<http://demo.fiz-karlsruhe.de/matwerk/E1248688> rdfs:label "Development of coupled ontologies and workflows for thermochemical treatments" ;
    mwo:mainTaskArea <http://demo.fiz-karlsruhe.de/matwerk/E1247883> ;
    mwo:relatedParticipantProject <http://demo.fiz-karlsruhe.de/matwerk/E1248223>,
        <http://demo.fiz-karlsruhe.de/matwerk/E1248298> ;
    mwo:relatedTaskArea <http://demo.fiz-karlsruhe.de/matwerk/E1247890> .

<http://demo.fiz-karlsruhe.de/matwerk/E1248727> rdfs:label "Alignment of application- and higher-level ontologies" ;
    mwo:mainTaskArea <http://demo.fiz-karlsruhe.de/matwerk/E1247883> ;
    mwo:relatedParticipantProject <http://demo.fiz-karlsruhe.de/matwerk/E1247975>,
        <http://demo.fiz-karlsruhe.de/matwerk/E1248013>,
        <http://demo.fiz-karlsruhe.de/matwerk/E1248083>,
        <http://demo.fiz-karlsruhe.de/matwerk/E1248157>,
        <http://demo.fiz-karlsruhe.de/matwerk/E1248298> ;
    mwo:relatedTaskArea <http://demo.fiz-karlsruhe.de/matwerk/E1247880> .

<http://demo.fiz-karlsruhe.de/matwerk/E1248767> rdfs:label "Co-creation environment for experts" ;
    mwo:mainTaskArea <http://demo.fiz-karlsruhe.de/matwerk/E1247883> ;
    mwo:relatedParticipantProject <http://demo.fiz-karlsruhe.de/matwerk/E1248083>,
        <http://demo.fiz-karlsruhe.de/matwerk/E1248298>,
        <http://demo.fiz-karlsruhe.de/matwerk/E1248325> ;
    mwo:relatedTaskArea <http://demo.fiz-karlsruhe.de/matwerk/E1247890> .

<http://demo.fiz-karlsruhe.de/matwerk/E1248808> rdfs:label "Adaptive automated characterization pipelines and meta data schemas for high throughput experiments" ;
    mwo:mainTaskArea <http://demo.fiz-karlsruhe.de/matwerk/E1247883> ;
    mwo:relatedParticipantProject <http://demo.fiz-karlsruhe.de/matwerk/E1247962>,
        <http://demo.fiz-karlsruhe.de/matwerk/E1248067> ;
    mwo:relatedTaskArea <http://demo.fiz-karlsruhe.de/matwerk/E1247881>,
        <http://demo.fiz-karlsruhe.de/matwerk/E1247890> .

<http://demo.fiz-karlsruhe.de/matwerk/E1248850> rdfs:label "Method- and scale-bridging workflows and data structures for tomography" ;
    mwo:mainTaskArea <http://demo.fiz-karlsruhe.de/matwerk/E1247883> ;
    mwo:relatedParticipantProject <http://demo.fiz-karlsruhe.de/matwerk/E1248118>,
        <http://demo.fiz-karlsruhe.de/matwerk/E1248178> ;
    mwo:relatedTaskArea <http://demo.fiz-karlsruhe.de/matwerk/E1247886>,
        <http://demo.fiz-karlsruhe.de/matwerk/E1247890> .

<http://demo.fiz-karlsruhe.de/matwerk/E1248893> rdfs:label "Unified ontology for matrix-inclusion microstructure and composites" ;
    mwo:mainTaskArea <http://demo.fiz-karlsruhe.de/matwerk/E1247883> ;
    mwo:relatedParticipantProject <http://demo.fiz-karlsruhe.de/matwerk/E1247983>,
        <http://demo.fiz-karlsruhe.de/matwerk/E1248118> ;
    mwo:relatedTaskArea <http://demo.fiz-karlsruhe.de/matwerk/E1247881>,
        <http://demo.fiz-karlsruhe.de/matwerk/E1247890> .

<http://demo.fiz-karlsruhe.de/matwerk/E1248937> rdfs:label "Ontologies for defects in crystals" ;
    mwo:mainTaskArea <http://demo.fiz-karlsruhe.de/matwerk/E1247883> ;
    mwo:relatedParticipantProject <http://demo.fiz-karlsruhe.de/matwerk/E1247962>,
        <http://demo.fiz-karlsruhe.de/matwerk/E1247968>,
        <http://demo.fiz-karlsruhe.de/matwerk/E1248157>,
        <http://demo.fiz-karlsruhe.de/matwerk/E1248223> ;
    mwo:relatedTaskArea <http://demo.fiz-karlsruhe.de/matwerk/E1247886>,
        <http://demo.fiz-karlsruhe.de/matwerk/E1247890> .

<http://demo.fiz-karlsruhe.de/matwerk/E12629> a nfdicore:Person ;
    rdfs:label "PD Dr.  Franz  Roters" ;
    mwo:emailAddress "f.roters@mpie.de"^^xsd:string ;
    mwo:hasAffiliation <http://demo.fiz-karlsruhe.de/matwerk/E1001> ;
    mwo:hasExpertiseIn <http://demo.fiz-karlsruhe.de/matwerk/E49517>,
        <http://demo.fiz-karlsruhe.de/matwerk/E622056>,
        <http://demo.fiz-karlsruhe.de/matwerk/E65262> ;
    mwo:hasORCID <https://orcid.org/0000-0002-9098-9566> ;
    owl:sameAs <http://www.wikidata.org/entity/Q96103750> ;
    foaf:firstName "Franz "^^xsd:string ;
    foaf:surname "Roters"^^xsd:string ;
    foaf:title "PD Dr. "^^xsd:string .

<http://demo.fiz-karlsruhe.de/matwerk/E12782> a nfdicore:Person ;
    rdfs:label "Prof. Dr. Erica Lilleodden" ;
    mwo:emailAddress "erica.lilleodden@imws.fraunhofer.de"^^xsd:string ;
    mwo:hasAffiliation <http://demo.fiz-karlsruhe.de/matwerk/E1172> ;
    mwo:hasExpertiseIn <http://demo.fiz-karlsruhe.de/matwerk/E50142> ;
    mwo:hasORCID <https://orcid.org/0000-0002-4014-0986> ;
    owl:sameAs <http://www.wikidata.org/entity/Q111358936> ;
    foaf:depiction <https://ams3.digitaloceanspaces.com/externalpublic/57/a85ce9a5-d376-4ff3-bd68-96a0946e4ee0/conversions/34079649-d517-4fff-b111-b3e18b316098-md.jpg?X-Amz-Content-Sha256=UNSIGNED-PAYLOAD&X-Amz-Algorithm=AWS4-HMAC-SHA256&X-Amz-Credential=KVC4ZMO47JLTBHVHEFZ4%2F20230512%2Fams3%2Fs3%2Faws4_request&X-Amz-Date=20230512T150442Z&X-Amz-SignedHeaders=host&X-Amz-Expires=7200&X-Amz-Signature=953ece3eaf8d78b540257f64cef19e03e8dd3dcbd4537c4f5aa3f2119e2c61af> ;
    foaf:firstName "Erica"^^xsd:string ;
    foaf:surname "Lilleodden"^^xsd:string ;
    foaf:title "Prof. Dr."^^xsd:string .

<http://demo.fiz-karlsruhe.de/matwerk/E12936> a nfdicore:Person ;
    rdfs:label "Prof. Dr.-Ing.  Tilmann Beck" ;
    mwo:emailAddress "beck@mv.uni-kl.de"^^xsd:string ;
    mwo:hasAffiliation <http://demo.fiz-karlsruhe.de/matwerk/E1191> ;
    mwo:hasExpertiseIn <http://demo.fiz-karlsruhe.de/matwerk/E50456>,
        <http://demo.fiz-karlsruhe.de/matwerk/E50771>,
        <http://demo.fiz-karlsruhe.de/matwerk/E51087>,
        <http://demo.fiz-karlsruhe.de/matwerk/E65621> ;
    foaf:depiction <https://ams3.digitaloceanspaces.com/externalpublic/57/bd5a8a8d-0e4d-4e72-ba03-9914cd36a845/conversions/9c38505a-7fe9-4b8a-b4c6-f48969cb9f61-md.jpg?X-Amz-Content-Sha256=UNSIGNED-PAYLOAD&X-Amz-Algorithm=AWS4-HMAC-SHA256&X-Amz-Credential=KVC4ZMO47JLTBHVHEFZ4%2F20230512%2Fams3%2Fs3%2Faws4_request&X-Amz-Date=20230512T150442Z&X-Amz-SignedHeaders=host&X-Amz-Expires=7200&X-Amz-Signature=60361c5243596af44efc1c7524a4a22a620a7b72f5c2d3c54a421ff59b688be0> ;
    foaf:firstName "Tilmann"^^xsd:string ;
    foaf:surname "Beck"^^xsd:string ;
    foaf:title "Prof. Dr.-Ing. "^^xsd:string .

<http://demo.fiz-karlsruhe.de/matwerk/E13091> a nfdicore:Person ;
    rdfs:label "Prof. Dr.  Heike Leitte" ;
    mwo:emailAddress "leitte@cs.uni-kl.de"^^xsd:string ;
    mwo:hasAffiliation <http://demo.fiz-karlsruhe.de/matwerk/E1211> ;
    mwo:hasExpertiseIn <http://demo.fiz-karlsruhe.de/matwerk/E51404>,
        <http://demo.fiz-karlsruhe.de/matwerk/E51722>,
        <http://demo.fiz-karlsruhe.de/matwerk/E52041> ;
    mwo:hasORCID <https://orcid.org/0000-0002-7112-2190> ;
    owl:sameAs <http://www.wikidata.org/entity/Q89560401> ;
    foaf:firstName "Heike"^^xsd:string ;
    foaf:surname "Leitte"^^xsd:string ;
    foaf:title "Prof. Dr. "^^xsd:string .

<http://demo.fiz-karlsruhe.de/matwerk/E13247> a nfdicore:Person ;
    rdfs:label "Dr. Matthias Steinbacher" ;
    mwo:emailAddress "steinbacher@iwt-bremen.de"^^xsd:string ;
    mwo:hasAffiliation <http://demo.fiz-karlsruhe.de/matwerk/E1232> ;
    mwo:hasExpertiseIn <http://demo.fiz-karlsruhe.de/matwerk/E52361> ;
    mwo:hasORCID <https://orcid.org/0000-0003-4461-6539> ;
    owl:sameAs <http://www.wikidata.org/entity/Q89659331> ;
    foaf:firstName "Matthias"^^xsd:string ;
    foaf:surname "Steinbacher"^^xsd:string ;
    foaf:title "Dr."^^xsd:string .

<http://demo.fiz-karlsruhe.de/matwerk/E13404> a nfdicore:Person ;
    rdfs:label "Dr. Joachim  Meier" ;
    mwo:emailAddress "joachim.meier@ptb.de"^^xsd:string ;
    mwo:hasAffiliation <http://demo.fiz-karlsruhe.de/matwerk/E1254> ;
    foaf:firstName "Joachim "^^xsd:string ;
    foaf:surname "Meier"^^xsd:string ;
    foaf:title "Dr."^^xsd:string .

<http://demo.fiz-karlsruhe.de/matwerk/E13562> a nfdicore:Person ;
    rdfs:label "Prof. Dr.  Christoph Eberl" ;
    mwo:emailAddress "chris.eberl@iwm.fraunhofer.de"^^xsd:string ;
    mwo:hasAffiliation <http://demo.fiz-karlsruhe.de/matwerk/E1106> ;
    mwo:hasExpertiseIn <http://demo.fiz-karlsruhe.de/matwerk/E52682> ;
    mwo:hasORCID <https://orcid.org/0000-0001-9449-9583> ;
    owl:sameAs <http://www.wikidata.org/entity/Q98155960> ;
    foaf:depiction <https://ams3.digitaloceanspaces.com/externalpublic/57/74fc2cc4-9a89-4298-9b4c-79097af0dbe7/conversions/6d51c0a0-becc-4060-8c35-1021943e22be-md.jpg?X-Amz-Content-Sha256=UNSIGNED-PAYLOAD&X-Amz-Algorithm=AWS4-HMAC-SHA256&X-Amz-Credential=KVC4ZMO47JLTBHVHEFZ4%2F20230512%2Fams3%2Fs3%2Faws4_request&X-Amz-Date=20230512T150442Z&X-Amz-SignedHeaders=host&X-Amz-Expires=7200&X-Amz-Signature=fac28d1c91da919233adae3f177596b3689735ad3f5f743c0cddc1546113f79b> ;
    foaf:firstName "Christoph"^^xsd:string ;
    foaf:surname "Eberl"^^xsd:string ;
    foaf:title "Prof. Dr. "^^xsd:string .

<http://demo.fiz-karlsruhe.de/matwerk/E14042> a nfdicore:Person ;
    rdfs:label "Prof. Dr. Frank Mücklich" ;
    mwo:emailAddress "muecke@matsci.uni-sb.de"^^xsd:string ;
    mwo:hasAffiliation <http://demo.fiz-karlsruhe.de/matwerk/E1154> ;
    foaf:depiction <https://ams3.digitaloceanspaces.com/externalpublic/57/5386ddab-65ce-4f25-9aad-ee7d36d1d924/conversions/342ad2e8-ce70-442e-a5d7-603d25c96b0f-md.jpg?X-Amz-Content-Sha256=UNSIGNED-PAYLOAD&X-Amz-Algorithm=AWS4-HMAC-SHA256&X-Amz-Credential=KVC4ZMO47JLTBHVHEFZ4%2F20230512%2Fams3%2Fs3%2Faws4_request&X-Amz-Date=20230512T150442Z&X-Amz-SignedHeaders=host&X-Amz-Expires=7200&X-Amz-Signature=8e21a16ecb628470bc5100240653fbffacad9ec9908ea1caf063dfd63d7e25e2> ;
    foaf:firstName "Frank"^^xsd:string ;
    foaf:surname "Mücklich"^^xsd:string ;
    foaf:title "Prof. Dr."^^xsd:string .

<http://demo.fiz-karlsruhe.de/matwerk/E14204> a nfdicore:Person ;
    rdfs:label "Prof. Dr. Erik Bitzek" ;
    mwo:emailAddress "e.bitzek@mpie.de"^^xsd:string ;
    mwo:hasAffiliation <http://demo.fiz-karlsruhe.de/matwerk/E1001> ;
    mwo:hasExpertiseIn <http://demo.fiz-karlsruhe.de/matwerk/E1245805>,
        <http://demo.fiz-karlsruhe.de/matwerk/E1245827>,
        <http://demo.fiz-karlsruhe.de/matwerk/E1245850>,
        <http://demo.fiz-karlsruhe.de/matwerk/E1245874>,
        <http://demo.fiz-karlsruhe.de/matwerk/E1245899>,
        <http://demo.fiz-karlsruhe.de/matwerk/E65981> ;
    mwo:hasORCID <https://orcid.org/0000-0001-7430-3694> ;
    owl:sameAs <http://www.wikidata.org/entity/Q58569085> ;
    foaf:depiction <https://ams3.digitaloceanspaces.com/externalpublic/57/395b3869-8621-47ba-a4b3-0d5d51766a63/conversions/58de6ff0-6503-4ed2-9bb7-e905fbaff9c9-md.jpg?X-Amz-Content-Sha256=UNSIGNED-PAYLOAD&X-Amz-Algorithm=AWS4-HMAC-SHA256&X-Amz-Credential=KVC4ZMO47JLTBHVHEFZ4%2F20230512%2Fams3%2Fs3%2Faws4_request&X-Amz-Date=20230512T150442Z&X-Amz-SignedHeaders=host&X-Amz-Expires=7200&X-Amz-Signature=d14d93e2896992daccbe9494e0886aa97688cd97e1eb3f60965973de427138a1> ;
    foaf:firstName "Erik"^^xsd:string ;
    foaf:surname "Bitzek"^^xsd:string ;
    foaf:title "Prof. Dr."^^xsd:string .

<http://demo.fiz-karlsruhe.de/matwerk/E14367> a nfdicore:Person ;
    rdfs:label "Prof. Dr. Peter Gumbsch" ;
    mwo:emailAddress "peter.gumbsch@iwm.fraunhofer.de"^^xsd:string ;
    mwo:hasAffiliation <http://demo.fiz-karlsruhe.de/matwerk/E1106> ;
    mwo:hasExpertiseIn <http://demo.fiz-karlsruhe.de/matwerk/E1245925>,
        <http://demo.fiz-karlsruhe.de/matwerk/E54629> ;
    mwo:hasORCID <https://orcid.org/0000-0001-7995-228X> ;
    owl:sameAs <http://www.wikidata.org/entity/Q2075335> ;
    foaf:depiction <https://ams3.digitaloceanspaces.com/externalpublic/57/86de12dc-3c9c-4f30-aaee-52b0ac559127/conversions/e271c80f-41bb-4271-973f-dc12b4f265ec-md.jpg?X-Amz-Content-Sha256=UNSIGNED-PAYLOAD&X-Amz-Algorithm=AWS4-HMAC-SHA256&X-Amz-Credential=KVC4ZMO47JLTBHVHEFZ4%2F20230512%2Fams3%2Fs3%2Faws4_request&X-Amz-Date=20230512T150442Z&X-Amz-SignedHeaders=host&X-Amz-Expires=7200&X-Amz-Signature=841d2d4b32164149156f7d07b0a3b2f05f01a4180654417e58de8f308a04541a> ;
    foaf:firstName "Peter"^^xsd:string ;
    foaf:surname "Gumbsch"^^xsd:string ;
    foaf:title "Prof. Dr."^^xsd:string .

<http://demo.fiz-karlsruhe.de/matwerk/E14531> a nfdicore:Person ;
    rdfs:label "Dr. Tilmann Hickel" ;
    mwo:emailAddress "hickel@mpie.de"^^xsd:string ;
    mwo:hasAffiliation <http://demo.fiz-karlsruhe.de/matwerk/E1001>,
        <http://demo.fiz-karlsruhe.de/matwerk/E1245640> ;
    mwo:hasExpertiseIn <http://demo.fiz-karlsruhe.de/matwerk/E1245952>,
        <http://demo.fiz-karlsruhe.de/matwerk/E1245980>,
        <http://demo.fiz-karlsruhe.de/matwerk/E1246009>,
        <http://demo.fiz-karlsruhe.de/matwerk/E1246039>,
        <http://demo.fiz-karlsruhe.de/matwerk/E1246070>,
        <http://demo.fiz-karlsruhe.de/matwerk/E63836> ;
    mwo:hasORCID <https://orcid.org/0000-0003-0698-4891> ;
    owl:sameAs <http://www.wikidata.org/entity/Q45899344> ;
    foaf:depiction <https://ams3.digitaloceanspaces.com/externalpublic/57/eba635e9-6da7-4cd3-9c6a-3b796cc56d54/conversions/09d08d4f-63e7-4596-9568-bb3cb8d54cc5-md.jpg?X-Amz-Content-Sha256=UNSIGNED-PAYLOAD&X-Amz-Algorithm=AWS4-HMAC-SHA256&X-Amz-Credential=KVC4ZMO47JLTBHVHEFZ4%2F20230512%2Fams3%2Fs3%2Faws4_request&X-Amz-Date=20230512T150442Z&X-Amz-SignedHeaders=host&X-Amz-Expires=7200&X-Amz-Signature=e1ea74e8840a8384eccb8a8d2cbb0a6d3a54380de5d0228493ec31376cf83fc9> ;
    foaf:firstName "Tilmann"^^xsd:string ;
    foaf:surname "Hickel"^^xsd:string ;
    foaf:title "Dr."^^xsd:string .

<http://demo.fiz-karlsruhe.de/matwerk/E14696> a nfdicore:Person ;
    rdfs:label "Prof. Dr. Matthias S. Müller" ;
    mwo:emailAddress "mueller@itc.rwth-aachen.de"^^xsd:string ;
    mwo:hasAffiliation <http://demo.fiz-karlsruhe.de/matwerk/E1326> ;
    mwo:hasExpertiseIn <http://demo.fiz-karlsruhe.de/matwerk/E56946> ;
    foaf:depiction <https://ams3.digitaloceanspaces.com/externalpublic/57/93b34cee-702d-45ea-b5ee-d50baf9e957d/conversions/a2325573-76b0-4b99-ba40-fced0fdf02ac-md.jpg?X-Amz-Content-Sha256=UNSIGNED-PAYLOAD&X-Amz-Algorithm=AWS4-HMAC-SHA256&X-Amz-Credential=KVC4ZMO47JLTBHVHEFZ4%2F20230512%2Fams3%2Fs3%2Faws4_request&X-Amz-Date=20230512T150442Z&X-Amz-SignedHeaders=host&X-Amz-Expires=7200&X-Amz-Signature=6ee90a07c4ae5d54708df2539241f6e4b3833abba1cdf04f51b2979c1fb02476> ;
    foaf:firstName "Matthias S."^^xsd:string ;
    foaf:surname "Müller"^^xsd:string ;
    foaf:title "Prof. Dr."^^xsd:string .

<http://demo.fiz-karlsruhe.de/matwerk/E15029> a nfdicore:Person ;
    rdfs:label "Prof. Dr. Philipp Slusallek" ;
    mwo:emailAddress "slusallek@cg.uni-saarland.de"^^xsd:string ;
    mwo:hasAffiliation <http://demo.fiz-karlsruhe.de/matwerk/E1352> ;
    mwo:hasExpertiseIn <http://demo.fiz-karlsruhe.de/matwerk/E1246102>,
        <http://demo.fiz-karlsruhe.de/matwerk/E1246135>,
        <http://demo.fiz-karlsruhe.de/matwerk/E1246169>,
        <http://demo.fiz-karlsruhe.de/matwerk/E1246204>,
        <http://demo.fiz-karlsruhe.de/matwerk/E57954> ;
    mwo:hasORCID <https://orcid.org/0000-0002-2189-2429> ;
    owl:sameAs <http://www.wikidata.org/entity/Q20243272> ;
    foaf:depiction <https://ams3.digitaloceanspaces.com/externalpublic/57/c57b6729-806e-478a-9e60-fa2ebf62e0e4/conversions/15e2ad65-10d0-4ec2-8f29-0ffaeaf85b38-md.jpg?X-Amz-Content-Sha256=UNSIGNED-PAYLOAD&X-Amz-Algorithm=AWS4-HMAC-SHA256&X-Amz-Credential=KVC4ZMO47JLTBHVHEFZ4%2F20230512%2Fams3%2Fs3%2Faws4_request&X-Amz-Date=20230512T150442Z&X-Amz-SignedHeaders=host&X-Amz-Expires=7200&X-Amz-Signature=17f91e976078f4c52de33b67aab9e938bae1e1e67ccfc7c9fa011c6f854ca944> ;
    foaf:firstName "Philipp"^^xsd:string ;
    foaf:surname "Slusallek"^^xsd:string ;
    foaf:title "Prof. Dr."^^xsd:string .

<http://demo.fiz-karlsruhe.de/matwerk/E15197> a nfdicore:Person ;
    rdfs:label "Prof. Dr. Achim Streit" ;
    mwo:emailAddress "achim.streit@kit.edu"^^xsd:string ;
    mwo:hasAffiliation <http://demo.fiz-karlsruhe.de/matwerk/E1121> ;
    mwo:hasExpertiseIn <http://demo.fiz-karlsruhe.de/matwerk/E59654> ;
    mwo:hasORCID <https://orcid.org/0000-0002-5065-469X> ;
    owl:sameAs <http://www.wikidata.org/entity/Q111440065> ;
    foaf:depiction <https://ams3.digitaloceanspaces.com/externalpublic/57/fd2e9a3a-606e-412b-963d-82b08913e210/conversions/05dada8b-7cab-488c-92a5-3c804f7bcd54-md.jpg?X-Amz-Content-Sha256=UNSIGNED-PAYLOAD&X-Amz-Algorithm=AWS4-HMAC-SHA256&X-Amz-Credential=KVC4ZMO47JLTBHVHEFZ4%2F20230512%2Fams3%2Fs3%2Faws4_request&X-Amz-Date=20230512T150442Z&X-Amz-SignedHeaders=host&X-Amz-Expires=7200&X-Amz-Signature=e3c4bb2abaf895802b753dc8e9be4e4c68ffd72c905a526c1fa4162ca60f2568> ;
    foaf:firstName "Achim"^^xsd:string ;
    foaf:surname "Streit"^^xsd:string ;
    foaf:title "Prof. Dr."^^xsd:string .

<http://demo.fiz-karlsruhe.de/matwerk/E15366> a nfdicore:Person ;
    rdfs:label "Prof. Dr. Martina Zimmermann" ;
    mwo:emailAddress "martina.zimmermann@iws.fraunhofer.de"^^xsd:string ;
    mwo:hasAffiliation <http://demo.fiz-karlsruhe.de/matwerk/E1407> ;
    mwo:hasExpertiseIn <http://demo.fiz-karlsruhe.de/matwerk/E59997> ;
    foaf:depiction <https://ams3.digitaloceanspaces.com/externalpublic/57/09c805ec-ff80-4ccd-a662-c89c8dfaea38/conversions/564801df-764c-444d-84a6-d3a48749c5f3-md.jpg?X-Amz-Content-Sha256=UNSIGNED-PAYLOAD&X-Amz-Algorithm=AWS4-HMAC-SHA256&X-Amz-Credential=KVC4ZMO47JLTBHVHEFZ4%2F20230512%2Fams3%2Fs3%2Faws4_request&X-Amz-Date=20230512T150442Z&X-Amz-SignedHeaders=host&X-Amz-Expires=7200&X-Amz-Signature=0f65b149649c128df308c1b67341a1adddff212484dfd41ce71fdbca79407b5f> ;
    foaf:firstName "Martina"^^xsd:string ;
    foaf:surname "Zimmermann"^^xsd:string ;
    foaf:title "Prof. Dr."^^xsd:string .

<http://demo.fiz-karlsruhe.de/matwerk/E15536> a nfdicore:Person ;
    rdfs:label "Dr. Rainer Stotzka" ;
    mwo:emailAddress "rainer.stotzka@kit.edu"^^xsd:string ;
    mwo:hasAffiliation <http://demo.fiz-karlsruhe.de/matwerk/E1121> ;
    mwo:hasExpertiseIn <http://demo.fiz-karlsruhe.de/matwerk/E1245710>,
        <http://demo.fiz-karlsruhe.de/matwerk/E60341>,
        <http://demo.fiz-karlsruhe.de/matwerk/E66342> ;
    mwo:hasORCID <https://orcid.org/0000-0003-3642-1264> ;
    foaf:firstName "Rainer"^^xsd:string ;
    foaf:surname "Stotzka"^^xsd:string ;
    foaf:title "Dr."^^xsd:string .

<http://demo.fiz-karlsruhe.de/matwerk/E15707> a nfdicore:Person ;
    rdfs:label "Dr. Rossella Aversa" ;
    mwo:emailAddress "rossella.aversa@kit.edu"^^xsd:string ;
    mwo:hasAffiliation <http://demo.fiz-karlsruhe.de/matwerk/E1121> ;
    mwo:hasExpertiseIn <http://demo.fiz-karlsruhe.de/matwerk/E38402>,
        <http://demo.fiz-karlsruhe.de/matwerk/E66342> ;
    mwo:hasORCID <https://orcid.org/0000-0003-2534-0063> ;
    foaf:firstName "Rossella"^^xsd:string ;
    foaf:surname "Aversa"^^xsd:string ;
    foaf:title "Dr."^^xsd:string .

<http://demo.fiz-karlsruhe.de/matwerk/E15879> a nfdicore:Person ;
    rdfs:label "Ebrahim Norouzi" ;
    mwo:emailAddress "ebrahim.norouzi@fiz-karlsruhe.de"^^xsd:string ;
    mwo:hasAffiliation <http://demo.fiz-karlsruhe.de/matwerk/E1016> ;
    mwo:hasExpertiseIn <http://demo.fiz-karlsruhe.de/matwerk/E1245258>,
        <http://demo.fiz-karlsruhe.de/matwerk/E1246240> ;
    mwo:hasORCID <https://orcid.org/0000-0002-2691-6995> ;
    owl:sameAs <http://www.wikidata.org/entity/Q118232637> ;
    foaf:depiction <https://www.fiz-karlsruhe.de/sites/default/files/styles/contact_image/public/FIZ/Bilder/Personen/ebrahim-norouzi.jpg?itok=h0iFGsaA> ;
    foaf:firstName "Ebrahim"^^xsd:string ;
    foaf:surname "Norouzi"^^xsd:string .

<http://demo.fiz-karlsruhe.de/matwerk/E16052> a nfdicore:Person ;
    rdfs:label "Dr. Jörg Waitelonis" ;
    mwo:emailAddress "joerg.waitelonis@fiz-karlsruhe.de"^^xsd:string ;
    mwo:hasAffiliation <http://demo.fiz-karlsruhe.de/matwerk/E1016> ;
    mwo:hasExpertiseIn <http://demo.fiz-karlsruhe.de/matwerk/E1245258>,
        <http://demo.fiz-karlsruhe.de/matwerk/E59654> ;
    mwo:hasORCID <https://orcid.org/0000-0001-7192-7143> ;
    foaf:firstName "Jörg"^^xsd:string ;
    foaf:surname "Waitelonis"^^xsd:string ;
    foaf:title "Dr."^^xsd:string .

<http://demo.fiz-karlsruhe.de/matwerk/E18956> a nfdicore:Person ;
    rdfs:label "PD Dr. Steffen Brinckmann" ;
    mwo:hasAffiliation <http://demo.fiz-karlsruhe.de/matwerk/E1022> ;
    mwo:hasExpertiseIn <http://demo.fiz-karlsruhe.de/matwerk/E1245665>,
        <http://demo.fiz-karlsruhe.de/matwerk/E1245745>,
        <http://demo.fiz-karlsruhe.de/matwerk/E1245764> ;
    mwo:hasORCID <https://orcid.org/0000-0003-0930-082X> ;
    foaf:firstName "Steffen"^^xsd:string ;
    foaf:surname "Brinckmann"^^xsd:string ;
    foaf:title "PD Dr."^^xsd:string .

<http://demo.fiz-karlsruhe.de/matwerk/E38951> owl:sameAs <http://www.wikidata.org/entity/Q180160> .

<http://demo.fiz-karlsruhe.de/matwerk/E411872> a nfdicore:Software,
        mwo:ResearchSoftware ;
    rdfs:label "Calphy" ;
    nfdicore:fundingProject <http://demo.fiz-karlsruhe.de/matwerk/E1247022>,
        <http://demo.fiz-karlsruhe.de/matwerk/E851861> ;
    nfdicore:programmingLanguage <http://demo.fiz-karlsruhe.de/matwerk/E836279> ;
    dcterms:description "Python library and command line tool for calculation of free energies"^^xsd:string ;
    mwo:hasContactPoint <http://demo.fiz-karlsruhe.de/matwerk/E8627> ;
    mwo:hasContributor <http://demo.fiz-karlsruhe.de/matwerk/E3416> ;
    mwo:hasDiscipline <http://demo.fiz-karlsruhe.de/matwerk/E67431>,
        <http://demo.fiz-karlsruhe.de/matwerk/E70379> ;
    mwo:hasDocumentation <http://demo.fiz-karlsruhe.de/matwerk/E91952> ;
    mwo:hasRelatedResource <http://demo.fiz-karlsruhe.de/matwerk/E626522>,
        <http://demo.fiz-karlsruhe.de/matwerk/E627641>,
        <http://demo.fiz-karlsruhe.de/matwerk/E628761>,
        <http://demo.fiz-karlsruhe.de/matwerk/E629882> ;
    mwo:hasRepository <http://demo.fiz-karlsruhe.de/matwerk/E159204> ;
    mwo:hasVersion "1.1.4" ;
    mwo:hasWebsite <http://demo.fiz-karlsruhe.de/matwerk/E91952> ;
    mwo:usesMethod <http://demo.fiz-karlsruhe.de/matwerk/E616496>,
        <http://demo.fiz-karlsruhe.de/matwerk/E63482> ;
    ns3:has_license <http://demo.fiz-karlsruhe.de/matwerk/E738506> ;
    schema:citation <http://demo.fiz-karlsruhe.de/matwerk/E880802> ;
    schema:operatingSystem ns3:SWO_0000021,
        ns3:SWO_0000022 .

<http://demo.fiz-karlsruhe.de/matwerk/E412779> a nfdicore:Software,
        mwo:ComputationalWorkflow ;
    rdfs:label "Melting temperature computational workflow" ;
    nfdicore:fundingProject <http://demo.fiz-karlsruhe.de/matwerk/E1247022> ;
    dcterms:description "A repository illustrating the calculation of melting temperature through atomistic simulations using pyiron and calphy"^^xsd:string ;
    mwo:hasContactPoint <http://demo.fiz-karlsruhe.de/matwerk/E8627> ;
    mwo:hasContributor <http://demo.fiz-karlsruhe.de/matwerk/E3416> ;
    mwo:hasDiscipline <http://demo.fiz-karlsruhe.de/matwerk/E67431>,
        <http://demo.fiz-karlsruhe.de/matwerk/E70379> ;
    mwo:hasDocumentation <http://demo.fiz-karlsruhe.de/matwerk/E242861> ;
    mwo:hasRepository <http://demo.fiz-karlsruhe.de/matwerk/E159767> ;
    mwo:usesMethod <http://demo.fiz-karlsruhe.de/matwerk/E616496>,
        <http://demo.fiz-karlsruhe.de/matwerk/E63482> .

<http://demo.fiz-karlsruhe.de/matwerk/E413687> a nfdicore:Software,
        mwo:ProcessingSoftware,
        mwo:ResearchSoftware ;
    rdfs:label "Pyscal" ;
    nfdicore:programmingLanguage <http://demo.fiz-karlsruhe.de/matwerk/E828542>,
        <http://demo.fiz-karlsruhe.de/matwerk/E836279> ;
    dcterms:description "Python library written in C++ for calculation of local atomic structural environment"^^xsd:string ;
    mwo:hasContactPoint <http://demo.fiz-karlsruhe.de/matwerk/E8627> ;
    mwo:hasDiscipline <http://demo.fiz-karlsruhe.de/matwerk/E67431> ;
    mwo:hasDocumentation <http://demo.fiz-karlsruhe.de/matwerk/E92379> ;
    mwo:hasRelatedResource <http://demo.fiz-karlsruhe.de/matwerk/E631004>,
        <http://demo.fiz-karlsruhe.de/matwerk/E632127>,
        <http://demo.fiz-karlsruhe.de/matwerk/E633251>,
        <http://demo.fiz-karlsruhe.de/matwerk/E634376> ;
    mwo:hasRepository <http://demo.fiz-karlsruhe.de/matwerk/E160331> ;
    mwo:hasVersion "2.10.15" ;
    mwo:hasWebsite <http://demo.fiz-karlsruhe.de/matwerk/E92379> ;
    mwo:usesMethod <http://demo.fiz-karlsruhe.de/matwerk/E616496>,
        <http://demo.fiz-karlsruhe.de/matwerk/E63482> ;
    ns3:has_license <http://demo.fiz-karlsruhe.de/matwerk/E739721> ;
    schema:citation <http://demo.fiz-karlsruhe.de/matwerk/E882129> ;
    schema:operatingSystem ns3:SWO_0000021,
        ns3:SWO_0000022,
        ns3:SWO_9000072 .

<http://demo.fiz-karlsruhe.de/matwerk/E414596> a nfdicore:Software,
        mwo:ResearchSoftware ;
    rdfs:label "EQ2PC" ;
    nfdicore:programmingLanguage <http://demo.fiz-karlsruhe.de/matwerk/E836279> ;
    dcterms:description "A python script to implement the generation of discrete periodic structures with identical 2-point correlation."^^xsd:string ;
    mwo:hasContactPoint <http://demo.fiz-karlsruhe.de/matwerk/E16226> ;
    mwo:hasDiscipline <http://demo.fiz-karlsruhe.de/matwerk/E49517> ;
    mwo:hasDocumentation <http://demo.fiz-karlsruhe.de/matwerk/E243557> ;
    mwo:hasRepository <http://demo.fiz-karlsruhe.de/matwerk/E160896> ;
    schema:citation <http://demo.fiz-karlsruhe.de/matwerk/E883457> .

<http://demo.fiz-karlsruhe.de/matwerk/E415506> a nfdicore:Software,
        mwo:ResearchSoftware ;
    rdfs:label "MinimumEnergyPoints" ;
    nfdicore:fundingProject <http://demo.fiz-karlsruhe.de/matwerk/E853166>,
        <http://demo.fiz-karlsruhe.de/matwerk/E854472>,
        <http://demo.fiz-karlsruhe.de/matwerk/E855779> ;
    nfdicore:programmingLanguage <http://demo.fiz-karlsruhe.de/matwerk/E838866> ;
    dcterms:description "An algorithm implementing the minimum energy without nonlinear constraints. Distributes points on hyperspheres such that user-defined energy is minimized."^^xsd:string ;
    mwo:hasContactPoint <http://demo.fiz-karlsruhe.de/matwerk/E16401>,
        <http://demo.fiz-karlsruhe.de/matwerk/E16577> ;
    mwo:hasDiscipline <http://demo.fiz-karlsruhe.de/matwerk/E67067>,
        <http://demo.fiz-karlsruhe.de/matwerk/E67431> ;
    mwo:hasRepository <http://demo.fiz-karlsruhe.de/matwerk/E161462> ;
    ns3:has_license <http://demo.fiz-karlsruhe.de/matwerk/E740937> ;
    schema:citation <http://demo.fiz-karlsruhe.de/matwerk/E884786> .

<http://demo.fiz-karlsruhe.de/matwerk/E416417> a nfdicore:Software,
        mwo:ResearchSoftware ;
    rdfs:label "ConcentricInterpolation" ;
    nfdicore:fundingProject <http://demo.fiz-karlsruhe.de/matwerk/E857087> ;
    nfdicore:programmingLanguage <http://demo.fiz-karlsruhe.de/matwerk/E828542> ;
    dcterms:description "Interpolate and differentiate data in arbitrary dimensions efficiently in a concentric manner."^^xsd:string ;
    mwo:hasContactPoint <http://demo.fiz-karlsruhe.de/matwerk/E16401>,
        <http://demo.fiz-karlsruhe.de/matwerk/E16577> ;
    mwo:hasDiscipline <http://demo.fiz-karlsruhe.de/matwerk/E67067>,
        <http://demo.fiz-karlsruhe.de/matwerk/E67796> ;
    mwo:hasRepository <http://demo.fiz-karlsruhe.de/matwerk/E162029> ;
    ns3:has_license <http://demo.fiz-karlsruhe.de/matwerk/E1246803> ;
    schema:citation <http://demo.fiz-karlsruhe.de/matwerk/E884786>,
        <http://demo.fiz-karlsruhe.de/matwerk/E966356> .

<http://demo.fiz-karlsruhe.de/matwerk/E417329> a nfdicore:Software,
        mwo:ResearchSoftware ;
    rdfs:label "Image based prediction of the heat conduction tensor" ;
    nfdicore:fundingProject <http://demo.fiz-karlsruhe.de/matwerk/E857087> ;
    nfdicore:programmingLanguage <http://demo.fiz-karlsruhe.de/matwerk/E836279> ;
    dcterms:description "An open-source code providing a graphical user interface to predict the effective heat conductivity of microstructures and requires only the image data as input. The deployed methods are proposed and validated in the related paper, doi: 10.3390/mca24020057."^^xsd:string ;
    mwo:hasContactPoint <http://demo.fiz-karlsruhe.de/matwerk/E16577>,
        <http://demo.fiz-karlsruhe.de/matwerk/E16754> ;
    mwo:hasDiscipline <http://demo.fiz-karlsruhe.de/matwerk/E67431>,
        <http://demo.fiz-karlsruhe.de/matwerk/E68162> ;
    mwo:hasRepository <http://demo.fiz-karlsruhe.de/matwerk/E162597> ;
    mwo:usesMethod <http://demo.fiz-karlsruhe.de/matwerk/E609857> ;
    schema:citation <http://demo.fiz-karlsruhe.de/matwerk/E886116> .

<http://demo.fiz-karlsruhe.de/matwerk/E418242> a nfdicore:Software,
        mwo:ResearchSoftware ;
    rdfs:label "Finite Element Analysis Program" ;
    dcterms:description "A general purpose finite element analysis program which is designed for research and educational use."^^xsd:string ;
    mwo:hasAcronym "FEAP"^^xsd:string ;
    mwo:hasContactPoint <http://demo.fiz-karlsruhe.de/matwerk/E688379> ;
    mwo:hasDiscipline <http://demo.fiz-karlsruhe.de/matwerk/E67431> ;
    mwo:hasDocumentation <http://demo.fiz-karlsruhe.de/matwerk/E244254> ;
    mwo:hasVersion "8.6" ;
    mwo:hasWebsite <http://demo.fiz-karlsruhe.de/matwerk/E92807> ;
    mwo:usesMethod <http://demo.fiz-karlsruhe.de/matwerk/E610961> ;
    ns3:has_license <http://demo.fiz-karlsruhe.de/matwerk/E743372> ;
    schema:operatingSystem ns3:SWO_0000020,
        ns3:SWO_0000022,
        ns3:SWO_0000149,
        ns3:SWO_9000072 .

<http://demo.fiz-karlsruhe.de/matwerk/E420071> a nfdicore:Software,
        mwo:VisualizationSoftware ;
    rdfs:label "The Visualization Toolkit" ;
    dcterms:description "The Visualization Toolkit (VTK) is open source software for manipulating and displaying scientific data. It comes with state-of-the-art tools for 3D rendering, a suite of widgets for 3D interaction, and extensive 2D plotting capability."^^xsd:string ;
    mwo:hasAcronym "VTK"^^xsd:string ;
    mwo:hasContactPoint <http://demo.fiz-karlsruhe.de/matwerk/E689552> ;
    mwo:hasDiscipline <http://demo.fiz-karlsruhe.de/matwerk/E68897>,
        <http://demo.fiz-karlsruhe.de/matwerk/E70007> ;
    mwo:hasRelatedResource <http://demo.fiz-karlsruhe.de/matwerk/E419156> ;
    mwo:hasRepository <http://demo.fiz-karlsruhe.de/matwerk/E163736> ;
    mwo:hasVersion "9.2.0" ;
    mwo:hasWebsite <http://demo.fiz-karlsruhe.de/matwerk/E93666> ;
    ns3:has_license <http://demo.fiz-karlsruhe.de/matwerk/E745811> ;
    schema:citation <http://demo.fiz-karlsruhe.de/matwerk/E887447> .

<http://demo.fiz-karlsruhe.de/matwerk/E420987> a nfdicore:Software,
        mwo:ProcessingSoftware,
        mwo:ResearchSoftware,
        mwo:VisualizationSoftware ;
    rdfs:label "pyXIT" ;
    nfdicore:programmingLanguage <http://demo.fiz-karlsruhe.de/matwerk/E836279> ;
    dcterms:description "Volume Reconstrution Software for X-ray computed tomography data: reconstruction of set of 2D projections to a 3D volume based on mathematical algorithms"^^xsd:string ;
    mwo:hasDiscipline <http://demo.fiz-karlsruhe.de/matwerk/E69266>,
        <http://demo.fiz-karlsruhe.de/matwerk/E69636> ;
    mwo:hasVersion "1.1.5" ;
    mwo:hasWebsite <http://demo.fiz-karlsruhe.de/matwerk/E94097> ;
    mwo:usesMethod <http://demo.fiz-karlsruhe.de/matwerk/E612066> ;
    ns3:has_license <http://demo.fiz-karlsruhe.de/matwerk/E747032> .

<http://demo.fiz-karlsruhe.de/matwerk/E421904> a nfdicore:Software,
        mwo:ProcessingSoftware,
        mwo:ResearchSoftware,
        mwo:VisualizationSoftware ;
    rdfs:label "Avizo Software" ;
    dcterms:description "image data processing, visualization and analysis especially for 3D data sets like X-ray tomography"^^xsd:string ;
    mwo:hasDiscipline <http://demo.fiz-karlsruhe.de/matwerk/E69266>,
        <http://demo.fiz-karlsruhe.de/matwerk/E70007> ;
    mwo:hasVersion "2019.3" ;
    mwo:hasWebsite <http://demo.fiz-karlsruhe.de/matwerk/E94529> ;
    ns3:has_license <http://demo.fiz-karlsruhe.de/matwerk/E748254> .

<http://demo.fiz-karlsruhe.de/matwerk/E425582> a nfdicore:Software,
        mwo:ResearchSoftware ;
    rdfs:label "Vienna Ab initio Simulation Package" ;
    nfdicore:programmingLanguage <http://demo.fiz-karlsruhe.de/matwerk/E841457> ;
    dcterms:description "The Vienna Ab initio Simulation Package (VASP) is a computer program for atomic scale materials modelling, e.g. electronic structure calculations and quantum-mechanical molecular dynamics, from first principles."^^xsd:string ;
    mwo:hasAcronym "VASP"^^xsd:string ;
    mwo:hasContactPoint <http://demo.fiz-karlsruhe.de/matwerk/E690726> ;
    mwo:hasDiscipline <http://demo.fiz-karlsruhe.de/matwerk/E67431> ;
    mwo:hasDocumentation <http://demo.fiz-karlsruhe.de/matwerk/E246351> ;
    mwo:hasVersion "6.X" ;
    mwo:hasWebsite <http://demo.fiz-karlsruhe.de/matwerk/E96267> ;
    mwo:usesMethod <http://demo.fiz-karlsruhe.de/matwerk/E613172> ;
    ns3:has_license <http://demo.fiz-karlsruhe.de/matwerk/E753152> ;
    owl:sameAs <http://www.wikidata.org/entity/Q7928305> ;
    schema:citation <http://demo.fiz-karlsruhe.de/matwerk/E888779> .

<http://demo.fiz-karlsruhe.de/matwerk/E426504> a nfdicore:Software,
        mwo:ResearchSoftware ;
    rdfs:label "CAmbridge Serial Total Energy Package" ;
    dcterms:description "CASTEP is a full-featured materials modelling code based on a first-principles quantum mechanical description of electrons and nuclei. It uses the robust methods of a plane-wave basis set and pseudopotentials."^^xsd:string ;
    mwo:hasAcronym "CASTEP"^^xsd:string ;
    mwo:hasDiscipline <http://demo.fiz-karlsruhe.de/matwerk/E67431> ;
    mwo:hasDocumentation <http://demo.fiz-karlsruhe.de/matwerk/E247052> ;
    mwo:hasVersion "21.1.1" ;
    mwo:hasWebsite <http://demo.fiz-karlsruhe.de/matwerk/E96704> ;
    mwo:usesMethod <http://demo.fiz-karlsruhe.de/matwerk/E613172> ;
    ns3:has_license <http://demo.fiz-karlsruhe.de/matwerk/E753152> ;
    schema:citation <http://demo.fiz-karlsruhe.de/matwerk/E890112> .

<http://demo.fiz-karlsruhe.de/matwerk/E427427> a nfdicore:Software,
        mwo:ResearchSoftware ;
    rdfs:label "Carr Parrinello Molecular Dynamics" ;
    nfdicore:programmingLanguage <http://demo.fiz-karlsruhe.de/matwerk/E841457> ;
    dcterms:description "The CPMD code is a parallelized plane wave / pseudopotential implementation of Density Functional Theory, particularly designed for ab-initio molecular dynamics."^^xsd:string ;
    mwo:hasAcronym "CPMD"^^xsd:string ;
    mwo:hasDiscipline <http://demo.fiz-karlsruhe.de/matwerk/E67431> ;
    mwo:hasDocumentation <http://demo.fiz-karlsruhe.de/matwerk/E247754> ;
    mwo:hasWebsite <http://demo.fiz-karlsruhe.de/matwerk/E97142> ;
    mwo:usesMethod <http://demo.fiz-karlsruhe.de/matwerk/E613172> ;
    ns3:has_license <http://demo.fiz-karlsruhe.de/matwerk/E754379> ;
    schema:citation <http://demo.fiz-karlsruhe.de/matwerk/E891446> ;
    schema:operatingSystem ns3:SWO_0000022 .

<http://demo.fiz-karlsruhe.de/matwerk/E428351> a nfdicore:Software,
        mwo:ResearchSoftware ;
    rdfs:label "ABINIT" ;
    nfdicore:programmingLanguage <http://demo.fiz-karlsruhe.de/matwerk/E836279>,
        <http://demo.fiz-karlsruhe.de/matwerk/E841457> ;
    dcterms:description "ABINIT is a software suite to calculate the optical, mechanical, vibrational, and other observable properties of materials. Starting from the quantum equations of density functional theory, you can build up to advanced applications with perturbation theories based on DFT, and many-body Green's functions (GW and DMFT)"^^xsd:string ;
    mwo:hasContactPoint <http://demo.fiz-karlsruhe.de/matwerk/E691901> ;
    mwo:hasDiscipline <http://demo.fiz-karlsruhe.de/matwerk/E67431> ;
    mwo:hasDocumentation <http://demo.fiz-karlsruhe.de/matwerk/E248457> ;
    mwo:hasRepository <http://demo.fiz-karlsruhe.de/matwerk/E166026> ;
    mwo:hasVersion "9.6" ;
    mwo:hasWebsite <http://demo.fiz-karlsruhe.de/matwerk/E97581> ;
    mwo:usesMethod <http://demo.fiz-karlsruhe.de/matwerk/E613172> ;
    ns3:has_license <http://demo.fiz-karlsruhe.de/matwerk/E755607> ;
    owl:sameAs <http://www.wikidata.org/entity/Q4033170> ;
    schema:citation <http://demo.fiz-karlsruhe.de/matwerk/E892781> .

<http://demo.fiz-karlsruhe.de/matwerk/E429276> a nfdicore:Software,
        mwo:ResearchSoftware ;
    rdfs:label "BigDFT" ;
    dcterms:description "A fast, precise, and flexible DFT code for ab-initio atomistic simulation"^^xsd:string ;
    mwo:hasDiscipline <http://demo.fiz-karlsruhe.de/matwerk/E67431> ;
    mwo:hasRelatedResource <http://demo.fiz-karlsruhe.de/matwerk/E1234236>,
        <http://demo.fiz-karlsruhe.de/matwerk/E638886> ;
    mwo:hasRepository <http://demo.fiz-karlsruhe.de/matwerk/E166601> ;
    mwo:hasVersion "1.8.3" ;
    mwo:hasWebsite <http://demo.fiz-karlsruhe.de/matwerk/E98021> ;
    mwo:usesMethod <http://demo.fiz-karlsruhe.de/matwerk/E613172> ;
    ns3:has_license <http://demo.fiz-karlsruhe.de/matwerk/E755607> ;
    owl:sameAs <http://www.wikidata.org/entity/Q4904861> ;
    schema:citation <http://demo.fiz-karlsruhe.de/matwerk/E894117> .

<http://demo.fiz-karlsruhe.de/matwerk/E431129> a nfdicore:Software,
        mwo:ResearchSoftware ;
    rdfs:label "Parallel total energy" ;
    dcterms:description "It is a parallel plane wave pseudopotential program for atomistic total energy calculation based on density functional theory. It is designed for large system simulations to be run on large parallel computers like IBM SP machines at NERSC, and linux cluster machines. "^^xsd:string ;
    mwo:hasAcronym "PEtot"^^xsd:string ;
    mwo:hasDiscipline <http://demo.fiz-karlsruhe.de/matwerk/E67431> ;
    mwo:hasVersion "3" ;
    mwo:hasWebsite <http://demo.fiz-karlsruhe.de/matwerk/E98904> ;
    mwo:usesMethod <http://demo.fiz-karlsruhe.de/matwerk/E613172> ;
    ns3:has_license <http://demo.fiz-karlsruhe.de/matwerk/E756836> .

<http://demo.fiz-karlsruhe.de/matwerk/E432057> a nfdicore:Software,
        mwo:ResearchSoftware ;
    rdfs:label "JDTFx" ;
    dcterms:description "JDFTx is a plane-wave density-functional theory (DFT) code designed to be as easy to develop with as it is easy to use. "^^xsd:string ;
    mwo:hasDiscipline <http://demo.fiz-karlsruhe.de/matwerk/E67431> ;
    mwo:hasDocumentation <http://demo.fiz-karlsruhe.de/matwerk/E249866> ;
    mwo:hasRepository <http://demo.fiz-karlsruhe.de/matwerk/E167754> ;
    mwo:hasVersion "1.7.0" ;
    mwo:hasWebsite <http://demo.fiz-karlsruhe.de/matwerk/E99347> ;
    mwo:usesMethod <http://demo.fiz-karlsruhe.de/matwerk/E613172> ;
    ns3:has_license <http://demo.fiz-karlsruhe.de/matwerk/E755607> ;
    schema:citation <http://demo.fiz-karlsruhe.de/matwerk/E896792> .

<http://demo.fiz-karlsruhe.de/matwerk/E432986> a nfdicore:Software,
        mwo:ResearchSoftware ;
    rdfs:label "PARSEC" ;
    dcterms:description "PARSEC is a computer code that solves the Kohn-Sham equations by expressing electron wave-functions directly in real space, without the use of explicit basis sets. It uses norm-conserving pseudopotentials (Troullier-Martins and other varieties). It is designed for ab initio quantum-mechanical calculations of the electronic structure of matter, within density-functional theory."^^xsd:string ;
    mwo:hasDiscipline <http://demo.fiz-karlsruhe.de/matwerk/E67431> ;
    mwo:hasRepository <http://demo.fiz-karlsruhe.de/matwerk/E168332> ;
    mwo:hasVersion "1.4" ;
    mwo:hasWebsite <http://demo.fiz-karlsruhe.de/matwerk/E99791> ;
    mwo:usesMethod <http://demo.fiz-karlsruhe.de/matwerk/E613172> ;
    ns3:has_license <http://demo.fiz-karlsruhe.de/matwerk/E755607> ;
    owl:sameAs <http://www.wikidata.org/entity/Q7118228> ;
    schema:citation <http://demo.fiz-karlsruhe.de/matwerk/E898131> .

<http://demo.fiz-karlsruhe.de/matwerk/E433916> a nfdicore:Software,
        mwo:ResearchSoftware ;
    rdfs:label "CP2K" ;
    nfdicore:programmingLanguage <http://demo.fiz-karlsruhe.de/matwerk/E836279>,
        <http://demo.fiz-karlsruhe.de/matwerk/E841457> ;
    dcterms:description "CP2K is a quantum chemistry and solid state physics software package that can perform atomistic simulations of solid state, liquid, molecular, periodic, material, crystal, and biological systems. CP2K provides a general framework for different modeling methods such as DFT using the mixed Gaussian and plane waves approaches GPW and GAPW. Supported theory levels include DFTB, LDA, GGA, MP2, RPA, semi-empirical methods (AM1, PM3, PM6, RM1, MNDO, …), and classical force fields (AMBER, CHARMM, …). CP2K can do simulations of molecular dynamics, metadynamics, Monte Carlo, Ehrenfest dynamics, vibrational analysis, core level spectroscopy, energy minimization, and transition state optimization using NEB or dimer method."^^xsd:string ;
    mwo:hasDiscipline <http://demo.fiz-karlsruhe.de/matwerk/E67431> ;
    mwo:hasDocumentation <http://demo.fiz-karlsruhe.de/matwerk/E250572> ;
    mwo:hasRepository <http://demo.fiz-karlsruhe.de/matwerk/E168911> ;
    mwo:hasVersion "9.1" ;
    mwo:hasWebsite <http://demo.fiz-karlsruhe.de/matwerk/E100236> ;
    mwo:usesMethod <http://demo.fiz-karlsruhe.de/matwerk/E613172>,
        <http://demo.fiz-karlsruhe.de/matwerk/E614279>,
        <http://demo.fiz-karlsruhe.de/matwerk/E615387>,
        <http://demo.fiz-karlsruhe.de/matwerk/E616496>,
        <http://demo.fiz-karlsruhe.de/matwerk/E617606>,
        <http://demo.fiz-karlsruhe.de/matwerk/E618717>,
        <http://demo.fiz-karlsruhe.de/matwerk/E619829>,
        <http://demo.fiz-karlsruhe.de/matwerk/E63482> ;
    ns3:has_license <http://demo.fiz-karlsruhe.de/matwerk/E755607> ;
    owl:sameAs <http://www.wikidata.org/entity/Q5013592> .

<http://demo.fiz-karlsruhe.de/matwerk/E434847> a nfdicore:Software,
        mwo:ResearchSoftware ;
    rdfs:label "GPAW" ;
    nfdicore:programmingLanguage <http://demo.fiz-karlsruhe.de/matwerk/E836279> ;
    dcterms:description "GPAW is a density-functional theory (DFT) Python code based on the projector-augmented wave (PAW) method and the atomic simulation environment (ASE). "^^xsd:string ;
    mwo:hasDiscipline <http://demo.fiz-karlsruhe.de/matwerk/E67431> ;
    mwo:hasDocumentation <http://demo.fiz-karlsruhe.de/matwerk/E251279> ;
    mwo:hasRelatedResource <http://demo.fiz-karlsruhe.de/matwerk/E641147> ;
    mwo:hasRepository <http://demo.fiz-karlsruhe.de/matwerk/E169491> ;
    mwo:hasVersion "22.1" ;
    mwo:hasWebsite <http://demo.fiz-karlsruhe.de/matwerk/E100682> ;
    mwo:usesMethod <http://demo.fiz-karlsruhe.de/matwerk/E613172> ;
    ns3:has_license <http://demo.fiz-karlsruhe.de/matwerk/E755607> ;
    schema:citation <http://demo.fiz-karlsruhe.de/matwerk/E899471> .

<http://demo.fiz-karlsruhe.de/matwerk/E435779> a nfdicore:Software,
        mwo:ResearchSoftware ;
    rdfs:label "S/PHI/nX" ;
    dcterms:description "S/PHI/nX is a C++ library for materials simulation, mostly electronic-structure theory. It also is a program (sphinx) to perform such simulations using density-functional theory, and k.p theory. In addition, the package offers dozens of specialized programs (add-ons) for smaller tasks related to setup, analysis, post-processing, and other types of simulations."^^xsd:string ;
    mwo:hasAcronym "SPHINX"^^xsd:string ;
    mwo:hasContactPoint <http://demo.fiz-karlsruhe.de/matwerk/E18579> ;
    mwo:hasContributor <http://demo.fiz-karlsruhe.de/matwerk/E3416> ;
    mwo:hasDiscipline <http://demo.fiz-karlsruhe.de/matwerk/E67431> ;
    mwo:hasRepository <http://demo.fiz-karlsruhe.de/matwerk/E170072> ;
    mwo:hasVersion "3.0.9" ;
    mwo:hasWebsite <http://demo.fiz-karlsruhe.de/matwerk/E101129> ;
    mwo:usesMethod <http://demo.fiz-karlsruhe.de/matwerk/E613172> ;
    ns3:has_license <http://demo.fiz-karlsruhe.de/matwerk/E758066> .

<http://demo.fiz-karlsruhe.de/matwerk/E436712> a nfdicore:Software,
        mwo:ResearchSoftware ;
    rdfs:label "Qbox First-Principles Molecular Dynamics" ;
    nfdicore:programmingLanguage <http://demo.fiz-karlsruhe.de/matwerk/E828542> ;
    dcterms:description """Qbox is a C++/MPI scalable parallel implementation of first-principles molecular dynamics (FPMD) based on the plane-wave, pseudopotential formalism. Qbox is designed for operation on large parallel computers.\r
\r
"""^^xsd:string ;
    mwo:hasDiscipline <http://demo.fiz-karlsruhe.de/matwerk/E67431> ;
    mwo:hasDocumentation <http://demo.fiz-karlsruhe.de/matwerk/E251987> ;
    mwo:hasRepository <http://demo.fiz-karlsruhe.de/matwerk/E170654> ;
    mwo:hasVersion "1.74.4" ;
    mwo:hasWebsite <http://demo.fiz-karlsruhe.de/matwerk/E101577> ;
    mwo:usesMethod <http://demo.fiz-karlsruhe.de/matwerk/E613172> ;
    ns3:has_license <http://demo.fiz-karlsruhe.de/matwerk/E755607> .

<http://demo.fiz-karlsruhe.de/matwerk/E437646> a nfdicore:Software,
        mwo:ResearchSoftware ;
    rdfs:label "DFTK.jl" ;
    nfdicore:programmingLanguage <http://demo.fiz-karlsruhe.de/matwerk/E842754> ;
    dcterms:description "The density-functional toolkit, DFTK for short, is a library of Julia routines for playing with plane-wave density-functional theory (DFT) algorithms. In its basic formulation it solves periodic Kohn-Sham equations. The unique feature of the code is its emphasis on simplicity and flexibility with the goal of facilitating methodological development and interdisciplinary collaboration. "^^xsd:string ;
    mwo:hasDiscipline <http://demo.fiz-karlsruhe.de/matwerk/E67431> ;
    mwo:hasDocumentation <http://demo.fiz-karlsruhe.de/matwerk/E102026> ;
    mwo:hasRepository <http://demo.fiz-karlsruhe.de/matwerk/E171237> ;
    mwo:hasVersion "0.5" ;
    mwo:hasWebsite <http://demo.fiz-karlsruhe.de/matwerk/E102026> ;
    mwo:usesMethod <http://demo.fiz-karlsruhe.de/matwerk/E613172> ;
    ns3:has_license <http://demo.fiz-karlsruhe.de/matwerk/E759297> ;
    schema:citation <http://demo.fiz-karlsruhe.de/matwerk/E900812> .

<http://demo.fiz-karlsruhe.de/matwerk/E438581> a nfdicore:Software,
        mwo:ResearchSoftware ;
    rdfs:label "density of Montréal" ;
    dcterms:description "deMon (density of Montréal) is a software package for density functional theory (DFT) calculations. It uses the linear combination of Gaussian-type orbital (LCGTO) approach for the self-consistent solution of the Kohn-Sham (KS) DFT equations. The calculation of the four-center electron repulsion integrals is avoided by introducing an auxiliary function basis for the variational fitting of the Coulomb potential. "^^xsd:string ;
    mwo:hasAcronym "deMon2k"^^xsd:string ;
    mwo:hasContactPoint <http://demo.fiz-karlsruhe.de/matwerk/E695432> ;
    mwo:hasDiscipline <http://demo.fiz-karlsruhe.de/matwerk/E67431> ;
    mwo:hasVersion "5" ;
    mwo:hasWebsite <http://demo.fiz-karlsruhe.de/matwerk/E102476> ;
    mwo:usesMethod <http://demo.fiz-karlsruhe.de/matwerk/E613172> .

<http://demo.fiz-karlsruhe.de/matwerk/E439517> a nfdicore:Software,
        mwo:ResearchSoftware ;
    rdfs:label "SIESTA" ;
    dcterms:description "SIESTA is both a method and its computer program implementation, to perform efficient electronic structure calculations and ab initio molecular dynamics simulations of molecules and solids. SIESTA's efficiency stems from the use of a basis set of strictly-localized atomic orbitals. A very important feature of the code is that its accuracy and cost can be tuned in a wide range, from quick exploratory calculations to highly accurate simulations matching the quality of other approaches, such as plane-wave methods."^^xsd:string ;
    mwo:hasDiscipline <http://demo.fiz-karlsruhe.de/matwerk/E67431> ;
    mwo:hasDocumentation <http://demo.fiz-karlsruhe.de/matwerk/E252696> ;
    mwo:hasRepository <http://demo.fiz-karlsruhe.de/matwerk/E171821> ;
    mwo:hasVersion "4" ;
    mwo:hasWebsite <http://demo.fiz-karlsruhe.de/matwerk/E102927> ;
    mwo:usesMethod <http://demo.fiz-karlsruhe.de/matwerk/E613172> ;
    ns3:has_license <http://demo.fiz-karlsruhe.de/matwerk/E755607> ;
    owl:sameAs <http://www.wikidata.org/entity/Q7390304> ;
    schema:citation <http://demo.fiz-karlsruhe.de/matwerk/E902154> .

<http://demo.fiz-karlsruhe.de/matwerk/E440454> a nfdicore:Software,
        mwo:ResearchSoftware ;
    rdfs:label "CRYSTAL" ;
    dcterms:description """The CRYSTAL package performs ab initio calculations of the ground state energy, energy\r
gradient, electronic wave function and properties of periodic systems. Hartree-Fock or KohnSham Hamiltonians (that adopt an Exchange-Correlation potential following the postulates of\r
Density-Functional Theory) can be used. """^^xsd:string ;
    mwo:hasAcronym "CRYSTAL17"^^xsd:string ;
    mwo:hasDiscipline <http://demo.fiz-karlsruhe.de/matwerk/E67431> ;
    mwo:hasVersion "1.0.2" ;
    mwo:hasWebsite <http://demo.fiz-karlsruhe.de/matwerk/E103379> ;
    mwo:usesMethod <http://demo.fiz-karlsruhe.de/matwerk/E613172> ;
    ns3:has_license <http://demo.fiz-karlsruhe.de/matwerk/E760529> ;
    owl:sameAs <http://www.wikidata.org/entity/Q3648912> ;
    schema:citation <http://demo.fiz-karlsruhe.de/matwerk/E903497> ;
    schema:operatingSystem ns3:SWO_0000020,
        ns3:SWO_0000022,
        ns3:SWO_0000149,
        ns3:SWO_9000072 .

<http://demo.fiz-karlsruhe.de/matwerk/E441392> a nfdicore:Software,
        mwo:ResearchSoftware ;
    rdfs:label "FHI-AIMS" ;
    dcterms:description "FHI-aims is an all-electron electronic structure code based on numeric atom-centered orbitals. It enables first-principles simulations with very high numerical accuracy for production calculations, with excellent scalability up to very large system sizes (thousands of atoms) and up to very large, massively parallel supercomputers (ten thousand CPU cores)."^^xsd:string ;
    mwo:hasContactPoint <http://demo.fiz-karlsruhe.de/matwerk/E696611> ;
    mwo:hasDiscipline <http://demo.fiz-karlsruhe.de/matwerk/E67431> ;
    mwo:hasWebsite <http://demo.fiz-karlsruhe.de/matwerk/E103832> ;
    mwo:usesMethod <http://demo.fiz-karlsruhe.de/matwerk/E613172> ;
    ns3:has_license <http://demo.fiz-karlsruhe.de/matwerk/E760529> .

<http://demo.fiz-karlsruhe.de/matwerk/E442331> a nfdicore:Software,
        mwo:ResearchSoftware ;
    rdfs:label "FPLO" ;
    dcterms:description "The FPLO® package is a full-potential local-orbital code to solve the Kohn-Sham equations on a regular lattice or with free boundary conditions (finite systems). Relativistic effects are treated either in a scalar-relativistic or a full 4-component formalism. Available functionals are LSDA, GGA (PBE 96) and LSDA/GGA+U. "^^xsd:string ;
    mwo:hasContactPoint <http://demo.fiz-karlsruhe.de/matwerk/E17111> ;
    mwo:hasDiscipline <http://demo.fiz-karlsruhe.de/matwerk/E67431> ;
    mwo:hasVersion "22" ;
    mwo:hasWebsite <http://demo.fiz-karlsruhe.de/matwerk/E104286> ;
    mwo:usesMethod <http://demo.fiz-karlsruhe.de/matwerk/E613172> ;
    ns3:has_license <http://demo.fiz-karlsruhe.de/matwerk/E761762> ;
    schema:citation <http://demo.fiz-karlsruhe.de/matwerk/E904841> .

<http://demo.fiz-karlsruhe.de/matwerk/E443271> a nfdicore:Software,
        mwo:ResearchSoftware ;
    rdfs:label "Open source package for Material eXplorer" ;
    dcterms:description "OpenMX (Open source package for Material eXplorer) is a software package for nano-scale material simulations based on density functional theories (DFT), norm-conserving pseudopotentials, and pseudo-atomic localized basis functions . The methods and algorithms used in OpenMX and their implementation are carefully designed for the realization of large-scale ab initio electronic structure calculations on parallel computers based on the MPI or MPI/OpenMP hybrid parallelism. "^^xsd:string ;
    mwo:hasAcronym "OpenMX"^^xsd:string ;
    mwo:hasDiscipline <http://demo.fiz-karlsruhe.de/matwerk/E67431> ;
    mwo:hasDocumentation <http://demo.fiz-karlsruhe.de/matwerk/E253406> ;
    mwo:hasVersion "3.9.9" ;
    mwo:hasWebsite <http://demo.fiz-karlsruhe.de/matwerk/E104741> ;
    mwo:usesMethod <http://demo.fiz-karlsruhe.de/matwerk/E613172> ;
    ns3:has_license <http://demo.fiz-karlsruhe.de/matwerk/E762996> .

<http://demo.fiz-karlsruhe.de/matwerk/E444212> a nfdicore:Software,
        mwo:ResearchSoftware ;
    rdfs:label "Elk" ;
    dcterms:description "An all-electron full-potential linearised augmented-plane wave (LAPW) code with many advanced features. Written originally at Karl-Franzens-Universität Graz as a milestone of the EXCITING EU Research and Training Network, the code is designed to be as simple as possible so that new developments in the field of density functional theory (DFT) can be added quickly and reliably. "^^xsd:string ;
    mwo:hasDiscipline <http://demo.fiz-karlsruhe.de/matwerk/E67431> ;
    mwo:hasDocumentation <http://demo.fiz-karlsruhe.de/matwerk/E254117> ;
    mwo:hasVersion "8.5.2" ;
    mwo:hasWebsite <http://demo.fiz-karlsruhe.de/matwerk/E105197> ;
    mwo:usesMethod <http://demo.fiz-karlsruhe.de/matwerk/E613172> ;
    ns3:has_license <http://demo.fiz-karlsruhe.de/matwerk/E755607> ;
    owl:sameAs <http://www.wikidata.org/entity/Q114833975> .

<http://demo.fiz-karlsruhe.de/matwerk/E445154> a nfdicore:Software,
        mwo:ResearchSoftware ;
    rdfs:label "exciting" ;
    nfdicore:fundingProject <http://demo.fiz-karlsruhe.de/matwerk/E858396> ;
    dcterms:description "exciting is a full-potential all-electron density-functional-theory package implementing the families of linearized augmented planewave methods. It can be applied to all kinds of materials, irrespective of the atomic species involved, and also allows for exploring the physics of core electrons. A particular focus are excited states within many-body perturbation theory."^^xsd:string ;
    mwo:hasContributor <http://demo.fiz-karlsruhe.de/matwerk/E3486> ;
    mwo:hasDiscipline <http://demo.fiz-karlsruhe.de/matwerk/E67431> ;
    mwo:hasDocumentation <http://demo.fiz-karlsruhe.de/matwerk/E254829> ;
    mwo:hasRepository <http://demo.fiz-karlsruhe.de/matwerk/E172406> ;
    mwo:hasVersion "oxygen" ;
    mwo:hasWebsite <http://demo.fiz-karlsruhe.de/matwerk/E105654> ;
    mwo:usesMethod <http://demo.fiz-karlsruhe.de/matwerk/E613172> ;
    ns3:has_license <http://demo.fiz-karlsruhe.de/matwerk/E764231> ;
    schema:operatingSystem ns3:SWO_0000020,
        ns3:SWO_0000022 .

<http://demo.fiz-karlsruhe.de/matwerk/E446097> a nfdicore:Software,
        mwo:ResearchSoftware ;
    rdfs:label "FLEUR" ;
    nfdicore:programmingLanguage <http://demo.fiz-karlsruhe.de/matwerk/E836279>,
        <http://demo.fiz-karlsruhe.de/matwerk/E841457>,
        <http://demo.fiz-karlsruhe.de/matwerk/E844052> ;
    dcterms:description "FLEUR is a feature-full, freely available FLAPW (full-potential linearized augmented planewave) code, based on density-functional theory. "^^xsd:string ;
    mwo:hasContributor <http://demo.fiz-karlsruhe.de/matwerk/E1022> ;
    mwo:hasDiscipline <http://demo.fiz-karlsruhe.de/matwerk/E67431> ;
    mwo:hasDocumentation <http://demo.fiz-karlsruhe.de/matwerk/E255542> ;
    mwo:hasRepository <http://demo.fiz-karlsruhe.de/matwerk/E172992> ;
    mwo:hasVersion "MaX-6.0" ;
    mwo:hasWebsite <http://demo.fiz-karlsruhe.de/matwerk/E106112> ;
    mwo:usesMethod <http://demo.fiz-karlsruhe.de/matwerk/E613172> ;
    ns3:has_license <http://demo.fiz-karlsruhe.de/matwerk/E759297> ;
    owl:sameAs <http://www.wikidata.org/entity/Q108241750> .

<http://demo.fiz-karlsruhe.de/matwerk/E447041> a nfdicore:Software,
        mwo:ResearchSoftware ;
    rdfs:label "WIEN2k" ;
    nfdicore:fundingProject <http://demo.fiz-karlsruhe.de/matwerk/E858396> ;
    dcterms:description "The program package WIEN2k allows to perform electronic structure calculations of solids using density functional theory (DFT). It is based on the full-potential (linearized) augmented plane-wave ((L)APW) + local orbitals (lo) method, one among the most accurate schemes for band structure calculations. WIEN2k is an all-electron scheme including relativistic effects and has many features."^^xsd:string ;
    mwo:hasContactPoint <http://demo.fiz-karlsruhe.de/matwerk/E17291> ;
    mwo:hasDiscipline <http://demo.fiz-karlsruhe.de/matwerk/E67431> ;
    mwo:hasDocumentation <http://demo.fiz-karlsruhe.de/matwerk/E256256> ;
    mwo:hasVersion "21.1" ;
    mwo:hasWebsite <http://demo.fiz-karlsruhe.de/matwerk/E106571> ;
    mwo:usesMethod <http://demo.fiz-karlsruhe.de/matwerk/E613172> ;
    ns3:has_license <http://demo.fiz-karlsruhe.de/matwerk/E760529> ;
    owl:sameAs <http://www.wikidata.org/entity/Q2749650> .

<http://demo.fiz-karlsruhe.de/matwerk/E447986> a nfdicore:Software,
        mwo:ResearchSoftware ;
    rdfs:label "Large-scale Atomic/Molecular Massively Parallel Simulator" ;
    nfdicore:programmingLanguage <http://demo.fiz-karlsruhe.de/matwerk/E828542>,
        <http://demo.fiz-karlsruhe.de/matwerk/E841457> ;
    dcterms:description " classical molecular dynamics code with a focus on materials modeling"^^xsd:string ;
    mwo:hasAcronym "LAMMPS"^^xsd:string ;
    mwo:hasDiscipline <http://demo.fiz-karlsruhe.de/matwerk/E67431> ;
    mwo:hasDocumentation <http://demo.fiz-karlsruhe.de/matwerk/E256971> ;
    mwo:hasRepository <http://demo.fiz-karlsruhe.de/matwerk/E173579> ;
    mwo:hasVersion "23-Jun-22" ;
    mwo:hasWebsite <http://demo.fiz-karlsruhe.de/matwerk/E107031> ;
    mwo:usesMethod <http://demo.fiz-karlsruhe.de/matwerk/E616496>,
        <http://demo.fiz-karlsruhe.de/matwerk/E63482> ;
    ns3:has_license <http://demo.fiz-karlsruhe.de/matwerk/E765467> ;
    owl:sameAs <http://www.wikidata.org/entity/Q4042577> ;
    schema:citation <http://demo.fiz-karlsruhe.de/matwerk/E906186> .

<http://demo.fiz-karlsruhe.de/matwerk/E448932> a nfdicore:Software,
        mwo:ResearchSoftware ;
    rdfs:label "The ITAP Molecular Dynamics Program" ;
    nfdicore:fundingProject <http://demo.fiz-karlsruhe.de/matwerk/E859706> ;
    nfdicore:programmingLanguage <http://demo.fiz-karlsruhe.de/matwerk/E828542>,
        <http://demo.fiz-karlsruhe.de/matwerk/E844052> ;
    dcterms:description "IMD is a software package for classical molecular dynamics simulations. Several types of interactions are supported, such as central pair potentials, EAM potentials for metals, Stillinger-Weber and Tersoff potentials for covalent systems, and Gay-Berne potentials for liquid crystals."^^xsd:string ;
    mwo:hasAcronym "IMD"^^xsd:string ;
    mwo:hasContactPoint <http://demo.fiz-karlsruhe.de/matwerk/E700154> ;
    mwo:hasDiscipline <http://demo.fiz-karlsruhe.de/matwerk/E67431> ;
    mwo:hasDocumentation <http://demo.fiz-karlsruhe.de/matwerk/E257687> ;
    mwo:hasRepository <http://demo.fiz-karlsruhe.de/matwerk/E174167> ;
    mwo:hasWebsite <http://demo.fiz-karlsruhe.de/matwerk/E107492> ;
    mwo:usesMethod <http://demo.fiz-karlsruhe.de/matwerk/E616496>,
        <http://demo.fiz-karlsruhe.de/matwerk/E63482> ;
    ns3:has_license <http://demo.fiz-karlsruhe.de/matwerk/E762996> ;
    schema:citation <http://demo.fiz-karlsruhe.de/matwerk/E907532> .

<http://demo.fiz-karlsruhe.de/matwerk/E449879> a nfdicore:Software,
        mwo:ResearchSoftware ;
    rdfs:label "GROMACS" ;
    dcterms:description "molecular dynamics with a focus on simulations of proteins, lipids, and nucleic acids"^^xsd:string ;
    mwo:hasDiscipline <http://demo.fiz-karlsruhe.de/matwerk/E67431> ;
    mwo:hasDocumentation <http://demo.fiz-karlsruhe.de/matwerk/E258404> ;
    mwo:hasRepository <http://demo.fiz-karlsruhe.de/matwerk/E174756> ;
    mwo:hasVersion "2022" ;
    mwo:hasWebsite <http://demo.fiz-karlsruhe.de/matwerk/E107954> ;
    mwo:usesMethod <http://demo.fiz-karlsruhe.de/matwerk/E616496>,
        <http://demo.fiz-karlsruhe.de/matwerk/E63482> ;
    ns3:has_license <http://demo.fiz-karlsruhe.de/matwerk/E764231> ;
    owl:sameAs <http://www.wikidata.org/entity/Q905302> ;
    schema:citation <http://demo.fiz-karlsruhe.de/matwerk/E908879> .

<http://demo.fiz-karlsruhe.de/matwerk/E450827> a nfdicore:Software,
        mwo:ResearchSoftware ;
    rdfs:label "MD++" ;
    nfdicore:programmingLanguage <http://demo.fiz-karlsruhe.de/matwerk/E828542> ;
    dcterms:description "MD++ is a molecular dynamics simulation package written in C++."^^xsd:string ;
    mwo:hasDiscipline <http://demo.fiz-karlsruhe.de/matwerk/E67431> ;
    mwo:hasWebsite <http://demo.fiz-karlsruhe.de/matwerk/E108417> ;
    mwo:usesMethod <http://demo.fiz-karlsruhe.de/matwerk/E616496>,
        <http://demo.fiz-karlsruhe.de/matwerk/E63482> .

<http://demo.fiz-karlsruhe.de/matwerk/E451776> a nfdicore:Software,
        mwo:ResearchSoftware ;
    rdfs:label "Thermo-Calc" ;
    dcterms:description "Thermo-Calc, is used by materials scientists and engineers to generate material properties data, gain insights about materials, understand a specific observation, and answer direct questions related to a specific material and/or its processing. Used in conjunction with suitable databases, Thermo-Calc can be used for a wide variety of applications."^^xsd:string ;
    mwo:hasDiscipline <http://demo.fiz-karlsruhe.de/matwerk/E67431>,
        <http://demo.fiz-karlsruhe.de/matwerk/E70379> ;
    mwo:hasVersion "2022b" ;
    mwo:hasWebsite <http://demo.fiz-karlsruhe.de/matwerk/E108881> ;
    ns3:has_license <http://demo.fiz-karlsruhe.de/matwerk/E766704> .

<http://demo.fiz-karlsruhe.de/matwerk/E452726> a nfdicore:Software,
        mwo:ResearchSoftware ;
    rdfs:label "OpenPhase" ;
    nfdicore:programmingLanguage <http://demo.fiz-karlsruhe.de/matwerk/E828542> ;
    dcterms:description "OpenPhase Studio is a powerful microstructure simulation suite made for metallic materials, ceramics and minerals. Using multi-physics models embedded in the phase-field method, materials processes such as solidification, heat treatment, mechanical testing and many more can be simulated."^^xsd:string ;
    mwo:hasContributor <http://demo.fiz-karlsruhe.de/matwerk/E1037>,
        <http://demo.fiz-karlsruhe.de/matwerk/E4656> ;
    mwo:hasDiscipline <http://demo.fiz-karlsruhe.de/matwerk/E67431>,
        <http://demo.fiz-karlsruhe.de/matwerk/E70379> ;
    mwo:hasWebsite <http://demo.fiz-karlsruhe.de/matwerk/E109346> ;
    mwo:usesMethod <http://demo.fiz-karlsruhe.de/matwerk/E620942> ;
    ns3:has_license <http://demo.fiz-karlsruhe.de/matwerk/E766704> .

<http://demo.fiz-karlsruhe.de/matwerk/E453677> a nfdicore:Software,
        mwo:ResearchSoftware ;
    rdfs:label "Multiphysics Object Oriented Simulation Environment" ;
    nfdicore:programmingLanguage <http://demo.fiz-karlsruhe.de/matwerk/E828542>,
        <http://demo.fiz-karlsruhe.de/matwerk/E836279> ;
    dcterms:description "The Multiphysics Object-Oriented Simulation Environment (MOOSE) is a finite-element, multiphysics framework primarily developed by Idaho National Laboratory. "^^xsd:string ;
    mwo:hasAcronym "MOOSE"^^xsd:string ;
    mwo:hasDiscipline <http://demo.fiz-karlsruhe.de/matwerk/E67431> ;
    mwo:hasRepository <http://demo.fiz-karlsruhe.de/matwerk/E175346> ;
    mwo:hasWebsite <http://demo.fiz-karlsruhe.de/matwerk/E109812> ;
    mwo:usesMethod <http://demo.fiz-karlsruhe.de/matwerk/E610961> ;
    ns3:has_license <http://demo.fiz-karlsruhe.de/matwerk/E767942> ;
    owl:sameAs <http://www.wikidata.org/entity/Q17069813> .

<http://demo.fiz-karlsruhe.de/matwerk/E454629> a nfdicore:Software,
        mwo:ResearchSoftware ;
    rdfs:label "Abaqus" ;
    dcterms:description "The Abaqus Unified FEA product suite offers powerful and complete solutions for both routine and sophisticated engineering problems covering a vast spectrum of industrial applications. "^^xsd:string ;
    mwo:hasContributor <http://demo.fiz-karlsruhe.de/matwerk/E3702> ;
    mwo:hasDiscipline <http://demo.fiz-karlsruhe.de/matwerk/E67431> ;
    mwo:hasVersion "2022" ;
    mwo:hasWebsite <http://demo.fiz-karlsruhe.de/matwerk/E110279> ;
    mwo:usesMethod <http://demo.fiz-karlsruhe.de/matwerk/E610961> ;
    ns3:has_license <http://demo.fiz-karlsruhe.de/matwerk/E766704> ;
    owl:sameAs <http://www.wikidata.org/entity/Q728658> ;
    schema:operatingSystem ns3:SWO_0000022,
        ns3:SWO_9000072 .

<http://demo.fiz-karlsruhe.de/matwerk/E455582> a nfdicore:Software,
        mwo:ResearchSoftware ;
    rdfs:label "FeniCS Project" ;
    nfdicore:programmingLanguage <http://demo.fiz-karlsruhe.de/matwerk/E828542>,
        <http://demo.fiz-karlsruhe.de/matwerk/E836279> ;
    dcterms:description "FEniCSx is a popular open-source computing platform for solving partial differential equations (PDEs). FEniCSx enables users to quickly translate scientific models into efficient finite element code."^^xsd:string ;
    mwo:hasDiscipline <http://demo.fiz-karlsruhe.de/matwerk/E67431> ;
    mwo:hasDocumentation <http://demo.fiz-karlsruhe.de/matwerk/E259122> ;
    mwo:hasRepository <http://demo.fiz-karlsruhe.de/matwerk/E175937> ;
    mwo:hasVersion "0.4" ;
    mwo:hasWebsite <http://demo.fiz-karlsruhe.de/matwerk/E110747> ;
    mwo:usesMethod <http://demo.fiz-karlsruhe.de/matwerk/E610961> ;
    ns3:has_license <http://demo.fiz-karlsruhe.de/matwerk/E762996> ;
    schema:operatingSystem ns3:SWO_0000022,
        ns3:SWO_0000149,
        ns3:SWO_9000072 .

<http://demo.fiz-karlsruhe.de/matwerk/E456536> a nfdicore:Software,
        mwo:ResearchSoftware ;
    rdfs:label "Dusseldorf Advanced Material Simulation Kit" ;
    nfdicore:programmingLanguage <http://demo.fiz-karlsruhe.de/matwerk/E836279>,
        <http://demo.fiz-karlsruhe.de/matwerk/E841457> ;
    dcterms:description """DAMASK is a unified multi-physics crystal plasticity simulation package. The solution of continuum mechanical boundary value problems requires a constitutive response that connects deformation and stress at each material point. This problem is solved in DAMASK on the basis of crystal plasticity using a variety of constitutive models and homogenization approaches. However, treating mechanics in isolation is no longer sufficient to study emergent advanced high-strength materials. In these materials, deformation happens interrelated with displacive phase transformation, significant heating, and potential damage evolution. Therefore, DAMASK is capable of handling multi-physics problems. Following a modular approach, additional field equations are solved in a fully coupled way using a staggered approach.\r
\r
"""^^xsd:string ;
    mwo:hasAcronym "DAMASK"^^xsd:string ;
    mwo:hasContactPoint <http://demo.fiz-karlsruhe.de/matwerk/E701337> ;
    mwo:hasContributor <http://demo.fiz-karlsruhe.de/matwerk/E3416> ;
    mwo:hasDiscipline <http://demo.fiz-karlsruhe.de/matwerk/E67431> ;
    mwo:hasDocumentation <http://demo.fiz-karlsruhe.de/matwerk/E259841> ;
    mwo:hasRepository <http://demo.fiz-karlsruhe.de/matwerk/E176529> ;
    mwo:hasVersion "3" ;
    mwo:hasWebsite <http://demo.fiz-karlsruhe.de/matwerk/E111216> ;
    mwo:usesMethod <http://demo.fiz-karlsruhe.de/matwerk/E622056> ;
    ns3:has_license <http://demo.fiz-karlsruhe.de/matwerk/E769181> ;
    schema:citation <http://demo.fiz-karlsruhe.de/matwerk/E910227> .

<http://demo.fiz-karlsruhe.de/matwerk/E458447> a nfdicore:Software,
        mwo:ResearchSoftware,
        mwo:WorkflowEnvironment ;
    rdfs:label "Automated interactive infrastructure and database for computational science" ;
    nfdicore:programmingLanguage <http://demo.fiz-karlsruhe.de/matwerk/E836279> ;
    dcterms:description "workflow manager for computational science with a strong focus on provenance, performance and extensibility."^^xsd:string ;
    mwo:hasAcronym "AiiDA"^^xsd:string ;
    mwo:hasDiscipline <http://demo.fiz-karlsruhe.de/matwerk/E67431> ;
    mwo:hasDocumentation <http://demo.fiz-karlsruhe.de/matwerk/E261282> ;
    mwo:hasRepository <http://demo.fiz-karlsruhe.de/matwerk/E177716> ;
    mwo:hasVersion "2" ;
    mwo:hasWebsite <http://demo.fiz-karlsruhe.de/matwerk/E112157> ;
    ns3:has_license <http://demo.fiz-karlsruhe.de/matwerk/E759297> ;
    schema:citation <http://demo.fiz-karlsruhe.de/matwerk/E912926> .

<http://demo.fiz-karlsruhe.de/matwerk/E459404> a nfdicore:Software,
        mwo:ResearchSoftware,
        mwo:WorkflowEnvironment ;
    rdfs:label "SimStack" ;
    dcterms:description "workflow environment"^^xsd:string ;
    mwo:hasDiscipline <http://demo.fiz-karlsruhe.de/matwerk/E67431> ;
    mwo:hasDocumentation <http://demo.fiz-karlsruhe.de/matwerk/E262004> ;
    mwo:hasWebsite <http://demo.fiz-karlsruhe.de/matwerk/E112629> ;
    ns3:has_license <http://demo.fiz-karlsruhe.de/matwerk/E770421> ;
    schema:operatingSystem ns3:SWO_0000022,
        ns3:SWO_9000072 .

<http://demo.fiz-karlsruhe.de/matwerk/E460362> a nfdicore:Software,
        mwo:ProcessingSoftware,
        mwo:ResearchSoftware,
        mwo:VisualizationSoftware ;
    rdfs:label "Atomic Simulation Environment" ;
    nfdicore:programmingLanguage <http://demo.fiz-karlsruhe.de/matwerk/E836279> ;
    dcterms:description "set of tools and Python modules for setting up, manipulating, running, visualizing and analyzing atomistic simulations"^^xsd:string ;
    mwo:hasAcronym "ASE"^^xsd:string ;
    mwo:hasDiscipline <http://demo.fiz-karlsruhe.de/matwerk/E67431> ;
    mwo:hasDocumentation <http://demo.fiz-karlsruhe.de/matwerk/E262727> ;
    mwo:hasRepository <http://demo.fiz-karlsruhe.de/matwerk/E178311> ;
    mwo:hasVersion "3.22.1" ;
    mwo:hasWebsite <http://demo.fiz-karlsruhe.de/matwerk/E113102> ;
    mwo:usesMethod <http://demo.fiz-karlsruhe.de/matwerk/E63482> ;
    ns3:has_license <http://demo.fiz-karlsruhe.de/matwerk/E771662> ;
    schema:operatingSystem ns3:SWO_0000022,
        ns3:SWO_0000149 .

<http://demo.fiz-karlsruhe.de/matwerk/E461321> a nfdicore:Software ;
    rdfs:label "OVITO basic" ;
    dcterms:description "visualization and analysis for data generated in MD, atomistic Monte-Carlo and other particle-based simulations"^^xsd:string ;
    mwo:hasAcronym "OVITO"^^xsd:string ;
    mwo:hasDocumentation <http://demo.fiz-karlsruhe.de/matwerk/E263451> ;
    mwo:hasVersion "3.7.7" ;
    mwo:hasWebsite <http://demo.fiz-karlsruhe.de/matwerk/E113576> ;
    ns3:has_license <http://demo.fiz-karlsruhe.de/matwerk/E772904> ;
    schema:operatingSystem ns3:SWO_0000022,
        ns3:SWO_0000149,
        ns3:SWO_9000072 .

<http://demo.fiz-karlsruhe.de/matwerk/E462281> a nfdicore:Software ;
    rdfs:label "Jmol" ;
    dcterms:description "open-source Java viewer for chemical structures in 3D with features for chemicals, crystals, materials and biomolecules"^^xsd:string ;
    mwo:hasDocumentation <http://demo.fiz-karlsruhe.de/matwerk/E264176> ;
    mwo:hasVersion "14" ;
    mwo:hasWebsite <http://demo.fiz-karlsruhe.de/matwerk/E114051> ;
    ns3:has_license <http://demo.fiz-karlsruhe.de/matwerk/E764231> ;
    owl:sameAs <http://www.wikidata.org/entity/Q1689854> .

<http://demo.fiz-karlsruhe.de/matwerk/E463242> a nfdicore:Software ;
    rdfs:label "Visualization for electronic and structural analysis" ;
    dcterms:description "3D visualization program for structural models, volumetric data such as electron/nuclear densities, and crystal morphologies"^^xsd:string ;
    mwo:hasAcronym "VESTA"^^xsd:string ;
    mwo:hasDocumentation <http://demo.fiz-karlsruhe.de/matwerk/E264902> ;
    mwo:hasVersion "3" ;
    mwo:hasWebsite <http://demo.fiz-karlsruhe.de/matwerk/E114527> ;
    ns3:has_license <http://demo.fiz-karlsruhe.de/matwerk/E774147> ;
    schema:operatingSystem ns3:SWO_0000022,
        ns3:SWO_0000149,
        ns3:SWO_9000072 .

<http://demo.fiz-karlsruhe.de/matwerk/E464204> a nfdicore:Software ;
    rdfs:label "X-window crystalline structures and densities" ;
    dcterms:description "crystalline and molecular structure visualisation program aiming at display of isosurfaces and contours"^^xsd:string ;
    mwo:hasAcronym "XcrySDen"^^xsd:string ;
    mwo:hasDocumentation <http://demo.fiz-karlsruhe.de/matwerk/E265629> ;
    mwo:hasVersion "1.6.2" ;
    mwo:hasWebsite <http://demo.fiz-karlsruhe.de/matwerk/E115004> ;
    ns3:has_license <http://demo.fiz-karlsruhe.de/matwerk/E755607> ;
    schema:operatingSystem ns3:SWO_0000021,
        ns3:SWO_0000022 .

<http://demo.fiz-karlsruhe.de/matwerk/E465167> a nfdicore:Software ;
    rdfs:label "Visual Molecular Dynamics" ;
    dcterms:description "molecular modelling and visualization computer program"^^xsd:string ;
    mwo:hasAcronym "VMD"^^xsd:string ;
    mwo:hasDocumentation <http://demo.fiz-karlsruhe.de/matwerk/E266357> ;
    mwo:hasVersion "1.9.4" ;
    mwo:hasWebsite <http://demo.fiz-karlsruhe.de/matwerk/E115482> ;
    ns3:has_license <http://demo.fiz-karlsruhe.de/matwerk/E775391> ;
    owl:sameAs <http://www.wikidata.org/entity/Q7936565> ;
    schema:operatingSystem ns3:SWO_0000022,
        ns3:SWO_0000149,
        ns3:SWO_9000072 .

<http://demo.fiz-karlsruhe.de/matwerk/E466131> a nfdicore:Software ;
    rdfs:label "py4vasp" ;
    nfdicore:programmingLanguage <http://demo.fiz-karlsruhe.de/matwerk/E828542>,
        <http://demo.fiz-karlsruhe.de/matwerk/E836279> ;
    dcterms:description "Python interface to extract data from VASP calculations"^^xsd:string ;
    mwo:hasRepository <http://demo.fiz-karlsruhe.de/matwerk/E178907> ;
    mwo:hasVersion "0.4" ;
    mwo:hasWebsite <http://demo.fiz-karlsruhe.de/matwerk/E115961> ;
    ns3:has_license <http://demo.fiz-karlsruhe.de/matwerk/E765467> ;
    schema:operatingSystem ns3:SWO_0000022,
        ns3:SWO_0000149,
        ns3:SWO_9000072 .

<http://demo.fiz-karlsruhe.de/matwerk/E467096> a nfdicore:Software ;
    rdfs:label "phonopy" ;
    nfdicore:programmingLanguage <http://demo.fiz-karlsruhe.de/matwerk/E836279>,
        <http://demo.fiz-karlsruhe.de/matwerk/E844052> ;
    dcterms:description "open source package for phonon calculations at harmonic and quasi-harmonic levels"^^xsd:string ;
    mwo:hasDocumentation <http://demo.fiz-karlsruhe.de/matwerk/E267086> ;
    mwo:hasRepository <http://demo.fiz-karlsruhe.de/matwerk/E179504> ;
    mwo:hasVersion "2.15.0" ;
    mwo:hasWebsite <http://demo.fiz-karlsruhe.de/matwerk/E116441> ;
    ns3:has_license <http://demo.fiz-karlsruhe.de/matwerk/E739721> .

<http://demo.fiz-karlsruhe.de/matwerk/E468062> a nfdicore:Software ;
    rdfs:label "Soprano" ;
    nfdicore:programmingLanguage <http://demo.fiz-karlsruhe.de/matwerk/E836279> ;
    dcterms:description "Python library for common tasks in computational NMR crystallography and simulations to generate, manipulate, run calculations on and analyse large data sets of crystal structures, with a particular attention to the output of ab-initio random structure searching"^^xsd:string ;
    mwo:hasRepository <http://demo.fiz-karlsruhe.de/matwerk/E180102> ;
    mwo:hasWebsite <http://demo.fiz-karlsruhe.de/matwerk/E116922> ;
    ns3:has_license <http://demo.fiz-karlsruhe.de/matwerk/E776636> ;
    owl:sameAs <http://www.wikidata.org/entity/Q3110464> .

<http://demo.fiz-karlsruhe.de/matwerk/E469029> a nfdicore:Software ;
    rdfs:label "CASINO" ;
    dcterms:description "Quantum Monte Carlo (QMC) electronic structure calculations"^^xsd:string ;
    mwo:hasVersion "2.12" ;
    mwo:hasWebsite <http://demo.fiz-karlsruhe.de/matwerk/E117404> ;
    ns3:has_license <http://demo.fiz-karlsruhe.de/matwerk/E777882> ;
    owl:sameAs <http://www.wikidata.org/entity/Q5008866> .

<http://demo.fiz-karlsruhe.de/matwerk/E469997> a nfdicore:Software ;
    rdfs:label "Graphical Interface for Materials Simulations" ;
    dcterms:description "browser-based toolbox for electronic structure codes and supports the generation of input files for first-principles electronic structure calculations and workflows, as well as the analysis and visualization of the resulting data extracted from the output files."^^xsd:string ;
    mwo:hasAcronym "GIMS"^^xsd:string ;
    mwo:hasWebsite <http://demo.fiz-karlsruhe.de/matwerk/E117887> ;
    schema:operatingSystem ns3:SWO_0000021 .

<http://demo.fiz-karlsruhe.de/matwerk/E470966> a nfdicore:Software ;
    rdfs:label "FHI-vibes" ;
    dcterms:description "python package for calculating, analyzing, and understanding the vibrational properties of solids from first principles. FHI-vibes is intended to seamlessly bridge between the harmonic approximation and fully anharmonic molecular dynamics simulations."^^xsd:string ;
    mwo:hasDocumentation <http://demo.fiz-karlsruhe.de/matwerk/E267816> ;
    mwo:hasRepository <http://demo.fiz-karlsruhe.de/matwerk/E180701> ;
    mwo:hasVersion "1.0.3" ;
    mwo:hasWebsite <http://demo.fiz-karlsruhe.de/matwerk/E118371> ;
    ns3:has_license <http://demo.fiz-karlsruhe.de/matwerk/E759297> .

<http://demo.fiz-karlsruhe.de/matwerk/E471936> a nfdicore:Software ;
    rdfs:label "CIF2Cell" ;
    nfdicore:programmingLanguage <http://demo.fiz-karlsruhe.de/matwerk/E836279> ;
    dcterms:description "tool to generate the geometrical setup for various electronic structure codes from a CIF (Crystallographic Information Framework) file"^^xsd:string ;
    mwo:hasRepository <http://demo.fiz-karlsruhe.de/matwerk/E181301> ;
    ns3:has_license <http://demo.fiz-karlsruhe.de/matwerk/E779129> ;
    schema:citation <http://demo.fiz-karlsruhe.de/matwerk/E914277> .

<http://demo.fiz-karlsruhe.de/matwerk/E472907> a nfdicore:Software ;
    rdfs:label "Avogadro" ;
    nfdicore:programmingLanguage <http://demo.fiz-karlsruhe.de/matwerk/E828542> ;
    dcterms:description "molecule editor and visualizer designed for cross-platform use in computational chemistry, molecular modeling, bioinformatics, materials science, and related areas"^^xsd:string ;
    mwo:hasDocumentation <http://demo.fiz-karlsruhe.de/matwerk/E268547> ;
    mwo:hasRepository <http://demo.fiz-karlsruhe.de/matwerk/E181902> ;
    mwo:hasVersion "1.95" ;
    mwo:hasWebsite <http://demo.fiz-karlsruhe.de/matwerk/E118856> ;
    owl:sameAs <http://www.wikidata.org/entity/Q851800> ;
    schema:citation <http://demo.fiz-karlsruhe.de/matwerk/E915629> .

<http://demo.fiz-karlsruhe.de/matwerk/E473879> a nfdicore:Software ;
    rdfs:label "AML" ;
    nfdicore:programmingLanguage <http://demo.fiz-karlsruhe.de/matwerk/E836279> ;
    dcterms:description "Python package to automatically build the reference set for the training of Neural Network Potentials (NNPs), and eventually other machine-learned potentials, in an automated, data-driven fashion."^^xsd:string ;
    mwo:hasRepository <http://demo.fiz-karlsruhe.de/matwerk/E182504> ;
    ns3:has_license <http://demo.fiz-karlsruhe.de/matwerk/E779129> ;
    schema:citation <http://demo.fiz-karlsruhe.de/matwerk/E916982> .

<http://demo.fiz-karlsruhe.de/matwerk/E474852> a nfdicore:Software ;
    rdfs:label "pycp2k" ;
    nfdicore:programmingLanguage <http://demo.fiz-karlsruhe.de/matwerk/E836279> ;
    dcterms:description "Python Cp2k interface"^^xsd:string ;
    mwo:hasRepository <http://demo.fiz-karlsruhe.de/matwerk/E183107> ;
    ns3:has_license <http://demo.fiz-karlsruhe.de/matwerk/E780377> .

<http://demo.fiz-karlsruhe.de/matwerk/E475826> a nfdicore:Software ;
    rdfs:label "Pyretis" ;
    nfdicore:programmingLanguage <http://demo.fiz-karlsruhe.de/matwerk/E836279> ;
    dcterms:description "Python library for rare event molecular simulations with emphasis on methods based on transition interface sampling and replica exchange transition interface sampling"^^xsd:string ;
    mwo:hasRepository <http://demo.fiz-karlsruhe.de/matwerk/E183711> ;
    mwo:hasVersion "2.5.0" ;
    mwo:hasWebsite <http://demo.fiz-karlsruhe.de/matwerk/E119342> ;
    ns3:has_license <http://demo.fiz-karlsruhe.de/matwerk/E781626> ;
    schema:citation <http://demo.fiz-karlsruhe.de/matwerk/E918336> .

<http://demo.fiz-karlsruhe.de/matwerk/E476801> a nfdicore:Software ;
    rdfs:label "OpenPathSampling" ;
    nfdicore:programmingLanguage <http://demo.fiz-karlsruhe.de/matwerk/E836279> ;
    dcterms:description "Python library to facilitate path sampling algorithms."^^xsd:string ;
    mwo:hasRepository <http://demo.fiz-karlsruhe.de/matwerk/E184316> ;
    mwo:hasVersion "1.5.3" ;
    mwo:hasWebsite <http://demo.fiz-karlsruhe.de/matwerk/E119829> ;
    ns3:has_license <http://demo.fiz-karlsruhe.de/matwerk/E759297> ;
    schema:citation <http://demo.fiz-karlsruhe.de/matwerk/E919691> .

<http://demo.fiz-karlsruhe.de/matwerk/E477777> a nfdicore:Software ;
    rdfs:label "SeeK-path" ;
    nfdicore:programmingLanguage <http://demo.fiz-karlsruhe.de/matwerk/E836279> ;
    dcterms:description "A module to obtain and visualize k-vector coefficients and obtain band paths in the Brillouin zone of crystal structures"^^xsd:string ;
    mwo:hasRepository <http://demo.fiz-karlsruhe.de/matwerk/E184922> ;
    mwo:hasWebsite <http://demo.fiz-karlsruhe.de/matwerk/E120317> ;
    ns3:has_license <http://demo.fiz-karlsruhe.de/matwerk/E759297> .

<http://demo.fiz-karlsruhe.de/matwerk/E478754> a nfdicore:Software ;
    rdfs:label "Python Materials Genomics" ;
    nfdicore:programmingLanguage <http://demo.fiz-karlsruhe.de/matwerk/E836279> ;
    dcterms:description "materials analysis code that defines core object representations for structures and molecules with support for many electronic structure codes. It is currently the core analysis code powering the Materials Project."^^xsd:string ;
    mwo:hasAcronym "Pymatgen"^^xsd:string ;
    mwo:hasDocumentation <http://demo.fiz-karlsruhe.de/matwerk/E269279> ;
    mwo:hasRepository <http://demo.fiz-karlsruhe.de/matwerk/E185529> ;
    mwo:hasVersion "V2022.0" ;
    mwo:hasWebsite <http://demo.fiz-karlsruhe.de/matwerk/E120806> ;
    ns3:has_license <http://demo.fiz-karlsruhe.de/matwerk/E759297> .

<http://demo.fiz-karlsruhe.de/matwerk/E479732> a nfdicore:Software ;
    rdfs:label "Qe-tools" ;
    nfdicore:programmingLanguage <http://demo.fiz-karlsruhe.de/matwerk/E836279> ;
    dcterms:description "A set of useful tools for Quantum ESPRESSO"^^xsd:string ;
    mwo:hasRepository <http://demo.fiz-karlsruhe.de/matwerk/E186137> ;
    ns3:has_license <http://demo.fiz-karlsruhe.de/matwerk/E759297> .

<http://demo.fiz-karlsruhe.de/matwerk/E480711> a nfdicore:Software ;
    rdfs:label "TAMkin" ;
    nfdicore:programmingLanguage <http://demo.fiz-karlsruhe.de/matwerk/E836279> ;
    dcterms:description "post-processing toolkit for normal mode analysis, thermochemistry and reaction kinetics."^^xsd:string ;
    mwo:hasDocumentation <http://demo.fiz-karlsruhe.de/matwerk/E270012> ;
    mwo:hasRepository <http://demo.fiz-karlsruhe.de/matwerk/E186746> ;
    mwo:hasWebsite <http://demo.fiz-karlsruhe.de/matwerk/E121296> ;
    ns3:has_license <http://demo.fiz-karlsruhe.de/matwerk/E782876> ;
    schema:citation <http://demo.fiz-karlsruhe.de/matwerk/E921047> .

<http://demo.fiz-karlsruhe.de/matwerk/E481691> a nfdicore:Software ;
    rdfs:label "Pizza.py Toolkit" ;
    nfdicore:programmingLanguage <http://demo.fiz-karlsruhe.de/matwerk/E836279> ;
    dcterms:description "Pizza.py is a loosely integrated collection of tools, many of which provide pre- and post-processing capability for the LAMMPS molecular dynamics, ChemCell cell modeling, and SPPARKS kinetic Monte Carlo packages. There are tools to create input files, convert between file formats, process log and dump files, create plots, and visualize and animate simulation snapshots. "^^xsd:string ;
    mwo:hasDocumentation <http://demo.fiz-karlsruhe.de/matwerk/E270746> ;
    mwo:hasRepository <http://demo.fiz-karlsruhe.de/matwerk/E187356> ;
    mwo:hasWebsite <http://demo.fiz-karlsruhe.de/matwerk/E121787> ;
    ns3:has_license <http://demo.fiz-karlsruhe.de/matwerk/E784127> .

<http://demo.fiz-karlsruhe.de/matwerk/E482672> a nfdicore:Software ;
    rdfs:label "MDTraj" ;
    dcterms:description "Read, write and analyze MD trajectories with only a few lines of Python code."^^xsd:string ;
    mwo:hasWebsite <http://demo.fiz-karlsruhe.de/matwerk/E122279> .

<http://demo.fiz-karlsruhe.de/matwerk/E483654> a nfdicore:Software ;
    rdfs:label "freud" ;
    nfdicore:programmingLanguage <http://demo.fiz-karlsruhe.de/matwerk/E828542>,
        <http://demo.fiz-karlsruhe.de/matwerk/E836279> ;
    dcterms:description "The freud Python library provides a simple, flexible, powerful set of tools for analyzing trajectories obtained from molecular dynamics or Monte Carlo simulations. "^^xsd:string ;
    mwo:hasDocumentation <http://demo.fiz-karlsruhe.de/matwerk/E271481> ;
    mwo:hasRepository <http://demo.fiz-karlsruhe.de/matwerk/E187967> ;
    mwo:hasVersion "2.11.0" .

<http://demo.fiz-karlsruhe.de/matwerk/E484637> a nfdicore:Software ;
    rdfs:label "NGLview" ;
    nfdicore:programmingLanguage <http://demo.fiz-karlsruhe.de/matwerk/E836279> ;
    dcterms:description "Jupyter widget to interactively view molecular structures and trajectories"^^xsd:string ;
    mwo:hasRepository <http://demo.fiz-karlsruhe.de/matwerk/E188579> ;
    mwo:hasVersion "3.0.3" ;
    mwo:hasWebsite <http://demo.fiz-karlsruhe.de/matwerk/E122772> ;
    ns3:has_license <http://demo.fiz-karlsruhe.de/matwerk/E759297> ;
    schema:citation <http://demo.fiz-karlsruhe.de/matwerk/E922404> .

<http://demo.fiz-karlsruhe.de/matwerk/E485621> a nfdicore:Software ;
    rdfs:label "QuickFF" ;
    nfdicore:programmingLanguage <http://demo.fiz-karlsruhe.de/matwerk/E836279> ;
    dcterms:description "Python package developed at the Center for Molecular Modeling (CMM) to quickly derive accurate force fields from ab initio calculations. "^^xsd:string ;
    mwo:hasContactPoint <http://demo.fiz-karlsruhe.de/matwerk/E17472> ;
    mwo:hasRepository <http://demo.fiz-karlsruhe.de/matwerk/E189192> ;
    mwo:hasVersion "2.2.7" ;
    mwo:hasWebsite <http://demo.fiz-karlsruhe.de/matwerk/E123266> ;
    ns3:has_license <http://demo.fiz-karlsruhe.de/matwerk/E785379> ;
    schema:citation <http://demo.fiz-karlsruhe.de/matwerk/E923762> .

<http://demo.fiz-karlsruhe.de/matwerk/E486606> a nfdicore:Software ;
    rdfs:label "PyLammpsMPI" ;
    nfdicore:programmingLanguage <http://demo.fiz-karlsruhe.de/matwerk/E836279> ;
    dcterms:description "Parallel Lammps Python interface"^^xsd:string ;
    mwo:hasRepository <http://demo.fiz-karlsruhe.de/matwerk/E189806> ;
    ns3:has_license <http://demo.fiz-karlsruhe.de/matwerk/E739721> .

<http://demo.fiz-karlsruhe.de/matwerk/E487592> a nfdicore:Software ;
    rdfs:label "Yet another force field" ;
    nfdicore:programmingLanguage <http://demo.fiz-karlsruhe.de/matwerk/E836279>,
        <http://demo.fiz-karlsruhe.de/matwerk/E844052> ;
    dcterms:description " pythonic force-field (FF) code used at the Center for Molecular Modeling (CMM) to test-drive new FF models"^^xsd:string ;
    mwo:hasAcronym "Yaff "^^xsd:string ;
    mwo:hasDocumentation <http://demo.fiz-karlsruhe.de/matwerk/E272217> ;
    mwo:hasRepository <http://demo.fiz-karlsruhe.de/matwerk/E190421> ;
    mwo:hasVersion "1.6.0" ;
    mwo:hasWebsite <http://demo.fiz-karlsruhe.de/matwerk/E123761> ;
    ns3:has_license <http://demo.fiz-karlsruhe.de/matwerk/E785379> .

<http://demo.fiz-karlsruhe.de/matwerk/E488579> a nfdicore:Software ;
    rdfs:label "Cluster Expansion in Atomic Simulation Environment" ;
    dcterms:description "package that automates the cumbersome setup and construction procedure of cluster expansion (CE). It provides a comprehensive list of tools for specifying parameters for CE, generating training structures, fitting effective cluster interaction (ECI) values and running Monte Carlo simulations."^^xsd:string ;
    mwo:hasAcronym "CLEASE"^^xsd:string ;
    mwo:hasDocumentation <http://demo.fiz-karlsruhe.de/matwerk/E272954> ;
    mwo:hasRepository <http://demo.fiz-karlsruhe.de/matwerk/E191037> ;
    mwo:hasVersion "0.10.9" ;
    mwo:hasWebsite <http://demo.fiz-karlsruhe.de/matwerk/E124257> ;
    ns3:has_license <http://demo.fiz-karlsruhe.de/matwerk/E786632> ;
    schema:citation <http://demo.fiz-karlsruhe.de/matwerk/E925121> .

<http://demo.fiz-karlsruhe.de/matwerk/E489567> a nfdicore:Software ;
    rdfs:label "icet" ;
    nfdicore:programmingLanguage <http://demo.fiz-karlsruhe.de/matwerk/E836279> ;
    dcterms:description "icet is a python tool for the construction and sampling of alloy cluster expansions."^^xsd:string ;
    mwo:hasRepository <http://demo.fiz-karlsruhe.de/matwerk/E191654> ;
    mwo:hasVersion "2.1" ;
    ns3:has_license <http://demo.fiz-karlsruhe.de/matwerk/E786632> ;
    schema:citation <http://demo.fiz-karlsruhe.de/matwerk/E926481> .

<http://demo.fiz-karlsruhe.de/matwerk/E490556> a nfdicore:Software ;
    rdfs:label "DynaPhoPy" ;
    nfdicore:programmingLanguage <http://demo.fiz-karlsruhe.de/matwerk/E836279> ;
    dcterms:description "Dynaphopy allows to calculate anharmonic phonon linewidhts and frequency shifts using the mode descomposition technique."^^xsd:string ;
    mwo:hasRepository <http://demo.fiz-karlsruhe.de/matwerk/E192272> ;
    ns3:has_license <http://demo.fiz-karlsruhe.de/matwerk/E759297> ;
    schema:citation <http://demo.fiz-karlsruhe.de/matwerk/E927842> .

<http://demo.fiz-karlsruhe.de/matwerk/E491546> a nfdicore:Software ;
    rdfs:label "Extensible Self-optimizing Phase Equilibria Infrastructure" ;
    nfdicore:programmingLanguage <http://demo.fiz-karlsruhe.de/matwerk/E836279> ;
    dcterms:description "tool for creating CALPHAD databases and evaluating the uncertainty of CALPHAD models."^^xsd:string ;
    mwo:hasAcronym "ESPEI"^^xsd:string ;
    mwo:hasRepository <http://demo.fiz-karlsruhe.de/matwerk/E192891> ;
    mwo:hasVersion "0.8.9" ;
    ns3:has_license <http://demo.fiz-karlsruhe.de/matwerk/E759297> ;
    schema:citation <http://demo.fiz-karlsruhe.de/matwerk/E929204> .

<http://demo.fiz-karlsruhe.de/matwerk/E492537> a nfdicore:Software ;
    rdfs:label "pycalphad" ;
    nfdicore:programmingLanguage <http://demo.fiz-karlsruhe.de/matwerk/E836279>,
        <http://demo.fiz-karlsruhe.de/matwerk/E845351> ;
    dcterms:description "Python library for computational thermodynamics using the CALPHAD method."^^xsd:string ;
    mwo:hasRepository <http://demo.fiz-karlsruhe.de/matwerk/E193511> ;
    mwo:hasVersion "0.10.1" ;
    mwo:hasWebsite <http://demo.fiz-karlsruhe.de/matwerk/E124754> ;
    ns3:has_license <http://demo.fiz-karlsruhe.de/matwerk/E759297> ;
    schema:citation <http://demo.fiz-karlsruhe.de/matwerk/E930567> .

<http://demo.fiz-karlsruhe.de/matwerk/E493529> a nfdicore:Software ;
    rdfs:label "pymatnest" ;
    nfdicore:programmingLanguage <http://demo.fiz-karlsruhe.de/matwerk/E836279>,
        <http://demo.fiz-karlsruhe.de/matwerk/E846651> ;
    dcterms:description "the pymatnest package is a software library for carrying out nested sampling calculations. It can be used to explore the energy landscape of different materials (both clusters and bulk materials), calculate thermodynamic variables at arbitrary temperatures, locate phase transitions and calculate the phase diagram. "^^xsd:string ;
    mwo:hasRepository <http://demo.fiz-karlsruhe.de/matwerk/E194132> ;
    ns3:has_license <http://demo.fiz-karlsruhe.de/matwerk/E785379> ;
    schema:citation <http://demo.fiz-karlsruhe.de/matwerk/E931931> .

<http://demo.fiz-karlsruhe.de/matwerk/E494522> a nfdicore:Software ;
    rdfs:label "KIM-based Learning-Integrated Fitting Framework" ;
    nfdicore:programmingLanguage <http://demo.fiz-karlsruhe.de/matwerk/E828542>,
        <http://demo.fiz-karlsruhe.de/matwerk/E836279> ;
    dcterms:description "KLIFF is an interatomic potential fitting package that can be used to fit both physics-motivated potentials (e.g. the Stillinger-Weber potential) and machine learning potentials (e.g. neural network potential). "^^xsd:string ;
    mwo:hasAcronym "KLIFF"^^xsd:string ;
    mwo:hasDocumentation <http://demo.fiz-karlsruhe.de/matwerk/E273692> ;
    mwo:hasRepository <http://demo.fiz-karlsruhe.de/matwerk/E194754> ;
    mwo:hasVersion "0.4.0" ;
    ns3:has_license <http://demo.fiz-karlsruhe.de/matwerk/E787886> ;
    schema:citation <http://demo.fiz-karlsruhe.de/matwerk/E933296> .

<http://demo.fiz-karlsruhe.de/matwerk/E495516> a nfdicore:Software ;
    rdfs:label "n2p2" ;
    nfdicore:programmingLanguage <http://demo.fiz-karlsruhe.de/matwerk/E828542>,
        <http://demo.fiz-karlsruhe.de/matwerk/E836279> ;
    dcterms:description "high-dimensional neural network potentials in computational physics and chemistry"^^xsd:string ;
    mwo:hasRepository <http://demo.fiz-karlsruhe.de/matwerk/E195377> ;
    mwo:hasVersion "2.2.0" ;
    mwo:hasWebsite <http://demo.fiz-karlsruhe.de/matwerk/E125252> ;
    ns3:has_license <http://demo.fiz-karlsruhe.de/matwerk/E762996> ;
    schema:citation <http://demo.fiz-karlsruhe.de/matwerk/E934662> .

<http://demo.fiz-karlsruhe.de/matwerk/E496511> a nfdicore:Software ;
    rdfs:label "FitSNAP" ;
    nfdicore:programmingLanguage <http://demo.fiz-karlsruhe.de/matwerk/E836279>,
        <http://demo.fiz-karlsruhe.de/matwerk/E845351> ;
    dcterms:description "A Python Package For Training SNAP Interatomic Potentials for use in the LAMMPS molecular dynamics package"^^xsd:string ;
    mwo:hasRepository <http://demo.fiz-karlsruhe.de/matwerk/E196001> ;
    mwo:hasWebsite <http://demo.fiz-karlsruhe.de/matwerk/E125751> ;
    ns3:has_license <http://demo.fiz-karlsruhe.de/matwerk/E765467> .

<http://demo.fiz-karlsruhe.de/matwerk/E497507> a nfdicore:Software ;
    rdfs:label "matminer" ;
    nfdicore:programmingLanguage <http://demo.fiz-karlsruhe.de/matwerk/E836279> ;
    dcterms:description "Python library for data mining the properties of materials."^^xsd:string ;
    mwo:hasRepository <http://demo.fiz-karlsruhe.de/matwerk/E196626> ;
    mwo:hasVersion "0.7.6" ;
    mwo:hasWebsite <http://demo.fiz-karlsruhe.de/matwerk/E126251> ;
    ns3:has_license <http://demo.fiz-karlsruhe.de/matwerk/E789141> ;
    schema:citation <http://demo.fiz-karlsruhe.de/matwerk/E936029> .

<http://demo.fiz-karlsruhe.de/matwerk/E498504> a nfdicore:Software ;
    rdfs:label "Matbench" ;
    nfdicore:programmingLanguage <http://demo.fiz-karlsruhe.de/matwerk/E836279> ;
    dcterms:description "Matbench is an ImageNet for materials science; a curated set of 13 supervised, pre-cleaned, ready-to-use ML tasks for benchmarking and fair comparison. The tasks span a wide domain of inorganic materials science applications including electronic, thermodynamic, mechanical, and thermal properties among crystals, 2D materials, disordered metals, and more."^^xsd:string ;
    mwo:hasRepository <http://demo.fiz-karlsruhe.de/matwerk/E197252> ;
    mwo:hasVersion "0.6" ;
    mwo:hasWebsite <http://demo.fiz-karlsruhe.de/matwerk/E126752> ;
    ns3:has_license <http://demo.fiz-karlsruhe.de/matwerk/E759297> ;
    schema:citation <http://demo.fiz-karlsruhe.de/matwerk/E937397> .

<http://demo.fiz-karlsruhe.de/matwerk/E499502> a nfdicore:Software ;
    rdfs:label "mendeleev" ;
    nfdicore:programmingLanguage <http://demo.fiz-karlsruhe.de/matwerk/E836279> ;
    dcterms:description "A python package for accessing various properties of elements, ions and isotopes in the periodic table of elements."^^xsd:string ;
    mwo:hasDocumentation <http://demo.fiz-karlsruhe.de/matwerk/E274431> ;
    mwo:hasRepository <http://demo.fiz-karlsruhe.de/matwerk/E197879> ;
    mwo:hasVersion "0.10.0" ;
    ns3:has_license <http://demo.fiz-karlsruhe.de/matwerk/E759297> .

<http://demo.fiz-karlsruhe.de/matwerk/E500501> a nfdicore:Software ;
    rdfs:label "TEMMETA" ;
    nfdicore:programmingLanguage <http://demo.fiz-karlsruhe.de/matwerk/E836279> ;
    dcterms:description "TEMMETA is a library for transmission electron microscopy (TEM) (meta)data manipulation. The aim is to offer a one stop place for very basic to intermediate level operations on (S)TEM data, and be a kind of python version of ImageJ + Digital Micrograph + Velox."^^xsd:string ;
    mwo:hasRepository <http://demo.fiz-karlsruhe.de/matwerk/E198507> ;
    mwo:hasVersion "0.0.6" ;
    ns3:has_license <http://demo.fiz-karlsruhe.de/matwerk/E762996> .

<http://demo.fiz-karlsruhe.de/matwerk/E502502> a nfdicore:Software ;
    rdfs:label "High-Throughput Molecular Dynamics" ;
    nfdicore:programmingLanguage <http://demo.fiz-karlsruhe.de/matwerk/E836279> ;
    dcterms:description "HTMD is a programmable, extensible platform written in Python. It provides a complete workspace for simulation-based discovery through molecular simulations while aiming to solve the data generation and analysis problem as well as increase reproducibility."^^xsd:string ;
    mwo:hasAcronym "HTMD"^^xsd:string ;
    mwo:hasRepository <http://demo.fiz-karlsruhe.de/matwerk/E199766> ;
    mwo:hasVersion "1.13.1" ;
    ns3:has_license <http://demo.fiz-karlsruhe.de/matwerk/E790397> .

<http://demo.fiz-karlsruhe.de/matwerk/E503504> a nfdicore:Software ;
    rdfs:label "hiPhive" ;
    nfdicore:programmingLanguage <http://demo.fiz-karlsruhe.de/matwerk/E836279> ;
    dcterms:description "hiPhive is a tool for efficiently extracting high-order force constants from atomistic simulations, most commonly density functional theory calculations."^^xsd:string ;
    mwo:hasRepository <http://demo.fiz-karlsruhe.de/matwerk/E200397> ;
    mwo:hasVersion "1.13.1" ;
    mwo:hasWebsite <http://demo.fiz-karlsruhe.de/matwerk/E127757> ;
    ns3:has_license <http://demo.fiz-karlsruhe.de/matwerk/E759297> ;
    schema:citation <http://demo.fiz-karlsruhe.de/matwerk/E940136> .

<http://demo.fiz-karlsruhe.de/matwerk/E504507> a nfdicore:Software ;
    rdfs:label "WulffPack" ;
    nfdicore:programmingLanguage <http://demo.fiz-karlsruhe.de/matwerk/E836279> ;
    dcterms:description "WulffPack is a Python package for making Wulff constructions, typically for finding equilibrium shapes of nanoparticles. WulffPack constructs both continuum models and atomistic structures for further modeling with, e.g., molecular dynamics or density functional theory."^^xsd:string ;
    mwo:hasRepository <http://demo.fiz-karlsruhe.de/matwerk/E201029> ;
    mwo:hasVersion "1.2" ;
    mwo:hasWebsite <http://demo.fiz-karlsruhe.de/matwerk/E128261> ;
    ns3:has_license <http://demo.fiz-karlsruhe.de/matwerk/E786632> ;
    schema:citation <http://demo.fiz-karlsruhe.de/matwerk/E941507> .

<http://demo.fiz-karlsruhe.de/matwerk/E505511> a nfdicore:Software ;
    rdfs:label "dynasor" ;
    dcterms:description "dynasor is a simple tool for calculating total and partial dynamical structure factors as well as current correlation functions from molecular dynamics (MD) simulations."^^xsd:string ;
    mwo:hasRepository <http://demo.fiz-karlsruhe.de/matwerk/E201662> ;
    mwo:hasWebsite <http://demo.fiz-karlsruhe.de/matwerk/E128766> ;
    ns3:has_license <http://demo.fiz-karlsruhe.de/matwerk/E759297> ;
    schema:citation <http://demo.fiz-karlsruhe.de/matwerk/E942879> .

<http://demo.fiz-karlsruhe.de/matwerk/E506516> a nfdicore:Software ;
    rdfs:label "The Science Hub for Atomic-scale Research at Chalmers" ;
    dcterms:description "Dielectric functions of metallic alloys calculated with time-dependent density functional theory.  Atoms under pressure - Electron configuration and electronegativity of the atoms under compression.  Wulff construction - The classic method for calculating equilibrium nanoparticle shapes in a modern setting. SQS – Generate special quasirandom atomic structures with a few clicks in your browser."^^xsd:string ;
    mwo:hasAcronym "sharc"^^xsd:string ;
    mwo:hasWebsite <http://demo.fiz-karlsruhe.de/matwerk/E129272> ;
    schema:operatingSystem ns3:SWO_0000021 .

<http://demo.fiz-karlsruhe.de/matwerk/E507522> a nfdicore:Software ;
    rdfs:label "Vcsgc-lammps" ;
    dcterms:description "The vcsgc-lammps package is an extension for the popular molecular dynamics code LAMMPS, which enables efficient Monte Carlo simulations in the semi-grand-canonical (SGC) and variance constrained SGC ensembles."^^xsd:string ;
    mwo:hasRepository <http://demo.fiz-karlsruhe.de/matwerk/E202296> ;
    mwo:hasWebsite <http://demo.fiz-karlsruhe.de/matwerk/E129779> ;
    schema:citation <http://demo.fiz-karlsruhe.de/matwerk/E944252> .

<http://demo.fiz-karlsruhe.de/matwerk/E508529> a nfdicore:Software ;
    rdfs:label "kanapy" ;
    dcterms:description "Kanapy is a python package for generating three-dimensional synthetic polycrystals based on characteristic microstructural features."^^xsd:string ;
    mwo:hasContactPoint <http://demo.fiz-karlsruhe.de/matwerk/E12176> ;
    mwo:hasRepository <http://demo.fiz-karlsruhe.de/matwerk/E202931> ;
    mwo:hasVersion "2.0.0" ;
    ns3:has_license <http://demo.fiz-karlsruhe.de/matwerk/E791654> .

<http://demo.fiz-karlsruhe.de/matwerk/E509537> a nfdicore:Software ;
    rdfs:label "Python Laboratory for Finite Element Analysis" ;
    dcterms:description "The pyLabFEA package introduces a simple version of FEA for solid mechanics and elastic-plastic materials, which is fully written in Python. Due to its simplicity, it is well-suited for teaching, and its flexibility in constitutive modeling of materials makes it a useful research tool."^^xsd:string ;
    mwo:hasAcronym "pyLabFEA"^^xsd:string ;
    mwo:hasContactPoint <http://demo.fiz-karlsruhe.de/matwerk/E12176> ;
    mwo:hasDocumentation <http://demo.fiz-karlsruhe.de/matwerk/E275171> ;
    mwo:hasRepository <http://demo.fiz-karlsruhe.de/matwerk/E203567> ;
    ns3:has_license <http://demo.fiz-karlsruhe.de/matwerk/E792912> .

<http://demo.fiz-karlsruhe.de/matwerk/E510546> a nfdicore:Software ;
    rdfs:label "Pyrho" ;
    dcterms:description "Pyrho is a real-space DFT code written in Python. It is not built to be super-fast or scalable- instead, it is built to be super-readable.  There's a tutorial notebook (tutorial.ipynb) to guide you through the process of building Pyrho from scratch (starting with the 1D Schroedinger equation). This notebook is based on interactive lectures given by Prof. Joerg Neugebauer."^^xsd:string ;
    mwo:hasRepository <http://demo.fiz-karlsruhe.de/matwerk/E204204> ;
    ns3:has_license <http://demo.fiz-karlsruhe.de/matwerk/E794171> .

<http://demo.fiz-karlsruhe.de/matwerk/E512567> a nfdicore:Software ;
    rdfs:label "Aachen (Aix) Virtual Platform for Materials Processing" ;
    dcterms:description "AixViPMaP is a platform on which different software tools in the field of material and process simulation can be coupled efficiently and effectively."^^xsd:string ;
    mwo:hasAcronym "AixViPMaP"^^xsd:string ;
    mwo:hasContactPoint <http://demo.fiz-karlsruhe.de/matwerk/E704892> ;
    mwo:hasRepository <http://demo.fiz-karlsruhe.de/matwerk/E205481> ;
    mwo:hasWebsite <http://demo.fiz-karlsruhe.de/matwerk/E130287> ;
    schema:citation <http://demo.fiz-karlsruhe.de/matwerk/E947001> .

<http://demo.fiz-karlsruhe.de/matwerk/E513579> a nfdicore:Software ;
    rdfs:label "MuPIF" ;
    dcterms:description "MuPIF is open-source, modular, object-oriented integration platform allowing to create complex, distributed, multiphysics simulation workflows across the scales and processing chains by combining existing simulation tools. "^^xsd:string ;
    mwo:hasRepository <http://demo.fiz-karlsruhe.de/matwerk/E206121> ;
    mwo:hasVersion "2.0.0" ;
    mwo:hasWebsite <http://demo.fiz-karlsruhe.de/matwerk/E130796> ;
    ns3:has_license <http://demo.fiz-karlsruhe.de/matwerk/E796692> ;
    schema:citation <http://demo.fiz-karlsruhe.de/matwerk/E948377> .

<http://demo.fiz-karlsruhe.de/matwerk/E514592> a nfdicore:Software ;
    rdfs:label "SimPhoNy" ;
    dcterms:description "Simulation framework for multi-scale phenomena in micro- and nanosystems"^^xsd:string ;
    mwo:hasRepository <http://demo.fiz-karlsruhe.de/matwerk/E206762> ;
    mwo:hasWebsite <http://demo.fiz-karlsruhe.de/matwerk/E131306> .

<http://demo.fiz-karlsruhe.de/matwerk/E515606> a nfdicore:Software ;
    rdfs:label "MpCCI" ;
    dcterms:description "The MpCCI interface software is a vendor neutral solution for co-simulation and file-based data transfer. MpCCI supports a growing number of commercial as well as research simulation tools in different engineering disciplines."^^xsd:string ;
    mwo:hasWebsite <http://demo.fiz-karlsruhe.de/matwerk/E131817> ;
    ns3:has_license <http://demo.fiz-karlsruhe.de/matwerk/E797954> .

<http://demo.fiz-karlsruhe.de/matwerk/E516621> a nfdicore:Software ;
    rdfs:label "Virtual materials Marketplace" ;
    dcterms:description "VIMMP Marketplace facilitates and promotes the exchange between all materials modelling stakeholders for the benefit of increased innovation in the European manufacturing industry."^^xsd:string ;
    mwo:hasAcronym "VIMMP"^^xsd:string ;
    mwo:hasWebsite <http://demo.fiz-karlsruhe.de/matwerk/E132329> .

<http://demo.fiz-karlsruhe.de/matwerk/E517637> a nfdicore:Software ;
    rdfs:label "Open Model" ;
    dcterms:description "OpenModel aims to design, create, provide, and maintain a sustainable integrated open platform for innovation which delivers predictable, validated, and traceable simulation workflows integrating seamlessly third-party physics-based models, solvers, post-processors and databases."^^xsd:string ;
    mwo:hasContactPoint <http://demo.fiz-karlsruhe.de/matwerk/E17654> ;
    mwo:hasWebsite <http://demo.fiz-karlsruhe.de/matwerk/E132842> .

<http://demo.fiz-karlsruhe.de/matwerk/E518654> a nfdicore:Software ;
    rdfs:label "Cluster GB" ;
    dcterms:description "ClusterGB is a set of Python scripts designed to facilitate easy calculations of planar grain boundaries (GBs) using LAMMPS. In order to accommodate even low-symmetry boundaries, ClusterGB uses vacuum clusters to eliminate the need for periodic boundary conditions."^^xsd:string ;
    mwo:hasRepository <http://demo.fiz-karlsruhe.de/matwerk/E207404> ;
    ns3:has_license <http://demo.fiz-karlsruhe.de/matwerk/E759297> ;
    schema:citation <http://demo.fiz-karlsruhe.de/matwerk/E949754> ;
    schema:operatingSystem ns3:SWO_0000020 .

<http://demo.fiz-karlsruhe.de/matwerk/E519672> a nfdicore:Software ;
    rdfs:label "DIST toolkit" ;
    dcterms:description "Generate atomic structures for common defects in materials"^^xsd:string ;
    mwo:hasRepository <http://demo.fiz-karlsruhe.de/matwerk/E208047> ;
    mwo:hasVersion "1" ;
    ns3:has_license <http://demo.fiz-karlsruhe.de/matwerk/E794171> ;
    schema:citation <http://demo.fiz-karlsruhe.de/matwerk/E951132> .

<http://demo.fiz-karlsruhe.de/matwerk/E520691> a nfdicore:Software ;
    rdfs:label "GB_code" ;
    dcterms:description "This python package helps you create orthogonal grain boundary supercells for atomistic calculations. The code is based on the coincident site lattice (CSL) formulations for cubic materials (sc, bcc, fcc, diamond). The code produces a final structure to be read in LAMMPS or VASP."^^xsd:string ;
    mwo:hasRepository <http://demo.fiz-karlsruhe.de/matwerk/E208691> ;
    mwo:hasVersion "1.0.2" ;
    ns3:has_license <http://demo.fiz-karlsruhe.de/matwerk/E759297> ;
    schema:citation <http://demo.fiz-karlsruhe.de/matwerk/E952511> .

<http://demo.fiz-karlsruhe.de/matwerk/E521711> a nfdicore:Software ;
    rdfs:label "paraprobe-toolbox" ;
    dcterms:description "Strong-scaling distributed- and shared-memory CPU-parallelized tools for mining atom probe tomography data and GPU-parallelized tools for atom probe crystallography."^^xsd:string ;
    mwo:hasDocumentation <http://demo.fiz-karlsruhe.de/matwerk/E276654> ;
    mwo:hasRepository <http://demo.fiz-karlsruhe.de/matwerk/E209336> ;
    ns3:has_license <http://demo.fiz-karlsruhe.de/matwerk/E762996> ;
    schema:citation <http://demo.fiz-karlsruhe.de/matwerk/E953891> .

<http://demo.fiz-karlsruhe.de/matwerk/E522732> a nfdicore:Software ;
    rdfs:label "pySTEM" ;
    dcterms:description "Automatic segmentation of Scanning Transmission Electron Microscope (STEM) images with unsupervised machine learning"^^xsd:string ;
    mwo:hasRepository <http://demo.fiz-karlsruhe.de/matwerk/E209982> ;
    ns3:has_license <http://demo.fiz-karlsruhe.de/matwerk/E762996> ;
    schema:citation <http://demo.fiz-karlsruhe.de/matwerk/E955272> .

<http://demo.fiz-karlsruhe.de/matwerk/E523754> a nfdicore:Software ;
    rdfs:label "Stabix" ;
    dcterms:description "A Matlab toolbox to analyze slip transfer through grain boundaries"^^xsd:string ;
    mwo:hasDocumentation <http://demo.fiz-karlsruhe.de/matwerk/E277397> ;
    mwo:hasRepository <http://demo.fiz-karlsruhe.de/matwerk/E210629> ;
    mwo:hasVersion "2" ;
    ns3:has_license <http://demo.fiz-karlsruhe.de/matwerk/E791654> ;
    schema:citation <http://demo.fiz-karlsruhe.de/matwerk/E956654> .

<http://demo.fiz-karlsruhe.de/matwerk/E524777> a nfdicore:Software ;
    rdfs:label "Voro++" ;
    dcterms:description "Voro++ is a open source software library for the computation of the Voronoi diagram, a widely-used tessellation that has applications in many scientific fields."^^xsd:string ;
    mwo:hasContactPoint <http://demo.fiz-karlsruhe.de/matwerk/E18767> ;
    mwo:hasDocumentation <http://demo.fiz-karlsruhe.de/matwerk/E278141> ;
    mwo:hasVersion "0.4.6" ;
    mwo:hasWebsite <http://demo.fiz-karlsruhe.de/matwerk/E133356> ;
    ns3:has_license <http://demo.fiz-karlsruhe.de/matwerk/E747032> ;
    schema:citation <http://demo.fiz-karlsruhe.de/matwerk/E958037> ;
    schema:operatingSystem ns3:SWO_0000022,
        ns3:SWO_0000149,
        ns3:SWO_9000072 .

<http://demo.fiz-karlsruhe.de/matwerk/E525801> a nfdicore:Software ;
    rdfs:label "Qhull" ;
    dcterms:description "Qhull computes the convex hull, Delaunay triangulation, Voronoi diagram, halfspace intersection about a point, furthest-site Delaunay triangulation, and furthest-site Voronoi diagram. The source code runs in 2-d, 3-d, 4-d, and higher dimensions. "^^xsd:string ;
    mwo:hasContactPoint <http://demo.fiz-karlsruhe.de/matwerk/E708456> ;
    mwo:hasDocumentation <http://demo.fiz-karlsruhe.de/matwerk/E278886> ;
    mwo:hasVersion "2020.2" ;
    mwo:hasWebsite <http://demo.fiz-karlsruhe.de/matwerk/E133871> ;
    ns3:has_license <http://demo.fiz-karlsruhe.de/matwerk/E799217> ;
    schema:citation <http://demo.fiz-karlsruhe.de/matwerk/E959421> ;
    schema:operatingSystem ns3:SWO_0000022,
        ns3:SWO_0000149,
        ns3:SWO_9000072 .

<http://demo.fiz-karlsruhe.de/matwerk/E526826> a nfdicore:Software ;
    rdfs:label "Pasta ELN" ;
    dcterms:description "This ELN combines raw-data with rich metadata to allow advanced data science. In the database, one can fully adapt and improvise the metadata definitions to generate something novel. PASTA uses a local-first approach: store all data and metadata locally (always accessible to user) and synchronize with a server upon user request."^^xsd:string ;
    mwo:hasRepository <http://demo.fiz-karlsruhe.de/matwerk/E211277> ;
    mwo:hasVersion "1.2.2" ;
    mwo:hasWebsite <http://demo.fiz-karlsruhe.de/matwerk/E134387> ;
    ns3:has_license <http://demo.fiz-karlsruhe.de/matwerk/E759297> ;
    schema:operatingSystem ns3:SWO_0000022,
        ns3:SWO_0000149,
        ns3:SWO_9000072 .

<http://demo.fiz-karlsruhe.de/matwerk/E527852> a nfdicore:Software ;
    rdfs:label "eLabFTW" ;
    dcterms:description "eLabFTW is an electronic lab notebook manager for research teams. It lets you store and organize your research experiments easily. It also features a database where any kind of objects (such as antibodies, plasmids, cell lines, boxes, etc.) can be stored. It is accessed via the browser"^^xsd:string ;
    mwo:hasDocumentation <http://demo.fiz-karlsruhe.de/matwerk/E279632> ;
    mwo:hasRepository <http://demo.fiz-karlsruhe.de/matwerk/E211926> ;
    mwo:hasVersion "4.3.9" ;
    mwo:hasWebsite <http://demo.fiz-karlsruhe.de/matwerk/E134904> ;
    ns3:has_license <http://demo.fiz-karlsruhe.de/matwerk/E791654> ;
    owl:sameAs <http://www.wikidata.org/entity/Q85758859> ;
    schema:operatingSystem ns3:SWO_0000022,
        ns3:SWO_0000149,
        ns3:SWO_9000072 .

<http://demo.fiz-karlsruhe.de/matwerk/E528879> a nfdicore:Software ;
    rdfs:label "Karlsruhe Data Infrastructure for Materials Science" ;
    dcterms:description "The focus on the repository component is on warm data, i.e. unpublished data that is yet to be analysed further, while in the ELN component it is on the automated and documented execution of heterogeneous workflows. The components are therefore best described as community repository and ELN 2.0 respectively. In this way, a virtual research environment is created that facilitates collaboration between researchers. "^^xsd:string ;
    mwo:hasAcronym "Kadi4Mat"^^xsd:string ;
    mwo:hasDocumentation <http://demo.fiz-karlsruhe.de/matwerk/E280379> ;
    mwo:hasRepository <http://demo.fiz-karlsruhe.de/matwerk/E212576> ;
    mwo:hasVersion "0.26.0" ;
    mwo:hasWebsite <http://demo.fiz-karlsruhe.de/matwerk/E135422> ;
    ns3:has_license <http://demo.fiz-karlsruhe.de/matwerk/E800481> ;
    schema:citation <http://demo.fiz-karlsruhe.de/matwerk/E960806> .

<http://demo.fiz-karlsruhe.de/matwerk/E529907> a nfdicore:Software ;
    rdfs:label "Metador" ;
    dcterms:description "File uplad service with resumable uploads and rich metadata requirements"^^xsd:string ;
    mwo:hasDocumentation <http://demo.fiz-karlsruhe.de/matwerk/E281127> ;
    mwo:hasRepository <http://demo.fiz-karlsruhe.de/matwerk/E213227> ;
    ns3:has_license <http://demo.fiz-karlsruhe.de/matwerk/E759297> ;
    schema:operatingSystem ns3:SWO_0000021 .

<http://demo.fiz-karlsruhe.de/matwerk/E530936> a nfdicore:Software ;
    rdfs:label "Atomsk" ;
    mwo:hasWebsite <http://demo.fiz-karlsruhe.de/matwerk/E135941> .

<http://demo.fiz-karlsruhe.de/matwerk/E531966> a nfdicore:Software ;
    rdfs:label "Atomman" ;
    mwo:hasWebsite <http://demo.fiz-karlsruhe.de/matwerk/E136461> .

<http://demo.fiz-karlsruhe.de/matwerk/E532997> a nfdicore:Software ;
    rdfs:label "iprPy High Throughput Computational Framework" ;
    mwo:hasWebsite <http://demo.fiz-karlsruhe.de/matwerk/E136982> .

<http://demo.fiz-karlsruhe.de/matwerk/E534029> a nfdicore:Software ;
    rdfs:label "Kim API" ;
    mwo:hasWebsite <http://demo.fiz-karlsruhe.de/matwerk/E137504> ;
    schema:citation <http://demo.fiz-karlsruhe.de/matwerk/E962192> .

<http://demo.fiz-karlsruhe.de/matwerk/E536096> a nfdicore:Software ;
    rdfs:label "FireWorks" ;
    mwo:hasWebsite <http://demo.fiz-karlsruhe.de/matwerk/E138551> .

<http://demo.fiz-karlsruhe.de/matwerk/E538167> a nfdicore:Software ;
    rdfs:label "EMMOntoPy" ;
    dcterms:description "Python API for the Elemental Multiperspective Material Ontology (EMMO)."^^xsd:string ;
    mwo:hasRepository <http://demo.fiz-karlsruhe.de/matwerk/E213879> ;
    mwo:hasWebsite <http://demo.fiz-karlsruhe.de/matwerk/E139602> .

<http://demo.fiz-karlsruhe.de/matwerk/E539204> a nfdicore:Software ;
    rdfs:label "yambo" ;
    mwo:hasWebsite <http://demo.fiz-karlsruhe.de/matwerk/E140129> .

<http://demo.fiz-karlsruhe.de/matwerk/E540242> a nfdicore:Software ;
    rdfs:label "wannier90" ;
    mwo:hasWebsite <http://demo.fiz-karlsruhe.de/matwerk/E140657> .

<http://demo.fiz-karlsruhe.de/matwerk/E541281> a nfdicore:Software ;
    rdfs:label "The High-Throughput Toolkit (httk)" ;
    mwo:hasDocumentation <http://demo.fiz-karlsruhe.de/matwerk/E281876> ;
    mwo:hasRelatedResource <http://demo.fiz-karlsruhe.de/matwerk/E643412> .

<http://demo.fiz-karlsruhe.de/matwerk/E542321> a nfdicore:Software ;
    rdfs:label "SIRIUS" ;
    mwo:hasRepository <http://demo.fiz-karlsruhe.de/matwerk/E214532> .

<http://demo.fiz-karlsruhe.de/matwerk/E544404> a nfdicore:Software ;
    rdfs:label "Coscine" ;
    mwo:hasWebsite <http://demo.fiz-karlsruhe.de/matwerk/E141716> .

<http://demo.fiz-karlsruhe.de/matwerk/E545447> a nfdicore:Software ;
    rdfs:label "kadi-apy" ;
    mwo:hasRepository <http://demo.fiz-karlsruhe.de/matwerk/E212576> .

<http://demo.fiz-karlsruhe.de/matwerk/E547536> a nfdicore:Software ;
    rdfs:label "Materials Project API" ;
    mwo:hasDocumentation <http://demo.fiz-karlsruhe.de/matwerk/E284129> .

<http://demo.fiz-karlsruhe.de/matwerk/E548582> a nfdicore:Software ;
    rdfs:label "PyTorch" ;
    mwo:hasWebsite <http://demo.fiz-karlsruhe.de/matwerk/E142247> ;
    owl:sameAs <http://www.wikidata.org/entity/Q47509047> .

<http://demo.fiz-karlsruhe.de/matwerk/E549629> a nfdicore:Software ;
    rdfs:label "scikit-learn" ;
    mwo:hasWebsite <http://demo.fiz-karlsruhe.de/matwerk/E142779> ;
    owl:sameAs <http://www.wikidata.org/entity/Q1026367> .

<http://demo.fiz-karlsruhe.de/matwerk/E550677> a nfdicore:Software ;
    rdfs:label "TensorFlow" ;
    mwo:hasWebsite <http://demo.fiz-karlsruhe.de/matwerk/E143312> ;
    owl:sameAs <http://www.wikidata.org/entity/Q21447895> .

<http://demo.fiz-karlsruhe.de/matwerk/E551726> a nfdicore:Software ;
    rdfs:label "OpenBIS" ;
    dcterms:description "The openBIS platform has three primary functionalities: 1. Inventory management of laboratory samples, materials, protocols, equipment. 2. Laboratory notebook, to document lab experiments. 3. Data management, to store all data related to lab experiments (raw, processed, analysed data, scripts, Jupyter notebooks, etc.)."^^xsd:string ;
    mwo:hasContactPoint <http://demo.fiz-karlsruhe.de/matwerk/E683698> ;
    mwo:hasWebsite <http://demo.fiz-karlsruhe.de/matwerk/E143846> ;
    owl:sameAs <http://www.wikidata.org/entity/Q106929673> .

<http://demo.fiz-karlsruhe.de/matwerk/E552776> a nfdicore:Software ;
    rdfs:label "Atomic Simulation Recipes" ;
    nfdicore:programmingLanguage <http://demo.fiz-karlsruhe.de/matwerk/E836279> ;
    dcterms:description """Recipes for Atomic Scale Materials Research. Collection of python recipes for common (and not so common)\r
tasks perfomed in atomic scale materials research. These tasks include\r
relaxation of structures, calculating ground states, calculating band\r
structures, calculating dielectric functions and so on."""^^xsd:string ;
    mwo:hasAcronym "ASR"^^xsd:string ;
    mwo:hasRelatedResource <http://demo.fiz-karlsruhe.de/matwerk/E641147> ;
    mwo:hasRepository <http://demo.fiz-karlsruhe.de/matwerk/E215841> .

<http://demo.fiz-karlsruhe.de/matwerk/E553827> a nfdicore:Software,
        mwo:ResearchSoftware ;
    rdfs:label "TURBOMOLE" ;
    dcterms:description "Program Package for Electronic Structure Calculations"^^xsd:string ;
    mwo:hasContributor <http://demo.fiz-karlsruhe.de/matwerk/E3851> ;
    mwo:hasDiscipline <http://demo.fiz-karlsruhe.de/matwerk/E70752>,
        <http://demo.fiz-karlsruhe.de/matwerk/E71126>,
        <http://demo.fiz-karlsruhe.de/matwerk/E71501> ;
    mwo:hasDocumentation <http://demo.fiz-karlsruhe.de/matwerk/E284882> ;
    mwo:hasVersion "7.6" ;
    mwo:hasWebsite <http://demo.fiz-karlsruhe.de/matwerk/E144381> ;
    mwo:usesMethod <http://demo.fiz-karlsruhe.de/matwerk/E623171>,
        <http://demo.fiz-karlsruhe.de/matwerk/E624287> ;
    owl:sameAs <http://www.wikidata.org/entity/Q2385566> ;
    schema:citation <http://demo.fiz-karlsruhe.de/matwerk/E963579> ;
    schema:operatingSystem ns3:SWO_0000022,
        ns3:SWO_0000149,
        ns3:SWO_9000072 .

<http://demo.fiz-karlsruhe.de/matwerk/E554879> a nfdicore:Software ;
    rdfs:label "DREAM.3D" ;
    mwo:hasWebsite <http://demo.fiz-karlsruhe.de/matwerk/E144917> .

<http://demo.fiz-karlsruhe.de/matwerk/E555932> a nfdicore:Software ;
    rdfs:label "MTEX" ;
    mwo:hasWebsite <http://demo.fiz-karlsruhe.de/matwerk/E145454> .

<http://demo.fiz-karlsruhe.de/matwerk/E556986> a nfdicore:Software ;
    rdfs:label "Gmsh" ;
    mwo:hasWebsite <http://demo.fiz-karlsruhe.de/matwerk/E145992> ;
    owl:sameAs <http://www.wikidata.org/entity/Q3109412> .

<http://demo.fiz-karlsruhe.de/matwerk/E558041> a nfdicore:Software ;
    rdfs:label "Neper" ;
    mwo:hasWebsite <http://demo.fiz-karlsruhe.de/matwerk/E146531> .

<http://demo.fiz-karlsruhe.de/matwerk/E559097> a nfdicore:Software ;
    rdfs:label "PETSc" ;
    mwo:hasWebsite <http://demo.fiz-karlsruhe.de/matwerk/E147071> ;
    owl:sameAs <http://www.wikidata.org/entity/Q4047262> .

<http://demo.fiz-karlsruhe.de/matwerk/E560154> a nfdicore:Software ;
    rdfs:label "deal.II" ;
    mwo:hasWebsite <http://demo.fiz-karlsruhe.de/matwerk/E147612> ;
    owl:sameAs <http://www.wikidata.org/entity/Q5245828> .

<http://demo.fiz-karlsruhe.de/matwerk/E561212> a nfdicore:Software ;
    rdfs:label "DUNE-FEM" ;
    mwo:hasRepository <http://demo.fiz-karlsruhe.de/matwerk/E216497> .

<http://demo.fiz-karlsruhe.de/matwerk/E562271> a nfdicore:Software ;
    rdfs:label "Firedrake" ;
    mwo:hasWebsite <http://demo.fiz-karlsruhe.de/matwerk/E148154> .

<http://demo.fiz-karlsruhe.de/matwerk/E563331> a nfdicore:Software ;
    rdfs:label "FreeFEM" ;
    mwo:hasWebsite <http://demo.fiz-karlsruhe.de/matwerk/E148697> .

<http://demo.fiz-karlsruhe.de/matwerk/E564392> a nfdicore:Software ;
    rdfs:label "hIPPYlib" ;
    mwo:hasWebsite <http://demo.fiz-karlsruhe.de/matwerk/E149241> .

<http://demo.fiz-karlsruhe.de/matwerk/E565454> a nfdicore:Software ;
    rdfs:label "MoFEM" ;
    mwo:hasWebsite <http://demo.fiz-karlsruhe.de/matwerk/E149786> .

<http://demo.fiz-karlsruhe.de/matwerk/E566517> a nfdicore:Software ;
    rdfs:label "OOFEM" ;
    mwo:hasWebsite <http://demo.fiz-karlsruhe.de/matwerk/E150332> ;
    owl:sameAs <http://www.wikidata.org/entity/Q7072787> .

<http://demo.fiz-karlsruhe.de/matwerk/E567581> a nfdicore:Software ;
    rdfs:label "preCICE" ;
    mwo:hasWebsite <http://demo.fiz-karlsruhe.de/matwerk/E150879> ;
    owl:sameAs <http://www.wikidata.org/entity/Q67123602> .

<http://demo.fiz-karlsruhe.de/matwerk/E568646> a nfdicore:Software ;
    rdfs:label "Clawpack" ;
    mwo:hasWebsite <http://demo.fiz-karlsruhe.de/matwerk/E151427> .

<http://demo.fiz-karlsruhe.de/matwerk/E569712> a nfdicore:Software ;
    rdfs:label "aviary" ;
    mwo:hasRepository <http://demo.fiz-karlsruhe.de/matwerk/E217154> .

<http://demo.fiz-karlsruhe.de/matwerk/E570779> a nfdicore:Software ;
    rdfs:label "BIOVIA Materials Studio" ;
    mwo:hasWebsite <http://demo.fiz-karlsruhe.de/matwerk/E151976> .

<http://demo.fiz-karlsruhe.de/matwerk/E571847> a nfdicore:Software ;
    rdfs:label "Computational Autonomy for Materials Discovery" ;
    mwo:hasAcronym "CAMD"^^xsd:string ;
    mwo:hasRepository <http://demo.fiz-karlsruhe.de/matwerk/E217812> .

<http://demo.fiz-karlsruhe.de/matwerk/E572916> a nfdicore:Software ;
    rdfs:label "Compositionally-Restricted Attention-Based Network" ;
    mwo:hasAcronym "CrabNet"^^xsd:string ;
    mwo:hasRepository <http://demo.fiz-karlsruhe.de/matwerk/E218471> .

<http://demo.fiz-karlsruhe.de/matwerk/E573986> a nfdicore:Software ;
    rdfs:label "cclib" ;
    mwo:hasWebsite <http://demo.fiz-karlsruhe.de/matwerk/E152526> .

<http://demo.fiz-karlsruhe.de/matwerk/E575057> a nfdicore:Software ;
    rdfs:label "cctbx" ;
    mwo:hasWebsite <http://demo.fiz-karlsruhe.de/matwerk/E153077> .

<http://demo.fiz-karlsruhe.de/matwerk/E576129> a nfdicore:Software ;
    rdfs:label "Datamol" ;
    mwo:hasRepository <http://demo.fiz-karlsruhe.de/matwerk/E219131> .

<http://demo.fiz-karlsruhe.de/matwerk/E577202> a nfdicore:Software ;
    rdfs:label "matador" ;
    mwo:hasRepository <http://demo.fiz-karlsruhe.de/matwerk/E219792> .

<http://demo.fiz-karlsruhe.de/matwerk/E578276> a nfdicore:Software ;
    rdfs:label "mat_discover" ;
    mwo:hasWebsite <http://demo.fiz-karlsruhe.de/matwerk/E153629> .

<http://demo.fiz-karlsruhe.de/matwerk/E579351> a nfdicore:Software ;
    rdfs:label "NIST Materials Data Curation System" ;
    mwo:hasAcronym "MDCS"^^xsd:string ;
    mwo:hasWebsite <http://demo.fiz-karlsruhe.de/matwerk/E154182> .

<http://demo.fiz-karlsruhe.de/matwerk/E580427> a nfdicore:Software ;
    rdfs:label "MedeA" ;
    mwo:hasWebsite <http://demo.fiz-karlsruhe.de/matwerk/E154736> .

<http://demo.fiz-karlsruhe.de/matwerk/E581504> a nfdicore:Software ;
    rdfs:label "Material Optimal Descriptor Network" ;
    mwo:hasAcronym "MODNet"^^xsd:string ;
    mwo:hasRepository <http://demo.fiz-karlsruhe.de/matwerk/E220454> .

<http://demo.fiz-karlsruhe.de/matwerk/E582582> a nfdicore:Software ;
    rdfs:label "Organizing Assistant for Comprehensive and Interactive Simulations" ;
    mwo:hasAcronym "OACIS"^^xsd:string ;
    mwo:hasWebsite <http://demo.fiz-karlsruhe.de/matwerk/E155291> .

<http://demo.fiz-karlsruhe.de/matwerk/E583661> a nfdicore:Software,
        ns3:SWO_0000001 ;
    rdfs:label "OPTIMADE python tools" ;
    mwo:hasRepository <http://demo.fiz-karlsruhe.de/matwerk/E221117> .

<http://demo.fiz-karlsruhe.de/matwerk/E584741> a nfdicore:Software ;
    rdfs:label "piro" ;
    mwo:hasRepository <http://demo.fiz-karlsruhe.de/matwerk/E221781> .

<http://demo.fiz-karlsruhe.de/matwerk/E585822> a nfdicore:Software ;
    rdfs:label "Pymatflow" ;
    mwo:hasRepository <http://demo.fiz-karlsruhe.de/matwerk/E222446> .

<http://demo.fiz-karlsruhe.de/matwerk/E586904> a nfdicore:Software ;
    rdfs:label "PyMKS" ;
    mwo:hasRepository <http://demo.fiz-karlsruhe.de/matwerk/E223112> .

<http://demo.fiz-karlsruhe.de/matwerk/E587987> a nfdicore:Software ;
    rdfs:label "QMFlows" ;
    mwo:hasRepository <http://demo.fiz-karlsruhe.de/matwerk/E223779> .

<http://demo.fiz-karlsruhe.de/matwerk/E589071> a nfdicore:Software ;
    rdfs:label "RDKit" ;
    mwo:hasRepository <http://demo.fiz-karlsruhe.de/matwerk/E224447> ;
    owl:sameAs <http://www.wikidata.org/entity/Q54152347> .

<http://demo.fiz-karlsruhe.de/matwerk/E590156> a nfdicore:Software ;
    rdfs:label "Simulation Environment for Atomistic and Molecular Modeling" ;
    mwo:hasAcronym "SEAMM"^^xsd:string ;
    mwo:hasWebsite <http://demo.fiz-karlsruhe.de/matwerk/E155847> .

<http://demo.fiz-karlsruhe.de/matwerk/E591242> a nfdicore:Software ;
    rdfs:label "Tilde" ;
    mwo:hasRepository <http://demo.fiz-karlsruhe.de/matwerk/E225116> .

<http://demo.fiz-karlsruhe.de/matwerk/E593417> a nfdicore:Software ;
    rdfs:label "ro-crate-py" ;
    nfdicore:programmingLanguage <http://demo.fiz-karlsruhe.de/matwerk/E836279> ;
    dcterms:description "ro-crate-py is a Python library to create and consume Research Object Crates. It currently supports the RO-Crate 1.1 specification."^^xsd:string ;
    mwo:hasRelatedResource <http://demo.fiz-karlsruhe.de/matwerk/E646817> ;
    mwo:hasRepository <http://demo.fiz-karlsruhe.de/matwerk/E225786> ;
    mwo:hasVersion "0.7.0" ;
    ns3:has_license <http://demo.fiz-karlsruhe.de/matwerk/E801746> ;
    schema:citation <http://demo.fiz-karlsruhe.de/matwerk/E964967> .

<http://demo.fiz-karlsruhe.de/matwerk/E594506> a nfdicore:Software ;
    rdfs:label "Simmate" ;
    dcterms:description "The Simulated Materials Ecosystem (Simmate) is a toolbox and framework for computational materials research. It lets you explore various crystal databases, predict new materials, and quickly calculate properties."^^xsd:string ;
    mwo:hasDocumentation <http://demo.fiz-karlsruhe.de/matwerk/E285636> ;
    mwo:hasRepository <http://demo.fiz-karlsruhe.de/matwerk/E226457> ;
    mwo:hasWebsite <http://demo.fiz-karlsruhe.de/matwerk/E156962> .

<http://demo.fiz-karlsruhe.de/matwerk/E595596> a nfdicore:Software,
        ns3:SWO_0000001 ;
    rdfs:label "Materials Data Curation System" ;
    dcterms:description "The NIST Materials Data Curation System (MDCS) provides a means for capturing, sharing, and transforming materials data into a structured format that is XML based amenable to transformation to other formats. The data are organized using user-selected templates encoded in XML Schema. These templates are used to create data entry forms. The documents are saved in a non-relational (NoSQL) database, namely MongoDB. The data can be searched and retrieved by a template-driven web-based form or by a RESTful API call. The system also enables the interconnection of MDCS repositories for federated searches."^^xsd:string ;
    mwo:hasRepository <http://demo.fiz-karlsruhe.de/matwerk/E154182> .

<http://demo.fiz-karlsruhe.de/matwerk/E596687> a nfdicore:Software ;
    rdfs:label "MAterials Simulation Toolkit (MAST)" ;
    mwo:hasWebsite <http://demo.fiz-karlsruhe.de/matwerk/E157521> .

<http://demo.fiz-karlsruhe.de/matwerk/E597779> a nfdicore:Software ;
    rdfs:label "DiffPy" ;
    dcterms:description "A free and open source software project to provide python software for diffraction analysis and the study of the atomic structure of materials."^^xsd:string ;
    mwo:hasWebsite <http://demo.fiz-karlsruhe.de/matwerk/E158081> .

<http://demo.fiz-karlsruhe.de/matwerk/E598872> a nfdicore:Software ;
    rdfs:label "pyDOE" ;
    mwo:hasWebsite <http://demo.fiz-karlsruhe.de/matwerk/E158642> .

<http://demo.fiz-karlsruhe.de/matwerk/E599966> a nfdicore:Software ;
    rdfs:label "NeXpy" ;
    mwo:hasRepository <http://demo.fiz-karlsruhe.de/matwerk/E227129> .

<http://demo.fiz-karlsruhe.de/matwerk/E601061> a nfdicore:Software ;
    rdfs:label "TomoPy" ;
    mwo:hasRepository <http://demo.fiz-karlsruhe.de/matwerk/E227802> ;
    owl:sameAs <http://www.wikidata.org/entity/Q22909437> .

<http://demo.fiz-karlsruhe.de/matwerk/E602157> a nfdicore:Software ;
    rdfs:label "MetaStore2" ;
    dcterms:description "General purpose metadata repository and schema registry service."^^xsd:string ;
    mwo:hasRepository <http://demo.fiz-karlsruhe.de/matwerk/E228476> .

<http://demo.fiz-karlsruhe.de/matwerk/E603254> a nfdicore:Software ;
    rdfs:label "FAIR-DOscope" ;
    nfdicore:programmingLanguage <http://demo.fiz-karlsruhe.de/matwerk/E847952>,
        <http://demo.fiz-karlsruhe.de/matwerk/E849254> ;
    dcterms:description "FAIR-DOscope is an easy-to-use, generic FAIR Digital Object viewer and browser accepting PIDs of FAIR DOs and presenting the associated PID record in a graphical and user-friendly way. It offers a tabular view of the contents of a PID record and a graphical representation of related FAIR DOs."^^xsd:string ;
    mwo:hasDocumentation <http://demo.fiz-karlsruhe.de/matwerk/E286391> ;
    mwo:hasRepository <http://demo.fiz-karlsruhe.de/matwerk/E229151> ;
    ns3:has_license <http://demo.fiz-karlsruhe.de/matwerk/E803012> .

<http://demo.fiz-karlsruhe.de/matwerk/E604352> a nfdicore:Software ;
    rdfs:label "Randspg" ;
    schema:citation <http://demo.fiz-karlsruhe.de/matwerk/E967746> .

<http://demo.fiz-karlsruhe.de/matwerk/E605451> a nfdicore:Software ;
    rdfs:label "Ontopanel" ;
    dcterms:description "Ontopanel is a plugin in diagrams.net that helps domain experts to build ontologies and method graph in a simpler way."^^xsd:string ;
    mwo:hasRepository <http://demo.fiz-karlsruhe.de/matwerk/E229827> .

<http://demo.fiz-karlsruhe.de/matwerk/E606551> a nfdicore:Software ;
    rdfs:label "BEXIS2" ;
    mwo:hasRepository <http://demo.fiz-karlsruhe.de/matwerk/E230504> .

<http://demo.fiz-karlsruhe.de/matwerk/E60686> owl:sameAs <http://www.wikidata.org/entity/Q110262588> .

<http://demo.fiz-karlsruhe.de/matwerk/E607652> a nfdicore:Software ;
    rdfs:label "KIT Data Manager" ;
    mwo:hasRepository <http://demo.fiz-karlsruhe.de/matwerk/E231182> .

<http://demo.fiz-karlsruhe.de/matwerk/E742154> owl:sameAs <http://www.wikidata.org/entity/Q18491847> .

<http://demo.fiz-karlsruhe.de/matwerk/E8876> a nfdicore:Person ;
    rdfs:label "Dr. Amir Laadhar" ;
    mwo:emailAddress "amir.laadhar@mib.uni-stuttgart.de"^^xsd:string ;
    mwo:hasAffiliation <http://demo.fiz-karlsruhe.de/matwerk/E1002> ;
    mwo:hasExpertiseIn <http://demo.fiz-karlsruhe.de/matwerk/E36779>,
        <http://demo.fiz-karlsruhe.de/matwerk/E37047>,
        <http://demo.fiz-karlsruhe.de/matwerk/E37316>,
        <http://demo.fiz-karlsruhe.de/matwerk/E37586> ;
    mwo:hasORCID <https://orcid.org/0000-0001-9106-8825> ;
    foaf:firstName "Amir"^^xsd:string ;
    foaf:surname "Laadhar"^^xsd:string ;
    foaf:title "Dr."^^xsd:string .

<http://demo.fiz-karlsruhe.de/matwerk/E9129> a nfdicore:Person ;
    rdfs:label "Dr. Jürgen Olbricht" ;
    mwo:emailAddress "juergen.olbricht@bam.de"^^xsd:string ;
    mwo:hasAffiliation <http://demo.fiz-karlsruhe.de/matwerk/E1245640> ;
    mwo:hasExpertiseIn <http://demo.fiz-karlsruhe.de/matwerk/E37857> ;
    mwo:hasORCID <https://orcid.org/0000-0002-2296-4930> ;
    foaf:firstName "Jürgen"^^xsd:string ;
    foaf:surname "Olbricht"^^xsd:string ;
    foaf:title "Dr."^^xsd:string .

<http://demo.fiz-karlsruhe.de/matwerk/E9257> a nfdicore:Person ;
    rdfs:label "Prof. Dr.-Ing. Stephan Wulfinghoff" ;
    mwo:emailAddress "swu@tf.uni-kiel.de"^^xsd:string ;
    mwo:hasAffiliation <http://demo.fiz-karlsruhe.de/matwerk/E1011> ;
    mwo:hasExpertiseIn <http://demo.fiz-karlsruhe.de/matwerk/E42042> ;
    foaf:depiction <https://ams3.digitaloceanspaces.com/externalpublic/57/5c733336-78f8-450d-bc38-cceb174c11b1/conversions/7c4cea63-5ebb-41f9-b6ec-1f9220751368-md.jpg?X-Amz-Content-Sha256=UNSIGNED-PAYLOAD&X-Amz-Algorithm=AWS4-HMAC-SHA256&X-Amz-Credential=KVC4ZMO47JLTBHVHEFZ4%2F20230512%2Fams3%2Fs3%2Faws4_request&X-Amz-Date=20230512T150442Z&X-Amz-SignedHeaders=host&X-Amz-Expires=7200&X-Amz-Signature=0f0f194674268b86a9377bcb7fb458791d73ce61e2ec1ac2778feabff1e3b08e> ;
    foaf:firstName "Stephan"^^xsd:string ;
    foaf:surname "Wulfinghoff"^^xsd:string ;
    foaf:title "Prof. Dr.-Ing."^^xsd:string .

<http://demo.fiz-karlsruhe.de/matwerk/E9386> a nfdicore:Person ;
    rdfs:label "Christian Dorn" ;
    mwo:emailAddress "cdo@tf.uni-kiel.de"^^xsd:string ;
    mwo:hasAffiliation <http://demo.fiz-karlsruhe.de/matwerk/E1011> ;
    mwo:hasExpertiseIn <http://demo.fiz-karlsruhe.de/matwerk/E42042> ;
    mwo:hasORCID <https://orcid.org/0000-0002-6426-1029> ;
    foaf:firstName "Christian"^^xsd:string ;
    foaf:surname "Dorn"^^xsd:string .

<http://demo.fiz-karlsruhe.de/matwerk/E9516> a nfdicore:Person ;
    rdfs:label "Thorge Petersen" ;
    mwo:emailAddress "petersen@rz.uni-kiel.de"^^xsd:string ;
    mwo:hasExpertiseIn <http://demo.fiz-karlsruhe.de/matwerk/E38402> ;
    mwo:hasORCID <https://orcid.org/0000-0002-2354-5914> ;
    foaf:firstName "Thorge"^^xsd:string ;
    foaf:surname "Petersen"^^xsd:string .

<http://demo.fiz-karlsruhe.de/matwerk/E9779> a nfdicore:Person ;
    rdfs:label "Dr.  Heike Fliegl" ;
    mwo:emailAddress "heike.fliegl@fiz-karlsruhe.de"^^xsd:string ;
    mwo:hasAffiliation <http://demo.fiz-karlsruhe.de/matwerk/E1016> ;
    mwo:hasExpertiseIn <http://demo.fiz-karlsruhe.de/matwerk/E38676> ;
    mwo:hasORCID <https://orcid.org/0000-0002-7541-115X> ;
    owl:sameAs <http://www.wikidata.org/entity/Q57605303> ;
    foaf:firstName "Heike"^^xsd:string ;
    foaf:surname "Fliegl"^^xsd:string ;
    foaf:title "Dr. "^^xsd:string .

<http://demo.fiz-karlsruhe.de/matwerk/E9912> a nfdicore:Person ;
    rdfs:label "Dr.  Volker Hofmann" ;
    mwo:emailAddress "v.hofmann@fz-juelich.de"^^xsd:string ;
    mwo:hasAffiliation <http://demo.fiz-karlsruhe.de/matwerk/E1022> ;
    mwo:hasExpertiseIn <http://demo.fiz-karlsruhe.de/matwerk/E1245727>,
        <http://demo.fiz-karlsruhe.de/matwerk/E38402> ;
    mwo:hasORCID <https://orcid.org/0000-0002-5149-603X> ;
    owl:sameAs <http://www.wikidata.org/entity/Q84561074> ;
    foaf:firstName "Volker"^^xsd:string ;
    foaf:surname "Hofmann"^^xsd:string ;
    foaf:title "Dr. "^^xsd:string .

emmo:EMMO_967080e5_2f42_4eb2_a3a9_c58143e835f9 a owl:AnnotationProperty .

nfdicore:Consortium a owl:Class ;
    rdfs:label "consortium"@en ;
    nfdicore:example "NFDI4Culture, NFDI-MatWerk, DataPLANT." ;
    rdfs:comment "NFDI consortia grouped by a discipline based in a science-led process managed by the German Research Foundation (DFG)."@en ;
    rdfs:subClassOf nfdicore:Organization .

nfdicore:ControlledVocabulary a nfdicore:SemanticExpressivity,
        owl:NamedIndividual ;
    rdfs:label "controlled vocabulary"@en ;
    rdfs:comment "A list of terms, natural language definitions and naming conventions. In comparisson to a glossary, there is a dedicated curation mechanism for new terms in a controlled vocabulary."@en .

nfdicore:Glossary a nfdicore:SemanticExpressivity,
        owl:NamedIndividual ;
    rdfs:label "glossary"@en ;
    rdfs:comment "A list of terms and their with natural language definitions."@en .

nfdicore:ProvidedResource a owl:Class ;
    rdfs:label "provided resource"@en ;
    rdfs:comment "A ressource that identifies a resource provided to the nfdi."@en ;
    rdfs:subClassOf nfdicore:Resource .

nfdicore:ServiceType a owl:Class ;
    rdfs:label "service type"@en ;
    nfdicore:example "Expertise, advertisement, curation"@en ;
    rdfs:comment "A resource that identifies the type of a service."@en .

nfdicore:Taxonomy a nfdicore:SemanticExpressivity,
        owl:NamedIndividual ;
    rdfs:label "taxonomy"@en ;
    rdfs:comment "A data model in a class hierarchy, where all concepts inherit their behaviour from the super-class concept. Taxonomies can be strict or non strict and can contain instances."@en .

nfdicore:Thesaurus a nfdicore:SemanticExpressivity,
        owl:NamedIndividual ;
    rdfs:label "thesaurus"@en ;
    rdfs:comment "A structured list of terms and relations between the terms, as e.g. broader/narrower."@en .

nfdicore:bestPractice a owl:ObjectProperty ;
    rdfs:label "best practice"@en ;
    rdfs:comment "The property is a relationship between a resource and the best practice."@en ;
    rdfs:domain nfdicore:Resource ;
    rdfs:range nfdicore:Specification ;
    owl:inverseOf nfdicore:bestPracticeOf .

nfdicore:country a owl:ObjectProperty ;
    rdfs:label "country"@en ;
    rdfs:comment "The property relates a city or a state to a country where it is located."@en ;
    rdfs:domain [ a owl:Class ;
            owl:unionOf ( nfdicore:City nfdicore:FederalState ) ] ;
    rdfs:range nfdicore:Country ;
    owl:inverseOf nfdicore:countryOf .

nfdicore:example a owl:AnnotationProperty .

nfdicore:federalState a owl:ObjectProperty ;
    rdfs:label "federal state"@en ;
    rdfs:comment "The property relates a city to a federal state where it is located."@en ;
    rdfs:domain nfdicore:City ;
    rdfs:range nfdicore:FederalState ;
    owl:inverseOf nfdicore:federalStateOf .

nfdicore:fundingOrganisation a owl:ObjectProperty ;
    rdfs:label "funding organisation"@en ;
    rdfs:comment "The property relates a resource or a project to the organisation that provided funding for it."@en ;
    rdfs:domain [ a owl:Class ;
            owl:unionOf ( nfdicore:Project nfdicore:Resource ) ] ;
    rdfs:range nfdicore:Organization ;
    rdfs:subPropertyOf nfdicore:funder ;
    owl:inverseOf nfdicore:fundingOrganisationOf .

nfdicore:location a owl:ObjectProperty ;
    rdfs:label "location"@en ;
    rdfs:comment "The property is a relationship between a thing and a place its located at. "@en ;
    rdfs:domain owl:Thing ;
    rdfs:range nfdicore:Place ;
    owl:inverseOf nfdicore:locationOf .

nfdicore:objectType a owl:ObjectProperty ;
    rdfs:label "object type"@en ;
    rdfs:comment "The property relates a data collection to the type of object it contains. "@en ;
    rdfs:domain nfdicore:Collection ;
    rdfs:range nfdicore:ObjectType ;
    owl:inverseOf nfdicore:objectTypeOf .

nfdicore:parentOrganisation a owl:ObjectProperty ;
    rdfs:label "parent organisation"@en ;
    rdfs:comment "The property is a parental relationship between organisations."@en ;
    rdfs:domain nfdicore:Organization ;
    rdfs:range nfdicore:Organization ;
    owl:inverseOf nfdicore:subsidiaryOrganization .

nfdicore:partnerOrganization a owl:ObjectProperty,
        owl:SymmetricProperty ;
    rdfs:domain nfdicore:Organization ;
    rdfs:range nfdicore:Organization .

nfdicore:programmingLanguage a owl:ObjectProperty ;
    rdfs:label "programming language"@en ;
    rdfs:comment "The property links software to a programming language it is written in." ;
    rdfs:domain nfdicore:Software ;
    rdfs:range nfdicore:ProgrammingLanguage ;
    owl:inverseOf nfdicore:programmingLanguageOf .

nfdicore:publisher a owl:ObjectProperty ;
    rdfs:label "publisher"@en ;
    rdfs:comment "The property is a relationship between a resource and an organisation or a person responsible for publishing it."@en ;
    rdfs:domain nfdicore:Resource ;
    rdfs:range [ a owl:Class ;
            owl:unionOf ( nfdicore:Organization nfdicore:Person ) ] ;
    owl:inverseOf nfdicore:publisherOf .

nfdicore:relatedProject a owl:ObjectProperty,
        owl:SymmetricProperty ;
    rdfs:label "related project"@en ;
    rdfs:comment "The property is a relationship between related projects. The property is symmetric."@en ;
    rdfs:domain nfdicore:Project ;
    rdfs:range nfdicore:Project .

nfdicore:semanticExpressivity a owl:ObjectProperty ;
    rdfs:label "semantic expressivity"@en ;
    rdfs:comment "The property relates a resource to its semantic expressivity spectrum."@en ;
    rdfs:domain mwo:SemanticResource ;
    rdfs:range nfdicore:SemanticExpressivity ;
    owl:inverseOf nfdicore:semanticExpressivityOf .

nfdicore:standard a owl:ObjectProperty ;
    rdfs:label "standard"@en ;
    rdfs:comment "The property relates a resource to the standard it relies on."@en ;
    rdfs:domain nfdicore:Resource ;
    rdfs:range nfdicore:Standard ;
    owl:inverseOf nfdicore:standardOf .

ns2:BFO_0000179 a owl:AnnotationProperty .

ns2:BFO_0000180 a owl:AnnotationProperty .

ns2:IAO_0000111 a owl:AnnotationProperty .

ns2:IAO_0000112 a owl:AnnotationProperty .

ns2:IAO_0000114 a owl:AnnotationProperty .

ns2:IAO_0000115 a owl:AnnotationProperty ;
    rdfs:label "definition",
        "textual definition",
        "definition"@en ;
    ns2:IAO_0000111 "definition",
        "textual definition",
        "definition"@en ;
    ns2:IAO_0000114 ns2:IAO_0000122 ;
    ns2:IAO_0000115 "The official OBI definition, explaining the meaning of a class or property. Shall be Aristotelian, formalized and normalized. Can be augmented with colloquial definitions."@en,
        "The official definition, explaining the meaning of a class or property. Shall be Aristotelian, formalized and normalized. Can be augmented with colloquial definitions."@en ;
    ns2:IAO_0000116 """2012-04-05: 
Barry Smith

The official OBI definition, explains the meaning of a class or property: 'Shall be Aristotelian, formalized and normalized. Can be augmented with colloquial definitions'  is terrible.

Can you fix to something like:

A statement of necessary and sufficient conditions explaining the meaning of an expression referring to a class or property.

Alan Ruttenberg

Your proposed definition is a reasonable candidate, except that it is very common that necessary and sufficient conditions are not given. Mostly they are necessary, occasionally they are necessary and sufficient or just sufficient. Often they use terms that are not themselves defined and so they effectively can't be evaluated by those criteria. 

On the specifics of the proposed definition:

We don't have definitions of 'meaning' or 'expression' or 'property'. For 'reference' in the intended sense I think we use the term 'denotation'. For 'expression', I think we you mean symbol, or identifier. For 'meaning' it differs for class and property. For class we want documentation that let's the intended reader determine whether an entity is instance of the class, or not. For property we want documentation that let's the intended reader determine, given a pair of potential relata, whether the assertion that the relation holds is true. The 'intended reader' part suggests that we also specify who, we expect, would be able to understand the definition, and also generalizes over human and computer reader to include textual and logical definition. 

Personally, I am more comfortable weakening definition to documentation, with instructions as to what is desirable. 

We also have the outstanding issue of how to aim different definitions to different audiences. A clinical audience reading chebi wants a different sort of definition documentation/definition from a chemistry trained audience, and similarly there is a need for a definition that is adequate for an ontologist to work with.  """@en ;
    ns2:IAO_0000117 "PERSON:Daniel Schober"@en ;
    ns2:IAO_0000119 "GROUP:OBI:<http://purl.obolibrary.org/obo/obi>"@en ;
    rdfs:isDefinedBy ns2:iao.owl .

ns2:IAO_0000116 a owl:AnnotationProperty .

ns2:IAO_0000117 a owl:AnnotationProperty .

ns2:IAO_0000118 a owl:AnnotationProperty .

ns2:IAO_0000119 a owl:AnnotationProperty .

ns2:IAO_0010000 a owl:AnnotationProperty .

ns2:NCIT_C42610 a owl:AnnotationProperty ;
    rdfs:label "abbreviation"@en ;
    ns2:IAO_0000115 "A shortened form of a word or phrase. [Definition Source: NCI]" ;
    rdfs:subPropertyOf skos:altLabel .

ns2:NCIT_C93495 a owl:AnnotationProperty ;
    rdfs:label "acronym"@en ;
    ns2:IAO_0000115 "The non-unique initials or abbreviated name used for identification. [Definition Source: NCI]" ;
    rdfs:subPropertyOf skos:altLabel .

dc:creator a owl:AnnotationProperty .

dc:date a owl:AnnotationProperty .

dc:description a owl:AnnotationProperty .

dc:title a owl:AnnotationProperty .

dcterms:abstract a owl:AnnotationProperty .

dcterms:bibliographicCitation a owl:AnnotationProperty .

dcterms:creator a owl:AnnotationProperty .

dcterms:description a owl:AnnotationProperty ;
    rdfs:label "description" .

dcterms:format a owl:AnnotationProperty ;
    rdfs:label "has format"@en,
        "Format"@en-us ;
    dcterms:bibliographicCitation "[MIME] http://www.iana.org/assignments/media-types/" ;
    rdfs:comment """The file format, physical medium, or dimensions of the resource.

Examples of dimensions include size and duration. Recommended best practice is to use a controlled vocabulary such as the list of Internet Media Types."""@en,
        "Examples of dimensions include size and duration. Recommended best practice is to use a controlled vocabulary such as the list of Internet Media Types [MIME]."@en-us ;
    rdfs:range dc:contributor ;
    rdfs:seeAlso <http://www.iana.org/assignments/media-types/> ;
    rdfs:subPropertyOf dc:format ;
    skos:definition "The file format, physical medium, or dimensions of the resource."@en-us .

dcterms:hasVersion a owl:AnnotationProperty .

dcterms:isPartOf a owl:ObjectProperty ;
    rdfs:domain nfdicore:TaskArea ;
    rdfs:range default1:Consortium .

dcterms:license a owl:AnnotationProperty .

dcterms:title a owl:AnnotationProperty,
        owl:DatatypeProperty ;
    rdfs:label "has title"@en ;
    rdfs:comment "A name given to a resource.  Typically, the title will be the name by which the resource is formally known."@en ;
    rdfs:domain nfdicore:Resource .

mwo: a owl:Ontology ;
    dc:contributor <https://orcid.org/0000-0001-7069-9804>,
        <https://orcid.org/0000-0001-9106-8825>,
        <https://orcid.org/0000-0001-9560-4728>,
        <https://orcid.org/0000-0002-2691-6995>,
        <https://orcid.org/0000-0002-5149-603X>,
        <https://orcid.org/0000-0003-4926-0068> ;
    dcterms:creator <https://orcid.org/0000-0001-7564-7990>,
        <https://orcid.org/0000-0002-1008-4530>,
        <https://orcid.org/0000-0002-2818-5890> ;
    dcterms:description "The MatWerk ontology represents research data and related activities of the MSE community. A first version of the ontology will be simplified, focusing on (i) community structure: researchers, research projects, universities, and institutions; (ii) infrastructure: software, workflows, ontologies, schemas, APIs, instruments, facilities, educational resources; and (iii) data: repositories, databases, scientific publications, published datasets and reference data." ;
    dcterms:license <https://creativecommons.org/licenses/by/4.0/>,
        <https://creativecommons.org/licenses/unspecified> ;
    dcterms:title "The MatWerk ontology" ;
    rdfs:comment "The purpose of the MatWerk Ontology is to represent the scientific and infrastructural status of the Materials Science and Engineering (MSE) community. It will be used as a backbone for the MSE Knowledge Graph."@en .

mwo:ChemistryDatabase a owl:Class ;
    rdfs:label "chemistry database"@en ;
    ns2:IAO_0000115 "A database containing chemistry data."@en ;
    rdfs:subClassOf mwo:Database .

mwo:ContactPerson a owl:Class ;
    rdfs:label "contact person"@en ;
    ns2:IAO_0000115 "A role which inheres in a bearer and is realised when this person acts as the contact point regarding a contribution."@en ;
    rdfs:subClassOf ns2:BFO_0000023,
        mwo:ContactPoint .

mwo:CrystallographyDatabase a owl:Class ;
    rdfs:label "crystallography database"@en ;
    ns2:IAO_0000115 "A database containing crystal structures and data on structural and mathematical crystallography, solid state physics and structural chemistry."@en ;
    rdfs:subClassOf mwo:Database .

mwo:DataCollector a owl:Class ;
    rdfs:label "data collector"@en ;
    ns2:IAO_0000115 "A role which inheres in a bearer and is realised when this bearer has participated in the gathering of data."@en ;
    rdfs:comment "The bearer in this definition might be a person or a software agent. Data may consist of subject data, object data or both."@en ;
    rdfs:subClassOf ns2:BFO_0000023 .

mwo:ElectronicLabNotebook a owl:Class ;
    rdfs:label "electronic lab notebook"@en ;
    ns2:IAO_0000115 "An Electronic Lab Notebook is a software tool that digitally replicates paper lab notebooks traditionally used in the sciences to record experimental results. It allows scientists to access, search, and share results from an experiment."@en ;
    ns4:hasExactSynonym "Electronic Laboratory Notebook"@en ;
    rdfs:subClassOf ns3:SWO_0000001 .

mwo:ExperimentalWorkflow a owl:Class ;
    rdfs:label "Experimental Workflow"@en ;
    ns2:IAO_0000115 "Experimental workflow is a workflow that describes an experimental process, including the design, preparation, measurement, and analysis of the data."@en ;
    rdfs:subClassOf mwo:Workflow .

mwo:GitRepository a owl:Class ;
    rdfs:label "git repository" ;
    ns2:IAO_0000115 "A repository that is created and managed using a Git version control system."@en ;
    rdfs:subClassOf mwo:Repository .

mwo:Lecture a owl:Class ;
    rdfs:label "Lecture" ;
    ns2:IAO_0000115 "An academic event which is intented to deliver instruction on a specific topic, most commonly to an audience of university students."@en ;
    rdfs:subClassOf mwo:EducationalEvent .

mwo:MaterialsDatabase a owl:Class ;
    rdfs:label "materials database"@en ;
    ns2:IAO_0000115 "A database containing data of experimental and computational properties of materials"@en ;
    rdfs:subClassOf mwo:Database .

mwo:OntologyRepository a owl:Class ;
    rdfs:label "ontology repository"@en ;
    ns2:IAO_0000115 "A repository which contains ontologies."@en ;
    rdfs:subClassOf mwo:Repository .

mwo:Patent a owl:Class ;
    rdfs:label "patent"@en ;
    ns2:IAO_0000115 "A patent is an exclusive right granted for an invention, which is a product or a process that provides, in general, a new way of doing something, or offers a new technical solution to a problem. To get a patent, technical information about the invention must be disclosed to the public in a patent application."@en ;
    ns4:hasDbXref <https://www.wipo.int/patents/en/> ;
    rdfs:subClassOf nfdicore:Specification .

mwo:PotentialsRepository a owl:Class ;
    rdfs:label "potentials repository"@en ;
    ns2:IAO_0000115 "A data repository which contains interatomic potentials or pseudopotentials for atomistic models."@en ;
    rdfs:subClassOf mwo:Repository .

mwo:ProjectLeader a owl:Class ;
    rdfs:label "project leader"@en ;
    ns2:IAO_0000115 "A role which inheres in a bearer and is realized when an person is responsible for 1) the coordination of project resources and 2) the operations carried out within it."@en ;
    ns4:hasDbXref <https://www.indeed.com/career-advice/finding-a-job/project-leader-vs-project-manager> ;
    ns4:hasRelatedSynonym mwo:ProjectManager ;
    rdfs:comment "In a project, a project leader might engage, motivate and support the team by establishing and maintaining productive operations"@en ;
    rdfs:subClassOf ns2:BFO_0000023 .

mwo:Seminar a owl:Class ;
    rdfs:label "Seminar"@en ;
    ns2:IAO_0000115 "An academic event where recuring meetings are held on a particular research topic, usually attended by academic and research staff."@en ;
    rdfs:subClassOf ns1:AcademicEvent .

mwo:SoftwareRepository a owl:Class ;
    rdfs:label "software repository"@en ;
    ns2:IAO_0000115 "A repository which contains software and its components, including libraries, scripts, etc."@en ;
    rdfs:subClassOf mwo:Repository .

mwo:SummerSchool a owl:Class ;
    rdfs:label "Summer School"@en ;
    ns2:IAO_0000115 "An academic event where a school session is conducted in summer enabling students to accelerate progress toward a diploma or degree, to make up credits lost through absence or failure, or to round out professional education."@en ;
    ns4:hasDbXref <https://www.merriam-webster.com/dictionary/summer%20school#:~:text=noun,to%20round%20out%20professional%20education> ;
    rdfs:subClassOf mwo:EducationalEvent .

mwo:TrainingCourse a owl:Class ;
    rdfs:label "Training Course"@en ;
    ns2:IAO_0000115 "An academic event where the objective is to teach skills needed for a particular task or job."@en ;
    rdfs:subClassOf mwo:EducationalEvent .

mwo:aboutMaterial a owl:ObjectProperty ;
    rdfs:label "about material"@en ;
    ns2:IAO_0000115 "A relation between a dataset and the material it contains data on."@en ;
    rdfs:domain nfdicore:Dataset ;
    rdfs:range emmo:EMMO_4207e895_8b83_4318_996a_72cfb32acd94 .

mwo:belongsTo a owl:ObjectProperty ;
    rdfs:label "belongs to"@en ;
    ns2:IAO_0000115 "A relation between a research group or large-scale facility and the organization it belongs to."@en ;
    rdfs:domain [ a owl:Class ;
            owl:unionOf ( mwo:LargeScaleFacility mwo:ResearchGroup ) ] ;
    rdfs:range nfdicore:Organization .

mwo:conformsToSpecification a owl:ObjectProperty ;
    rdfs:label "conforms to specification"@en ;
    ns2:IAO_0000115 "A relation between a resource and the specification it conforms to."@en ;
    rdfs:domain nfdicore:Resource ;
    rdfs:range nfdicore:Specification .

mwo:description a owl:DatatypeProperty ;
    rdfs:label "description"@en ;
    ns2:IAO_0000115 "A data property linking an entity to its description."@en .

mwo:emailAddress a owl:DatatypeProperty ;
    rdfs:label "email address"@en ;
    rdfs:domain [ a owl:Class ;
            owl:unionOf ( nfdicore:Organization nfdicore:Person ) ] .

mwo:hasAcronym a owl:DatatypeProperty ;
    rdfs:label "has acronym"@en ;
    ns2:IAO_0000115 "A data property indicating the acronym of an entity, often represented as an abbreviation of the initials of the name or title of the entity."@en .

mwo:hasAffiliation a owl:ObjectProperty ;
    rdfs:label "has affiliation"@en ;
    ns2:IAO_0000115 "a relation between a person and an organization to which the person is affiliated."@en ;
    rdfs:domain nfdicore:Person ;
    rdfs:range nfdicore:Organization .

mwo:hasContactPoint a owl:ObjectProperty ;
    rdfs:label "a relation between a thing and its contact point, which can be a person or website."@en,
        "has contact point"@en ;
    rdfs:domain owl:Thing ;
    rdfs:range mwo:ContactPoint .

mwo:hasContributor a owl:ObjectProperty ;
    rdfs:label "has contributor"@en ;
    owl:inverseOf mwo:isContributorOf .

mwo:hasCreator a owl:ObjectProperty ;
    rdfs:label "has creator" ;
    ns2:IAO_0000115 "A relation between a dataset and a person or organization, who has created the data."@en ;
    rdfs:domain nfdicore:Dataset ;
    rdfs:range [ a owl:Class ;
            owl:unionOf ( nfdicore:Organization nfdicore:Person ) ] ;
    rdfs:subPropertyOf mwo:hasAuthor .

mwo:hasDOI a owl:DatatypeProperty ;
    rdfs:label "has DOI" ;
    ns2:IAO_0000115 "A data property relating a work to its Digital Object Identifier (DOI)."@en ;
    rdfs:domain nfdicore:Resource ;
    rdfs:subPropertyOf dcterms:identifier .

mwo:hasDiscipline a owl:ObjectProperty ;
    rdfs:label "has discipline"@en ;
    ns2:IAO_0000115 "A relation between a resource or large-scale facility and the academic discipline of the produced work."@en ;
    rdfs:domain nfdicore:Resource ;
    rdfs:range nfdicore:AcademicDiscipline .

mwo:hasDocumentation a owl:ObjectProperty ;
    rdfs:label "has documentation"@en ;
    ns2:IAO_0000115 "A relation between a resource and its documentation."@en ;
    rdfs:domain nfdicore:Resource ;
    rdfs:range mwo:Documentation .

mwo:hasEndpointURL a owl:DatatypeProperty ;
    rdfs:label "has endpoint URL"@en ;
    ns2:IAO_0000115 "A data property relating a SPARQL EndPoint with its URL."@en ;
    rdfs:domain mwo:SparqlEndpoint ;
    rdfs:range xsd:anyURI ;
    rdfs:subPropertyOf nfdicore:url .

mwo:hasExpertiseIn a owl:ObjectProperty ;
    rdfs:label "has expertise in"@en ;
    ns2:IAO_0000115 "A relation between a person and an academic discipline or research topic, in which this person is an expert."@en ;
    rdfs:domain nfdicore:Person ;
    rdfs:range nfdicore:AcademicDiscipline .

mwo:hasFormat a owl:ObjectProperty ;
    rdfs:label "has format"@en ;
    ns2:IAO_0000115 "The file format of the resource"@en ;
    rdfs:domain nfdicore:Resource ;
    rdfs:range dcterms:FileFormat .

mwo:hasLeader a owl:ObjectProperty ;
    rdfs:label "has leader"@en ;
    ns2:IAO_0000115 "A relation between a research group and its leader."@en ;
    rdfs:domain mwo:ResearchGroup ;
    rdfs:range mwo:GroupLeader ;
    owl:inverseOf mwo:isLeaderOf .

mwo:hasLecturer a owl:ObjectProperty ;
    rdfs:label "has lecturer"@en ;
    ns2:IAO_0000115 "A relation between an academic event and a person, who participates in teaching capacity in the event."@en ;
    rdfs:domain [ a owl:Class ;
            owl:unionOf ( mwo:EducationalEvent mwo:EducationalResource ) ] ;
    rdfs:range nfdicore:Person .

mwo:hasManual a owl:ObjectProperty ;
    rdfs:label "has manual"@en ;
    ns2:IAO_0000115 "A relation between an instrument and its documentation."@en ;
    rdfs:domain modsci:Instrument ;
    rdfs:range mwo:Documentation .

mwo:hasMember a owl:ObjectProperty ;
    rdfs:label "has member"@en ;
    ns2:IAO_0000115 "A relation between a research project and its members."@en ;
    rdfs:domain nfdicore:Project ;
    rdfs:range mwo:ProjectMember ;
    owl:inverseOf mwo:memberOf .

mwo:hasORCID a owl:DatatypeProperty ;
    rdfs:label "has ORCID" ;
    ns2:IAO_0000115 "A data property relating a person to their Open Researcher and Contributor ID (ORCID)." ;
    rdfs:domain nfdicore:Person ;
    rdfs:subPropertyOf dcterms:identifier .

mwo:hasOwner a owl:ObjectProperty ;
    rdfs:label "has owner"@en ;
    ns2:IAO_0000115 "A relation between an instrument and the organization that acts as its owner."@en ;
    rdfs:domain modsci:Instrument ;
    rdfs:range nfdicore:Organization .

mwo:hasPostalCode a owl:DatatypeProperty ;
    rdfs:label "has postal code" ;
    ns2:IAO_0000115 "A data property indicating the postal code of an entity." ;
    rdfs:domain [ a owl:Class ;
            owl:unionOf ( nfdicore:Organization nfdicore:Person ) ] ;
    rdfs:subPropertyOf mwo:hasPostalAddress .

mwo:hasProjectIdentifier a owl:DatatypeProperty ;
    rdfs:label "has project identifier"@en ;
    ns2:IAO_0000115 "A data property relating a research project with a unique identifier, defined in a given context."@en ;
    rdfs:domain nfdicore:Project ;
    rdfs:subPropertyOf dcterms:identifier .

mwo:hasRORID a owl:DatatypeProperty ;
    rdfs:label "has ROR ID" ;
    ns2:IAO_0000115 "A data property relating an organization to its identifier within the Research Organization Registry (ROR)."@en ;
    rdfs:domain nfdicore:Organization ;
    rdfs:subPropertyOf dcterms:identifier .

mwo:hasRelatedResource a owl:ObjectProperty,
        owl:SymmetricProperty ;
    rdfs:label "has related resource"@en ;
    ns2:IAO_0000115 "A relation between two different resources, which indicates both are associated."@en ;
    rdfs:domain nfdicore:Resource ;
    rdfs:range nfdicore:Resource .

mwo:hasRepository a owl:ObjectProperty ;
    rdfs:label "has repository"@en ;
    ns2:IAO_0000115 "A relation between a software and the website of the repository where it is stored."@en ;
    rdfs:domain nfdicore:Resource ;
    rdfs:range mwo:Repository .

mwo:hasRole a owl:ObjectProperty ;
    rdfs:label "has role"@en ;
    ns2:IAO_0000115 "A relation between a person (the bearer) and a role, in which the role specifically depends on the bearer for its existence."@en ;
    rdfs:domain nfdicore:Person ;
    rdfs:range ns2:BFO_0000023 .

mwo:hasSerialNumber a owl:DatatypeProperty ;
    rdfs:label "has serial number"@en ;
    rdfs:comment "A data property linking something, for example a piece of equipment, to its serial number."@en ;
    rdfs:domain [ a owl:Class ;
            owl:unionOf ( <http://schema.org/Product> modsci:Instrument ) ] ;
    rdfs:subPropertyOf dcterms:identifier .

mwo:hasSparqlEndpoint a owl:ObjectProperty ;
    rdfs:label "has SPARQL endpoint"@en ;
    ns2:IAO_0000115 "A relation between a semantic resource and its SPARQL Endpoint."@en ;
    rdfs:domain mwo:SemanticResource ;
    rdfs:range mwo:SparqlEndpoint .

mwo:hasTopic a owl:ObjectProperty ;
    rdfs:label "has topic"@en ;
    ns2:IAO_0000115 "A relation between a research project and the topic of the research question it investigates."@en ;
    rdfs:domain nfdicore:Project ;
    rdfs:range mwo:ResearchTopic .

mwo:hasVersion a owl:DatatypeProperty ;
    rdfs:label "has version"@en ;
    ns2:IAO_0000115 "A number or string that identifies different variants or releases of a resource."@en ;
    rdfs:domain nfdicore:Resource .

mwo:hasWebsite a owl:ObjectProperty ;
    rdfs:label "has website"@en ;
    ns2:IAO_0000115 "a relation between a thing and its website."@en ;
    rdfs:domain owl:Thing ;
    rdfs:range nfdicore:Website .

mwo:instrumentModel a owl:DatatypeProperty ;
    rdfs:label "instrument model"@en ;
    ns2:IAO_0000115 "A data property relating an instrument with the model information."@en ;
    rdfs:domain modsci:Instrument .

mwo:isOnline a owl:DatatypeProperty ;
    rdfs:label "is online"@en ;
    ns2:IAO_0000115 "A flag to indicate an organized event or educational resource can be accessed online."@en ;
    rdfs:domain [ a owl:Class ;
            owl:unionOf ( mwo:EducationalResource ns1:OrganisedEvent ) ] ;
    rdfs:range xsd:boolean .

mwo:keyword a owl:DatatypeProperty ;
    rdfs:label "keywords"@en ;
    ns2:IAO_0000115 "A data property used for defining something with keywords."@en .

mwo:mainTaskArea a owl:ObjectProperty ;
    rdfs:domain mwo:UseCase ;
    rdfs:range nfdicore:TaskArea .

mwo:relatedParticipantProject a owl:ObjectProperty ;
    rdfs:domain mwo:UseCase ;
    rdfs:range mwo:ParticipantProject .

mwo:relatedTaskArea a owl:ObjectProperty ;
    rdfs:domain mwo:UseCase ;
    rdfs:range nfdicore:TaskArea .

mwo:requiredTool a owl:ObjectProperty ;
    rdfs:label "required tool"@en ;
    ns2:IAO_0000115 "A relation between an educational resource or academic event and the tools required to participate."@en ;
    rdfs:domain [ a owl:Class ;
            owl:unionOf ( mwo:EducationalEvent mwo:EducationalResource ) ] ;
    rdfs:range ns3:SWO_0000001 .

mwo:softwareCitation a owl:ObjectProperty ;
    rdfs:label "software citation"@en ;
    ns2:IAO_0000115 "A relation between a work and a cited software."@en ;
    rdfs:domain nfdicore:Resource ;
    rdfs:range nfdicore:Software ;
    rdfs:subPropertyOf schema:citation .

mwo:usesMethod a owl:ObjectProperty ;
    rdfs:label "uses method"@en ;
    ns2:IAO_0000115 "A relation between a resource and method it implements, uses or describes."@en ;
    rdfs:domain nfdicore:Resource ;
    rdfs:range mwo:Method .

mwo:usesTechnology a owl:ObjectProperty ;
    rdfs:label "uses technology"@en ;
    ns2:IAO_0000115 "A relation between an instrument and the technology it implements."@en ;
    rdfs:domain modsci:Instrument ;
    rdfs:range modsci:Technology .

mwo:workingOnTopic a owl:ObjectProperty ;
    rdfs:label "a relation between a research group and the topic in which it conducts research."@en,
        "working on topic"@en ;
    rdfs:domain mwo:ResearchGroup ;
    rdfs:range mwo:ResearchTopic .

void:feature a owl:AnnotationProperty .

ns3:SWO_0000082 a owl:ObjectProperty ;
    rdfs:label "uses software"@en ;
    ns2:IAO_0000112 "Cytoscape plugins would be linked to the Cytoscape application via uses software, while Microsoft Excel is linked to Microsoft Office via has_part." ;
    ns2:IAO_0000115 "This property allows the linkage of two different pieces of software such that one directly executes or uses the other. The has_part relationship should instead be used to describe related but independent members of a larger software package, and 'uses platform' relationship should be used to describe which operating system(s) a particular piece of software can use." ;
    ns2:IAO_0000119 "Allyson Lister" ;
    rdfs:domain ns3:SWO_0000001 ;
    rdfs:range ns3:SWO_0000001 ;
    owl:inverseOf ns3:SWO_0000157 .

ns3:SWO_0004001 a owl:ObjectProperty ;
    rdfs:label "has interface" ;
    ns2:IAO_0000115 "Provides a method of asserting what type of interactions are possible for the class in question. The interface must be from the 'software interface' hierarchy." ;
    ns2:IAO_0000119 "Allyson Lister",
        "Andy Brown" ;
    dcterms:creator "Andy Brown" ;
    rdfs:range ns3:SWO_9000050 .

<http://www.ebi.ac.uk/swo/interface/SWO_9000054> a owl:Class ;
    rdfs:label "application programming interface" ;
    ns2:IAO_0000115 "An application programming interface is a set of routines, protocols, and tools for building software applications. An API expresses a software component in terms of its operations, inputs, outputs, and underlying types. An API defines functionalities that are independent of their respective implementations, which allows definitions and implementations to vary without compromising each other. The API specifies how software components should interact." ;
    ns2:IAO_0000118 "API" ;
    ns2:IAO_0000119 "http://en.wikipedia.org/wiki/Application_programming_interface, accessed 25 November 2014." ;
    rdfs:subClassOf ns3:SWO_9000050 .

<http://www.ebi.ac.uk/swo/license/SWO_1000009> a owl:Class ;
    rdfs:label "License without restrictions on derivatives" ;
    rdfs:subClassOf ns3:SWO_0000002 .

<http://www.ebi.ac.uk/swo/license/SWO_1000048> a owl:ObjectProperty,
        owl:SymmetricProperty ;
    rdfs:label "is compatible license of"@en ;
    ns2:IAO_0000115 "'is compatible license of' provides a method of marking two software licenses as compatible and without conflicts, e.g. that the Apache License version 2 is compatible with GNU GPL version 3. If two licenses are connected with this property, it means code released under one license can be released with code from the other license in a larger program." ;
    ns2:IAO_0000119 "http://www.gnu.org/licenses/gpl-faq.html#WhatDoesCompatMean, accessed 12 June 2013." ;
    dcterms:creator "Allyson Lister" ;
    rdfs:domain ns3:SWO_0000002 ;
    rdfs:range ns3:SWO_0000002 .

<http://www.ebi.ac.uk/swo/license/SWO_1000056> a owl:Class ;
    rdfs:label "Artistic License" ;
    dcterms:creator "Allyson Lister" ;
    rdfs:subClassOf ns3:SWO_0000002 .

<http://www.ebi.ac.uk/swo/license/SWO_1000069> a owl:Class ;
    rdfs:label "GNU AGPL"@en ;
    rdfs:subClassOf ns3:SWO_0000002 .

<http://www.ebi.ac.uk/swo/license/SWO_1000095> a owl:Class ;
    rdfs:label "Open Data Commons"@en ;
    rdfs:subClassOf ns3:SWO_0000002 .

<http://www.ebi.ac.uk/swo/license/SWO_1000137> a owl:Class ;
    rdfs:label "Fee-Based Commercial License"@en ;
    ns2:IAO_0000115 "Fee-Based Commercial License is a license which, among its license clauses, states that commercial entities may use the resource for a fee." ;
    ns2:IAO_0000119 "Allyson Lister" ;
    dcterms:creator "Allyson Lister" ;
    rdfs:comment "Allyson Lister: This is a convenience class which combines multiple license clauses to create a defined class, such that any license type which meets the requirements will be inferred to fall into this category." ;
    rdfs:subClassOf ns3:SWO_0000002 .

<http://www.ebi.ac.uk/swo/license/SWO_1000140> a owl:Class ;
    rdfs:label "Non-Commercial No-Fee License"@en ;
    ns2:IAO_0000115 "Non-Commercial No-Fee License is a license which, among its license clauses, states that non-commercial entities may use the resource without a purchase or usage cost." ;
    ns2:IAO_0000119 "Allyson Lister" ;
    dcterms:creator "Allyson Lister" ;
    rdfs:comment "Allyson Lister: This is a convenience class which combines multiple license clauses to create a defined class, such that any license type which meets the requirements will be inferred to fall into this category." ;
    rdfs:subClassOf ns3:SWO_0000002 .

ns4:hasBroadSynonym a owl:AnnotationProperty ;
    rdfs:label "has_broad_synonym"@en ;
    ns4:hasDbXref [ ] ;
    ns4:hasDefinition [ ] ;
    rdfs:subPropertyOf ns4:hasSynonym .

ns4:hasDbXref a owl:AnnotationProperty ;
    rdfs:label "database_cross_reference" .

ns4:hasDefinition a owl:AnnotationProperty .

ns4:hasExactSynonym a owl:AnnotationProperty ;
    rdfs:label "has_exact_synonym"@en ;
    ns4:hasDbXref [ ] ;
    ns4:hasDefinition [ ] ;
    rdfs:subPropertyOf ns4:hasSynonym .

ns4:hasNarrowSynonym a owl:AnnotationProperty ;
    rdfs:label "has_narrow_synonym"@en ;
    ns4:hasDbXref [ ] ;
    ns4:hasDefinition [ ] ;
    rdfs:subPropertyOf ns4:hasSynonym .

ns4:hasRelatedSynonym a owl:AnnotationProperty ;
    rdfs:label "has_related_synonym"@en ;
    ns4:hasDbXref [ ] ;
    ns4:hasDefinition [ ] ;
    rdfs:subPropertyOf ns4:hasSynonym .

owl:versionInfo a owl:AnnotationProperty .

skos:definition a owl:AnnotationProperty .

skos:prefLabel a owl:AnnotationProperty .

foaf:firstName a owl:DatatypeProperty ;
    rdfs:domain nfdicore:Person ;
    rdfs:subPropertyOf mwo:hasPersonalInformation .

foaf:gender a owl:DatatypeProperty,
        owl:FunctionalProperty ;
    rdfs:label "gender" ;
    rdfs:comment "The gender of this Agent (typically but not necessarily 'male' or 'female')." ;
    rdfs:domain nfdicore:Person ;
    rdfs:isDefinedBy foaf: ;
    rdfs:subPropertyOf mwo:hasPersonalInformation .

foaf:surname a owl:DatatypeProperty ;
    rdfs:domain nfdicore:Person ;
    rdfs:subPropertyOf mwo:hasPersonalInformation .

foaf:title a owl:DatatypeProperty ;
    rdfs:label "title" ;
    rdfs:comment "Title (Mr, Mrs, Ms, Dr. etc)" ;
    rdfs:domain nfdicore:Person ;
    rdfs:isDefinedBy foaf: ;
    rdfs:subPropertyOf mwo:hasPersonalInformation .

<https://nfdi.fiz-karlsruhe.de/ontology> a owl:Ontology ;
    rdfs:label "Consortium module for NFDIcore Ontology" ;
    skos:definition "The NFDIcore ontology  (prefix nfdicore) describes resouces (datasets, data providers, persons, projects and other entities) in the data domain of NFDI (https://www.nfdi.de/). It serves as the basis for further domain specific ontologies, e.g. nfdi4culture ontology, nfdi4matwerk ontology. Mappings to numerous external vocabularies and ontologies are provided in an extra file."@en .

default1:ControlledVocabulary a owl:NamedIndividual ;
    rdfs:label "controlled vocabulary"@en ;
    rdfs:comment "A list of terms, natural language definitions and naming conventions. In comparisson to a glossary, there is a dedicated curation mechanism for new terms in a controlled vocabulary."@en .

default1:Glossary a owl:NamedIndividual ;
    rdfs:label "glossary"@en ;
    rdfs:comment "A list of terms and their with natural language definitions."@en .

default1:Ontology a owl:NamedIndividual ;
    rdfs:label "ontology"@en ;
    rdfs:comment "A complete, machine-readable specification of a conceptualization using URIs (and then IRIs) for all elements, properties and relationship types."@en .

default1:Taxonomy a owl:NamedIndividual ;
    rdfs:label "taxonomy"@en ;
    rdfs:comment "A data model in a class hierarchy, where all concepts inherit their behaviour from the super-class concept. Taxonomies can be strict or non strict and can contain instances."@en .

default1:Thesaurus a owl:NamedIndividual ;
    rdfs:label "thesaurus"@en ;
    rdfs:comment "A structured list of terms and relations between the terms, as e.g. broader/narrower."@en .

default1:acronym a owl:AnnotationProperty ;
    rdfs:label "nfdicore:acronym"@en .

default1:areaCode a owl:DatatypeProperty ;
    rdfs:label "area code"@en ;
    rdfs:domain default1:Organization ;
    rdfs:range rdfs:Literal .

default1:emailAddress a owl:DatatypeProperty ;
    rdfs:label "email address"@en ;
    rdfs:domain [ a owl:Class ;
            owl:unionOf ( default1:Organization default1:Person ) ] ;
    rdfs:range rdfs:Literal .

default1:example a owl:AnnotationProperty ;
    rdfs:label "nfdicore:example"@en .

default1:fileExtension a owl:DatatypeProperty ;
    rdfs:label "file extension" ;
    rdfs:comment "An identifier for a file format (e.g. txt for a text file) used as a suffix to the file name, don't use dot at start."@en ;
    default1:example "mp4",
        "ttl",
        "txt",
        "xml" .

default1:fundingOrganization a owl:ObjectProperty ;
    rdfs:label "funding organization"@en ;
    rdfs:comment "The property relates a resource or a project to the organization that provided funding for it."@en ;
    rdfs:range default1:Organization ;
    owl:inverseOf default1:fundingOrganizationOf .

default1:fundingProject a owl:ObjectProperty ;
    rdfs:label "funding project"@en ;
    rdfs:comment "The property relateds a resource to the project that provided funding for it."@en ;
    rdfs:range default1:Project ;
    owl:inverseOf default1:fundingProjectOf .

default1:parentOrganization a owl:ObjectProperty ;
    rdfs:label "parent organization"@en ;
    rdfs:comment "The property is a parental relationship between organizations."@en ;
    rdfs:domain default1:Organization ;
    rdfs:range default1:Organization .

default1:partnerOrganization a owl:ObjectProperty,
        owl:SymmetricProperty ;
    rdfs:label "partner organization"@en ;
    rdfs:comment "The property is a partner relationship between organizations. The property is symmetric."@en ;
    rdfs:domain default1:Organization ;
    rdfs:range default1:Organization .

default1:relatedProject a owl:ObjectProperty ;
    rdfs:label "related project"@en ;
    rdfs:comment "The property is a relationship between a project or a resource and related projects."@en ;
    rdfs:range default1:Project .

default1:url a owl:DatatypeProperty ;
    rdfs:label "url"@en ;
    rdfs:comment "URL of a thing"@en ;
    rdfs:domain owl:Thing ;
    rdfs:range xsd:anyURI .

ns1:Conference a owl:Class ;
    rdfs:label "Conference"@en ;
    rdfs:comment "A conference event."@en ;
    rdfs:subClassOf ns1:AcademicEvent .

ns1:Talk a owl:Class ;
    rdfs:label "Talk"@en ;
    rdfs:comment "A talk event."@en ;
    rdfs:subClassOf ns1:AcademicEvent .

ns1:Tutorial a owl:Class ;
    rdfs:label "Tutorial"@en ;
    rdfs:comment "An event which a teaching session is given to to an individual or very small group."@en ;
    rdfs:subClassOf mwo:EducationalEvent .

ns1:Workshop a owl:Class ;
    rdfs:label "Workshop"@en ;
    rdfs:comment "An event which is a long interactive meeting or educational session designed to create a specialized result. Workshops are smaller than conferences, and are usually only a day or two long and are dedicated to discussing a specific topic."@en ;
    rdfs:subClassOf ns1:AcademicEvent .

ns1:duration a owl:DatatypeProperty ;
    rdfs:label "duration"@en ;
    rdfs:comment "duration"@en ;
    rdfs:domain ns1:OrganisedEvent .

<https://w3id.org/seo#KeynoteSpeaker> a owl:Class ;
    rdfs:label "Keynote speaker"@en ;
    rdfs:comment "Someone who gives the main address at a formal gathering such as a conference ."@en ;
    rdfs:subClassOf <https://w3id.org/seo#InvitedSpeakers> .

modsci:LaboratoryInstrument a owl:Class ;
    rdfs:label "Laboratory Instrument"@en ;
    rdfs:comment "An instrument needed for operations in various laboratories, synthesis and analysis."@en ;
    rdfs:subClassOf modsci:Instrument ;
    owl:equivalentClass modsci:ScientificInstrument .

modsci:hasManufacturer a owl:ObjectProperty ;
    rdfs:label "has manufacturer"@en ;
    ns2:IAO_0000115 "A relation between company that makes goods for sale."@en ;
    rdfs:domain modsci:ScientificInstrument ;
    rdfs:range modsci:ScientificInstrumentManufacturer ;
    owl:inverseOf modsci:isManufacturerOf .

<http://demo.fiz-karlsruhe.de/matwerk/E1001406> a nfdicore:Publication ;
    rdfs:label "Bernstein, H. J., Bollinger, J. C., Brown, I. D., Gražulis, S., Hester, J. R., McMahon, B., Spadaccini, N., Westbrook, J. D. & Westrip, S. P. (2016). \"Specification of the Crystallographic Information File format, version 2.0\", J. Appl. Cryst. 49" .

<http://demo.fiz-karlsruhe.de/matwerk/E100236> a nfdicore:Website ;
    rdfs:label "https://www.cp2k.org/"^^xsd:anyURI ;
    nfdicore:url <https://www.cp2k.org/> .

<http://demo.fiz-karlsruhe.de/matwerk/E1002821> a nfdicore:Publication ;
    rdfs:label "https://doi.org/10.1107/S1600576714027575"^^xsd:anyURI ;
    nfdicore:url <https://doi.org/10.1107/S1600576714027575> .

<http://demo.fiz-karlsruhe.de/matwerk/E10046> a nfdicore:Person ;
    rdfs:label "Dr.-Ing Abril Azocar Guzman" ;
    mwo:emailAddress "a.azocar.guzman@fz-juelich.de"^^xsd:string ;
    mwo:hasAffiliation <http://demo.fiz-karlsruhe.de/matwerk/E1022> ;
    mwo:hasExpertiseIn <http://demo.fiz-karlsruhe.de/matwerk/E39504>,
        <http://demo.fiz-karlsruhe.de/matwerk/E42042>,
        <http://demo.fiz-karlsruhe.de/matwerk/E63836> ;
    mwo:hasORCID <https://orcid.org/0000-0001-7564-7990> ;
    owl:sameAs <http://www.wikidata.org/entity/Q104560161> ;
    foaf:firstName "Abril"^^xsd:string ;
    foaf:surname "Azocar Guzman"^^xsd:string ;
    foaf:title "Dr.-Ing"^^xsd:string .

<http://demo.fiz-karlsruhe.de/matwerk/E100682> a nfdicore:Website ;
    rdfs:label "https://wiki.fysik.dtu.dk/gpaw/"^^xsd:anyURI ;
    nfdicore:url <https://wiki.fysik.dtu.dk/gpaw/> .

<http://demo.fiz-karlsruhe.de/matwerk/E101129> a nfdicore:Website ;
    rdfs:label "https://sxrepo.mpie.de/projects/sphinx/wiki"^^xsd:anyURI ;
    nfdicore:url <https://sxrepo.mpie.de/projects/sphinx/wiki> .

<http://demo.fiz-karlsruhe.de/matwerk/E101577> a nfdicore:Website ;
    rdfs:label "http://qboxcode.org/"^^xsd:anyURI ;
    nfdicore:url <http://qboxcode.org/> .

<http://demo.fiz-karlsruhe.de/matwerk/E102476> a nfdicore:Website ;
    rdfs:label "http://www.demon-software.com/public_html/index.html"^^xsd:anyURI ;
    nfdicore:url <http://www.demon-software.com/public_html/index.html> .

<http://demo.fiz-karlsruhe.de/matwerk/E1027029> a nfdicore:DataPortal,
        ns3:SWO_0000001 ;
    rdfs:label "Materials Cloud" ;
    mwo:conformsToSpecification <http://demo.fiz-karlsruhe.de/matwerk/E1125251> ;
    mwo:description "Materials Cloud is built to enable the seamless sharing and dissemination of resources in computational materials science, offering educational, research, and archiving tools; simulation software and services; and curated and raw data. These underpin published results and empower data-based discovery, compliant with data management plans and the FAIR principles." ;
    mwo:hasContactPoint <http://demo.fiz-karlsruhe.de/matwerk/E724004> ;
    mwo:hasContributor <http://demo.fiz-karlsruhe.de/matwerk/E6461> ;
    mwo:hasRelatedResource <http://demo.fiz-karlsruhe.de/matwerk/E652512>,
        <http://demo.fiz-karlsruhe.de/matwerk/E657086>,
        <http://demo.fiz-karlsruhe.de/matwerk/E658232> ;
    mwo:hasRepository <http://demo.fiz-karlsruhe.de/matwerk/E390404> ;
    mwo:hasWebsite <http://demo.fiz-karlsruhe.de/matwerk/E348362> ;
    schema:citation <http://demo.fiz-karlsruhe.de/matwerk/E977504> .

<http://demo.fiz-karlsruhe.de/matwerk/E102927> a nfdicore:Website ;
    rdfs:label "http://www.icmab.es/siesta/"^^xsd:anyURI ;
    nfdicore:url <http://www.icmab.es/siesta/> .

<http://demo.fiz-karlsruhe.de/matwerk/E103379> a nfdicore:Website ;
    rdfs:label "https://www.crystal.unito.it/index.php"^^xsd:anyURI ;
    nfdicore:url <https://www.crystal.unito.it/index.php> .

<http://demo.fiz-karlsruhe.de/matwerk/E103832> a nfdicore:Website ;
    rdfs:label "https://fhi-aims.org/"^^xsd:anyURI ;
    nfdicore:url <https://fhi-aims.org/> .

<http://demo.fiz-karlsruhe.de/matwerk/E104286> a nfdicore:Website ;
    rdfs:label "http://www.fplo.de/"^^xsd:anyURI ;
    nfdicore:url <http://www.fplo.de/> .

<http://demo.fiz-karlsruhe.de/matwerk/E1046> a nfdicore:Organization ;
    rdfs:label "Institute for physical metallurgy and materials physics",
        "Institut für Metallkunde und Materialphysik"@de ;
    nfdicore:location <http://demo.fiz-karlsruhe.de/matwerk/E74154> ;
    nfdicore:parentOrganisation <http://demo.fiz-karlsruhe.de/matwerk/E3279> ;
    mwo:hasAcronym "IMM"^^xsd:string ;
    mwo:hasPostalCode "52062" ;
    mwo:hasWebsite <http://demo.fiz-karlsruhe.de/matwerk/E84029> .

<http://demo.fiz-karlsruhe.de/matwerk/E104741> a nfdicore:Website ;
    rdfs:label "http://www.openmx-square.org/"^^xsd:anyURI ;
    nfdicore:url <http://www.openmx-square.org/> .

<http://demo.fiz-karlsruhe.de/matwerk/E105197> a nfdicore:Website ;
    rdfs:label "http://elk.sourceforge.net/"^^xsd:anyURI ;
    nfdicore:url <http://elk.sourceforge.net/> .

<http://demo.fiz-karlsruhe.de/matwerk/E105654> a nfdicore:Website ;
    rdfs:label "http://exciting-code.org/"^^xsd:anyURI ;
    nfdicore:url <http://exciting-code.org/> .

<http://demo.fiz-karlsruhe.de/matwerk/E106112> a nfdicore:Website ;
    rdfs:label "http://www.flapw.de/"^^xsd:anyURI ;
    nfdicore:url <http://www.flapw.de/> .

<http://demo.fiz-karlsruhe.de/matwerk/E106571> a nfdicore:Website ;
    rdfs:label "http://www.wien2k.at/"^^xsd:anyURI ;
    nfdicore:url <http://www.wien2k.at/> .

<http://demo.fiz-karlsruhe.de/matwerk/E1067> a nfdicore:Organization ;
    rdfs:label "Rechenzentrum der Christian-Albrechts-Universität" ;
    nfdicore:location <http://demo.fiz-karlsruhe.de/matwerk/E73011> ;
    nfdicore:parentOrganisation <http://demo.fiz-karlsruhe.de/matwerk/E2486> ;
    mwo:hasAcronym "RZ"^^xsd:string ;
    mwo:hasPostalCode "24118" ;
    mwo:hasWebsite <http://demo.fiz-karlsruhe.de/matwerk/E82004> .

<http://demo.fiz-karlsruhe.de/matwerk/E107031> a nfdicore:Website ;
    rdfs:label "https://www.lammps.org/"^^xsd:anyURI ;
    nfdicore:url <https://www.lammps.org/> .

<http://demo.fiz-karlsruhe.de/matwerk/E107492> a nfdicore:Website ;
    rdfs:label "http://imd.itap.physik.uni-stuttgart.de/"^^xsd:anyURI ;
    nfdicore:url <http://imd.itap.physik.uni-stuttgart.de/> .

<http://demo.fiz-karlsruhe.de/matwerk/E1079> a nfdicore:Organization ;
    rdfs:label "Institute of Biology II",
        "Institut für Biologie II"@de ;
    nfdicore:location <http://demo.fiz-karlsruhe.de/matwerk/E76079> ;
    nfdicore:parentOrganisation <http://demo.fiz-karlsruhe.de/matwerk/E3017> ;
    mwo:hasPostalCode "79104" ;
    mwo:hasWebsite <http://demo.fiz-karlsruhe.de/matwerk/E85667> .

<http://demo.fiz-karlsruhe.de/matwerk/E107954> a nfdicore:Website ;
    rdfs:label "https://www.gromacs.org/"^^xsd:anyURI ;
    nfdicore:url <https://www.gromacs.org/> .

<http://demo.fiz-karlsruhe.de/matwerk/E108417> a nfdicore:Website ;
    rdfs:label "http://micro.stanford.edu/MDpp"^^xsd:anyURI ;
    nfdicore:url <http://micro.stanford.edu/MDpp> .

<http://demo.fiz-karlsruhe.de/matwerk/E108881> a nfdicore:Website ;
    rdfs:label "https://thermocalc.com/"^^xsd:anyURI ;
    nfdicore:url <https://thermocalc.com/> .

<http://demo.fiz-karlsruhe.de/matwerk/E1092> a nfdicore:Organization ;
    rdfs:label "Department of Microsystems Engineering",
        "Institut für Mikrosystemtechnik"@de ;
    nfdicore:location <http://demo.fiz-karlsruhe.de/matwerk/E76079> ;
    nfdicore:parentOrganisation <http://demo.fiz-karlsruhe.de/matwerk/E3017> ;
    mwo:hasAcronym "IMTEK"^^xsd:string ;
    mwo:hasPostalCode "79104" ;
    mwo:hasWebsite <http://demo.fiz-karlsruhe.de/matwerk/E86079> .

<http://demo.fiz-karlsruhe.de/matwerk/E109346> a nfdicore:Website ;
    rdfs:label "https://openphase-solutions.com/"^^xsd:anyURI ;
    nfdicore:url <https://openphase-solutions.com/> .

<http://demo.fiz-karlsruhe.de/matwerk/E109812> a nfdicore:Website ;
    rdfs:label "www.mooseframework.org" .

<http://demo.fiz-karlsruhe.de/matwerk/E110279> a nfdicore:Website ;
    rdfs:label "https://www.3ds.com/products-services/simulia/products/abaqus/"^^xsd:anyURI ;
    nfdicore:url <https://www.3ds.com/products-services/simulia/products/abaqus/> .

<http://demo.fiz-karlsruhe.de/matwerk/E110747> a nfdicore:Website ;
    rdfs:label "http://www.fenicsproject.org/"^^xsd:anyURI ;
    nfdicore:url <http://www.fenicsproject.org/> .

<http://demo.fiz-karlsruhe.de/matwerk/E111216> a nfdicore:Website ;
    rdfs:label "https://damask.mpie.de/"^^xsd:anyURI ;
    nfdicore:url <https://damask.mpie.de/> .

<http://demo.fiz-karlsruhe.de/matwerk/E1116272> a modsci:Technology ;
    rdfs:label "electron imaging, EDX, nano-CT" .

<http://demo.fiz-karlsruhe.de/matwerk/E111686> a nfdicore:Website ;
    rdfs:label "https://pyiron.org/"^^xsd:anyURI ;
    nfdicore:url <https://pyiron.org/> .

<http://demo.fiz-karlsruhe.de/matwerk/E112157> a nfdicore:Website ;
    rdfs:label "https://www.aiida.net/"^^xsd:anyURI ;
    nfdicore:url <https://www.aiida.net/> .

<http://demo.fiz-karlsruhe.de/matwerk/E112629> a nfdicore:Website ;
    rdfs:label "https://www.simstack.de/"^^xsd:anyURI ;
    nfdicore:url <https://www.simstack.de/> .

<http://demo.fiz-karlsruhe.de/matwerk/E113102> a nfdicore:Website ;
    rdfs:label "https://wiki.fysik.dtu.dk/ase/"^^xsd:anyURI ;
    nfdicore:url <https://wiki.fysik.dtu.dk/ase/> .

<http://demo.fiz-karlsruhe.de/matwerk/E113576> a nfdicore:Website ;
    rdfs:label "https://www.ovito.org/about/"^^xsd:anyURI ;
    nfdicore:url <https://www.ovito.org/about/> .

<http://demo.fiz-karlsruhe.de/matwerk/E114051> a nfdicore:Website ;
    rdfs:label "http://jmol.sourceforge.net/"^^xsd:anyURI ;
    nfdicore:url <http://jmol.sourceforge.net/> .

<http://demo.fiz-karlsruhe.de/matwerk/E114527> a nfdicore:Website ;
    rdfs:label "http://jp-minerals.org/vesta/en/"^^xsd:anyURI ;
    nfdicore:url <http://jp-minerals.org/vesta/en/> .

<http://demo.fiz-karlsruhe.de/matwerk/E115004> a nfdicore:Website ;
    rdfs:label "http://www.xcrysden.org/"^^xsd:anyURI ;
    nfdicore:url <http://www.xcrysden.org/> .

<http://demo.fiz-karlsruhe.de/matwerk/E115482> a nfdicore:Website ;
    rdfs:label "https://www.ks.uiuc.edu/Research/vmd/"^^xsd:anyURI ;
    nfdicore:url <https://www.ks.uiuc.edu/Research/vmd/> .

<http://demo.fiz-karlsruhe.de/matwerk/E115961> a nfdicore:Website ;
    rdfs:label "https://www.vasp.at/py4vasp/latest/"^^xsd:anyURI ;
    nfdicore:url <https://www.vasp.at/py4vasp/latest/> .

<http://demo.fiz-karlsruhe.de/matwerk/E1160004> a nfdicore:Resource,
        mwo:MetadataSchema ;
    rdfs:label "NeXus Data Format" ;
    mwo:description "NeXus is a common data format for neutron, x-ray, and muon science. It is being developed as an international standard by scientists and programmers representing major scientific facilities in order to facilitate greater cooperation in the analysis and visualization of neutron, x-ray, and muon data." ;
    mwo:hasDocumentation <http://demo.fiz-karlsruhe.de/matwerk/E329456> ;
    mwo:hasRepository <http://demo.fiz-karlsruhe.de/matwerk/E316616> ;
    ns3:has_license <http://demo.fiz-karlsruhe.de/matwerk/E787886> ;
    schema:citation <http://demo.fiz-karlsruhe.de/matwerk/E1002821> .

<http://demo.fiz-karlsruhe.de/matwerk/E116441> a nfdicore:Website ;
    rdfs:label "https://phonopy.github.io/phonopy/"^^xsd:anyURI ;
    nfdicore:url <https://phonopy.github.io/phonopy/> .

<http://demo.fiz-karlsruhe.de/matwerk/E116922> a nfdicore:Website ;
    rdfs:label "https://ccp-nc.github.io/soprano/"^^xsd:anyURI ;
    nfdicore:url <https://ccp-nc.github.io/soprano/> .

<http://demo.fiz-karlsruhe.de/matwerk/E1172> a nfdicore:Organization ;
    rdfs:label "Fraunhofer Institute for Microstructure of Materials and Systems",
        "Fraunhofer-Institut für Mikrostruktur von Werkstoffen und Systemen"@de ;
    nfdicore:location <http://demo.fiz-karlsruhe.de/matwerk/E76856> ;
    nfdicore:parentOrganisation <http://demo.fiz-karlsruhe.de/matwerk/E3081> ;
    mwo:hasAcronym "IMWS"^^xsd:string ;
    mwo:hasPostalCode "6120" ;
    mwo:hasWebsite <http://demo.fiz-karlsruhe.de/matwerk/E87321> .

<http://demo.fiz-karlsruhe.de/matwerk/E117404> a nfdicore:Website ;
    rdfs:label "https://vallico.net/casinoqmc/request-a-copy/"^^xsd:anyURI ;
    nfdicore:url <https://vallico.net/casinoqmc/request-a-copy/> .

<http://demo.fiz-karlsruhe.de/matwerk/E1178346> a emmo:EMMO_4207e895_8b83_4318_996a_72cfb32acd94 ;
    rdfs:label "Nickel" .

<http://demo.fiz-karlsruhe.de/matwerk/E117887> a nfdicore:Website ;
    rdfs:label "https://gims.ms1p.org/"^^xsd:anyURI ;
    nfdicore:url <https://gims.ms1p.org/> .

<http://demo.fiz-karlsruhe.de/matwerk/E1179881> a emmo:EMMO_4207e895_8b83_4318_996a_72cfb32acd94 ;
    rdfs:label "Nimonic 75 nickel-base alloy" .

<http://demo.fiz-karlsruhe.de/matwerk/E1181418> a emmo:EMMO_4207e895_8b83_4318_996a_72cfb32acd94 ;
    rdfs:label "EN AW-2618A" .

<http://demo.fiz-karlsruhe.de/matwerk/E1182954> a emmo:EMMO_4207e895_8b83_4318_996a_72cfb32acd94 ;
    rdfs:label "structural steel S355" .

<http://demo.fiz-karlsruhe.de/matwerk/E118371> a nfdicore:Website ;
    rdfs:label "https://vibes-developers.gitlab.io/vibes/"^^xsd:anyURI ;
    nfdicore:url <https://vibes-developers.gitlab.io/vibes/> .

<http://demo.fiz-karlsruhe.de/matwerk/E1184492> a nfdicore:AcademicDiscipline ;
    rdfs:label "Computational analysis; Dislocations; Grain boundaries; Vein structures" .

<http://demo.fiz-karlsruhe.de/matwerk/E1186031> a nfdicore:AcademicDiscipline ;
    rdfs:label "Generated data from the 2PC-equivalent structures." .

<http://demo.fiz-karlsruhe.de/matwerk/E1187571> a nfdicore:AcademicDiscipline ;
    rdfs:label "This dataset was used in the work \"Material modeling for parametric, anisotropic finite hyperelasticity based on machine learning with application in optimization of metamaterials" .

<http://demo.fiz-karlsruhe.de/matwerk/E11879> a nfdicore:Person ;
    rdfs:label "Dr.  Thomas Hanke" ;
    mwo:emailAddress "thomas.hanke@materials.fraunhofer.de"^^xsd:string ;
    mwo:hasAffiliation <http://demo.fiz-karlsruhe.de/matwerk/E1106> ;
    foaf:firstName "Thomas"^^xsd:string ;
    foaf:surname "Hanke"^^xsd:string ;
    foaf:title "Dr. "^^xsd:string .

<http://demo.fiz-karlsruhe.de/matwerk/E118856> a nfdicore:Website ;
    rdfs:label "https://avogadro.cc/"^^xsd:anyURI ;
    nfdicore:url <https://avogadro.cc/> .

<http://demo.fiz-karlsruhe.de/matwerk/E1189112> a nfdicore:AcademicDiscipline ;
    rdfs:label "This dataset was used in the work \"On-the-Fly Adaptivity for Nonlinear Twoscale Simulations Using Artificial Neural Networks and Reduced Order Modeling\" by F. Fritzen, M. Fernández,  and F. Larsson" .

<http://demo.fiz-karlsruhe.de/matwerk/E1190654> a nfdicore:AcademicDiscipline ;
    rdfs:label "high temperature mechanical behavior" .

<http://demo.fiz-karlsruhe.de/matwerk/E1191> a nfdicore:Organization ;
    rdfs:label "Institute of Materials Science and Engineering",
        "Lehrstuhl für Werkstoffkunde"@de ;
    nfdicore:location <http://demo.fiz-karlsruhe.de/matwerk/E77246> ;
    nfdicore:parentOrganisation <http://demo.fiz-karlsruhe.de/matwerk/E3146> ;
    mwo:hasAcronym "WKK"^^xsd:string ;
    mwo:hasPostalCode "67653" ;
    mwo:hasWebsite <http://demo.fiz-karlsruhe.de/matwerk/E87737> .

<http://demo.fiz-karlsruhe.de/matwerk/E1192197> a nfdicore:AcademicDiscipline ;
    rdfs:label "long-term aging" .

<http://demo.fiz-karlsruhe.de/matwerk/E119342> a nfdicore:Website ;
    rdfs:label "https://www.pyretis.org/current/index.html"^^xsd:anyURI ;
    nfdicore:url <https://www.pyretis.org/current/index.html> .

<http://demo.fiz-karlsruhe.de/matwerk/E1193741> a nfdicore:AcademicDiscipline ;
    rdfs:label "mechanical testing" ;
    owl:sameAs <http://www.wikidata.org/entity/Q76431588> .

<http://demo.fiz-karlsruhe.de/matwerk/E1195286> a nfdicore:Standard ;
    rdfs:label "ASTM E139 -11" .

<http://demo.fiz-karlsruhe.de/matwerk/E119829> a nfdicore:Website ;
    rdfs:label "http://openpathsampling.org"^^xsd:anyURI ;
    nfdicore:url <http://openpathsampling.org> .

<http://demo.fiz-karlsruhe.de/matwerk/E1198379> a nfdicore:ObjectType ;
    rdfs:label "Python scripts" .

<http://demo.fiz-karlsruhe.de/matwerk/E1199927> a nfdicore:ObjectType ;
    rdfs:label "Jupyter notebooks" .

<http://demo.fiz-karlsruhe.de/matwerk/E1201476> a nfdicore:ObjectType ;
    rdfs:label "HDF5 data" .

<http://demo.fiz-karlsruhe.de/matwerk/E1203026> a nfdicore:ObjectType ;
    rdfs:label "H5 data and Jupyter Notesbooks" .

<http://demo.fiz-karlsruhe.de/matwerk/E120317> a nfdicore:Website ;
    rdfs:label "https://www.materialscloud.org/work/tools/seekpath"^^xsd:anyURI ;
    nfdicore:url <https://www.materialscloud.org/work/tools/seekpath> .

<http://demo.fiz-karlsruhe.de/matwerk/E1204577> a nfdicore:ObjectType ;
    rdfs:label "tensorflow model and data" .

<http://demo.fiz-karlsruhe.de/matwerk/E1206129> a nfdicore:ObjectType ;
    rdfs:label "test data" .

<http://demo.fiz-karlsruhe.de/matwerk/E1207682> a nfdicore:ObjectType ;
    rdfs:label "compilation of test results" .

<http://demo.fiz-karlsruhe.de/matwerk/E120806> a nfdicore:Website ;
    rdfs:label "https://pymatgen.org/"^^xsd:anyURI ;
    nfdicore:url <https://pymatgen.org/> .

<http://demo.fiz-karlsruhe.de/matwerk/E1209236> a nfdicore:ObjectType ;
    rdfs:label "additional information on material" .

<http://demo.fiz-karlsruhe.de/matwerk/E1211> a nfdicore:Organization ;
    rdfs:label "Department of Computer Science",
        "Fachbereich Informatik"@de ;
    nfdicore:location <http://demo.fiz-karlsruhe.de/matwerk/E77246> ;
    nfdicore:parentOrganisation <http://demo.fiz-karlsruhe.de/matwerk/E3146> ;
    mwo:hasPostalCode "67653" ;
    mwo:hasWebsite <http://demo.fiz-karlsruhe.de/matwerk/E88154> .

<http://demo.fiz-karlsruhe.de/matwerk/E121296> a nfdicore:Website ;
    rdfs:label "https://molmod.ugent.be/software/tamkin"^^xsd:anyURI ;
    nfdicore:url <https://molmod.ugent.be/software/tamkin> .

<http://demo.fiz-karlsruhe.de/matwerk/E1213904> a nfdicore:ObjectType ;
    rdfs:label "hardness data" .

<http://demo.fiz-karlsruhe.de/matwerk/E1215462> a nfdicore:ObjectType ;
    rdfs:label "information on material" .

<http://demo.fiz-karlsruhe.de/matwerk/E1217021> a nfdicore:ObjectType ;
    rdfs:label "aging treatment" .

<http://demo.fiz-karlsruhe.de/matwerk/E121787> a nfdicore:Website ;
    rdfs:label "https://lammps.github.io/pizza/"^^xsd:anyURI ;
    nfdicore:url <https://lammps.github.io/pizza/> .

<http://demo.fiz-karlsruhe.de/matwerk/E1220142> a dcterms:FileFormat ;
    rdfs:label "EDN" .

<http://demo.fiz-karlsruhe.de/matwerk/E122279> a nfdicore:Website ;
    rdfs:label "https://www.mdtraj.org"^^xsd:anyURI ;
    nfdicore:url <https://www.mdtraj.org> .

<http://demo.fiz-karlsruhe.de/matwerk/E1223267> a dcterms:FileFormat ;
    rdfs:label "JSON" .

<http://demo.fiz-karlsruhe.de/matwerk/E1224831> a dcterms:FileFormat ;
    rdfs:label "smiles" .

<http://demo.fiz-karlsruhe.de/matwerk/E1226396> a dcterms:FileFormat ;
    rdfs:label "SFD" .

<http://demo.fiz-karlsruhe.de/matwerk/E122772> a nfdicore:Website ;
    rdfs:label "http://nglviewer.org/nglview/latest/"^^xsd:anyURI ;
    nfdicore:url <http://nglviewer.org/nglview/latest/> .

<http://demo.fiz-karlsruhe.de/matwerk/E1227962> a dcterms:FileFormat ;
    rdfs:label "CIF" .

<http://demo.fiz-karlsruhe.de/matwerk/E1229529> a nfdicore:Website ;
    rdfs:label "https://gate.hzdr.de/user/"^^xsd:anyURI ;
    nfdicore:url <https://gate.hzdr.de/user/> .

<http://demo.fiz-karlsruhe.de/matwerk/E1232> a nfdicore:Organization ;
    rdfs:label "Leibniz Institute for Materials Engineering",
        "Leibniz-Institut für Werkstofforientierte Technologien"@de ;
    nfdicore:location <http://demo.fiz-karlsruhe.de/matwerk/E77637> ;
    nfdicore:parentOrganisation <http://demo.fiz-karlsruhe.de/matwerk/E2597> ;
    mwo:hasAcronym "IWT Bremen"^^xsd:string ;
    mwo:hasPostalCode "28359" ;
    mwo:hasWebsite <http://demo.fiz-karlsruhe.de/matwerk/E88572> .

<http://demo.fiz-karlsruhe.de/matwerk/E123266> a nfdicore:Website ;
    rdfs:label "https://molmod.github.io/QuickFF/"^^xsd:anyURI ;
    nfdicore:url <https://molmod.github.io/QuickFF/> .

<http://demo.fiz-karlsruhe.de/matwerk/E1232666> a ns3:SWO_0000001 ;
    rdfs:label "scikit-image" .

<http://demo.fiz-karlsruhe.de/matwerk/E1235807> a ns3:SWO_0000001 ;
    rdfs:label "calphy" .

<http://demo.fiz-karlsruhe.de/matwerk/E1237379> a ns3:SWO_0000001 ;
    rdfs:label "runner" .

<http://demo.fiz-karlsruhe.de/matwerk/E123761> a nfdicore:Website ;
    rdfs:label "https://molmod.ugent.be/software/yaff"^^xsd:anyURI ;
    nfdicore:url <https://molmod.ugent.be/software/yaff> .

<http://demo.fiz-karlsruhe.de/matwerk/E1238952> a nfdicore:Software,
        ns3:SWO_0000001 ;
    rdfs:label "atomicrex" ;
    dcterms:description "atomicrex is a versatile tool for the construction of advanced atomistic models. It is written in C++ and Python.  It was primarily developed to fit interatomic potential models. Thanks to its flexible generic structure its application range, however, is larger. In a general sense, it allows one to develop models that describe a given property as a function of an atomic (or atom-like) configuration. The property in question can be scalar or vectorial in nature, and could represent e.g., total energies and forces."^^xsd:string ;
    mwo:hasRepository <http://demo.fiz-karlsruhe.de/matwerk/E199136> ;
    mwo:hasWebsite <http://demo.fiz-karlsruhe.de/matwerk/E127254> ;
    ns3:has_license <http://demo.fiz-karlsruhe.de/matwerk/E762996> ;
    schema:citation <http://demo.fiz-karlsruhe.de/matwerk/E938766> .

<http://demo.fiz-karlsruhe.de/matwerk/E124257> a nfdicore:Website ;
    rdfs:label "https://computationalmaterials.gitlab.io/clease/"^^xsd:anyURI ;
    nfdicore:url <https://computationalmaterials.gitlab.io/clease/> .

<http://demo.fiz-karlsruhe.de/matwerk/E1243677> a ns3:SWO_0000001 ;
    rdfs:label "Runner" .

<http://demo.fiz-karlsruhe.de/matwerk/E1245254> a ns3:SWO_0000001 ;
    rdfs:label "Atomicrex" .

<http://demo.fiz-karlsruhe.de/matwerk/E1245567> a nfdicore:AcademicDiscipline ;
    rdfs:label "Knowledge Graph Embedding" .

<http://demo.fiz-karlsruhe.de/matwerk/E1245569> a nfdicore:AcademicDiscipline ;
    rdfs:label "Machine Learning" .

<http://demo.fiz-karlsruhe.de/matwerk/E1245572> a nfdicore:AcademicDiscipline ;
    rdfs:label "NLP" .

<http://demo.fiz-karlsruhe.de/matwerk/E1245595> a nfdicore:Website ;
    rdfs:label "https://www.bam.de/Navigation/DE/Home/home.html"^^xsd:anyURI ;
    nfdicore:url <https://www.bam.de/Navigation/DE/Home/home.html> .

<http://demo.fiz-karlsruhe.de/matwerk/E1245610> a nfdicore:Organization ;
    rdfs:label "Max-Planck-Institut für Eisenforschung" ;
    nfdicore:location <http://demo.fiz-karlsruhe.de/matwerk/E71877> ;
    nfdicore:parentOrganisation <http://demo.fiz-karlsruhe.de/matwerk/E2379> ;
    mwo:hasAcronym "MPIE"^^xsd:string ;
    mwo:hasPostalCode "40237" ;
    mwo:hasWebsite <http://demo.fiz-karlsruhe.de/matwerk/E80402> .

<http://demo.fiz-karlsruhe.de/matwerk/E1245710> a nfdicore:AcademicDiscipline ;
    rdfs:label "Data Science" .

<http://demo.fiz-karlsruhe.de/matwerk/E1245727> a nfdicore:AcademicDiscipline ;
    rdfs:label "Metadata" .

<http://demo.fiz-karlsruhe.de/matwerk/E1245745> a nfdicore:AcademicDiscipline ;
    rdfs:label "Micromechanics" .

<http://demo.fiz-karlsruhe.de/matwerk/E1245764> a nfdicore:AcademicDiscipline ;
    rdfs:label "Tribology" .

<http://demo.fiz-karlsruhe.de/matwerk/E1245784> a nfdicore:AcademicDiscipline ;
    rdfs:label "Experimental and Model Based Mechanical Behaviour of Materials" .

<http://demo.fiz-karlsruhe.de/matwerk/E1245805> a nfdicore:AcademicDiscipline ;
    rdfs:label "Multi-Scale Modelling of Fracture" .

<http://demo.fiz-karlsruhe.de/matwerk/E1245827> a nfdicore:AcademicDiscipline ;
    rdfs:label "Nanomechanics and Small-Scale Plasticity" .

<http://demo.fiz-karlsruhe.de/matwerk/E1245850> a nfdicore:AcademicDiscipline ;
    rdfs:label "Mechanical Behavior of Interface-Dominated Materials" .

<http://demo.fiz-karlsruhe.de/matwerk/E1245874> a nfdicore:AcademicDiscipline ;
    rdfs:label "Deformation and Failure of Amorphous Materials" .

<http://demo.fiz-karlsruhe.de/matwerk/E1245899> a nfdicore:AcademicDiscipline ;
    rdfs:label "Plasticity and Fracture of Complex Crystals" .

<http://demo.fiz-karlsruhe.de/matwerk/E1245925> a nfdicore:AcademicDiscipline ;
    rdfs:label "material behavior under load" .

<http://demo.fiz-karlsruhe.de/matwerk/E1245952> a nfdicore:AcademicDiscipline ;
    rdfs:label "Ab initio determination of phase diagrams" .

<http://demo.fiz-karlsruhe.de/matwerk/E1245980> a nfdicore:AcademicDiscipline ;
    rdfs:label "Thermodynamics and kinetics of metallic alloys" .

<http://demo.fiz-karlsruhe.de/matwerk/E1246009> a nfdicore:AcademicDiscipline ;
    rdfs:label "Theory of magnetism" .

<http://demo.fiz-karlsruhe.de/matwerk/E1246039> a nfdicore:AcademicDiscipline ;
    rdfs:label "many-body theory" .

<http://demo.fiz-karlsruhe.de/matwerk/E1246070> a nfdicore:AcademicDiscipline ;
    rdfs:label "Shape memory alloys" .

<http://demo.fiz-karlsruhe.de/matwerk/E1246102> a nfdicore:AcademicDiscipline ;
    rdfs:label "massive model visualization" .

<http://demo.fiz-karlsruhe.de/matwerk/E1246135> a nfdicore:AcademicDiscipline ;
    rdfs:label "3D Internet technology" .

<http://demo.fiz-karlsruhe.de/matwerk/E1246169> a nfdicore:AcademicDiscipline ;
    rdfs:label "distributed media applications" .

<http://demo.fiz-karlsruhe.de/matwerk/E1246204> a nfdicore:AcademicDiscipline ;
    rdfs:label "novel 3D tomographic reconstructions" .

<http://demo.fiz-karlsruhe.de/matwerk/E1246240> a nfdicore:AcademicDiscipline ;
    rdfs:label "Materials Informatic" .

<http://demo.fiz-karlsruhe.de/matwerk/E1246243> a nfdicore:Organization ;
    rdfs:label "DFKI" .

<http://demo.fiz-karlsruhe.de/matwerk/E1246245> a nfdicore:Person ;
    rdfs:label "MSc. Alaukik Saxena" ;
    mwo:emailAddress "saxena@mpie.de"^^xsd:string ;
    mwo:hasAffiliation <http://demo.fiz-karlsruhe.de/matwerk/E1245610> ;
    mwo:hasORCID <https://orcid.org/0000-0001-6714-0954> ;
    foaf:firstName "Alaukik"^^xsd:string ;
    foaf:surname "Saxena"^^xsd:string ;
    foaf:title "MSc."^^xsd:string .

<http://demo.fiz-karlsruhe.de/matwerk/E1246248> a nfdicore:Person ;
    rdfs:label "Dr.-Ing. Markus Kühbach" ;
    mwo:emailAddress "kuehbacm@physik.hu-berlin.de"^^xsd:string ;
    mwo:hasAffiliation <http://demo.fiz-karlsruhe.de/matwerk/E3486> ;
    mwo:hasORCID <https://orcid.org/0000-0002-7117-5196> ;
    foaf:firstName "Markus"^^xsd:string ;
    foaf:surname "Kühbach"^^xsd:string ;
    foaf:title "Dr.-Ing."^^xsd:string .

<http://demo.fiz-karlsruhe.de/matwerk/E1246263> rdfs:label "gwyfile" .

<http://demo.fiz-karlsruhe.de/matwerk/E1246270> rdfs:label "numpy" .

<http://demo.fiz-karlsruhe.de/matwerk/E1246278> rdfs:label "matplotlib" .

<http://demo.fiz-karlsruhe.de/matwerk/E1246287> rdfs:label "skimage" .

<http://demo.fiz-karlsruhe.de/matwerk/E1246297> rdfs:label "pillow" .

<http://demo.fiz-karlsruhe.de/matwerk/E1246308> rdfs:label "Pyiron_atomistics" .

<http://demo.fiz-karlsruhe.de/matwerk/E1246320> rdfs:label "Pyiron_contrib" .

<http://demo.fiz-karlsruhe.de/matwerk/E1246333> rdfs:label "Pyiron_gpl" .

<http://demo.fiz-karlsruhe.de/matwerk/E1246347> rdfs:label "lammps" .

<http://demo.fiz-karlsruhe.de/matwerk/E1246395> rdfs:label "Paraprobe-toolbox" .

<http://demo.fiz-karlsruhe.de/matwerk/E1246413> a mwo:Repository ;
    rdfs:label "https://github.com/eisenforschung/CompositionSpace"^^xsd:anyURI ;
    nfdicore:url <https://github.com/eisenforschung/CompositionSpace> .

<http://demo.fiz-karlsruhe.de/matwerk/E1246432> a mwo:Repository ;
    rdfs:label "https://github.com/pyscal/pyscal_rdf"^^xsd:anyURI ;
    nfdicore:url <https://github.com/pyscal/pyscal_rdf> .

<http://demo.fiz-karlsruhe.de/matwerk/E1246452> a mwo:Repository ;
    rdfs:label "https://git.rwth-aachen.de/nfdi-matwerk/ta-wsd/user-journey-indentation/-/tree/imprint-estimate/ImprintEstimation"^^xsd:anyURI ;
    nfdicore:url <https://git.rwth-aachen.de/nfdi-matwerk/ta-wsd/user-journey-indentation/-/tree/imprint-estimate/ImprintEstimation> .

<http://demo.fiz-karlsruhe.de/matwerk/E1246473> a mwo:Repository ;
    rdfs:label "https://gitlab.mpcdf.mpg.de/smenon/elastic-constant-demo"^^xsd:anyURI ;
    nfdicore:url <https://gitlab.mpcdf.mpg.de/smenon/elastic-constant-demo> .

<http://demo.fiz-karlsruhe.de/matwerk/E1246518> a mwo:Documentation ;
    rdfs:label "https://compositionspace.readthedocs.io/en/latest/"^^xsd:anyURI ;
    nfdicore:url <https://compositionspace.readthedocs.io/en/latest/> .

<http://demo.fiz-karlsruhe.de/matwerk/E1246542> a mwo:Documentation ;
    rdfs:label "https://rdf.pyscal.org"^^xsd:anyURI ;
    nfdicore:url <https://rdf.pyscal.org> .

<http://demo.fiz-karlsruhe.de/matwerk/E1246567> a nfdicore:Software,
        mwo:ResearchSoftware ;
    rdfs:label "CompositionSpace" ;
    nfdicore:programmingLanguage <http://demo.fiz-karlsruhe.de/matwerk/E836279> ;
    dcterms:description "CompositionSpace is a python library for analysis of APT data. "^^xsd:string ;
    mwo:hasContributor <http://demo.fiz-karlsruhe.de/matwerk/E1246242> ;
    mwo:hasDiscipline <http://demo.fiz-karlsruhe.de/matwerk/E1245665> ;
    mwo:hasDocumentation <http://demo.fiz-karlsruhe.de/matwerk/E1246518> ;
    mwo:hasRepository <http://demo.fiz-karlsruhe.de/matwerk/E1246413> ;
    mwo:usesMethod <http://demo.fiz-karlsruhe.de/matwerk/E1246872> ;
    ns3:has_license <http://demo.fiz-karlsruhe.de/matwerk/E1246803> ;
    schema:operatingSystem ns3:SWO_0000022 .

<http://demo.fiz-karlsruhe.de/matwerk/E1246593> a nfdicore:Resource,
        nfdicore:Software,
        mwo:ResearchSoftware ;
    rdfs:label "pyscal_rdf" ;
    nfdicore:programmingLanguage <http://demo.fiz-karlsruhe.de/matwerk/E836279> ;
    dcterms:description "pyscal_rdf is a python tool for ontology-based creation, manipulation, and quering of structures. pyscal_rdf uses the Computational Material Sample Ontology (CMSO). "^^xsd:string ;
    mwo:hasContactPoint <http://demo.fiz-karlsruhe.de/matwerk/E8627> ;
    mwo:hasContributor <http://demo.fiz-karlsruhe.de/matwerk/E1246242> ;
    mwo:hasDiscipline <http://demo.fiz-karlsruhe.de/matwerk/E42042> ;
    mwo:hasDocumentation <http://demo.fiz-karlsruhe.de/matwerk/E1246542> ;
    mwo:hasRelatedResource <http://demo.fiz-karlsruhe.de/matwerk/E1247323> ;
    mwo:hasRepository <http://demo.fiz-karlsruhe.de/matwerk/E1246432> ;
    mwo:hasVersion "0.0.4" ;
    mwo:usesMethod <http://demo.fiz-karlsruhe.de/matwerk/E1246908> ;
    ns3:has_license <http://demo.fiz-karlsruhe.de/matwerk/E759297> ;
    schema:operatingSystem ns3:SWO_0000022,
        ns3:SWO_0000149,
        ns3:SWO_9000072 .

<http://demo.fiz-karlsruhe.de/matwerk/E1246648> a nfdicore:Resource,
        nfdicore:Software,
        mwo:ComputationalWorkflow ;
    rdfs:label "Elastic Constant Demo" ;
    nfdicore:fundingProject <http://demo.fiz-karlsruhe.de/matwerk/E1247022> ;
    nfdicore:programmingLanguage <http://demo.fiz-karlsruhe.de/matwerk/E836279> ;
    dcterms:description "Workflow to calculate elastic constants of Al alloy"^^xsd:string ;
    mwo:hasContactPoint <http://demo.fiz-karlsruhe.de/matwerk/E8627> ;
    mwo:hasContributor <http://demo.fiz-karlsruhe.de/matwerk/E1246242> ;
    mwo:hasDiscipline <http://demo.fiz-karlsruhe.de/matwerk/E42042> ;
    mwo:hasFormat <http://demo.fiz-karlsruhe.de/matwerk/E1246252> ;
    mwo:hasRelatedResource <http://demo.fiz-karlsruhe.de/matwerk/E1247418> ;
    mwo:hasRepository <http://demo.fiz-karlsruhe.de/matwerk/E1246473> ;
    mwo:keyword "Aluminium",
        "EAM",
        "Elastic Constants",
        "LAMMPS",
        "MEAM",
        "Silicon" ;
    mwo:usesMethod <http://demo.fiz-karlsruhe.de/matwerk/E1246983> ;
    ns3:SWO_0000082 <http://demo.fiz-karlsruhe.de/matwerk/E1246308>,
        <http://demo.fiz-karlsruhe.de/matwerk/E1246320>,
        <http://demo.fiz-karlsruhe.de/matwerk/E1246333>,
        <http://demo.fiz-karlsruhe.de/matwerk/E1246347>,
        <http://demo.fiz-karlsruhe.de/matwerk/E1246362>,
        <http://demo.fiz-karlsruhe.de/matwerk/E457491> ;
    ns3:has_license <http://demo.fiz-karlsruhe.de/matwerk/E740937> ;
    schema:dateCreated "4/20/2023"^^xsd:time ;
    schema:datePublished "4/20/2023"^^xsd:time ;
    schema:operatingSystem ns3:SWO_0000022,
        ns3:SWO_0000149,
        ns3:SWO_9000072 .

<http://demo.fiz-karlsruhe.de/matwerk/E1246908> a mwo:Method ;
    rdfs:label "Atomistic simulations" .

<http://demo.fiz-karlsruhe.de/matwerk/E1246945> a mwo:Method ;
    rdfs:label "Image processing" .

<http://demo.fiz-karlsruhe.de/matwerk/E1247323> a nfdicore:Resource,
        mwo:SemanticResource ;
    rdfs:label "Computational Material Sample Ontology" ;
    nfdicore:relatedProject <http://demo.fiz-karlsruhe.de/matwerk/E1247022> ;
    nfdicore:semanticExpressivity nfdicore:Ontology ;
    mwo:description "CMSO is an ontology that aims to describe computational materials science samples (or structures), including crystalline defects." ;
    mwo:hasAcronym "CMSO"^^xsd:string ;
    mwo:hasContactPoint <http://demo.fiz-karlsruhe.de/matwerk/E10046> ;
    mwo:hasDiscipline <http://demo.fiz-karlsruhe.de/matwerk/E42042> ;
    mwo:hasFormat <http://demo.fiz-karlsruhe.de/matwerk/E1247808> ;
    mwo:hasRelatedResource <http://demo.fiz-karlsruhe.de/matwerk/E1246593> ;
    mwo:hasRepository <http://demo.fiz-karlsruhe.de/matwerk/E1247672> ;
    mwo:keyword "computational materials science",
        "defects",
        "ontology" ;
    ns3:has_license <http://demo.fiz-karlsruhe.de/matwerk/E759297> .

<http://demo.fiz-karlsruhe.de/matwerk/E1247418> a nfdicore:Dataset,
        nfdicore:Resource ;
    rdfs:label "Elastic Constant Demo Data" ;
    nfdicore:fileExtension ".h5" ;
    mwo:aboutMaterial <http://demo.fiz-karlsruhe.de/matwerk/E1247872>,
        <http://demo.fiz-karlsruhe.de/matwerk/E1247879> ;
    mwo:description "Data containing elastic constants of Al alloy" ;
    mwo:hasCreator <http://demo.fiz-karlsruhe.de/matwerk/E8627> ;
    mwo:hasDiscipline <http://demo.fiz-karlsruhe.de/matwerk/E42042> ;
    mwo:hasRelatedResource <http://demo.fiz-karlsruhe.de/matwerk/E1246648> ;
    mwo:hasRepository <http://demo.fiz-karlsruhe.de/matwerk/E1247854> ;
    mwo:keyword "Aluminium",
        "EAM",
        "Elastic Constants",
        "LAMMPS",
        "MEAM",
        "Silicon" ;
    mwo:usesMethod <http://demo.fiz-karlsruhe.de/matwerk/E1246983> ;
    ns3:has_license <http://demo.fiz-karlsruhe.de/matwerk/E740937> ;
    schema:datePublished "4/20/2023" .

<http://demo.fiz-karlsruhe.de/matwerk/E1247533> a modsci:ScientificInstrumentManufacturer ;
    rdfs:label "Fischerscope" .

<http://demo.fiz-karlsruhe.de/matwerk/E1247539> a modsci:ScientificInstrumentManufacturer ;
    rdfs:label "LEXT" .

<http://demo.fiz-karlsruhe.de/matwerk/E124754> a nfdicore:Website ;
    rdfs:label "https://pycalphad.org/"^^xsd:anyURI ;
    nfdicore:url <https://pycalphad.org/> .

<http://demo.fiz-karlsruhe.de/matwerk/E1247563> a modsci:ScientificInstrumentManufacturer ;
    rdfs:label "HBM" .

<http://demo.fiz-karlsruhe.de/matwerk/E1247573> a modsci:ScientificInstrumentManufacturer ;
    rdfs:label "BAM 5.2" .

<http://demo.fiz-karlsruhe.de/matwerk/E1247584> a modsci:Technology ;
    rdfs:label "Vickers nanoindentation" .

<http://demo.fiz-karlsruhe.de/matwerk/E1247596> a modsci:Technology ;
    rdfs:label "Confocal microscopy" .

<http://demo.fiz-karlsruhe.de/matwerk/E1247638> a modsci:Technology ;
    rdfs:label "Displacement measurement" .

<http://demo.fiz-karlsruhe.de/matwerk/E1247654> a modsci:Technology ;
    rdfs:label "Temperature calibration" .

<http://demo.fiz-karlsruhe.de/matwerk/E1247672> a mwo:Repository ;
    rdfs:label "https://github.com/Materials-Data-Science-and-Informatics/cmso-ontology"^^xsd:anyURI ;
    nfdicore:url <https://github.com/Materials-Data-Science-and-Informatics/cmso-ontology> .

<http://demo.fiz-karlsruhe.de/matwerk/E1247675> a mwo:Repository ;
    rdfs:label "https://git.rwth-aachen.de/nfdi-matwerk/ta-mdi/demonstrator_iuc02/-/blob/main/Data%20Schema%20IUC02/04.04.23_PP18_JSON_Schema.json"^^xsd:anyURI ;
    nfdicore:url <https://git.rwth-aachen.de/nfdi-matwerk/ta-mdi/demonstrator_iuc02/-/blob/main/Data%20Schema%20IUC02/04.04.23_PP18_JSON_Schema.json> .

<http://demo.fiz-karlsruhe.de/matwerk/E1247678> a mwo:Documentation ;
    rdfs:label "https://fairmat-experimental.github.io/nexus-fairmat-proposal/9636feecb79bb32b828b1a9804269573256d7696/index.html"^^xsd:anyURI ;
    nfdicore:url <https://fairmat-experimental.github.io/nexus-fairmat-proposal/9636feecb79bb32b828b1a9804269573256d7696/index.html> .

<http://demo.fiz-karlsruhe.de/matwerk/E1247727> a nfdicore:Resource,
        nfdicore:Specification ;
    rdfs:label "User Journey: Indentation" ;
    nfdicore:relatedProject <http://demo.fiz-karlsruhe.de/matwerk/E1247022> ;
    mwo:description "an EN AW 1050A sample is polished and indented and the load-displacement curve is recorded, which is used to calculate the Young's modulus according to the Oliver-Pharr Method. Afterwards the surface height profile is measured." ;
    mwo:hasContactPoint <http://demo.fiz-karlsruhe.de/matwerk/E1245575> ;
    mwo:hasDiscipline <http://demo.fiz-karlsruhe.de/matwerk/E1245665> ;
    mwo:hasFormat <http://demo.fiz-karlsruhe.de/matwerk/E1247825> ;
    mwo:hasRelatedResource <http://demo.fiz-karlsruhe.de/matwerk/E1247370>,
        <http://demo.fiz-karlsruhe.de/matwerk/E1247866> ;
    mwo:hasRepository <http://demo.fiz-karlsruhe.de/matwerk/E1247673> ;
    mwo:keyword "Aluminium",
        "Elastic Constants",
        "Indentation",
        "Young's modulus" ;
    mwo:usesMethod <http://demo.fiz-karlsruhe.de/matwerk/E1247857> ;
    ns3:has_license <http://demo.fiz-karlsruhe.de/matwerk/E1247861> ;
    schema:dateCreated "20:23:00-03:00"^^xsd:time ;
    schema:datePublished "2023-04-20T00:00:00.000Z" .

<http://demo.fiz-karlsruhe.de/matwerk/E1247777> a nfdicore:Organization ;
    rdfs:label "KIT"@de .

<http://demo.fiz-karlsruhe.de/matwerk/E1247808> a dcterms:FileFormat ;
    rdfs:label ".owl" .

<http://demo.fiz-karlsruhe.de/matwerk/E1247845> a emmo:EMMO_4207e895_8b83_4318_996a_72cfb32acd94 ;
    rdfs:label "EN AW 2618A" .

<http://demo.fiz-karlsruhe.de/matwerk/E1247850> a nfdicore:AcademicDiscipline ;
    rdfs:label "Quantitative microstructural analysis of transmission electron microscopy (TEM)" .

<http://demo.fiz-karlsruhe.de/matwerk/E1247851> a nfdicore:Organization ;
    rdfs:label "Max-Planck-Institut für Eisenforschung (MPIE"@de .

<http://demo.fiz-karlsruhe.de/matwerk/E1247854> a mwo:Repository ;
    rdfs:label "http://hdl.handle.net/21.11102/7f78d0ed-4855-4fdf-b764-0bea725f8821"^^xsd:anyURI ;
    nfdicore:url <http://hdl.handle.net/21.11102/7f78d0ed-4855-4fdf-b764-0bea725f8821> .

<http://demo.fiz-karlsruhe.de/matwerk/E1247879> a emmo:EMMO_4207e895_8b83_4318_996a_72cfb32acd94 ;
    rdfs:label "Silicon" .

<http://demo.fiz-karlsruhe.de/matwerk/E1247895> a nfdicore:Project ;
    rdfs:label "WP SD-1.1 Develop Processes for Translating Community Needs into Infrastructure; WP SD-1.2 Develop and Implement Consortium Governance; WP SD-1.3 IUC-Management; WP SD-1.4 Community Participation in Strategy Development; WP SD-2.1 Community Needs" .

<http://demo.fiz-karlsruhe.de/matwerk/E1247901> a nfdicore:Project ;
    rdfs:label "Surveys and Evaluation; WP SD-2.2 Stakeholder Management; WP SD-2.3 Development of Consortium Branding; WP SD-2.4 Public Affairs; WP SD-3.1 Sharing and Curating Incentives; WP SD-3.2 Research Game-Theory Approaches for Interactions; WP SD-3.3 Business models; WP SD-4.1 Consortium Coordination; WP SD-4.2 Quality Assurance; WP SD-4.3 Project Management and Reporting Toolbox; WP SD-4.4 Fostering International Relations; WP SD-4.5 Infrastructure Issue Tracking; WP SD-5.1 Ensure compliance with NFDI; WP SD-5.2 Data Protection Guidelines; WP SD-5.3 Ownership and Sovereignty" .

<http://demo.fiz-karlsruhe.de/matwerk/E1247908> a nfdicore:Project ;
    rdfs:label "WP MDI-1.1 Administrative Graph Database; WP MDI-1.2 Data Registration and Ingestion Interfaces; WP MDI-1.3 (Meta-) Data Formats; WP MDI-1.4 Compute & Data Sharing Interfaces; WP MDI-1.5 Operating Model; WP MDI-1.6 Peer-to-peer Client; WP MDI-1.7 Local Version Control; WP MDI-2.1 Website; WP MDI-2.2 Community-Hub; WP MDI-2.3 App Store Infrastructure; WP MDI-2.4 Meta-Search Interface; WP MDI-3.1 Infrastructure Services; WP MDI-3.2 Integration of Ontologies; WP MDI-3.3 Search; WP MDI-3.4 High-level Services; WP MDI-4.1 Identity Space; WP MDI-4.2 Role and Group Management; WP MDI-4.3 Monitoring & Data Usage Analytics; WP MDI-4.4 Reference Applications; WP MDI-5.1 Coordination; WP MDI-5.2 Requirements Analysis & Feedback; WP MDI-5.3 Knowledge Base & Dissemination; WP MDI-5.4 Support; WP MDI-5.5 Infrastructure Use Cases; WP MDI-5.6 Operation Model" .

<http://demo.fiz-karlsruhe.de/matwerk/E1247916> a nfdicore:Project ;
    rdfs:label "Cost & Compensation Model;" .

<http://demo.fiz-karlsruhe.de/matwerk/E1247925> a nfdicore:Project ;
    rdfs:label "WP OMS-1.1 Support foundation and manage interaction of ontology working groups; WP OMS-1.2 Link and coordinate ontology working groups with existing community efforts; WP OMS-2.1 Requirement Analysis; WP OMS-2.2 A Collaborative Ontology Design Environment and Tools; WP OMS-2.3 Metadata Schemes; WP OMS-2.4 Ontology Design; WP OMS-2.5 Demonstrators for MSE Ontology; WP OMS-2.6 Ontology Evaluation; WP OMS-3.1 A “Simplified” Knowledge Graph; WP OMS-3.2 Distributed Infrastructure and Index; WP OMS-3.3 MSE Knowledge Graph; WP OMS-3.4 NFDI-MatWerk FAIR Linked (Open) Data; WP OMS-4.1 Workshops for Ontology Working Group interaction; WP OMS-4.2: MSE Ontology applications; WP OMS-4.3 MSE Ontology education and training;" .

<http://demo.fiz-karlsruhe.de/matwerk/E1247935> a nfdicore:Project ;
    rdfs:label "WP CI-1.1 Organizing; WP CI-1.2 Training courses for international students; WP CI-2.1 Academic teaching material; WP CI-2.2 Technical teaching material; WP CI-3.1 Content management; WP CI-4.1 Stimulating awareness and critical discourse; WP CI-5.1 Contact person; WP CI-5.2 Templates; WP CI-6.1 Conference and Meetings; WP CI-6.2 Events; WP CI-6.3 Expert Committees; WP CI-7.1 Elaboration of guidelines and standards; WP CI-8.1 Exemplary Guidelines; WP CI-9.1 Current state; WP CI-9.2 Journal interaction; WP CI-10.1 Management" .

<http://demo.fiz-karlsruhe.de/matwerk/E1247946> a nfdicore:Project ;
    rdfs:label "WP WSD-1.1 Coordination; WP WSD-1.2 Version Control; WP WSD-1.3 Automated Installation; WP WSD-1.4 Execution Framework; WP WDS-1.5 Support; WP WSD-2.1 Basic System; WP WSD-2.2 Graphical Language; WP WSD-2.3 Jupyter and SciPy Integration; WP WSD-2.4 ImageJ (Fiji) Integration; WP WSD-3.1 Basic System; WP WSD-3.2 Access Control; WP WSD-3.3 Citeability; WP WSD-4.1 Job managemen; WP WSD-4.2 Data storage; WP WSD-4.3 Interface to Ontology; WP WSD-4.4 Parser; WP WSD-4.5 IDE; WP WSD-5.1 Mechanical testing and characterization workflows; WP WSD-5.2 Workflows for high-throughput and data-intensive experiments; WP WSD-5.3 Electronic lab books (ELNs); WP WSD-5.4 Workflows for multiscale simulations; WP WSD-6.1 Error bars; WP WSD-6.2 Parser for experiment; WP WSD-6.3 High-throughput; WP WSD-6.4 Convergence; WP WSD-6.5 Error propagation; WP WSD-6.6 Data consistency; WP WSD-7.1 Basic Platform; WP WSD-7.2 Integration with DME; WP WSD-7.3 Data Splitting Support; WP WSD-7.4 Validation Engine;" .

<http://demo.fiz-karlsruhe.de/matwerk/E125252> a nfdicore:Website ;
    rdfs:label "https://compphysvienna.github.io/n2p2/"^^xsd:anyURI ;
    nfdicore:url <https://compphysvienna.github.io/n2p2/> .

<http://demo.fiz-karlsruhe.de/matwerk/E1254> a nfdicore:Organization ;
    rdfs:label "National Metrology Institute of Germany",
        "Physikalisch-Technische Bundesanstalt"@de ;
    nfdicore:location <http://demo.fiz-karlsruhe.de/matwerk/E78029> ;
    mwo:hasAcronym "PTB"^^xsd:string ;
    mwo:hasPostalCode "38116" ;
    mwo:hasWebsite <http://demo.fiz-karlsruhe.de/matwerk/E88991> .

<http://demo.fiz-karlsruhe.de/matwerk/E125751> a nfdicore:Website ;
    rdfs:label "https://hackingmaterials.lbl.gov/matminer/"^^xsd:anyURI ;
    nfdicore:url <https://hackingmaterials.lbl.gov/matminer/> .

<http://demo.fiz-karlsruhe.de/matwerk/E126251> a nfdicore:Website ;
    rdfs:label "https://hackingmaterials.lbl.gov/matminer/#"^^xsd:anyURI ;
    nfdicore:url <https://hackingmaterials.lbl.gov/matminer/#> .

<http://demo.fiz-karlsruhe.de/matwerk/E126752> a nfdicore:Website ;
    rdfs:label "https://matbench.materialsproject.org/"^^xsd:anyURI ;
    nfdicore:url <https://matbench.materialsproject.org/> .

<http://demo.fiz-karlsruhe.de/matwerk/E127254> a nfdicore:Website ;
    rdfs:label "https://atomicrex.org/"^^xsd:anyURI ;
    nfdicore:url <https://atomicrex.org/> .

<http://demo.fiz-karlsruhe.de/matwerk/E127757> a nfdicore:Website ;
    rdfs:label "https://hiphive.materialsmodeling.org/"^^xsd:anyURI ;
    nfdicore:url <https://hiphive.materialsmodeling.org/> .

<http://demo.fiz-karlsruhe.de/matwerk/E128261> a nfdicore:Website ;
    rdfs:label "https://wulffpack.materialsmodeling.org/"^^xsd:anyURI ;
    nfdicore:url <https://wulffpack.materialsmodeling.org/> .

<http://demo.fiz-karlsruhe.de/matwerk/E128766> a nfdicore:Website ;
    rdfs:label "https://dynasor.materialsmodeling.org/"^^xsd:anyURI ;
    nfdicore:url <https://dynasor.materialsmodeling.org/> .

<http://demo.fiz-karlsruhe.de/matwerk/E129272> a nfdicore:Website ;
    rdfs:label "https://sharc.materialsmodeling.org/"^^xsd:anyURI ;
    nfdicore:url <https://sharc.materialsmodeling.org/> .

<http://demo.fiz-karlsruhe.de/matwerk/E129779> a nfdicore:Website ;
    rdfs:label "https://vcsgc-lammps.materialsmodeling.org/"^^xsd:anyURI ;
    nfdicore:url <https://vcsgc-lammps.materialsmodeling.org/> .

<http://demo.fiz-karlsruhe.de/matwerk/E130287> a nfdicore:Website ;
    rdfs:label "http://aixvipmap.de/"^^xsd:anyURI ;
    nfdicore:url <http://aixvipmap.de/> .

<http://demo.fiz-karlsruhe.de/matwerk/E130796> a nfdicore:Website ;
    rdfs:label "https://www.mupif.org/"^^xsd:anyURI ;
    nfdicore:url <https://www.mupif.org/> .

<http://demo.fiz-karlsruhe.de/matwerk/E131306> a nfdicore:Website ;
    rdfs:label "https://www.simphony-project.eu/en/about-simphony.html"^^xsd:anyURI ;
    nfdicore:url <https://www.simphony-project.eu/en/about-simphony.html> .

<http://demo.fiz-karlsruhe.de/matwerk/E131817> a nfdicore:Website ;
    rdfs:label "https://www.mpcci.de/"^^xsd:anyURI ;
    nfdicore:url <https://www.mpcci.de/> .

<http://demo.fiz-karlsruhe.de/matwerk/E132329> a nfdicore:Website ;
    rdfs:label "https://www.vimmp.eu/"^^xsd:anyURI ;
    nfdicore:url <https://www.vimmp.eu/> .

<http://demo.fiz-karlsruhe.de/matwerk/E1326> a nfdicore:Organization ;
    rdfs:label "Lehrstuhl für Informatik" ;
    nfdicore:location <http://demo.fiz-karlsruhe.de/matwerk/E74154> ;
    nfdicore:parentOrganisation <http://demo.fiz-karlsruhe.de/matwerk/E3279> ;
    mwo:hasPostalCode "52062" ;
    mwo:hasWebsite <http://demo.fiz-karlsruhe.de/matwerk/E90254> .

<http://demo.fiz-karlsruhe.de/matwerk/E132842> a nfdicore:Website ;
    rdfs:label "https://open-model.eu"^^xsd:anyURI ;
    nfdicore:url <https://open-model.eu> .

<http://demo.fiz-karlsruhe.de/matwerk/E133356> a nfdicore:Website ;
    rdfs:label "https://math.lbl.gov/voro++/"^^xsd:anyURI ;
    nfdicore:url <https://math.lbl.gov/voro++/> .

<http://demo.fiz-karlsruhe.de/matwerk/E133871> a nfdicore:Website ;
    rdfs:label "http://www.qhull.org/"^^xsd:anyURI ;
    nfdicore:url <http://www.qhull.org/> .

<http://demo.fiz-karlsruhe.de/matwerk/E134387> a nfdicore:Website ;
    rdfs:label "https://pasta-eln.github.io/"^^xsd:anyURI ;
    nfdicore:url <https://pasta-eln.github.io/> .

<http://demo.fiz-karlsruhe.de/matwerk/E134904> a nfdicore:Website ;
    rdfs:label "https://www.elabftw.net/"^^xsd:anyURI ;
    nfdicore:url <https://www.elabftw.net/> .

<http://demo.fiz-karlsruhe.de/matwerk/E135422> a nfdicore:Website ;
    rdfs:label "https://kadi.iam-cms.kit.edu/"^^xsd:anyURI ;
    nfdicore:url <https://kadi.iam-cms.kit.edu/> .

<http://demo.fiz-karlsruhe.de/matwerk/E135941> a nfdicore:Website ;
    rdfs:label "https://atomsk.univ-lille.fr/"^^xsd:anyURI ;
    nfdicore:url <https://atomsk.univ-lille.fr/> .

<http://demo.fiz-karlsruhe.de/matwerk/E136461> a nfdicore:Website ;
    rdfs:label "https://www.ctcms.nist.gov/potentials/atomman/"^^xsd:anyURI ;
    nfdicore:url <https://www.ctcms.nist.gov/potentials/atomman/> .

<http://demo.fiz-karlsruhe.de/matwerk/E136982> a nfdicore:Website ;
    rdfs:label "https://www.ctcms.nist.gov/potentials/iprPy/"^^xsd:anyURI ;
    nfdicore:url <https://www.ctcms.nist.gov/potentials/iprPy/> .

<http://demo.fiz-karlsruhe.de/matwerk/E13721> a nfdicore:Person ;
    rdfs:label "Prof. Dr. Ruth Schwaiger" ;
    mwo:emailAddress "r.schwaiger@fz-juelich.de"^^xsd:string ;
    mwo:hasAffiliation <http://demo.fiz-karlsruhe.de/matwerk/E1022> ;
    mwo:hasORCID <https://orcid.org/0000-0001-8940-2361> ;
    owl:sameAs <http://www.wikidata.org/entity/Q41592315> ;
    foaf:firstName "Ruth"^^xsd:string ;
    foaf:surname "Schwaiger"^^xsd:string ;
    foaf:title "Prof. Dr."^^xsd:string .

<http://demo.fiz-karlsruhe.de/matwerk/E137504> a nfdicore:Website ;
    rdfs:label "https://openkim.org/kim-api/"^^xsd:anyURI ;
    nfdicore:url <https://openkim.org/kim-api/> .

<http://demo.fiz-karlsruhe.de/matwerk/E138027> a nfdicore:Website ;
    rdfs:label "https://atomate.org/"^^xsd:anyURI ;
    nfdicore:url <https://atomate.org/> .

<http://demo.fiz-karlsruhe.de/matwerk/E138551> a nfdicore:Website ;
    rdfs:label "https://materialsproject.github.io/fireworks/"^^xsd:anyURI ;
    nfdicore:url <https://materialsproject.github.io/fireworks/> .

<http://demo.fiz-karlsruhe.de/matwerk/E139076> a nfdicore:Website ;
    rdfs:label "https://materialsproject.github.io/custodian/"^^xsd:anyURI ;
    nfdicore:url <https://materialsproject.github.io/custodian/> .

<http://demo.fiz-karlsruhe.de/matwerk/E139602> a nfdicore:Website ;
    rdfs:label "https://emmo-repo.github.io/EMMO-python/0.3.1/"^^xsd:anyURI ;
    nfdicore:url <https://emmo-repo.github.io/EMMO-python/0.3.1/> .

<http://demo.fiz-karlsruhe.de/matwerk/E140129> a nfdicore:Website ;
    rdfs:label "https://www.yambo-code.eu/"^^xsd:anyURI ;
    nfdicore:url <https://www.yambo-code.eu/> .

<http://demo.fiz-karlsruhe.de/matwerk/E140657> a nfdicore:Website ;
    rdfs:label "http://www.wannier.org/"^^xsd:anyURI ;
    nfdicore:url <http://www.wannier.org/> .

<http://demo.fiz-karlsruhe.de/matwerk/E1407> a nfdicore:Organization ;
    rdfs:label "Fraunhofer Institute for Material and Beam Technology",
        "Fraunhofer-Institut für Werkstoff- und Strahltechnik"@de ;
    nfdicore:location <http://demo.fiz-karlsruhe.de/matwerk/E79211> ;
    nfdicore:parentOrganisation <http://demo.fiz-karlsruhe.de/matwerk/E3081> ;
    mwo:hasAcronym "IWS"^^xsd:string ;
    mwo:hasPostalCode "1277" ;
    mwo:hasWebsite <http://demo.fiz-karlsruhe.de/matwerk/E91526> .

<http://demo.fiz-karlsruhe.de/matwerk/E141186> a nfdicore:Website ;
    rdfs:label "https://colabfit.org/"^^xsd:anyURI ;
    nfdicore:url <https://colabfit.org/> .

<http://demo.fiz-karlsruhe.de/matwerk/E141716> a nfdicore:Website ;
    rdfs:label "https://www.coscine.de/en/"^^xsd:anyURI ;
    nfdicore:url <https://www.coscine.de/en/> .

<http://demo.fiz-karlsruhe.de/matwerk/E142247> a nfdicore:Website ;
    rdfs:label "https://pytorch.org/"^^xsd:anyURI ;
    nfdicore:url <https://pytorch.org/> .

<http://demo.fiz-karlsruhe.de/matwerk/E142779> a nfdicore:Website ;
    rdfs:label "https://scikit-learn.org/stable/"^^xsd:anyURI ;
    nfdicore:url <https://scikit-learn.org/stable/> .

<http://demo.fiz-karlsruhe.de/matwerk/E143312> a nfdicore:Website ;
    rdfs:label "https://www.tensorflow.org/"^^xsd:anyURI ;
    nfdicore:url <https://www.tensorflow.org/> .

<http://demo.fiz-karlsruhe.de/matwerk/E143846> a nfdicore:Website ;
    rdfs:label "https://openbis.ch/"^^xsd:anyURI ;
    nfdicore:url <https://openbis.ch/> .

<http://demo.fiz-karlsruhe.de/matwerk/E144381> a nfdicore:Website ;
    rdfs:label "https://www.turbomole.org/"^^xsd:anyURI ;
    nfdicore:url <https://www.turbomole.org/> .

<http://demo.fiz-karlsruhe.de/matwerk/E144917> a nfdicore:Website ;
    rdfs:label "http://dream3d.bluequartz.net/"^^xsd:anyURI ;
    nfdicore:url <http://dream3d.bluequartz.net/> .

<http://demo.fiz-karlsruhe.de/matwerk/E145454> a nfdicore:Website ;
    rdfs:label "https://mtex-toolbox.github.io/"^^xsd:anyURI ;
    nfdicore:url <https://mtex-toolbox.github.io/> .

<http://demo.fiz-karlsruhe.de/matwerk/E145992> a nfdicore:Website ;
    rdfs:label "https://gmsh.info/"^^xsd:anyURI ;
    nfdicore:url <https://gmsh.info/> .

<http://demo.fiz-karlsruhe.de/matwerk/E146531> a nfdicore:Website ;
    rdfs:label "https://neper.info/"^^xsd:anyURI ;
    nfdicore:url <https://neper.info/> .

<http://demo.fiz-karlsruhe.de/matwerk/E147071> a nfdicore:Website ;
    rdfs:label "https://petsc.org/"^^xsd:anyURI ;
    nfdicore:url <https://petsc.org/> .

<http://demo.fiz-karlsruhe.de/matwerk/E147612> a nfdicore:Website ;
    rdfs:label "https://www.dealii.org/"^^xsd:anyURI ;
    nfdicore:url <https://www.dealii.org/> .

<http://demo.fiz-karlsruhe.de/matwerk/E148154> a nfdicore:Website ;
    rdfs:label "https://www.firedrakeproject.org/"^^xsd:anyURI ;
    nfdicore:url <https://www.firedrakeproject.org/> .

<http://demo.fiz-karlsruhe.de/matwerk/E148697> a nfdicore:Website ;
    rdfs:label "https://freefem.org/"^^xsd:anyURI ;
    nfdicore:url <https://freefem.org/> .

<http://demo.fiz-karlsruhe.de/matwerk/E149241> a nfdicore:Website ;
    rdfs:label "https://hippylib.github.io/"^^xsd:anyURI ;
    nfdicore:url <https://hippylib.github.io/> .

<http://demo.fiz-karlsruhe.de/matwerk/E149786> a nfdicore:Website ;
    rdfs:label "http://mofem.eng.gla.ac.uk/mofem/html/"^^xsd:anyURI ;
    nfdicore:url <http://mofem.eng.gla.ac.uk/mofem/html/> .

<http://demo.fiz-karlsruhe.de/matwerk/E150332> a nfdicore:Website ;
    rdfs:label "http://www.oofem.org/doku.php?id=en:oofem"^^xsd:anyURI ;
    nfdicore:url <http://www.oofem.org/doku.php?id=en:oofem> .

<http://demo.fiz-karlsruhe.de/matwerk/E150879> a nfdicore:Website ;
    rdfs:label "https://precice.org/"^^xsd:anyURI ;
    nfdicore:url <https://precice.org/> .

<http://demo.fiz-karlsruhe.de/matwerk/E151427> a nfdicore:Website ;
    rdfs:label "http://www.clawpack.org/"^^xsd:anyURI ;
    nfdicore:url <http://www.clawpack.org/> .

<http://demo.fiz-karlsruhe.de/matwerk/E151976> a nfdicore:Website ;
    rdfs:label "https://www.3ds.com/products-services/biovia/products/molecular-modeling-simulation/biovia-materials-studio/"^^xsd:anyURI ;
    nfdicore:url <https://www.3ds.com/products-services/biovia/products/molecular-modeling-simulation/biovia-materials-studio/> .

<http://demo.fiz-karlsruhe.de/matwerk/E152526> a nfdicore:Website ;
    rdfs:label "https://cclib.github.io/"^^xsd:anyURI ;
    nfdicore:url <https://cclib.github.io/> .

<http://demo.fiz-karlsruhe.de/matwerk/E153077> a nfdicore:Website ;
    rdfs:label "https://cctbx.github.io/"^^xsd:anyURI ;
    nfdicore:url <https://cctbx.github.io/> .

<http://demo.fiz-karlsruhe.de/matwerk/E153629> a nfdicore:Website ;
    rdfs:label "https://mat-discover.readthedocs.io/en/latest/"^^xsd:anyURI ;
    nfdicore:url <https://mat-discover.readthedocs.io/en/latest/> .

<http://demo.fiz-karlsruhe.de/matwerk/E154736> a nfdicore:Website ;
    rdfs:label "https://www.materialsdesign.com/medea-software"^^xsd:anyURI ;
    nfdicore:url <https://www.materialsdesign.com/medea-software> .

<http://demo.fiz-karlsruhe.de/matwerk/E155291> a nfdicore:Website ;
    rdfs:label "https://crest-cassia.github.io/oacis/en/"^^xsd:anyURI ;
    nfdicore:url <https://crest-cassia.github.io/oacis/en/> .

<http://demo.fiz-karlsruhe.de/matwerk/E155847> a nfdicore:Website ;
    rdfs:label "https://molssi-seamm.github.io/"^^xsd:anyURI ;
    nfdicore:url <https://molssi-seamm.github.io/> .

<http://demo.fiz-karlsruhe.de/matwerk/E156404> a nfdicore:Website ;
    rdfs:label "https://hybrid3-database.readthedocs.io/en/latest/"^^xsd:anyURI ;
    nfdicore:url <https://hybrid3-database.readthedocs.io/en/latest/> .

<http://demo.fiz-karlsruhe.de/matwerk/E156962> a nfdicore:Website ;
    rdfs:label "https://simmate.org/"^^xsd:anyURI ;
    nfdicore:url <https://simmate.org/> .

<http://demo.fiz-karlsruhe.de/matwerk/E157521> a nfdicore:Website ;
    rdfs:label "https://pythonhosted.org/MAST/index.html"^^xsd:anyURI ;
    nfdicore:url <https://pythonhosted.org/MAST/index.html> .

<http://demo.fiz-karlsruhe.de/matwerk/E158081> a nfdicore:Website ;
    rdfs:label "https://www.diffpy.org/"^^xsd:anyURI ;
    nfdicore:url <https://www.diffpy.org/> .

<http://demo.fiz-karlsruhe.de/matwerk/E158642> a nfdicore:Website ;
    rdfs:label "https://pythonhosted.org/pyDOE/#"^^xsd:anyURI ;
    nfdicore:url <https://pythonhosted.org/pyDOE/#> .

<http://demo.fiz-karlsruhe.de/matwerk/E159204> a mwo:Repository ;
    rdfs:label "https://github.com/ICAMS/calphy"^^xsd:anyURI ;
    nfdicore:url <https://github.com/ICAMS/calphy> .

<http://demo.fiz-karlsruhe.de/matwerk/E159767> a mwo:Repository ;
    rdfs:label "https://github.com/workflow-gallery/calphy"^^xsd:anyURI ;
    nfdicore:url <https://github.com/workflow-gallery/calphy> .

<http://demo.fiz-karlsruhe.de/matwerk/E160331> a mwo:Repository ;
    rdfs:label "https://github.com/pyscal/pyscal"^^xsd:anyURI ;
    nfdicore:url <https://github.com/pyscal/pyscal> .

<http://demo.fiz-karlsruhe.de/matwerk/E160896> a mwo:Repository ;
    rdfs:label "https://github.com/DataAnalyticsEngineering/EQ2PC"^^xsd:anyURI ;
    nfdicore:url <https://github.com/DataAnalyticsEngineering/EQ2PC> .

<http://demo.fiz-karlsruhe.de/matwerk/E161462> a mwo:Repository ;
    rdfs:label "https://github.com/EMMA-Group/MinimumEnergyPoints"^^xsd:anyURI ;
    nfdicore:url <https://github.com/EMMA-Group/MinimumEnergyPoints> .

<http://demo.fiz-karlsruhe.de/matwerk/E162029> a mwo:Repository ;
    rdfs:label "https://github.com/EMMA-Group/ConcentricInterpolation"^^xsd:anyURI ;
    nfdicore:url <https://github.com/EMMA-Group/ConcentricInterpolation> .

<http://demo.fiz-karlsruhe.de/matwerk/E162597> a mwo:Repository ;
    rdfs:label "https://github.com/J-lissner/image-property-linkage"^^xsd:anyURI ;
    nfdicore:url <https://github.com/J-lissner/image-property-linkage> .

<http://demo.fiz-karlsruhe.de/matwerk/E163166> a mwo:Repository ;
    rdfs:label "https://gitlab.kitware.com/paraview/paraview"^^xsd:anyURI ;
    nfdicore:url <https://gitlab.kitware.com/paraview/paraview> .

<http://demo.fiz-karlsruhe.de/matwerk/E163736> a mwo:Repository ;
    rdfs:label "https://gitlab.kitware.com/vtk"^^xsd:anyURI ;
    nfdicore:url <https://gitlab.kitware.com/vtk> .

<http://demo.fiz-karlsruhe.de/matwerk/E164307> a mwo:Repository ;
    rdfs:label "https://github.com/fiji/fiji"^^xsd:anyURI ;
    nfdicore:url <https://github.com/fiji/fiji> .

<http://demo.fiz-karlsruhe.de/matwerk/E164879> a mwo:Repository ;
    rdfs:label "https://github.com/imagej/ImageJ2"^^xsd:anyURI ;
    nfdicore:url <https://github.com/imagej/ImageJ2> .

<http://demo.fiz-karlsruhe.de/matwerk/E165452> a mwo:Repository ;
    rdfs:label "https://github.com/imagej/imagej2"^^xsd:anyURI ;
    nfdicore:url <https://github.com/imagej/imagej2> .

<http://demo.fiz-karlsruhe.de/matwerk/E166026> a mwo:Repository ;
    rdfs:label "https://github.com/abinit"^^xsd:anyURI ;
    nfdicore:url <https://github.com/abinit> .

<http://demo.fiz-karlsruhe.de/matwerk/E166601> a mwo:Repository ;
    rdfs:label "https://gitlab.com/l_sim/bigdft-suite"^^xsd:anyURI ;
    nfdicore:url <https://gitlab.com/l_sim/bigdft-suite> .

<http://demo.fiz-karlsruhe.de/matwerk/E167177> a mwo:Repository ;
    rdfs:label "https://gitlab.com/QEF/q-e"^^xsd:anyURI ;
    nfdicore:url <https://gitlab.com/QEF/q-e> .

<http://demo.fiz-karlsruhe.de/matwerk/E167754> a mwo:Repository ;
    rdfs:label "https://github.com/shankar1729/jdftx"^^xsd:anyURI ;
    nfdicore:url <https://github.com/shankar1729/jdftx> .

<http://demo.fiz-karlsruhe.de/matwerk/E168332> a mwo:Repository ;
    rdfs:label "https://gitlab.com/real-space/parsec/"^^xsd:anyURI ;
    nfdicore:url <https://gitlab.com/real-space/parsec/> .

<http://demo.fiz-karlsruhe.de/matwerk/E168911> a mwo:Repository ;
    rdfs:label "https://github.com/cp2k"^^xsd:anyURI ;
    nfdicore:url <https://github.com/cp2k> .

<http://demo.fiz-karlsruhe.de/matwerk/E169491> a mwo:Repository ;
    rdfs:label "https://gitlab.com/gpaw/gpaw"^^xsd:anyURI ;
    nfdicore:url <https://gitlab.com/gpaw/gpaw> .

<http://demo.fiz-karlsruhe.de/matwerk/E170072> a mwo:Repository ;
    rdfs:label "https://gitlab.com/sphinxlib/sxaccelerate"^^xsd:anyURI ;
    nfdicore:url <https://gitlab.com/sphinxlib/sxaccelerate> .

<http://demo.fiz-karlsruhe.de/matwerk/E170654> a mwo:Repository ;
    rdfs:label "http://scherzo.ucdavis.edu/qbox/qbox-public"^^xsd:anyURI ;
    nfdicore:url <http://scherzo.ucdavis.edu/qbox/qbox-public> .

<http://demo.fiz-karlsruhe.de/matwerk/E17111> a nfdicore:Person ;
    foaf:firstName "Manuel"^^xsd:string ;
    foaf:surname "Richter"^^xsd:string .

<http://demo.fiz-karlsruhe.de/matwerk/E171237> a mwo:Repository ;
    rdfs:label "https://github.com/JuliaMolSim/DFTK.jl"^^xsd:anyURI ;
    nfdicore:url <https://github.com/JuliaMolSim/DFTK.jl> .

<http://demo.fiz-karlsruhe.de/matwerk/E171821> a mwo:Repository ;
    rdfs:label "https://gitlab.com/siesta-project/siesta"^^xsd:anyURI ;
    nfdicore:url <https://gitlab.com/siesta-project/siesta> .

<http://demo.fiz-karlsruhe.de/matwerk/E172406> a mwo:Repository ;
    rdfs:label "https://github.com/exciting/exciting"^^xsd:anyURI ;
    nfdicore:url <https://github.com/exciting/exciting> .

<http://demo.fiz-karlsruhe.de/matwerk/E17291> a nfdicore:Person ;
    foaf:firstName "Prof."^^xsd:string ;
    foaf:surname "Peter"^^xsd:string .

<http://demo.fiz-karlsruhe.de/matwerk/E172992> a mwo:Repository ;
    rdfs:label "https://iffgit.fz-juelich.de/fleur/fleur"^^xsd:anyURI ;
    nfdicore:url <https://iffgit.fz-juelich.de/fleur/fleur> .

<http://demo.fiz-karlsruhe.de/matwerk/E173579> a mwo:Repository ;
    rdfs:label "https://github.com/lammps"^^xsd:anyURI ;
    nfdicore:url <https://github.com/lammps> .

<http://demo.fiz-karlsruhe.de/matwerk/E174167> a mwo:Repository ;
    rdfs:label "https://github.com/itapmd"^^xsd:anyURI ;
    nfdicore:url <https://github.com/itapmd> .

<http://demo.fiz-karlsruhe.de/matwerk/E17472> a nfdicore:Person ;
    foaf:firstName "Louis"^^xsd:string ;
    foaf:surname "Vanduyfhuys"^^xsd:string .

<http://demo.fiz-karlsruhe.de/matwerk/E174756> a mwo:Repository ;
    rdfs:label "https://gitlab.com/gromacs/gromacs"^^xsd:anyURI ;
    nfdicore:url <https://gitlab.com/gromacs/gromacs> .

<http://demo.fiz-karlsruhe.de/matwerk/E175346> a mwo:Repository ;
    rdfs:label "https://github.com/idaholab/moose"^^xsd:anyURI ;
    nfdicore:url <https://github.com/idaholab/moose> .

<http://demo.fiz-karlsruhe.de/matwerk/E175937> a mwo:Repository ;
    rdfs:label "https://github.com/FEniCS/"^^xsd:anyURI ;
    nfdicore:url <https://github.com/FEniCS/> .

<http://demo.fiz-karlsruhe.de/matwerk/E176529> a mwo:Repository ;
    rdfs:label "https://github.com/eisenforschung/damask"^^xsd:anyURI ;
    nfdicore:url <https://github.com/eisenforschung/damask> .

<http://demo.fiz-karlsruhe.de/matwerk/E17654> a nfdicore:Person ;
    foaf:firstName "Welchy"^^xsd:string ;
    foaf:surname "Leite"^^xsd:string .

<http://demo.fiz-karlsruhe.de/matwerk/E177122> a mwo:Repository ;
    rdfs:label "https://github.com/pyiron"^^xsd:anyURI ;
    nfdicore:url <https://github.com/pyiron> .

<http://demo.fiz-karlsruhe.de/matwerk/E177716> a mwo:Repository ;
    rdfs:label "https://github.com/aiidateam"^^xsd:anyURI ;
    nfdicore:url <https://github.com/aiidateam> .

<http://demo.fiz-karlsruhe.de/matwerk/E178311> a mwo:Repository ;
    rdfs:label "https://gitlab.com/ase/ase"^^xsd:anyURI ;
    nfdicore:url <https://gitlab.com/ase/ase> .

<http://demo.fiz-karlsruhe.de/matwerk/E178907> a mwo:Repository ;
    rdfs:label "https://github.com/orest-d/p4vasp"^^xsd:anyURI ;
    nfdicore:url <https://github.com/orest-d/p4vasp> .

<http://demo.fiz-karlsruhe.de/matwerk/E179504> a mwo:Repository ;
    rdfs:label "https://github.com/phonopy/phonopy"^^xsd:anyURI ;
    nfdicore:url <https://github.com/phonopy/phonopy> .

<http://demo.fiz-karlsruhe.de/matwerk/E180102> a mwo:Repository ;
    rdfs:label "https://github.com/CCP-NC/soprano"^^xsd:anyURI ;
    nfdicore:url <https://github.com/CCP-NC/soprano> .

<http://demo.fiz-karlsruhe.de/matwerk/E180701> a mwo:Repository ;
    rdfs:label "https://gitlab.com/vibes-developers/vibes"^^xsd:anyURI ;
    nfdicore:url <https://gitlab.com/vibes-developers/vibes> .

<http://demo.fiz-karlsruhe.de/matwerk/E181301> a mwo:Repository ;
    rdfs:label "https://github.com/torbjornbjorkman/cif2cell"^^xsd:anyURI ;
    nfdicore:url <https://github.com/torbjornbjorkman/cif2cell> .

<http://demo.fiz-karlsruhe.de/matwerk/E181902> a mwo:Repository ;
    rdfs:label "https://github.com/avogadro"^^xsd:anyURI ;
    nfdicore:url <https://github.com/avogadro> .

<http://demo.fiz-karlsruhe.de/matwerk/E182504> a mwo:Repository ;
    rdfs:label "https://github.com/MarsalekGroup/aml"^^xsd:anyURI ;
    nfdicore:url <https://github.com/MarsalekGroup/aml> .

<http://demo.fiz-karlsruhe.de/matwerk/E183107> a mwo:Repository ;
    rdfs:label "https://github.com/SINGROUP/pycp2k"^^xsd:anyURI ;
    nfdicore:url <https://github.com/SINGROUP/pycp2k> .

<http://demo.fiz-karlsruhe.de/matwerk/E183711> a mwo:Repository ;
    rdfs:label "https://gitlab.com/pyretis/pyretis"^^xsd:anyURI ;
    nfdicore:url <https://gitlab.com/pyretis/pyretis> .

<http://demo.fiz-karlsruhe.de/matwerk/E184316> a mwo:Repository ;
    rdfs:label "https://github.com/openpathsampling/openpathsampling"^^xsd:anyURI ;
    nfdicore:url <https://github.com/openpathsampling/openpathsampling> .

<http://demo.fiz-karlsruhe.de/matwerk/E184922> a mwo:Repository ;
    rdfs:label "https://github.com/giovannipizzi/seekpath"^^xsd:anyURI ;
    nfdicore:url <https://github.com/giovannipizzi/seekpath> .

<http://demo.fiz-karlsruhe.de/matwerk/E185529> a mwo:Repository ;
    rdfs:label "https://github.com/materialsproject/pymatgen"^^xsd:anyURI ;
    nfdicore:url <https://github.com/materialsproject/pymatgen> .

<http://demo.fiz-karlsruhe.de/matwerk/E18579> a nfdicore:Person ;
    foaf:firstName "Christoph"^^xsd:string ;
    foaf:surname "Freysoldt"^^xsd:string .

<http://demo.fiz-karlsruhe.de/matwerk/E186137> a mwo:Repository ;
    rdfs:label "https://github.com/aiidateam/qe-tools"^^xsd:anyURI ;
    nfdicore:url <https://github.com/aiidateam/qe-tools> .

<http://demo.fiz-karlsruhe.de/matwerk/E1862> a nfdicore:Organization ;
    rdfs:label "Karlsruher Institut für Technologie" ;
    mwo:hasRORID "https://ror.org/04t3en479" ;
    owl:sameAs <http://www.wikidata.org/entity/Q309988> .

<http://demo.fiz-karlsruhe.de/matwerk/E186746> a mwo:Repository ;
    rdfs:label "https://github.com/molmod/tamkin"^^xsd:anyURI ;
    nfdicore:url <https://github.com/molmod/tamkin> .

<http://demo.fiz-karlsruhe.de/matwerk/E187356> a mwo:Repository ;
    rdfs:label "https://github.com/lammps/pizza"^^xsd:anyURI ;
    nfdicore:url <https://github.com/lammps/pizza> .

<http://demo.fiz-karlsruhe.de/matwerk/E18767> a nfdicore:Person ;
    foaf:firstName "Chris"^^xsd:string ;
    foaf:surname "H."^^xsd:string .

<http://demo.fiz-karlsruhe.de/matwerk/E187967> a mwo:Repository ;
    rdfs:label "https://github.com/glotzerlab/freud"^^xsd:anyURI ;
    nfdicore:url <https://github.com/glotzerlab/freud> .

<http://demo.fiz-karlsruhe.de/matwerk/E188579> a mwo:Repository ;
    rdfs:label "https://github.com/nglviewer/nglview"^^xsd:anyURI ;
    nfdicore:url <https://github.com/nglviewer/nglview> .

<http://demo.fiz-karlsruhe.de/matwerk/E189192> a mwo:Repository ;
    rdfs:label "https://github.com/molmod/QuickFF"^^xsd:anyURI ;
    nfdicore:url <https://github.com/molmod/QuickFF> .

<http://demo.fiz-karlsruhe.de/matwerk/E189806> a mwo:Repository ;
    rdfs:label "https://github.com/pyiron/pylammpsmpi"^^xsd:anyURI ;
    nfdicore:url <https://github.com/pyiron/pylammpsmpi> .

<http://demo.fiz-karlsruhe.de/matwerk/E190421> a mwo:Repository ;
    rdfs:label "https://github.com/molmod/yaff"^^xsd:anyURI ;
    nfdicore:url <https://github.com/molmod/yaff> .

<http://demo.fiz-karlsruhe.de/matwerk/E191037> a mwo:Repository ;
    rdfs:label "https://gitlab.com/computationalmaterials/clease/activity"^^xsd:anyURI ;
    nfdicore:url <https://gitlab.com/computationalmaterials/clease/activity> .

<http://demo.fiz-karlsruhe.de/matwerk/E191654> a mwo:Repository ;
    rdfs:label "https://gitlab.com/materials-modeling/icet"^^xsd:anyURI ;
    nfdicore:url <https://gitlab.com/materials-modeling/icet> .

<http://demo.fiz-karlsruhe.de/matwerk/E192272> a mwo:Repository ;
    rdfs:label "https://github.com/abelcarreras/DynaPhoPy"^^xsd:anyURI ;
    nfdicore:url <https://github.com/abelcarreras/DynaPhoPy> .

<http://demo.fiz-karlsruhe.de/matwerk/E192891> a mwo:Repository ;
    rdfs:label "https://github.com/PhasesResearchLab/ESPEI"^^xsd:anyURI ;
    nfdicore:url <https://github.com/PhasesResearchLab/ESPEI> .

<http://demo.fiz-karlsruhe.de/matwerk/E193511> a mwo:Repository ;
    rdfs:label "https://github.com/pycalphad/pycalphad"^^xsd:anyURI ;
    nfdicore:url <https://github.com/pycalphad/pycalphad> .

<http://demo.fiz-karlsruhe.de/matwerk/E194132> a mwo:Repository ;
    rdfs:label "https://github.com/libAtoms/pymatnest"^^xsd:anyURI ;
    nfdicore:url <https://github.com/libAtoms/pymatnest> .

<http://demo.fiz-karlsruhe.de/matwerk/E194754> a mwo:Repository ;
    rdfs:label "https://github.com/openkim/kliff"^^xsd:anyURI ;
    nfdicore:url <https://github.com/openkim/kliff> .

<http://demo.fiz-karlsruhe.de/matwerk/E19529> a nfdicore:Person ;
    mwo:hasAffiliation <http://demo.fiz-karlsruhe.de/matwerk/E1037> ;
    foaf:firstName "Jutta"^^xsd:string ;
    foaf:surname "Rogal"^^xsd:string .

<http://demo.fiz-karlsruhe.de/matwerk/E195377> a mwo:Repository ;
    rdfs:label "https://github.com/CompPhysVienna/n2p2"^^xsd:anyURI ;
    nfdicore:url <https://github.com/CompPhysVienna/n2p2> .

<http://demo.fiz-karlsruhe.de/matwerk/E196001> a mwo:Repository ;
    rdfs:label "https://github.com/FitSNAP"^^xsd:anyURI ;
    nfdicore:url <https://github.com/FitSNAP> .

<http://demo.fiz-karlsruhe.de/matwerk/E196626> a mwo:Repository ;
    rdfs:label "https://github.com/hackingmaterials/matminer"^^xsd:anyURI ;
    nfdicore:url <https://github.com/hackingmaterials/matminer> .

<http://demo.fiz-karlsruhe.de/matwerk/E197252> a mwo:Repository ;
    rdfs:label "https://github.com/materialsproject/matbench"^^xsd:anyURI ;
    nfdicore:url <https://github.com/materialsproject/matbench> .

<http://demo.fiz-karlsruhe.de/matwerk/E197879> a mwo:Repository ;
    rdfs:label "https://github.com/lmmentel/mendeleev"^^xsd:anyURI ;
    nfdicore:url <https://github.com/lmmentel/mendeleev> .

<http://demo.fiz-karlsruhe.de/matwerk/E198507> a mwo:Repository ;
    rdfs:label "https://github.com/din14970/TEMMETA"^^xsd:anyURI ;
    nfdicore:url <https://github.com/din14970/TEMMETA> .

<http://demo.fiz-karlsruhe.de/matwerk/E199136> a mwo:Repository ;
    rdfs:label "https://gitlab.com/atomicrex/atomicrex"^^xsd:anyURI ;
    nfdicore:url <https://gitlab.com/atomicrex/atomicrex> .

<http://demo.fiz-karlsruhe.de/matwerk/E19916> a nfdicore:Person ;
    mwo:hasAffiliation <http://demo.fiz-karlsruhe.de/matwerk/E4656> ;
    foaf:firstName "Grisell"^^xsd:string ;
    foaf:surname "Díaz"^^xsd:string .

<http://demo.fiz-karlsruhe.de/matwerk/E199766> a mwo:Repository ;
    rdfs:label "https://github.com/Acellera/htmd"^^xsd:anyURI ;
    nfdicore:url <https://github.com/Acellera/htmd> .

<http://demo.fiz-karlsruhe.de/matwerk/E200397> a mwo:Repository ;
    rdfs:label "https://gitlab.com/materials-modeling/hiphive"^^xsd:anyURI ;
    nfdicore:url <https://gitlab.com/materials-modeling/hiphive> .

<http://demo.fiz-karlsruhe.de/matwerk/E201029> a mwo:Repository ;
    rdfs:label "https://gitlab.com/materials-modeling/wulffpack"^^xsd:anyURI ;
    nfdicore:url <https://gitlab.com/materials-modeling/wulffpack> .

<http://demo.fiz-karlsruhe.de/matwerk/E20111> a nfdicore:Person ;
    mwo:emailAddress "lars.pastewka@imtek.uni-freiburg.de"^^xsd:string ;
    foaf:firstName "Lars"^^xsd:string ;
    foaf:surname "Pastewka"^^xsd:string .

<http://demo.fiz-karlsruhe.de/matwerk/E201662> a mwo:Repository ;
    rdfs:label "https://gitlab.com/materials-modeling/dynasor"^^xsd:anyURI ;
    nfdicore:url <https://gitlab.com/materials-modeling/dynasor> .

<http://demo.fiz-karlsruhe.de/matwerk/E202296> a mwo:Repository ;
    rdfs:label "https://gitlab.com/materials-modeling/vcsgc-lammps"^^xsd:anyURI ;
    nfdicore:url <https://gitlab.com/materials-modeling/vcsgc-lammps> .

<http://demo.fiz-karlsruhe.de/matwerk/E202931> a mwo:Repository ;
    rdfs:label "https://github.com/ICAMS/Kanapy"^^xsd:anyURI ;
    nfdicore:url <https://github.com/ICAMS/Kanapy> .

<http://demo.fiz-karlsruhe.de/matwerk/E20307> a nfdicore:Person ;
    mwo:emailAddress "atz.togo@gmail.com"^^xsd:string ;
    foaf:firstName "Atsushi"^^xsd:string ;
    foaf:surname "Togo"^^xsd:string .

<http://demo.fiz-karlsruhe.de/matwerk/E203567> a mwo:Repository ;
    rdfs:label "https://github.com/ICAMS/pyLabFEA"^^xsd:anyURI ;
    nfdicore:url <https://github.com/ICAMS/pyLabFEA> .

<http://demo.fiz-karlsruhe.de/matwerk/E204204> a mwo:Repository ;
    rdfs:label "https://github.com/ashtonmv/pyrho"^^xsd:anyURI ;
    nfdicore:url <https://github.com/ashtonmv/pyrho> .

<http://demo.fiz-karlsruhe.de/matwerk/E204842> a mwo:Repository ;
    rdfs:label "https://github.com/ICAMS/python-ace"^^xsd:anyURI ;
    nfdicore:url <https://github.com/ICAMS/python-ace> .

<http://demo.fiz-karlsruhe.de/matwerk/E20504> a nfdicore:Person ;
    rdfs:label "Niklas Siemer" ;
    mwo:hasAffiliation <http://demo.fiz-karlsruhe.de/matwerk/E3416> ;
    foaf:firstName "Niklas"^^xsd:string ;
    foaf:surname "Siemer"^^xsd:string .

<http://demo.fiz-karlsruhe.de/matwerk/E205481> a mwo:Repository ;
    rdfs:label "https://github.com/aixvipmap"^^xsd:anyURI ;
    nfdicore:url <https://github.com/aixvipmap> .

<http://demo.fiz-karlsruhe.de/matwerk/E206121> a mwo:Repository ;
    rdfs:label "https://github.com/mupif"^^xsd:anyURI ;
    nfdicore:url <https://github.com/mupif> .

<http://demo.fiz-karlsruhe.de/matwerk/E206762> a mwo:Repository ;
    rdfs:label "https://github.com/simphony"^^xsd:anyURI ;
    nfdicore:url <https://github.com/simphony> .

<http://demo.fiz-karlsruhe.de/matwerk/E20702> a nfdicore:Person ;
    rdfs:label "Liam Huber" ;
    mwo:hasAffiliation <http://demo.fiz-karlsruhe.de/matwerk/E3279> ;
    foaf:firstName "Liam"^^xsd:string ;
    foaf:surname "Huber"^^xsd:string .

<http://demo.fiz-karlsruhe.de/matwerk/E207404> a mwo:Repository ;
    rdfs:label "https://github.com/liamhuber/clustergb"^^xsd:anyURI ;
    nfdicore:url <https://github.com/liamhuber/clustergb> .

<http://demo.fiz-karlsruhe.de/matwerk/E208047> a mwo:Repository ;
    rdfs:label "https://github.com/peizong/DIST-Toolkit"^^xsd:anyURI ;
    nfdicore:url <https://github.com/peizong/DIST-Toolkit> .

<http://demo.fiz-karlsruhe.de/matwerk/E208691> a mwo:Repository ;
    rdfs:label "https://github.com/oekosheri/GB_code"^^xsd:anyURI ;
    nfdicore:url <https://github.com/oekosheri/GB_code> .

<http://demo.fiz-karlsruhe.de/matwerk/E20901> a nfdicore:Person ;
    rdfs:label "Prof. Dr.  Sandra Korte-Kerzel" ;
    mwo:emailAddress "Korte-Kerzel@imm.rwth-aachen.de"^^xsd:string ;
    mwo:hasAffiliation <http://demo.fiz-karlsruhe.de/matwerk/E1046>,
        <http://demo.fiz-karlsruhe.de/matwerk/E3279> ;
    mwo:hasExpertiseIn <http://demo.fiz-karlsruhe.de/matwerk/E40622> ;
    mwo:hasORCID <https://orcid.org/0000-0002-4143-5129> ;
    owl:sameAs <http://www.wikidata.org/entity/Q58659836> ;
    foaf:depiction <https://ams3.digitaloceanspaces.com/externalpublic/57/938d750d-b7d8-4298-a0b4-b23f62d8b87c/conversions/a1d0cea4-0e64-4c26-948b-3024726bdcdf-md.jpg?X-Amz-Content-Sha256=UNSIGNED-PAYLOAD&X-Amz-Algorithm=AWS4-HMAC-SHA256&X-Amz-Credential=KVC4ZMO47JLTBHVHEFZ4%2F20230512%2Fams3%2Fs3%2Faws4_request&X-Amz-Date=20230512T150442Z&X-Amz-SignedHeaders=host&X-Amz-Expires=7200&X-Amz-Signature=3ebdd621f3424f84d715c6aa7be124d6dffb87854f0703f45d461cca5ccb5a25> ;
    foaf:firstName "Sandra"^^xsd:string ;
    foaf:surname "Korte-Kerzel"^^xsd:string ;
    foaf:title "Prof. Dr. "^^xsd:string .

<http://demo.fiz-karlsruhe.de/matwerk/E209336> a mwo:Repository ;
    rdfs:label "https://gitlab.com/paraprobe/paraprobe-toolbox"^^xsd:anyURI ;
    nfdicore:url <https://gitlab.com/paraprobe/paraprobe-toolbox> .

<http://demo.fiz-karlsruhe.de/matwerk/E209982> a mwo:Repository ;
    rdfs:label "https://github.com/NingWang1990/pySTEM"^^xsd:anyURI ;
    nfdicore:url <https://github.com/NingWang1990/pySTEM> .

<http://demo.fiz-karlsruhe.de/matwerk/E210629> a mwo:Repository ;
    rdfs:label "https://github.com/stabix/stabix"^^xsd:anyURI ;
    nfdicore:url <https://github.com/stabix/stabix> .

<http://demo.fiz-karlsruhe.de/matwerk/E21101> a nfdicore:Person ;
    rdfs:label "Prof. Dr.  Jörg Neugebauer" ;
    mwo:hasAffiliation <http://demo.fiz-karlsruhe.de/matwerk/E1001>,
        <http://demo.fiz-karlsruhe.de/matwerk/E3416> ;
    mwo:hasExpertiseIn <http://demo.fiz-karlsruhe.de/matwerk/E40904>,
        <http://demo.fiz-karlsruhe.de/matwerk/E41187>,
        <http://demo.fiz-karlsruhe.de/matwerk/E41471>,
        <http://demo.fiz-karlsruhe.de/matwerk/E41756>,
        <http://demo.fiz-karlsruhe.de/matwerk/E42042>,
        <http://demo.fiz-karlsruhe.de/matwerk/E63482>,
        <http://demo.fiz-karlsruhe.de/matwerk/E63836> ;
    mwo:hasORCID <https://orcid.org/0000-0002-7903-2472> ;
    owl:sameAs <http://www.wikidata.org/entity/Q51974528> ;
    foaf:depiction <https://ams3.digitaloceanspaces.com/externalpublic/57/39a82477-bb77-4278-bdab-b1906d585147/conversions/bd9d4eec-bffd-43c0-864b-be2c9685ea36-md.jpg?X-Amz-Content-Sha256=UNSIGNED-PAYLOAD&X-Amz-Algorithm=AWS4-HMAC-SHA256&X-Amz-Credential=KVC4ZMO47JLTBHVHEFZ4%2F20230512%2Fams3%2Fs3%2Faws4_request&X-Amz-Date=20230512T150442Z&X-Amz-SignedHeaders=host&X-Amz-Expires=7200&X-Amz-Signature=291f763afdb4f7a2f4a359deafb8e1f8965c953470d34c0b6d1c3585fc3603bd> ;
    foaf:firstName "Jörg"^^xsd:string ;
    foaf:surname "Neugebauer"^^xsd:string ;
    foaf:title "Prof. Dr. "^^xsd:string .

<http://demo.fiz-karlsruhe.de/matwerk/E211277> a mwo:Repository ;
    rdfs:label "https://github.com/PASTA-ELN"^^xsd:anyURI ;
    nfdicore:url <https://github.com/PASTA-ELN> .

<http://demo.fiz-karlsruhe.de/matwerk/E211926> a mwo:Repository ;
    rdfs:label "https://github.com/elabftw/elabftw"^^xsd:anyURI ;
    nfdicore:url <https://github.com/elabftw/elabftw> .

<http://demo.fiz-karlsruhe.de/matwerk/E213227> a mwo:Repository ;
    rdfs:label "https://github.com/Materials-Data-Science-and-Informatics/metador"^^xsd:anyURI ;
    nfdicore:url <https://github.com/Materials-Data-Science-and-Informatics/metador> .

<http://demo.fiz-karlsruhe.de/matwerk/E213879> a mwo:Repository ;
    rdfs:label "https://github.com/emmo-repo/EMMO-python"^^xsd:anyURI ;
    nfdicore:url <https://github.com/emmo-repo/EMMO-python> .

<http://demo.fiz-karlsruhe.de/matwerk/E214532> a mwo:Repository ;
    rdfs:label "https://github.com/electronic-structure/SIRIUS"^^xsd:anyURI ;
    nfdicore:url <https://github.com/electronic-structure/SIRIUS> .

<http://demo.fiz-karlsruhe.de/matwerk/E215186> a mwo:Repository ;
    rdfs:label "https://github.com/wolverton-research-group/qmpy"^^xsd:anyURI ;
    nfdicore:url <https://github.com/wolverton-research-group/qmpy> .

<http://demo.fiz-karlsruhe.de/matwerk/E215841> a mwo:Repository ;
    rdfs:label "https://gitlab.com/dtorel/asr"^^xsd:anyURI ;
    nfdicore:url <https://gitlab.com/dtorel/asr> .

<http://demo.fiz-karlsruhe.de/matwerk/E216497> a mwo:Repository ;
    rdfs:label "https://gitlab.dune-project.org/dune-fem/dune-fem"^^xsd:anyURI ;
    nfdicore:url <https://gitlab.dune-project.org/dune-fem/dune-fem> .

<http://demo.fiz-karlsruhe.de/matwerk/E217154> a mwo:Repository ;
    rdfs:label "https://github.com/CompRhys/aviary"^^xsd:anyURI ;
    nfdicore:url <https://github.com/CompRhys/aviary> .

<http://demo.fiz-karlsruhe.de/matwerk/E217812> a mwo:Repository ;
    rdfs:label "https://github.com/tri-amdd/camd"^^xsd:anyURI ;
    nfdicore:url <https://github.com/tri-amdd/camd> .

<http://demo.fiz-karlsruhe.de/matwerk/E218471> a mwo:Repository ;
    rdfs:label "https://github.com/anthony-wang/CrabNet"^^xsd:anyURI ;
    nfdicore:url <https://github.com/anthony-wang/CrabNet> .

<http://demo.fiz-karlsruhe.de/matwerk/E219131> a mwo:Repository ;
    rdfs:label "https://github.com/datamol-org/datamol"^^xsd:anyURI ;
    nfdicore:url <https://github.com/datamol-org/datamol> .

<http://demo.fiz-karlsruhe.de/matwerk/E219792> a mwo:Repository ;
    rdfs:label "https://github.com/ml-evs/matador"^^xsd:anyURI ;
    nfdicore:url <https://github.com/ml-evs/matador> .

<http://demo.fiz-karlsruhe.de/matwerk/E220454> a mwo:Repository ;
    rdfs:label "https://github.com/ppdebreuck/modnet"^^xsd:anyURI ;
    nfdicore:url <https://github.com/ppdebreuck/modnet> .

<http://demo.fiz-karlsruhe.de/matwerk/E221117> a mwo:Repository ;
    rdfs:label "https://github.com/Materials-Consortia/optimade-python-tools"^^xsd:anyURI ;
    nfdicore:url <https://github.com/Materials-Consortia/optimade-python-tools> .

<http://demo.fiz-karlsruhe.de/matwerk/E221781> a mwo:Repository ;
    rdfs:label "https://github.com/TRI-AMDD/piro"^^xsd:anyURI ;
    nfdicore:url <https://github.com/TRI-AMDD/piro> .

<http://demo.fiz-karlsruhe.de/matwerk/E222446> a mwo:Repository ;
    rdfs:label "https://github.com/DeqiTang/pymatflow"^^xsd:anyURI ;
    nfdicore:url <https://github.com/DeqiTang/pymatflow> .

<http://demo.fiz-karlsruhe.de/matwerk/E223112> a mwo:Repository ;
    rdfs:label "https://github.com/materialsinnovation/pymks"^^xsd:anyURI ;
    nfdicore:url <https://github.com/materialsinnovation/pymks> .

<http://demo.fiz-karlsruhe.de/matwerk/E223779> a mwo:Repository ;
    rdfs:label "https://github.com/SCM-NV/qmflows"^^xsd:anyURI ;
    nfdicore:url <https://github.com/SCM-NV/qmflows> .

<http://demo.fiz-karlsruhe.de/matwerk/E224447> a mwo:Repository ;
    rdfs:label "https://github.com/rdkit/rdkit"^^xsd:anyURI ;
    nfdicore:url <https://github.com/rdkit/rdkit> .

<http://demo.fiz-karlsruhe.de/matwerk/E225116> a mwo:Repository ;
    rdfs:label "https://github.com/tilde-lab/tilde"^^xsd:anyURI ;
    nfdicore:url <https://github.com/tilde-lab/tilde> .

<http://demo.fiz-karlsruhe.de/matwerk/E225786> a mwo:Repository ;
    rdfs:label "https://github.com/ResearchObject/ro-crate-py"^^xsd:anyURI ;
    nfdicore:url <https://github.com/ResearchObject/ro-crate-py> .

<http://demo.fiz-karlsruhe.de/matwerk/E226457> a mwo:Repository ;
    rdfs:label "https://github.com/jacksund/simmate"^^xsd:anyURI ;
    nfdicore:url <https://github.com/jacksund/simmate> .

<http://demo.fiz-karlsruhe.de/matwerk/E227129> a mwo:Repository ;
    rdfs:label "https://github.com/nexpy/nexpy"^^xsd:anyURI ;
    nfdicore:url <https://github.com/nexpy/nexpy> .

<http://demo.fiz-karlsruhe.de/matwerk/E227802> a mwo:Repository ;
    rdfs:label "https://github.com/tomopy/tomopy"^^xsd:anyURI ;
    nfdicore:url <https://github.com/tomopy/tomopy> .

<http://demo.fiz-karlsruhe.de/matwerk/E228476> a mwo:Repository ;
    rdfs:label "https://github.com/kit-data-manager/metastore2"^^xsd:anyURI ;
    nfdicore:url <https://github.com/kit-data-manager/metastore2> .

<http://demo.fiz-karlsruhe.de/matwerk/E229151> a mwo:Repository ;
    rdfs:label "https://github.com/kit-data-manager/fairdoscope"^^xsd:anyURI ;
    nfdicore:url <https://github.com/kit-data-manager/fairdoscope> .

<http://demo.fiz-karlsruhe.de/matwerk/E229827> a mwo:Repository ;
    rdfs:label "https://github.com/yuechenbam/Ontopanel-frontend"^^xsd:anyURI ;
    nfdicore:url <https://github.com/yuechenbam/Ontopanel-frontend> .

<http://demo.fiz-karlsruhe.de/matwerk/E230504> a mwo:Repository ;
    rdfs:label "https://github.com/BEXIS2"^^xsd:anyURI ;
    nfdicore:url <https://github.com/BEXIS2> .

<http://demo.fiz-karlsruhe.de/matwerk/E231182> a mwo:Repository ;
    rdfs:label "https://github.com/kit-data-manager"^^xsd:anyURI ;
    nfdicore:url <https://github.com/kit-data-manager> .

<http://demo.fiz-karlsruhe.de/matwerk/E231861> a nfdicore:Website ;
    rdfs:label "https://www.kitware.com/contact/"^^xsd:anyURI ;
    nfdicore:url <https://www.kitware.com/contact/> .

<http://demo.fiz-karlsruhe.de/matwerk/E242861> a mwo:Documentation ;
    rdfs:label "https://workflow-gallery.github.io/calphy/README.html"^^xsd:anyURI ;
    nfdicore:url <https://workflow-gallery.github.io/calphy/README.html> .

<http://demo.fiz-karlsruhe.de/matwerk/E2432> a nfdicore:Organization ;
    rdfs:label "Universität Stuttgart" ;
    mwo:hasRORID "https://ror.org/04vnq7t77" ;
    owl:sameAs <http://www.wikidata.org/entity/Q122453> .

<http://demo.fiz-karlsruhe.de/matwerk/E243557> a mwo:Documentation ;
    rdfs:label "https://github.com/DataAnalyticsEngineering/EQ2PC#readme"^^xsd:anyURI ;
    nfdicore:url <https://github.com/DataAnalyticsEngineering/EQ2PC#readme> .

<http://demo.fiz-karlsruhe.de/matwerk/E244254> a mwo:Documentation ;
    rdfs:label "http://feap.berkeley.edu/wiki/index.php?title=FEAP_Wiki_Main_Page"^^xsd:anyURI ;
    nfdicore:url <http://feap.berkeley.edu/wiki/index.php?title=FEAP_Wiki_Main_Page> .

<http://demo.fiz-karlsruhe.de/matwerk/E244952> a mwo:Documentation ;
    rdfs:label "https://www.paraview.org/documentation/"^^xsd:anyURI ;
    nfdicore:url <https://www.paraview.org/documentation/> .

<http://demo.fiz-karlsruhe.de/matwerk/E246351> a mwo:Documentation ;
    rdfs:label "https://www.vasp.at/wiki/index.php/The_VASP_Manual"^^xsd:anyURI ;
    nfdicore:url <https://www.vasp.at/wiki/index.php/The_VASP_Manual> .

<http://demo.fiz-karlsruhe.de/matwerk/E247052> a mwo:Documentation ;
    rdfs:label "http://www.castep.org/CASTEP/Documentation"^^xsd:anyURI ;
    nfdicore:url <http://www.castep.org/CASTEP/Documentation> .

<http://demo.fiz-karlsruhe.de/matwerk/E247754> a mwo:Documentation ;
    rdfs:label "https://www.cpmd.org/wordpress/index.php/documentation/"^^xsd:anyURI ;
    nfdicore:url <https://www.cpmd.org/wordpress/index.php/documentation/> .

<http://demo.fiz-karlsruhe.de/matwerk/E248457> a mwo:Documentation ;
    rdfs:label "https://docs.abinit.org/"^^xsd:anyURI ;
    nfdicore:url <https://docs.abinit.org/> .

<http://demo.fiz-karlsruhe.de/matwerk/E249161> a mwo:Documentation ;
    rdfs:label "https://www.quantum-espresso.org/documentation/"^^xsd:anyURI ;
    nfdicore:url <https://www.quantum-espresso.org/documentation/> .

<http://demo.fiz-karlsruhe.de/matwerk/E249866> a mwo:Documentation ;
    rdfs:label "http://jdftx.org/Using.html"^^xsd:anyURI ;
    nfdicore:url <http://jdftx.org/Using.html> .

<http://demo.fiz-karlsruhe.de/matwerk/E250572> a mwo:Documentation ;
    rdfs:label "https://manual.cp2k.org/#gsc.tab=0"^^xsd:anyURI ;
    nfdicore:url <https://manual.cp2k.org/#gsc.tab=0> .

<http://demo.fiz-karlsruhe.de/matwerk/E251279> a mwo:Documentation ;
    rdfs:label "https://wiki.fysik.dtu.dk/gpaw/documentation/documentation.html"^^xsd:anyURI ;
    nfdicore:url <https://wiki.fysik.dtu.dk/gpaw/documentation/documentation.html> .

<http://demo.fiz-karlsruhe.de/matwerk/E251987> a mwo:Documentation ;
    rdfs:label "http://qboxcode.org/doc/html/"^^xsd:anyURI ;
    nfdicore:url <http://qboxcode.org/doc/html/> .

<http://demo.fiz-karlsruhe.de/matwerk/E252696> a mwo:Documentation ;
    rdfs:label "https://departments.icmab.es/leem/siesta/Documentation/index.html"^^xsd:anyURI ;
    nfdicore:url <https://departments.icmab.es/leem/siesta/Documentation/index.html> .

<http://demo.fiz-karlsruhe.de/matwerk/E253406> a mwo:Documentation ;
    rdfs:label "http://www.openmx-square.org/openmx_man3.9/index.html"^^xsd:anyURI ;
    nfdicore:url <http://www.openmx-square.org/openmx_man3.9/index.html> .

<http://demo.fiz-karlsruhe.de/matwerk/E2541> a nfdicore:Organization ;
    rdfs:label "Universität des Saarlandes" ;
    mwo:hasRORID "https://ror.org/01jdpyv68" ;
    owl:sameAs <http://www.wikidata.org/entity/Q700758> .

<http://demo.fiz-karlsruhe.de/matwerk/E254117> a mwo:Documentation ;
    rdfs:label "https://elk.sourceforge.io/#documentation"^^xsd:anyURI ;
    nfdicore:url <https://elk.sourceforge.io/#documentation> .

<http://demo.fiz-karlsruhe.de/matwerk/E254829> a mwo:Documentation ;
    rdfs:label "http://exciting.wikidot.com/tutorials-oxygen"^^xsd:anyURI ;
    nfdicore:url <http://exciting.wikidot.com/tutorials-oxygen> .

<http://demo.fiz-karlsruhe.de/matwerk/E255542> a mwo:Documentation ;
    rdfs:label "https://www.flapw.de/MaX-6.0/documentation/userGuideOverview/"^^xsd:anyURI ;
    nfdicore:url <https://www.flapw.de/MaX-6.0/documentation/userGuideOverview/> .

<http://demo.fiz-karlsruhe.de/matwerk/E256256> a mwo:Documentation ;
    rdfs:label "http://www.wien2k.at/reg_user/textbooks/usersguide.pdf"^^xsd:anyURI ;
    nfdicore:url <http://www.wien2k.at/reg_user/textbooks/usersguide.pdf> .

<http://demo.fiz-karlsruhe.de/matwerk/E256971> a mwo:Documentation ;
    rdfs:label "https://docs.lammps.org/Manual.html"^^xsd:anyURI ;
    nfdicore:url <https://docs.lammps.org/Manual.html> .

<http://demo.fiz-karlsruhe.de/matwerk/E257687> a mwo:Documentation ;
    rdfs:label "http://imd.itap.physik.uni-stuttgart.de/userguide/imd.html"^^xsd:anyURI ;
    nfdicore:url <http://imd.itap.physik.uni-stuttgart.de/userguide/imd.html> .

<http://demo.fiz-karlsruhe.de/matwerk/E258404> a mwo:Documentation ;
    rdfs:label "https://manual.gromacs.org/current/index.html"^^xsd:anyURI ;
    nfdicore:url <https://manual.gromacs.org/current/index.html> .

<http://demo.fiz-karlsruhe.de/matwerk/E259122> a mwo:Documentation ;
    rdfs:label "https://docs.fenicsproject.org/"^^xsd:anyURI ;
    nfdicore:url <https://docs.fenicsproject.org/> .

<http://demo.fiz-karlsruhe.de/matwerk/E259841> a mwo:Documentation ;
    rdfs:label "https://damask.mpie.de/documentation/index.html"^^xsd:anyURI ;
    nfdicore:url <https://damask.mpie.de/documentation/index.html> .

<http://demo.fiz-karlsruhe.de/matwerk/E260561> a mwo:Documentation ;
    rdfs:label "https://pyiron.readthedocs.io/en/latest/"^^xsd:anyURI ;
    nfdicore:url <https://pyiron.readthedocs.io/en/latest/> .

<http://demo.fiz-karlsruhe.de/matwerk/E261282> a mwo:Documentation ;
    rdfs:label "https://aiida.readthedocs.io/projects/aiida-core/en/latest/"^^xsd:anyURI ;
    nfdicore:url <https://aiida.readthedocs.io/projects/aiida-core/en/latest/> .

<http://demo.fiz-karlsruhe.de/matwerk/E262004> a mwo:Documentation ;
    rdfs:label "https://simstack.readthedocs.io/en/latest/"^^xsd:anyURI ;
    nfdicore:url <https://simstack.readthedocs.io/en/latest/> .

<http://demo.fiz-karlsruhe.de/matwerk/E262727> a mwo:Documentation ;
    rdfs:label "https://wiki.fysik.dtu.dk/ase/ase/ase.html"^^xsd:anyURI ;
    nfdicore:url <https://wiki.fysik.dtu.dk/ase/ase/ase.html> .

<http://demo.fiz-karlsruhe.de/matwerk/E263451> a mwo:Documentation ;
    rdfs:label "https://www.ovito.org/docs/current/"^^xsd:anyURI ;
    nfdicore:url <https://www.ovito.org/docs/current/> .

<http://demo.fiz-karlsruhe.de/matwerk/E264176> a mwo:Documentation ;
    rdfs:label "http://jmol.sourceforge.net/docs/"^^xsd:anyURI ;
    nfdicore:url <http://jmol.sourceforge.net/docs/> .

<http://demo.fiz-karlsruhe.de/matwerk/E264902> a mwo:Documentation ;
    rdfs:label "http://jp-minerals.org/vesta/en/doc.html"^^xsd:anyURI ;
    nfdicore:url <http://jp-minerals.org/vesta/en/doc.html> .

<http://demo.fiz-karlsruhe.de/matwerk/E265629> a mwo:Documentation ;
    rdfs:label "http://www.xcrysden.org/Documentation.html"^^xsd:anyURI ;
    nfdicore:url <http://www.xcrysden.org/Documentation.html> .

<http://demo.fiz-karlsruhe.de/matwerk/E266357> a mwo:Documentation ;
    rdfs:label "https://www.ks.uiuc.edu/Research/vmd/current/ug/"^^xsd:anyURI ;
    nfdicore:url <https://www.ks.uiuc.edu/Research/vmd/current/ug/> .

<http://demo.fiz-karlsruhe.de/matwerk/E267086> a mwo:Documentation ;
    rdfs:label "https://phonopy.github.io/phonopy/#documentation"^^xsd:anyURI ;
    nfdicore:url <https://phonopy.github.io/phonopy/#documentation> .

<http://demo.fiz-karlsruhe.de/matwerk/E267816> a mwo:Documentation ;
    rdfs:label "https://vibes-developers.gitlab.io/vibes/Documentation/0_intro/"^^xsd:anyURI ;
    nfdicore:url <https://vibes-developers.gitlab.io/vibes/Documentation/0_intro/> .

<http://demo.fiz-karlsruhe.de/matwerk/E268547> a mwo:Documentation ;
    rdfs:label "https://avogadro.cc/docs/"^^xsd:anyURI ;
    nfdicore:url <https://avogadro.cc/docs/> .

<http://demo.fiz-karlsruhe.de/matwerk/E269279> a mwo:Documentation ;
    rdfs:label "https://pymatgen.org/usage.html"^^xsd:anyURI ;
    nfdicore:url <https://pymatgen.org/usage.html> .

<http://demo.fiz-karlsruhe.de/matwerk/E270012> a mwo:Documentation ;
    rdfs:label "http://molmod.github.io/tamkin/"^^xsd:anyURI ;
    nfdicore:url <http://molmod.github.io/tamkin/> .

<http://demo.fiz-karlsruhe.de/matwerk/E270746> a mwo:Documentation ;
    rdfs:label "https://lammps.github.io/pizza/doc/Manual.html"^^xsd:anyURI ;
    nfdicore:url <https://lammps.github.io/pizza/doc/Manual.html> .

<http://demo.fiz-karlsruhe.de/matwerk/E271481> a mwo:Documentation ;
    rdfs:label "https://freud.readthedocs.io/en/latest/"^^xsd:anyURI ;
    nfdicore:url <https://freud.readthedocs.io/en/latest/> .

<http://demo.fiz-karlsruhe.de/matwerk/E272217> a mwo:Documentation ;
    rdfs:label "http://molmod.github.io/yaff/"^^xsd:anyURI ;
    nfdicore:url <http://molmod.github.io/yaff/> .

<http://demo.fiz-karlsruhe.de/matwerk/E272954> a mwo:Documentation ;
    rdfs:label "https://computationalmaterials.gitlab.io/clease/api_doc.html"^^xsd:anyURI ;
    nfdicore:url <https://computationalmaterials.gitlab.io/clease/api_doc.html> .

<http://demo.fiz-karlsruhe.de/matwerk/E273692> a mwo:Documentation ;
    rdfs:label "https://kliff.readthedocs.io/en/latest/"^^xsd:anyURI ;
    nfdicore:url <https://kliff.readthedocs.io/en/latest/> .

<http://demo.fiz-karlsruhe.de/matwerk/E274431> a mwo:Documentation ;
    rdfs:label "https://mendeleev.readthedocs.io/en/stable/quick.html"^^xsd:anyURI ;
    nfdicore:url <https://mendeleev.readthedocs.io/en/stable/quick.html> .

<http://demo.fiz-karlsruhe.de/matwerk/E275171> a mwo:Documentation ;
    rdfs:label "https://ahartmaier.github.io/pyLabFEA/"^^xsd:anyURI ;
    nfdicore:url <https://ahartmaier.github.io/pyLabFEA/> .

<http://demo.fiz-karlsruhe.de/matwerk/E275912> a mwo:Documentation ;
    rdfs:label "https://pacemaker.readthedocs.io/en/latest/"^^xsd:anyURI ;
    nfdicore:url <https://pacemaker.readthedocs.io/en/latest/> .

<http://demo.fiz-karlsruhe.de/matwerk/E276654> a mwo:Documentation ;
    rdfs:label "https://paraprobe-toolbox.readthedocs.io/en/latest/"^^xsd:anyURI ;
    nfdicore:url <https://paraprobe-toolbox.readthedocs.io/en/latest/> .

<http://demo.fiz-karlsruhe.de/matwerk/E277397> a mwo:Documentation ;
    rdfs:label "https://stabix.readthedocs.io/en/latest/"^^xsd:anyURI ;
    nfdicore:url <https://stabix.readthedocs.io/en/latest/> .

<http://demo.fiz-karlsruhe.de/matwerk/E278141> a mwo:Documentation ;
    rdfs:label "https://math.lbl.gov/voro++/doc/"^^xsd:anyURI ;
    nfdicore:url <https://math.lbl.gov/voro++/doc/> .

<http://demo.fiz-karlsruhe.de/matwerk/E278886> a mwo:Documentation ;
    rdfs:label "http://www.qhull.org/html/index.htm"^^xsd:anyURI ;
    nfdicore:url <http://www.qhull.org/html/index.htm> .

<http://demo.fiz-karlsruhe.de/matwerk/E279632> a mwo:Documentation ;
    rdfs:label "https://doc.elabftw.net/"^^xsd:anyURI ;
    nfdicore:url <https://doc.elabftw.net/> .

<http://demo.fiz-karlsruhe.de/matwerk/E280379> a mwo:Documentation ;
    rdfs:label "https://kadi4mat.readthedocs.io/en/stable/index.html"^^xsd:anyURI ;
    nfdicore:url <https://kadi4mat.readthedocs.io/en/stable/index.html> .

<http://demo.fiz-karlsruhe.de/matwerk/E281127> a mwo:Documentation ;
    rdfs:label "https://github.com/Materials-Data-Science-and-Informatics/metador/blob/main/README.md"^^xsd:anyURI ;
    nfdicore:url <https://github.com/Materials-Data-Science-and-Informatics/metador/blob/main/README.md> .

<http://demo.fiz-karlsruhe.de/matwerk/E281876> a mwo:Documentation ;
    rdfs:label "https://docs.httk.org/en/latest/"^^xsd:anyURI ;
    nfdicore:url <https://docs.httk.org/en/latest/> .

<http://demo.fiz-karlsruhe.de/matwerk/E282626> a mwo:Documentation ;
    rdfs:label "https://colabfit.github.io/colabfit-tools/html/index.html"^^xsd:anyURI ;
    nfdicore:url <https://colabfit.github.io/colabfit-tools/html/index.html> .

<http://demo.fiz-karlsruhe.de/matwerk/E2831> a nfdicore:Organization ;
    rdfs:label "Universität Paderborn" ;
    mwo:hasRORID "https://ror.org/058kzsd48" ;
    owl:sameAs <http://www.wikidata.org/entity/Q679134> .

<http://demo.fiz-karlsruhe.de/matwerk/E283377> a mwo:Documentation ;
    rdfs:label "https://static.oqmd.org/static/docs/index.html"^^xsd:anyURI ;
    nfdicore:url <https://static.oqmd.org/static/docs/index.html> .

<http://demo.fiz-karlsruhe.de/matwerk/E284129> a mwo:Documentation ;
    rdfs:label "https://api.materialsproject.org/docs"^^xsd:anyURI ;
    nfdicore:url <https://api.materialsproject.org/docs> .

<http://demo.fiz-karlsruhe.de/matwerk/E284882> a mwo:Documentation ;
    rdfs:label "https://www.turbomole.org/turbomole/turbomole-documentation/"^^xsd:anyURI ;
    nfdicore:url <https://www.turbomole.org/turbomole/turbomole-documentation/> .

<http://demo.fiz-karlsruhe.de/matwerk/E285636> a mwo:Documentation ;
    rdfs:label "https://jacksund.github.io/simmate/home/"^^xsd:anyURI ;
    nfdicore:url <https://jacksund.github.io/simmate/home/> .

<http://demo.fiz-karlsruhe.de/matwerk/E286391> a mwo:Documentation ;
    rdfs:label "https://kit-data-manager.github.io/fairdoscope/"^^xsd:anyURI ;
    nfdicore:url <https://kit-data-manager.github.io/fairdoscope/> .

<http://demo.fiz-karlsruhe.de/matwerk/E287147> a nfdicore:Website ;
    rdfs:label "https://procon-x-ray.de/ct-alpha/"^^xsd:anyURI ;
    nfdicore:url <https://procon-x-ray.de/ct-alpha/> .

<http://demo.fiz-karlsruhe.de/matwerk/E287904> a nfdicore:Website ;
    rdfs:label "https://procon-x-ray.de/ct-nano/"^^xsd:anyURI ;
    nfdicore:url <https://procon-x-ray.de/ct-nano/> .

<http://demo.fiz-karlsruhe.de/matwerk/E288662> a mwo:Repository ;
    rdfs:label "https://doi.org/10.1016/j.dib.2019.104724"^^xsd:anyURI ;
    nfdicore:url <https://doi.org/10.1016/j.dib.2019.104724> .

<http://demo.fiz-karlsruhe.de/matwerk/E2892> a nfdicore:Organization ;
    rdfs:label "Technische Universität Darmstadt" ;
    mwo:hasRORID "https://ror.org/05n911h24" ;
    owl:sameAs <http://www.wikidata.org/entity/Q310695> .

<http://demo.fiz-karlsruhe.de/matwerk/E289421> a mwo:Repository ;
    rdfs:label "https://github.com/DataAnalyticsEngineering/EQ2PC/tree/master/data"^^xsd:anyURI ;
    nfdicore:url <https://github.com/DataAnalyticsEngineering/EQ2PC/tree/master/data> .

<http://demo.fiz-karlsruhe.de/matwerk/E290181> a mwo:Repository ;
    rdfs:label "https://github.com/CPShub/sim-data/tree/master/data/parametric_beam_lattice_metamaterials"^^xsd:anyURI ;
    nfdicore:url <https://github.com/CPShub/sim-data/tree/master/data/parametric_beam_lattice_metamaterials> .

<http://demo.fiz-karlsruhe.de/matwerk/E290942> a mwo:Repository ;
    rdfs:label "https://www.frontiersin.org/articles/10.3389/fmats.2019.00075/full#supplementary-material"^^xsd:anyURI ;
    nfdicore:url <https://www.frontiersin.org/articles/10.3389/fmats.2019.00075/full#supplementary-material> .

<http://demo.fiz-karlsruhe.de/matwerk/E291704> a mwo:Repository ;
    rdfs:label "https://doi.org/10.5281/zenodo.5106606"^^xsd:anyURI ;
    nfdicore:url <https://doi.org/10.5281/zenodo.5106606> .

<http://demo.fiz-karlsruhe.de/matwerk/E292467> a mwo:Repository ;
    rdfs:label "https://doi.org/10.5281/zenodo.6787085"^^xsd:anyURI ;
    nfdicore:url <https://doi.org/10.5281/zenodo.6787085> .

<http://demo.fiz-karlsruhe.de/matwerk/E293231> a mwo:Repository ;
    rdfs:label "https://doi.org/10.5281/zenodo.6778336"^^xsd:anyURI ;
    nfdicore:url <https://doi.org/10.5281/zenodo.6778336> .

<http://demo.fiz-karlsruhe.de/matwerk/E293996> a mwo:Documentation ;
    rdfs:label "https://doi.org/10.1016/j.msea.2019.138295"^^xsd:anyURI ;
    nfdicore:url <https://doi.org/10.1016/j.msea.2019.138295> .

<http://demo.fiz-karlsruhe.de/matwerk/E294762> a mwo:Documentation ;
    rdfs:label "https://doi.org/10.1098/rspa.2020.0568"^^xsd:anyURI ;
    nfdicore:url <https://doi.org/10.1098/rspa.2020.0568> .

<http://demo.fiz-karlsruhe.de/matwerk/E2954> a nfdicore:Organization ;
    rdfs:label "Technische Universität Clausthal" ;
    mwo:hasRORID "https://ror.org/04qb8nc58" ;
    owl:sameAs <http://www.wikidata.org/entity/Q447354> .

<http://demo.fiz-karlsruhe.de/matwerk/E295529> a mwo:Documentation ;
    rdfs:label "https://doi.org/10.1002/nme.6869"^^xsd:anyURI ;
    nfdicore:url <https://doi.org/10.1002/nme.6869> .

<http://demo.fiz-karlsruhe.de/matwerk/E296297> a mwo:Documentation ;
    rdfs:label "https://doi.org/10.3389/fmats.2019.00075"^^xsd:anyURI ;
    nfdicore:url <https://doi.org/10.3389/fmats.2019.00075> .

<http://demo.fiz-karlsruhe.de/matwerk/E29681> a nfdicore:Person ;
    rdfs:label "Said Fathalla" ;
    mwo:hasAffiliation <http://demo.fiz-karlsruhe.de/matwerk/E1022> ;
    foaf:firstName "Said"^^xsd:string ;
    foaf:surname "Fathalla"^^xsd:string .

<http://demo.fiz-karlsruhe.de/matwerk/E297066> a mwo:Documentation ;
    rdfs:label "https://doi.org/10.1007/s10853-020-05740-x"^^xsd:anyURI ;
    nfdicore:url <https://doi.org/10.1007/s10853-020-05740-x> .

<http://demo.fiz-karlsruhe.de/matwerk/E297067> a mwo:Documentation ;
    rdfs:label "https://doi.org/10.1016/j.msea.2018.01.033"^^xsd:anyURI ;
    nfdicore:url <https://doi.org/10.1016/j.msea.2018.01.033> .

<http://demo.fiz-karlsruhe.de/matwerk/E297836> a nfdicore:Website ;
    rdfs:label "https://www.desy.de"^^xsd:anyURI ;
    nfdicore:url <https://www.desy.de> .

<http://demo.fiz-karlsruhe.de/matwerk/E298607> a nfdicore:Website ;
    rdfs:label "https://www.rz.uni-kiel.de/en/our-portfolio/hiperf/hpc"^^xsd:anyURI ;
    nfdicore:url <https://www.rz.uni-kiel.de/en/our-portfolio/hiperf/hpc> .

<http://demo.fiz-karlsruhe.de/matwerk/E299379> a nfdicore:Website ;
    rdfs:label "https://www.fz-juelich.de/en/ias/jsc"^^xsd:anyURI ;
    nfdicore:url <https://www.fz-juelich.de/en/ias/jsc> .

<http://demo.fiz-karlsruhe.de/matwerk/E300152> a nfdicore:Website ;
    rdfs:label "https://www.scc.kit.edu/"^^xsd:anyURI ;
    nfdicore:url <https://www.scc.kit.edu/> .

<http://demo.fiz-karlsruhe.de/matwerk/E300926> a nfdicore:Website ;
    rdfs:label "https://www.hzdr.de/db/Cms?pNid=1984&pOid=40983"^^xsd:anyURI ;
    nfdicore:url <https://www.hzdr.de/db/Cms?pNid=1984&pOid=40983> .

<http://demo.fiz-karlsruhe.de/matwerk/E30162> a nfdicore:Person ;
    rdfs:label "Huanyu Li" ;
    mwo:hasAffiliation <http://demo.fiz-karlsruhe.de/matwerk/E4404> ;
    foaf:firstName "Huanyu"^^xsd:string ;
    foaf:surname "Li"^^xsd:string .

<http://demo.fiz-karlsruhe.de/matwerk/E304032> a mwo:Repository ;
    rdfs:label "https://zenodo.org/record/6513745#.YvS4gNJBwUH"^^xsd:anyURI ;
    nfdicore:url <https://zenodo.org/record/6513745#.YvS4gNJBwUH> .

<http://demo.fiz-karlsruhe.de/matwerk/E30404> a nfdicore:Person ;
    rdfs:label "Patrick Lambrix" ;
    mwo:hasAffiliation <http://demo.fiz-karlsruhe.de/matwerk/E4404> ;
    foaf:firstName "Patrick"^^xsd:string ;
    foaf:surname "Lambrix"^^xsd:string .

<http://demo.fiz-karlsruhe.de/matwerk/E304811> a mwo:Repository ;
    rdfs:label "https://github.com/Materials-Consortia/OPTIMADE"^^xsd:anyURI ;
    nfdicore:url <https://github.com/Materials-Consortia/OPTIMADE> .

<http://demo.fiz-karlsruhe.de/matwerk/E305591> a mwo:Repository ;
    rdfs:label "https://github.com/emmo-repo/EMMO"^^xsd:anyURI ;
    nfdicore:url <https://github.com/emmo-repo/EMMO> .

<http://demo.fiz-karlsruhe.de/matwerk/E306372> a mwo:Repository ;
    rdfs:label "https://github.com/tetherless-world/materialsmine"^^xsd:anyURI ;
    nfdicore:url <https://github.com/tetherless-world/materialsmine> .

<http://demo.fiz-karlsruhe.de/matwerk/E30647> a nfdicore:Person ;
    rdfs:label "Rickard Armiento" ;
    mwo:hasAffiliation <http://demo.fiz-karlsruhe.de/matwerk/E4404> ;
    foaf:firstName "Rickard"^^xsd:string ;
    foaf:surname "Armiento"^^xsd:string .

<http://demo.fiz-karlsruhe.de/matwerk/E307154> a mwo:Repository ;
    rdfs:label "https://github.com/Materials-Data-Science-and-Informatics/dislocation-ontology"^^xsd:anyURI ;
    nfdicore:url <https://github.com/Materials-Data-Science-and-Informatics/dislocation-ontology> .

<http://demo.fiz-karlsruhe.de/matwerk/E307937> a mwo:Repository ;
    rdfs:label "https://github.com/LiUSemWeb/Materials-Design-Ontology"^^xsd:anyURI ;
    nfdicore:url <https://github.com/LiUSemWeb/Materials-Design-Ontology> .

<http://demo.fiz-karlsruhe.de/matwerk/E308721> a mwo:Repository ;
    rdfs:label "https://github.com/iassouroko/AMontology"^^xsd:anyURI ;
    nfdicore:url <https://github.com/iassouroko/AMontology> .

<http://demo.fiz-karlsruhe.de/matwerk/E309506> a mwo:Repository ;
    rdfs:label "https://github.com/inovexcorp/MatOnto-Ontologies"^^xsd:anyURI ;
    nfdicore:url <https://github.com/inovexcorp/MatOnto-Ontologies> .

<http://demo.fiz-karlsruhe.de/matwerk/E310292> a mwo:Repository ;
    rdfs:label "https://matportal.org/ontologies/VIMMP_ONTOLOGIES"^^xsd:anyURI ;
    nfdicore:url <https://matportal.org/ontologies/VIMMP_ONTOLOGIES> .

<http://demo.fiz-karlsruhe.de/matwerk/E311079> a mwo:Repository ;
    rdfs:label "https://github.com/enanomapper/ontologies"^^xsd:anyURI ;
    nfdicore:url <https://github.com/enanomapper/ontologies> .

<http://demo.fiz-karlsruhe.de/matwerk/E31136> a nfdicore:Person ;
    rdfs:label "Vahid Samaee" ;
    foaf:firstName "Vahid"^^xsd:string ;
    foaf:surname "Samaee"^^xsd:string .

<http://demo.fiz-karlsruhe.de/matwerk/E311867> a mwo:Repository ;
    rdfs:label "https://github.com/Mat-O-Lab/MSEO"^^xsd:anyURI ;
    nfdicore:url <https://github.com/Mat-O-Lab/MSEO> .

<http://demo.fiz-karlsruhe.de/matwerk/E312656> a mwo:Repository ;
    rdfs:label "https://github.com/materialdigital/core-ontology"^^xsd:anyURI ;
    nfdicore:url <https://github.com/materialdigital/core-ontology> .

<http://demo.fiz-karlsruhe.de/matwerk/E313446> a mwo:Repository ;
    rdfs:label "http://www.nano-ontology.org/"^^xsd:anyURI ;
    nfdicore:url <http://www.nano-ontology.org/> .

<http://demo.fiz-karlsruhe.de/matwerk/E31382> a nfdicore:Person ;
    rdfs:label "Hosni Idrissi" ;
    mwo:hasAffiliation <http://demo.fiz-karlsruhe.de/matwerk/E7556> ;
    foaf:firstName "Hosni"^^xsd:string ;
    foaf:surname "Idrissi"^^xsd:string .

<http://demo.fiz-karlsruhe.de/matwerk/E314237> a mwo:Repository ;
    rdfs:label "https://github.com/daimoners/MAMBO"^^xsd:anyURI ;
    nfdicore:url <https://github.com/daimoners/MAMBO> .

<http://demo.fiz-karlsruhe.de/matwerk/E315029> a mwo:Repository ;
    rdfs:label "https://github.com/Exabyte-io/esse"^^xsd:anyURI ;
    nfdicore:url <https://github.com/Exabyte-io/esse> .

<http://demo.fiz-karlsruhe.de/matwerk/E315822> a mwo:Repository ;
    rdfs:label "https://gitlab.com/ElectronicStructureLibrary/escdf/escdf-specifications"^^xsd:anyURI ;
    nfdicore:url <https://gitlab.com/ElectronicStructureLibrary/escdf/escdf-specifications> .

<http://demo.fiz-karlsruhe.de/matwerk/E31629> a nfdicore:Person ;
    rdfs:label "Jonas Groten" ;
    mwo:hasAffiliation <http://demo.fiz-karlsruhe.de/matwerk/E7787> ;
    foaf:firstName "Jonas"^^xsd:string ;
    foaf:surname "Groten"^^xsd:string .

<http://demo.fiz-karlsruhe.de/matwerk/E316616> a mwo:Repository ;
    rdfs:label "https://github.com/nexusformat"^^xsd:anyURI ;
    nfdicore:url <https://github.com/nexusformat> .

<http://demo.fiz-karlsruhe.de/matwerk/E317411> a mwo:Repository ;
    rdfs:label "https://github.com/usnistgov/mgi-json-schema"^^xsd:anyURI ;
    nfdicore:url <https://github.com/usnistgov/mgi-json-schema> .

<http://demo.fiz-karlsruhe.de/matwerk/E318207> a mwo:Repository ;
    rdfs:label "https://github.com/rsc-ontologies/rsc-cmo"^^xsd:anyURI ;
    nfdicore:url <https://github.com/rsc-ontologies/rsc-cmo> .

<http://demo.fiz-karlsruhe.de/matwerk/E31877> a nfdicore:Person ;
    rdfs:label "Thomas Pardoen" ;
    mwo:hasAffiliation <http://demo.fiz-karlsruhe.de/matwerk/E7556> ;
    foaf:firstName "Thomas"^^xsd:string ;
    foaf:surname "Pardoen"^^xsd:string .

<http://demo.fiz-karlsruhe.de/matwerk/E319004> a mwo:Repository ;
    rdfs:label "https://github.com/emmo-repo/domain-characterisation-methodology"^^xsd:anyURI ;
    nfdicore:url <https://github.com/emmo-repo/domain-characterisation-methodology> .

<http://demo.fiz-karlsruhe.de/matwerk/E320601> a mwo:Documentation ;
    rdfs:label "https://www.optimade.org/"^^xsd:anyURI ;
    nfdicore:url <https://www.optimade.org/> .

<http://demo.fiz-karlsruhe.de/matwerk/E32126> a nfdicore:Person ;
    rdfs:label "Dominique Schryvers" ;
    foaf:firstName "Dominique"^^xsd:string ;
    foaf:surname "Schryvers"^^xsd:string .

<http://demo.fiz-karlsruhe.de/matwerk/E321401> a mwo:Documentation ;
    rdfs:label "https://materials-data-science-and-informatics.github.io/dislocation-ontology/"^^xsd:anyURI ;
    nfdicore:url <https://materials-data-science-and-informatics.github.io/dislocation-ontology/> .

<http://demo.fiz-karlsruhe.de/matwerk/E322202> a mwo:Documentation ;
    rdfs:label "w3id.org/mdo/full/1.0/" .

<http://demo.fiz-karlsruhe.de/matwerk/E323004> a mwo:Documentation ;
    rdfs:label "http://www.quantum-simulation.org/"^^xsd:anyURI ;
    nfdicore:url <http://www.quantum-simulation.org/> .

<http://demo.fiz-karlsruhe.de/matwerk/E323807> a mwo:Documentation ;
    rdfs:label "https://publications.jrc.ec.europa.eu/repository/handle/JRC75978"^^xsd:anyURI ;
    nfdicore:url <https://publications.jrc.ec.europa.eu/repository/handle/JRC75978> .

<http://demo.fiz-karlsruhe.de/matwerk/E324611> a mwo:Documentation ;
    rdfs:label "http://docs.oasis-open.org/materials/materials-matml-spec-pr-01.htm"^^xsd:anyURI ;
    nfdicore:url <http://docs.oasis-open.org/materials/materials-matml-spec-pr-01.htm> .

<http://demo.fiz-karlsruhe.de/matwerk/E325416> a mwo:Documentation ;
    rdfs:label "https://www.iucr.org/resources/cif"^^xsd:anyURI ;
    nfdicore:url <https://www.iucr.org/resources/cif> .

<http://demo.fiz-karlsruhe.de/matwerk/E326222> a mwo:Documentation ;
    rdfs:label "https://colabfit.org/about/"^^xsd:anyURI ;
    nfdicore:url <https://colabfit.org/about/> .

<http://demo.fiz-karlsruhe.de/matwerk/E327029> a mwo:Documentation ;
    rdfs:label "https://citrineinformatics.github.io/gemd-docs/"^^xsd:anyURI ;
    nfdicore:url <https://citrineinformatics.github.io/gemd-docs/> .

<http://demo.fiz-karlsruhe.de/matwerk/E327837> a mwo:Documentation ;
    rdfs:label "https://nomad-lab.eu/services/metainfo"^^xsd:anyURI ;
    nfdicore:url <https://nomad-lab.eu/services/metainfo> .

<http://demo.fiz-karlsruhe.de/matwerk/E328646> a mwo:Documentation ;
    rdfs:label "https://citrineinformatics.github.io/pif-documentation/index.html"^^xsd:anyURI ;
    nfdicore:url <https://citrineinformatics.github.io/pif-documentation/index.html> .

<http://demo.fiz-karlsruhe.de/matwerk/E32879> a nfdicore:Person ;
    rdfs:label "Sina Schriever" ;
    mwo:hasAffiliation <http://demo.fiz-karlsruhe.de/matwerk/E1245619>,
        <http://demo.fiz-karlsruhe.de/matwerk/E1245640> ;
    mwo:hasExpertiseIn <http://demo.fiz-karlsruhe.de/matwerk/E1245665> ;
    foaf:firstName "Sina"^^xsd:string ;
    foaf:surname "Schriever"^^xsd:string .

<http://demo.fiz-karlsruhe.de/matwerk/E329456> a mwo:Documentation ;
    rdfs:label "https://www.nexusformat.org/"^^xsd:anyURI ;
    nfdicore:url <https://www.nexusformat.org/> .

<http://demo.fiz-karlsruhe.de/matwerk/E330267> a mwo:Documentation ;
    rdfs:label "https://emmc.eu/moda/"^^xsd:anyURI ;
    nfdicore:url <https://emmc.eu/moda/> .

<http://demo.fiz-karlsruhe.de/matwerk/E331079> a mwo:Documentation ;
    rdfs:label "http://icatproject-contrib.github.io/CSMD/"^^xsd:anyURI ;
    nfdicore:url <http://icatproject-contrib.github.io/CSMD/> .

<http://demo.fiz-karlsruhe.de/matwerk/E331892> a mwo:Documentation ;
    rdfs:label "https://www.izus.uni-stuttgart.de/fokus/engmeta"^^xsd:anyURI ;
    nfdicore:url <https://www.izus.uni-stuttgart.de/fokus/engmeta> .

<http://demo.fiz-karlsruhe.de/matwerk/E33386> a nfdicore:Person ;
    rdfs:label "Philipp von Hartrott" ;
    mwo:hasAffiliation <http://demo.fiz-karlsruhe.de/matwerk/E1245619>,
        <http://demo.fiz-karlsruhe.de/matwerk/E1245640> ;
    foaf:firstName "Philipp"^^xsd:string ;
    foaf:surname "von Hartrott"^^xsd:string .

<http://demo.fiz-karlsruhe.de/matwerk/E334337> a nfdicore:Website ;
    rdfs:label "https://us3.list-manage.com/contact-form?u=16634d765b0c938ba69db3498&form_id=fa3029c68e8ab3aa138c7d816fca14f9"^^xsd:anyURI ;
    nfdicore:url <https://us3.list-manage.com/contact-form?u=16634d765b0c938ba69db3498&form_id=fa3029c68e8ab3aa138c7d816fca14f9> .

<http://demo.fiz-karlsruhe.de/matwerk/E335154> a nfdicore:Website ;
    rdfs:label "https://github.com/"^^xsd:anyURI ;
    nfdicore:url <https://github.com/> .

<http://demo.fiz-karlsruhe.de/matwerk/E335972> a nfdicore:Website ;
    rdfs:label "zenodo.org" .

<http://demo.fiz-karlsruhe.de/matwerk/E33641> a nfdicore:Person ;
    rdfs:label "Markus Schilling" ;
    mwo:hasAffiliation <http://demo.fiz-karlsruhe.de/matwerk/E1245619>,
        <http://demo.fiz-karlsruhe.de/matwerk/E1245640> ;
    foaf:firstName "Markus"^^xsd:string ;
    foaf:surname "Schilling"^^xsd:string .

<http://demo.fiz-karlsruhe.de/matwerk/E336791> a nfdicore:Website ;
    rdfs:label "https://datadryad.org/stash"^^xsd:anyURI ;
    nfdicore:url <https://datadryad.org/stash> .

<http://demo.fiz-karlsruhe.de/matwerk/E337611> a nfdicore:Website ;
    rdfs:label "https://osf.io/"^^xsd:anyURI ;
    nfdicore:url <https://osf.io/> .

<http://demo.fiz-karlsruhe.de/matwerk/E338432> a nfdicore:Website ;
    rdfs:label "https://figshare.com/"^^xsd:anyURI ;
    nfdicore:url <https://figshare.com/> .

<http://demo.fiz-karlsruhe.de/matwerk/E33897> a nfdicore:Person ;
    rdfs:label "Steffen Glaubitz" ;
    mwo:hasAffiliation <http://demo.fiz-karlsruhe.de/matwerk/E1245619>,
        <http://demo.fiz-karlsruhe.de/matwerk/E1245640> ;
    foaf:firstName "Steffen"^^xsd:string ;
    foaf:surname "Glaubitz"^^xsd:string .

<http://demo.fiz-karlsruhe.de/matwerk/E339254> a nfdicore:Website ;
    rdfs:label "https://cau-git.rz.uni-kiel.de"^^xsd:anyURI ;
    nfdicore:url <https://cau-git.rz.uni-kiel.de> .

<http://demo.fiz-karlsruhe.de/matwerk/E340077> a nfdicore:Website ;
    rdfs:label "https://opendata.uni-kiel.de"^^xsd:anyURI ;
    nfdicore:url <https://opendata.uni-kiel.de> .

<http://demo.fiz-karlsruhe.de/matwerk/E340901> a nfdicore:Website ;
    rdfs:label "https://www.ctcms.nist.gov/potentials/"^^xsd:anyURI ;
    nfdicore:url <https://www.ctcms.nist.gov/potentials/> .

<http://demo.fiz-karlsruhe.de/matwerk/E34154> a nfdicore:Person ;
    rdfs:label "Kathrin Matzak" ;
    mwo:hasAffiliation <http://demo.fiz-karlsruhe.de/matwerk/E1245619>,
        <http://demo.fiz-karlsruhe.de/matwerk/E1245640> ;
    foaf:firstName "Kathrin"^^xsd:string ;
    foaf:surname "Matzak"^^xsd:string .

<http://demo.fiz-karlsruhe.de/matwerk/E341726> a nfdicore:Website ;
    rdfs:label "https://openkim.org/"^^xsd:anyURI ;
    nfdicore:url <https://openkim.org/> .

<http://demo.fiz-karlsruhe.de/matwerk/E342552> a nfdicore:Website ;
    rdfs:label "http://www.atomistica.org/"^^xsd:anyURI ;
    nfdicore:url <http://www.atomistica.org/> .

<http://demo.fiz-karlsruhe.de/matwerk/E343379> a nfdicore:Website ;
    rdfs:label "https://www.ccpnc.ac.uk/database/"^^xsd:anyURI ;
    nfdicore:url <https://www.ccpnc.ac.uk/database/> .

<http://demo.fiz-karlsruhe.de/matwerk/E34412> a nfdicore:Person ;
    rdfs:label "Birgit Rehmer" ;
    mwo:hasAffiliation <http://demo.fiz-karlsruhe.de/matwerk/E1245619>,
        <http://demo.fiz-karlsruhe.de/matwerk/E1245640> ;
    foaf:firstName "Birgit"^^xsd:string ;
    foaf:surname "Rehmer"^^xsd:string .

<http://demo.fiz-karlsruhe.de/matwerk/E344207> a nfdicore:Website ;
    rdfs:label "https://www.ccpnc.ac.uk/pspot-site/"^^xsd:anyURI ;
    nfdicore:url <https://www.ccpnc.ac.uk/pspot-site/> .

<http://demo.fiz-karlsruhe.de/matwerk/E345036> a nfdicore:Website ;
    rdfs:label "https://pubchem.ncbi.nlm.nih.gov/"^^xsd:anyURI ;
    nfdicore:url <https://pubchem.ncbi.nlm.nih.gov/> .

<http://demo.fiz-karlsruhe.de/matwerk/E345866> a nfdicore:Website ;
    rdfs:label "https://www.cryst.ehu.es/"^^xsd:anyURI ;
    nfdicore:url <https://www.cryst.ehu.es/> .

<http://demo.fiz-karlsruhe.de/matwerk/E346697> a nfdicore:Website ;
    rdfs:label "http://www.crystallography.net/cod/"^^xsd:anyURI ;
    nfdicore:url <http://www.crystallography.net/cod/> .

<http://demo.fiz-karlsruhe.de/matwerk/E347529> a nfdicore:Website ;
    rdfs:label "https://materialsproject.org/"^^xsd:anyURI ;
    nfdicore:url <https://materialsproject.org/> .

<http://demo.fiz-karlsruhe.de/matwerk/E348362> a nfdicore:Website ;
    rdfs:label "https://www.materialscloud.org/discover/mc3d/dashboard/ptable"^^xsd:anyURI ;
    nfdicore:url <https://www.materialscloud.org/discover/mc3d/dashboard/ptable> .

<http://demo.fiz-karlsruhe.de/matwerk/E349196> a nfdicore:Website ;
    rdfs:label "https://nomad-lab.eu"^^xsd:anyURI ;
    nfdicore:url <https://nomad-lab.eu> .

<http://demo.fiz-karlsruhe.de/matwerk/E34931> a nfdicore:Person ;
    mwo:emailAddress "s.menon@mpie.de"^^xsd:string ;
    foaf:firstName "Joerg"^^xsd:string ;
    foaf:surname "Neugebauer"^^xsd:string ;
    foaf:title ""^^xsd:string .

<http://demo.fiz-karlsruhe.de/matwerk/E350031> a nfdicore:Website ;
    rdfs:label "https://matportal.org/"^^xsd:anyURI ;
    nfdicore:url <https://matportal.org/> .

<http://demo.fiz-karlsruhe.de/matwerk/E350867> a nfdicore:Website ;
    rdfs:label "http://atomistictools.org/"^^xsd:anyURI ;
    nfdicore:url <http://atomistictools.org/> .

<http://demo.fiz-karlsruhe.de/matwerk/E351704> a nfdicore:Website ;
    rdfs:label "http://aflow.org"^^xsd:anyURI ;
    nfdicore:url <http://aflow.org> .

<http://demo.fiz-karlsruhe.de/matwerk/E35192> a nfdicore:Person ;
    mwo:emailAddress "s.menon@mpie.de"^^xsd:string ;
    foaf:firstName "Michael"^^xsd:string ;
    foaf:surname "Finnis"^^xsd:string ;
    foaf:title ""^^xsd:string .

<http://demo.fiz-karlsruhe.de/matwerk/E352542> a nfdicore:Website ;
    rdfs:label "https://jarvis.nist.gov/"^^xsd:anyURI ;
    nfdicore:url <https://jarvis.nist.gov/> .

<http://demo.fiz-karlsruhe.de/matwerk/E353381> a nfdicore:Website ;
    rdfs:label "https://mpds.io/"^^xsd:anyURI ;
    nfdicore:url <https://mpds.io/> .

<http://demo.fiz-karlsruhe.de/matwerk/E354221> a nfdicore:Website ;
    rdfs:label "https://openmaterialsdb.se/"^^xsd:anyURI ;
    nfdicore:url <https://openmaterialsdb.se/> .

<http://demo.fiz-karlsruhe.de/matwerk/E355062> a nfdicore:Website ;
    rdfs:label "https://oqmd.org/"^^xsd:anyURI ;
    nfdicore:url <https://oqmd.org/> .

<http://demo.fiz-karlsruhe.de/matwerk/E355904> a nfdicore:Website ;
    rdfs:label "https://citrination.com/"^^xsd:anyURI ;
    nfdicore:url <https://citrination.com/> .

<http://demo.fiz-karlsruhe.de/matwerk/E356747> a nfdicore:Website ;
    rdfs:label "https://odin.jrc.ec.europa.eu/alcor/PortalController?query=Select&action=Refresh"^^xsd:anyURI ;
    nfdicore:url <https://odin.jrc.ec.europa.eu/alcor/PortalController?query=Select&action=Refresh> .

<http://demo.fiz-karlsruhe.de/matwerk/E357591> a nfdicore:Website ;
    rdfs:label "https://www.matdat.com/"^^xsd:anyURI ;
    nfdicore:url <https://www.matdat.com/> .

<http://demo.fiz-karlsruhe.de/matwerk/E358436> a nfdicore:Website ;
    rdfs:label "https://mdr.nims.go.jp"^^xsd:anyURI ;
    nfdicore:url <https://mdr.nims.go.jp> .

<http://demo.fiz-karlsruhe.de/matwerk/E359282> a nfdicore:Website ;
    rdfs:label "https://mits.nims.go.jp/en/"^^xsd:anyURI ;
    nfdicore:url <https://mits.nims.go.jp/en/> .

<http://demo.fiz-karlsruhe.de/matwerk/E360129> a nfdicore:Website ;
    rdfs:label "https://polymer.nims.go.jp/en/"^^xsd:anyURI ;
    nfdicore:url <https://polymer.nims.go.jp/en/> .

<http://demo.fiz-karlsruhe.de/matwerk/E360977> a nfdicore:Website ;
    rdfs:label "https://crystdb.nims.go.jp/en/"^^xsd:anyURI ;
    nfdicore:url <https://crystdb.nims.go.jp/en/> .

<http://demo.fiz-karlsruhe.de/matwerk/E361826> a nfdicore:Website ;
    rdfs:label "https://compes-x.nims.go.jp/en/"^^xsd:anyURI ;
    nfdicore:url <https://compes-x.nims.go.jp/en/> .

<http://demo.fiz-karlsruhe.de/matwerk/E36246> a nfdicore:AcademicDiscipline ;
    rdfs:label "software development" ;
    owl:sameAs <http://www.wikidata.org/entity/Q638608> .

<http://demo.fiz-karlsruhe.de/matwerk/E362676> a nfdicore:Website ;
    rdfs:label "https://diffusion.nims.go.jp/en/"^^xsd:anyURI ;
    nfdicore:url <https://diffusion.nims.go.jp/en/> .

<http://demo.fiz-karlsruhe.de/matwerk/E363527> a nfdicore:Website ;
    rdfs:label "https://thermophys.nims.go.jp/en/"^^xsd:anyURI ;
    nfdicore:url <https://thermophys.nims.go.jp/en/> .

<http://demo.fiz-karlsruhe.de/matwerk/E364379> a nfdicore:Website ;
    rdfs:label "https://metallicmaterials.nims.go.jp/en/"^^xsd:anyURI ;
    nfdicore:url <https://metallicmaterials.nims.go.jp/en/> .

<http://demo.fiz-karlsruhe.de/matwerk/E36512> a nfdicore:AcademicDiscipline ;
    rdfs:label "computational mechanics" ;
    owl:sameAs <http://www.wikidata.org/entity/Q919765> .

<http://demo.fiz-karlsruhe.de/matwerk/E365232> a nfdicore:Website ;
    rdfs:label "https://weldcct.nims.go.jp/en/"^^xsd:anyURI ;
    nfdicore:url <https://weldcct.nims.go.jp/en/> .

<http://demo.fiz-karlsruhe.de/matwerk/E366086> a nfdicore:Website ;
    rdfs:label "https://www.ccdc.cam.ac.uk/solutions/csd-core/components/csd/"^^xsd:anyURI ;
    nfdicore:url <https://www.ccdc.cam.ac.uk/solutions/csd-core/components/csd/> .

<http://demo.fiz-karlsruhe.de/matwerk/E366941> a nfdicore:Website ;
    rdfs:label "https://icsd.fiz-karlsruhe.de/index.xhtml"^^xsd:anyURI ;
    nfdicore:url <https://icsd.fiz-karlsruhe.de/index.xhtml> .

<http://demo.fiz-karlsruhe.de/matwerk/E36779> a nfdicore:AcademicDiscipline ;
    rdfs:label "Semantic web" ;
    owl:sameAs <http://www.wikidata.org/entity/Q54837> .

<http://demo.fiz-karlsruhe.de/matwerk/E367797> a nfdicore:Website ;
    rdfs:label "https://www.iochem-bd.org/"^^xsd:anyURI ;
    nfdicore:url <https://www.iochem-bd.org/> .

<http://demo.fiz-karlsruhe.de/matwerk/E368654> a nfdicore:Website ;
    rdfs:label "https://cmr.fysik.dtu.dk/#"^^xsd:anyURI ;
    nfdicore:url <https://cmr.fysik.dtu.dk/#> .

<http://demo.fiz-karlsruhe.de/matwerk/E369512> a nfdicore:Website ;
    rdfs:label "http://gurka.fysik.uu.se/ESP/"^^xsd:anyURI ;
    nfdicore:url <http://gurka.fysik.uu.se/ESP/> .

<http://demo.fiz-karlsruhe.de/matwerk/E3702> a nfdicore:Organization ;
    rdfs:label "Dassault Systèmes" .

<http://demo.fiz-karlsruhe.de/matwerk/E370371> a nfdicore:Website ;
    rdfs:label "https://materials.hybrid3.duke.edu/"^^xsd:anyURI ;
    nfdicore:url <https://materials.hybrid3.duke.edu/> .

<http://demo.fiz-karlsruhe.de/matwerk/E37047> a nfdicore:AcademicDiscipline ;
    rdfs:label "knowledge engineering" ;
    owl:sameAs <http://www.wikidata.org/entity/Q1540472> .

<http://demo.fiz-karlsruhe.de/matwerk/E371231> a nfdicore:Website ;
    rdfs:label "https://khazana.gatech.edu/"^^xsd:anyURI ;
    nfdicore:url <https://khazana.gatech.edu/> .

<http://demo.fiz-karlsruhe.de/matwerk/E372092> a nfdicore:Website ;
    rdfs:label "https://www.polymergenome.org/"^^xsd:anyURI ;
    nfdicore:url <https://www.polymergenome.org/> .

<http://demo.fiz-karlsruhe.de/matwerk/E372954> a nfdicore:Website ;
    rdfs:label "https://materialsdatafacility.org/"^^xsd:anyURI ;
    nfdicore:url <https://materialsdatafacility.org/> .

<http://demo.fiz-karlsruhe.de/matwerk/E37316> a nfdicore:AcademicDiscipline ;
    rdfs:label "semantic interoperability" ;
    owl:sameAs <http://www.wikidata.org/entity/Q5258530> .

<http://demo.fiz-karlsruhe.de/matwerk/E373817> a nfdicore:Website ;
    rdfs:label "http://mpod.cimav.edu.mx/"^^xsd:anyURI ;
    nfdicore:url <http://mpod.cimav.edu.mx/> .

<http://demo.fiz-karlsruhe.de/matwerk/E374681> a nfdicore:Website ;
    rdfs:label "https://nanohub.org/"^^xsd:anyURI ;
    nfdicore:url <https://nanohub.org/> .

<http://demo.fiz-karlsruhe.de/matwerk/E375546> a nfdicore:Website ;
    rdfs:label "https://materials.nrel.gov/"^^xsd:anyURI ;
    nfdicore:url <https://materials.nrel.gov/> .

<http://demo.fiz-karlsruhe.de/matwerk/E37586> a nfdicore:AcademicDiscipline ;
    rdfs:label "ontology matching" ;
    owl:sameAs <http://www.wikidata.org/entity/Q4339878> .

<http://demo.fiz-karlsruhe.de/matwerk/E376412> a nfdicore:Website ;
    rdfs:label "https://omdb.mathub.io/"^^xsd:anyURI ;
    nfdicore:url <https://omdb.mathub.io/> .

<http://demo.fiz-karlsruhe.de/matwerk/E377279> a nfdicore:Website ;
    rdfs:label "http://phonondb.mtl.kyoto-u.ac.jp/"^^xsd:anyURI ;
    nfdicore:url <http://phonondb.mtl.kyoto-u.ac.jp/> .

<http://demo.fiz-karlsruhe.de/matwerk/E3776> a nfdicore:Organization ;
    rdfs:label "LBNL" .

<http://demo.fiz-karlsruhe.de/matwerk/E378147> a nfdicore:Website ;
    rdfs:label "https://solsa.crystallography.net/rod/"^^xsd:anyURI ;
    nfdicore:url <https://solsa.crystallography.net/rod/> .

<http://demo.fiz-karlsruhe.de/matwerk/E379016> a nfdicore:Website ;
    rdfs:label "https://www.topologicalquantumchemistry.org/#/"^^xsd:anyURI ;
    nfdicore:url <https://www.topologicalquantumchemistry.org/#/> .

<http://demo.fiz-karlsruhe.de/matwerk/E379886> a nfdicore:Website ;
    rdfs:label "http://www.carolinamatdb.org/"^^xsd:anyURI ;
    nfdicore:url <http://www.carolinamatdb.org/> .

<http://demo.fiz-karlsruhe.de/matwerk/E380757> a nfdicore:Website ;
    rdfs:label "https://cascadesdb.org/"^^xsd:anyURI ;
    nfdicore:url <https://cascadesdb.org/> .

<http://demo.fiz-karlsruhe.de/matwerk/E381629> a nfdicore:Website ;
    rdfs:label "https://www.catalysis-hub.org/energies"^^xsd:anyURI ;
    nfdicore:url <https://www.catalysis-hub.org/energies> .

<http://demo.fiz-karlsruhe.de/matwerk/E382502> a nfdicore:Website ;
    rdfs:label "https://en.iric.imet-db.ru/"^^xsd:anyURI ;
    nfdicore:url <https://en.iric.imet-db.ru/> .

<http://demo.fiz-karlsruhe.de/matwerk/E383376> a nfdicore:Website ;
    rdfs:label "https://rxp.datamanager.kit.edu/"^^xsd:anyURI ;
    nfdicore:url <https://rxp.datamanager.kit.edu/> .

<http://demo.fiz-karlsruhe.de/matwerk/E384251> a nfdicore:Website ;
    rdfs:label "https://materialscommons.org/"^^xsd:anyURI ;
    nfdicore:url <https://materialscommons.org/> .

<http://demo.fiz-karlsruhe.de/matwerk/E3851> a nfdicore:Organization ;
    rdfs:label "Turbomole GmbH" .

<http://demo.fiz-karlsruhe.de/matwerk/E385127> a nfdicore:Website ;
    rdfs:label "https://trc.nist.gov/ThermoML/"^^xsd:anyURI ;
    nfdicore:url <https://trc.nist.gov/ThermoML/> .

<http://demo.fiz-karlsruhe.de/matwerk/E386004> a nfdicore:Website ;
    rdfs:label "http://www.physics.rutgers.edu/gbrv/"^^xsd:anyURI ;
    nfdicore:url <http://www.physics.rutgers.edu/gbrv/> .

<http://demo.fiz-karlsruhe.de/matwerk/E38676> a nfdicore:AcademicDiscipline ;
    rdfs:label "Computational Chemistry" ;
    owl:sameAs <http://www.wikidata.org/entity/Q369472> .

<http://demo.fiz-karlsruhe.de/matwerk/E387761> a mwo:Repository ;
    rdfs:label "https://github.com/CenterForOpenScience/"^^xsd:anyURI ;
    nfdicore:url <https://github.com/CenterForOpenScience/> .

<http://demo.fiz-karlsruhe.de/matwerk/E388641> a mwo:Repository ;
    rdfs:label "https://github.com/Atomistica/atomistica"^^xsd:anyURI ;
    nfdicore:url <https://github.com/Atomistica/atomistica> .

<http://demo.fiz-karlsruhe.de/matwerk/E389522> a mwo:Repository ;
    rdfs:label "https://github.com/materialsproject"^^xsd:anyURI ;
    nfdicore:url <https://github.com/materialsproject> .

<http://demo.fiz-karlsruhe.de/matwerk/E390404> a mwo:Repository ;
    rdfs:label "https://github.com/materialscloud-org"^^xsd:anyURI ;
    nfdicore:url <https://github.com/materialscloud-org> .

<http://demo.fiz-karlsruhe.de/matwerk/E391287> a mwo:Repository ;
    rdfs:label "https://gitlab.mpcdf.mpg.de/nomad-lab/nomad-FAIR"^^xsd:anyURI ;
    nfdicore:url <https://gitlab.mpcdf.mpg.de/nomad-lab/nomad-FAIR> .

<http://demo.fiz-karlsruhe.de/matwerk/E392171> a mwo:Repository ;
    rdfs:label "https://github.com/kit-data-manager/Data-Collections-Explorer"^^xsd:anyURI ;
    nfdicore:url <https://github.com/kit-data-manager/Data-Collections-Explorer> .

<http://demo.fiz-karlsruhe.de/matwerk/E393056> a mwo:Repository ;
    rdfs:label "https://github.com/materials-commons/materialscommons.org"^^xsd:anyURI ;
    nfdicore:url <https://github.com/materials-commons/materialscommons.org> .

<http://demo.fiz-karlsruhe.de/matwerk/E393942> a nfdicore:Website ;
    rdfs:label "https://www.mib.uni-stuttgart.de/teaching/course-offerings/dapro/"^^xsd:anyURI ;
    nfdicore:url <https://www.mib.uni-stuttgart.de/teaching/course-offerings/dapro/> .

<http://demo.fiz-karlsruhe.de/matwerk/E394829> a nfdicore:Website ;
    rdfs:label "https://www.mib.uni-stuttgart.de/teaching/course-offerings/dapro-ms/"^^xsd:anyURI ;
    nfdicore:url <https://www.mib.uni-stuttgart.de/teaching/course-offerings/dapro-ms/> .

<http://demo.fiz-karlsruhe.de/matwerk/E395717> a nfdicore:Website ;
    rdfs:label "https://www.youtube.com/c/ISEFIZKarlsruhe/about"^^xsd:anyURI ;
    nfdicore:url <https://www.youtube.com/c/ISEFIZKarlsruhe/about> .

<http://demo.fiz-karlsruhe.de/matwerk/E396606> a nfdicore:Website ;
    rdfs:label "https://open.hpi.de/courses/knowledgegraphs2020?locale=de"^^xsd:anyURI ;
    nfdicore:url <https://open.hpi.de/courses/knowledgegraphs2020?locale=de> .

<http://demo.fiz-karlsruhe.de/matwerk/E397496> a nfdicore:Website ;
    rdfs:label "https://open.hpi.de/courses/semanticweb2017"^^xsd:anyURI ;
    nfdicore:url <https://open.hpi.de/courses/semanticweb2017> .

<http://demo.fiz-karlsruhe.de/matwerk/E39782> a nfdicore:AcademicDiscipline ;
    rdfs:label "Atomistic modelling of light elements in steel" .

<http://demo.fiz-karlsruhe.de/matwerk/E398387> a nfdicore:Website ;
    rdfs:label "https://open.hpi.de/courses/semanticweb2016?locale=de"^^xsd:anyURI ;
    nfdicore:url <https://open.hpi.de/courses/semanticweb2016?locale=de> .

<http://demo.fiz-karlsruhe.de/matwerk/E399279> a nfdicore:Website ;
    rdfs:label "https://open.hpi.de/courses/semweb2015?locale=de"^^xsd:anyURI ;
    nfdicore:url <https://open.hpi.de/courses/semweb2015?locale=de> .

<http://demo.fiz-karlsruhe.de/matwerk/E400172> a nfdicore:Website ;
    rdfs:label "https://open.hpi.de/courses/semanticweb?locale=de"^^xsd:anyURI ;
    nfdicore:url <https://open.hpi.de/courses/semanticweb?locale=de> .

<http://demo.fiz-karlsruhe.de/matwerk/E40061> a nfdicore:AcademicDiscipline ;
    rdfs:label "Large-scale atomistic simulations" .

<http://demo.fiz-karlsruhe.de/matwerk/E401066> a nfdicore:Website ;
    rdfs:label "https://www.youtube.com/c/pyironIDE"^^xsd:anyURI ;
    nfdicore:url <https://www.youtube.com/c/pyironIDE> .

<http://demo.fiz-karlsruhe.de/matwerk/E401961> a nfdicore:Website ;
    rdfs:label "https://www.youtube.com/c/MaterialsCloud/"^^xsd:anyURI ;
    nfdicore:url <https://www.youtube.com/c/MaterialsCloud/> .

<http://demo.fiz-karlsruhe.de/matwerk/E402857> a nfdicore:Website ;
    rdfs:label "http://pyiron.org/potentials-workshop-2022/intro.html"^^xsd:anyURI ;
    nfdicore:url <http://pyiron.org/potentials-workshop-2022/intro.html> .

<http://demo.fiz-karlsruhe.de/matwerk/E40341> a nfdicore:AcademicDiscipline ;
    rdfs:label "Analytic bond-order potentials" .

<http://demo.fiz-karlsruhe.de/matwerk/E403754> a nfdicore:Website ;
    rdfs:label "https://pyiron.org/phasediagram-workshop-2020/Introduction.html"^^xsd:anyURI ;
    nfdicore:url <https://pyiron.org/phasediagram-workshop-2020/Introduction.html> .

<http://demo.fiz-karlsruhe.de/matwerk/E404652> a nfdicore:Website ;
    rdfs:label "https://pyiron.org/potentials-workshop-2021/README.html"^^xsd:anyURI ;
    nfdicore:url <https://pyiron.org/potentials-workshop-2021/README.html> .

<http://demo.fiz-karlsruhe.de/matwerk/E405551> a nfdicore:Website ;
    rdfs:label "http://pyiron.org/swimm-workshop-2021/README.html"^^xsd:anyURI ;
    nfdicore:url <http://pyiron.org/swimm-workshop-2021/README.html> .

<http://demo.fiz-karlsruhe.de/matwerk/E40622> a nfdicore:AcademicDiscipline ;
    rdfs:label "Materials Engineering" ;
    owl:sameAs <http://www.wikidata.org/entity/Q1710723> .

<http://demo.fiz-karlsruhe.de/matwerk/E407352> a nfdicore:Website ;
    rdfs:label "https://github.com/ISE-FIZKarlsruhe/ISE-teaching"^^xsd:anyURI ;
    nfdicore:url <https://github.com/ISE-FIZKarlsruhe/ISE-teaching> .

<http://demo.fiz-karlsruhe.de/matwerk/E408254> a nfdicore:Website ;
    rdfs:label "https://github.com/pyiron/potentials-workshop-2022"^^xsd:anyURI ;
    nfdicore:url <https://github.com/pyiron/potentials-workshop-2022> .

<http://demo.fiz-karlsruhe.de/matwerk/E40904> a nfdicore:AcademicDiscipline ;
    rdfs:label "Ab initio (parameter free) scale-bridging computer simulations" .

<http://demo.fiz-karlsruhe.de/matwerk/E409157> a nfdicore:Website ;
    rdfs:label "https://github.com/pyiron/phasediagram-workshop-2020"^^xsd:anyURI ;
    nfdicore:url <https://github.com/pyiron/phasediagram-workshop-2020> .

<http://demo.fiz-karlsruhe.de/matwerk/E410061> a nfdicore:Website ;
    rdfs:label "https://github.com/pyiron/potentials-workshop-2021"^^xsd:anyURI ;
    nfdicore:url <https://github.com/pyiron/potentials-workshop-2021> .

<http://demo.fiz-karlsruhe.de/matwerk/E410966> a nfdicore:Website ;
    rdfs:label "https://github.com/pyiron/swimm-workshop-2021"^^xsd:anyURI ;
    nfdicore:url <https://github.com/pyiron/swimm-workshop-2021> .

<http://demo.fiz-karlsruhe.de/matwerk/E41187> a nfdicore:AcademicDiscipline ;
    rdfs:label "Ab initio based thermodynamics and kinetics" .

<http://demo.fiz-karlsruhe.de/matwerk/E41471> a nfdicore:AcademicDiscipline ;
    rdfs:label "Surface and defect physics" .

<http://demo.fiz-karlsruhe.de/matwerk/E41756> a nfdicore:AcademicDiscipline ;
    rdfs:label "Theory on epitaxy and microstructure" .

<http://demo.fiz-karlsruhe.de/matwerk/E419156> a nfdicore:Resource,
        nfdicore:Software,
        mwo:ProcessingSoftware,
        mwo:ResearchSoftware,
        mwo:VisualizationSoftware ;
    rdfs:label "ParaView" ;
    nfdicore:programmingLanguage <http://demo.fiz-karlsruhe.de/matwerk/E828542>,
        <http://demo.fiz-karlsruhe.de/matwerk/E832406>,
        <http://demo.fiz-karlsruhe.de/matwerk/E841457>,
        <http://demo.fiz-karlsruhe.de/matwerk/E844052> ;
    dcterms:description "ParaView is an open-source, multi-platform data analysis and visualization application based on Visualization Toolkit (VTK)."^^xsd:string ;
    mwo:hasContactPoint <http://demo.fiz-karlsruhe.de/matwerk/E689552> ;
    mwo:hasDiscipline <http://demo.fiz-karlsruhe.de/matwerk/E68897>,
        <http://demo.fiz-karlsruhe.de/matwerk/E70007> ;
    mwo:hasDocumentation <http://demo.fiz-karlsruhe.de/matwerk/E244952> ;
    mwo:hasRelatedResource <http://demo.fiz-karlsruhe.de/matwerk/E635502> ;
    mwo:hasRepository <http://demo.fiz-karlsruhe.de/matwerk/E163166> ;
    mwo:hasVersion "5.10.1" ;
    mwo:hasWebsite <http://demo.fiz-karlsruhe.de/matwerk/E93236> ;
    ns3:has_license <http://demo.fiz-karlsruhe.de/matwerk/E744591> ;
    owl:sameAs <http://www.wikidata.org/entity/Q474635> ;
    schema:operatingSystem ns3:SWO_0000020,
        ns3:SWO_0000022,
        ns3:SWO_0000149,
        ns3:SWO_9000072 .

<http://demo.fiz-karlsruhe.de/matwerk/E42329> a nfdicore:AcademicDiscipline ;
    rdfs:label "Lightweight Design with Hybrid Systems" .

<http://demo.fiz-karlsruhe.de/matwerk/E42906> a nfdicore:AcademicDiscipline ;
    rdfs:label "Microstructure-mechanical property relationship for metallic materials" .

<http://demo.fiz-karlsruhe.de/matwerk/E43196> a nfdicore:AcademicDiscipline ;
    rdfs:label "Nanoindentation" ;
    owl:sameAs <http://www.wikidata.org/entity/Q1549892> .

<http://demo.fiz-karlsruhe.de/matwerk/E43487> a nfdicore:AcademicDiscipline ;
    rdfs:label "in-situ mechanical testing" .

<http://demo.fiz-karlsruhe.de/matwerk/E43779> a nfdicore:AcademicDiscipline ;
    rdfs:label "Nanocrystalline materials" .

<http://demo.fiz-karlsruhe.de/matwerk/E44072> a nfdicore:AcademicDiscipline ;
    rdfs:label "High temperature alloys" .

<http://demo.fiz-karlsruhe.de/matwerk/E44366> a nfdicore:AcademicDiscipline ;
    rdfs:label "Carbon coatings and thin films" .

<http://demo.fiz-karlsruhe.de/matwerk/E44661> a nfdicore:AcademicDiscipline ;
    rdfs:label "Scale bridging in mechanical properties" .

<http://demo.fiz-karlsruhe.de/matwerk/E44957> a nfdicore:AcademicDiscipline ;
    rdfs:label "Deformation and damage mechanisms" .

<http://demo.fiz-karlsruhe.de/matwerk/E45254> a nfdicore:AcademicDiscipline ;
    rdfs:label "Discrete element simulations" .

<http://demo.fiz-karlsruhe.de/matwerk/E45552> a nfdicore:AcademicDiscipline ;
    rdfs:label "data-driven methods" .

<http://demo.fiz-karlsruhe.de/matwerk/E45851> a nfdicore:AcademicDiscipline ;
    rdfs:label "Characterization of dislocation structures and plasticity with multiscale methods" .

<http://demo.fiz-karlsruhe.de/matwerk/E46151> a nfdicore:AcademicDiscipline ;
    rdfs:label "Biomimetics and Biomechanics" .

<http://demo.fiz-karlsruhe.de/matwerk/E46452> a nfdicore:AcademicDiscipline ;
    rdfs:label "Plant evolution" ;
    owl:sameAs <http://www.wikidata.org/entity/Q7201511> .

<http://demo.fiz-karlsruhe.de/matwerk/E46754> a nfdicore:AcademicDiscipline ;
    rdfs:label "Plant movement" .

<http://demo.fiz-karlsruhe.de/matwerk/E47057> a nfdicore:AcademicDiscipline ;
    rdfs:label "Chemistry & Physics of Interfaces" .

<http://demo.fiz-karlsruhe.de/matwerk/E47361> a nfdicore:AcademicDiscipline ;
    rdfs:label "Homogenization of elastic" .

<http://demo.fiz-karlsruhe.de/matwerk/E47666> a nfdicore:AcademicDiscipline ;
    rdfs:label "brittle-elastic and visco-plastic material properties" .

<http://demo.fiz-karlsruhe.de/matwerk/E47972> a nfdicore:AcademicDiscipline ;
    rdfs:label "Mathematical description of microstructures" .

<http://demo.fiz-karlsruhe.de/matwerk/E48279> a nfdicore:AcademicDiscipline ;
    rdfs:label "Localization and failure mechanisms" .

<http://demo.fiz-karlsruhe.de/matwerk/E48587> a nfdicore:AcademicDiscipline ;
    rdfs:label "Continuum mechanical modeling" ;
    owl:sameAs <http://www.wikidata.org/entity/Q193463> .

<http://demo.fiz-karlsruhe.de/matwerk/E50142> a nfdicore:AcademicDiscipline ;
    rdfs:label "Materials Mechanics" .

<http://demo.fiz-karlsruhe.de/matwerk/E50456> a nfdicore:AcademicDiscipline ;
    rdfs:label "Additive manufacturing" .

<http://demo.fiz-karlsruhe.de/matwerk/E50771> a nfdicore:AcademicDiscipline ;
    rdfs:label "metallic materials" .

<http://demo.fiz-karlsruhe.de/matwerk/E51087> a nfdicore:AcademicDiscipline ;
    rdfs:label "mechanical material testing" .

<http://demo.fiz-karlsruhe.de/matwerk/E511556> a nfdicore:Software,
        ns3:SWO_0000001 ;
    rdfs:label "pacemaker" ;
    dcterms:description "a tool for fitting of interatomic potentials in a general nonlinear Atomic Cluster Expansion (ACE) form. "^^xsd:string ;
    mwo:hasDocumentation <http://demo.fiz-karlsruhe.de/matwerk/E275912> ;
    mwo:hasRepository <http://demo.fiz-karlsruhe.de/matwerk/E204842> ;
    mwo:hasVersion "0.2.7" ;
    ns3:has_license <http://demo.fiz-karlsruhe.de/matwerk/E795431> ;
    schema:citation <http://demo.fiz-karlsruhe.de/matwerk/E945626> .

<http://demo.fiz-karlsruhe.de/matwerk/E51404> a nfdicore:AcademicDiscipline ;
    rdfs:label "Interactive visual data exploration" .

<http://demo.fiz-karlsruhe.de/matwerk/E51722> a nfdicore:AcademicDiscipline ;
    rdfs:label "Topological data analysis" .

<http://demo.fiz-karlsruhe.de/matwerk/E52041> a nfdicore:AcademicDiscipline ;
    rdfs:label "Machine learning in visualization" .

<http://demo.fiz-karlsruhe.de/matwerk/E52361> a nfdicore:AcademicDiscipline ;
    rdfs:label "Heat treatment" .

<http://demo.fiz-karlsruhe.de/matwerk/E52682> a nfdicore:AcademicDiscipline ;
    rdfs:label "Mechanics of Materials" .

<http://demo.fiz-karlsruhe.de/matwerk/E543362> a nfdicore:Resource,
        nfdicore:Software ;
    rdfs:label "colabfit-tools" ;
    mwo:hasDocumentation <http://demo.fiz-karlsruhe.de/matwerk/E282626> ;
    mwo:hasWebsite <http://demo.fiz-karlsruhe.de/matwerk/E141186> .

<http://demo.fiz-karlsruhe.de/matwerk/E54629> a nfdicore:AcademicDiscipline ;
    rdfs:label "mechanics of materials" .

<http://demo.fiz-karlsruhe.de/matwerk/E546491> a nfdicore:Resource,
        nfdicore:Software ;
    rdfs:label "qmpy" ;
    mwo:hasDocumentation <http://demo.fiz-karlsruhe.de/matwerk/E283377> ;
    mwo:hasRelatedResource <http://demo.fiz-karlsruhe.de/matwerk/E644546> ;
    mwo:hasRepository <http://demo.fiz-karlsruhe.de/matwerk/E215186> .

<http://demo.fiz-karlsruhe.de/matwerk/E56946> a nfdicore:AcademicDiscipline,
        mwo:LargeScaleFacility ;
    rdfs:label "High Performance Computing" ;
    nfdicore:location <http://demo.fiz-karlsruhe.de/matwerk/E73011>,
        <http://demo.fiz-karlsruhe.de/matwerk/E80004> ;
    mwo:belongsTo <http://demo.fiz-karlsruhe.de/matwerk/E2486> ;
    mwo:description "The University Computing Centre at Kiel University provides employees and faculties powerful resources for scientific computing. In addtiton it advises scientists in the scopes of system usage, parallelization, vectorization and optimization of scientific software and programs. The systems available for members of Kiel University are (1) Linux clusters (name “caucluster”) (2) the \"nesh\" cluster, a hybrid NEC HPC system, containing a Linux cluster, GPU and vector subsystem (NEC SX-Aurora TSUBASA) and (3) the HLRN Supercomputing System (via the North-German Supercomputing Alliance)." ;
    mwo:hasAcronym "HPC"^^xsd:string ;
    mwo:hasWebsite <http://demo.fiz-karlsruhe.de/matwerk/E298607> ;
    rdfs:comment "The CRC 1261 performs simulations on the “nesh” cluster." .

<http://demo.fiz-karlsruhe.de/matwerk/E57954> a nfdicore:AcademicDiscipline ;
    rdfs:label "high-performance graphics hardware and software" .

<http://demo.fiz-karlsruhe.de/matwerk/E592329> a nfdicore:Resource,
        nfdicore:Software ;
    rdfs:label "MatD3" ;
    mwo:hasRelatedResource <http://demo.fiz-karlsruhe.de/matwerk/E645681> ;
    mwo:hasWebsite <http://demo.fiz-karlsruhe.de/matwerk/E156404> .

<http://demo.fiz-karlsruhe.de/matwerk/E59997> a nfdicore:AcademicDiscipline ;
    rdfs:label "Materials Characterization and Testing" .

<http://demo.fiz-karlsruhe.de/matwerk/E60341> a nfdicore:AcademicDiscipline ;
    rdfs:label "Engineering" ;
    owl:sameAs <http://www.wikidata.org/entity/Q110262600> .

<http://demo.fiz-karlsruhe.de/matwerk/E609857> a mwo:Method ;
    rdfs:label "Machine learning" .

<http://demo.fiz-karlsruhe.de/matwerk/E612066> a mwo:Method ;
    rdfs:label "X-ray imaging" .

<http://demo.fiz-karlsruhe.de/matwerk/E614279> a mwo:Method ;
    rdfs:label "tight-binding" .

<http://demo.fiz-karlsruhe.de/matwerk/E6152> a nfdicore:Organization ;
    rdfs:label "University of Freiburg, Fraunhofer IWM" .

<http://demo.fiz-karlsruhe.de/matwerk/E615387> a mwo:Method ;
    rdfs:label "QM/MM" .

<http://demo.fiz-karlsruhe.de/matwerk/E617606> a mwo:Method ;
    rdfs:label "metadynamics" .

<http://demo.fiz-karlsruhe.de/matwerk/E618717> a mwo:Method ;
    rdfs:label "Monte Carlo" .

<http://demo.fiz-karlsruhe.de/matwerk/E619829> a mwo:Method ;
    rdfs:label "nudged elastic band" .

<http://demo.fiz-karlsruhe.de/matwerk/E62076> a nfdicore:AcademicDiscipline ;
    rdfs:label "machine learning; multiscale modelling" .

<http://demo.fiz-karlsruhe.de/matwerk/E620942> a mwo:Method ;
    rdfs:label "Phase-field" .

<http://demo.fiz-karlsruhe.de/matwerk/E623171> a mwo:Method ;
    rdfs:label "DFT" .

<http://demo.fiz-karlsruhe.de/matwerk/E624287> a mwo:Method ;
    rdfs:label "Coupled-Cluster" .

<http://demo.fiz-karlsruhe.de/matwerk/E6254> a nfdicore:Organization ;
    rdfs:label "University of the Basque country" .

<http://demo.fiz-karlsruhe.de/matwerk/E626522> a nfdicore:Resource ;
    rdfs:label "Calphy uses LAMMPS" .

<http://demo.fiz-karlsruhe.de/matwerk/E627641> a nfdicore:Resource ;
    rdfs:label "pylammpsmpi" .

<http://demo.fiz-karlsruhe.de/matwerk/E62777> a nfdicore:AcademicDiscipline ;
    rdfs:label "X-ray microscopy" .

<http://demo.fiz-karlsruhe.de/matwerk/E628761> a nfdicore:Resource ;
    rdfs:label "pyscal" .

<http://demo.fiz-karlsruhe.de/matwerk/E629882> a nfdicore:Resource ;
    rdfs:label "Mendeleev" .

<http://demo.fiz-karlsruhe.de/matwerk/E631004> a nfdicore:Resource ;
    rdfs:label "Pyscal uses ASE" .

<http://demo.fiz-karlsruhe.de/matwerk/E632127> a nfdicore:Resource ;
    rdfs:label "h5py" .

<http://demo.fiz-karlsruhe.de/matwerk/E633251> a nfdicore:Resource ;
    rdfs:label "pybind11" .

<http://demo.fiz-karlsruhe.de/matwerk/E634376> a nfdicore:Resource ;
    rdfs:label "(optionally) LAMMPS" .

<http://demo.fiz-karlsruhe.de/matwerk/E635502> a nfdicore:Resource ;
    rdfs:label "VTK" .

<http://demo.fiz-karlsruhe.de/matwerk/E6357> a nfdicore:Organization ;
    rdfs:label "University of Cambridge" .

<http://demo.fiz-karlsruhe.de/matwerk/E638886> a nfdicore:Resource ;
    rdfs:label "Nextmol" .

<http://demo.fiz-karlsruhe.de/matwerk/E64191> a nfdicore:AcademicDiscipline ;
    rdfs:label "bond order potentials (BOP)" .

<http://demo.fiz-karlsruhe.de/matwerk/E642279> a nfdicore:Resource ;
    rdfs:label "Fireworks" .

<http://demo.fiz-karlsruhe.de/matwerk/E643412> a nfdicore:DataPortal,
        nfdicore:Resource ;
    rdfs:label "Open Materials Database" ;
    mwo:conformsToSpecification <http://demo.fiz-karlsruhe.de/matwerk/E1125251> ;
    mwo:description "The Open Materials Database is a publicly available, searchable database for information on the properties of materials created by people who work in computational materials design research. " ;
    mwo:hasContactPoint <http://demo.fiz-karlsruhe.de/matwerk/E727616> ;
    mwo:hasRelatedResource <http://demo.fiz-karlsruhe.de/matwerk/E660527> ;
    mwo:hasWebsite <http://demo.fiz-karlsruhe.de/matwerk/E354221> .

<http://demo.fiz-karlsruhe.de/matwerk/E644546> a nfdicore:Resource ;
    rdfs:label "oqmd" .

<http://demo.fiz-karlsruhe.de/matwerk/E64547> a nfdicore:AcademicDiscipline ;
    rdfs:label "Focused Ion Beam (FIB)" .

<http://demo.fiz-karlsruhe.de/matwerk/E645681> a nfdicore:Resource ;
    rdfs:label "HybridD3" .

<http://demo.fiz-karlsruhe.de/matwerk/E6461> a nfdicore:Organization ;
    rdfs:label "EPFL, Swiss National Supercomputing Center (CSCS)" .

<http://demo.fiz-karlsruhe.de/matwerk/E646817> a nfdicore:Resource ;
    rdfs:label "RO-Crate 1.1 specification" .

<http://demo.fiz-karlsruhe.de/matwerk/E647954> a nfdicore:Resource ;
    rdfs:label "Qbox" .

<http://demo.fiz-karlsruhe.de/matwerk/E649092> a nfdicore:Resource ;
    rdfs:label "Atomic Simulation Environment (ASE)" .

<http://demo.fiz-karlsruhe.de/matwerk/E650231> a nfdicore:Resource ;
    rdfs:label "Large-scale Atomic/Molecular Massively Parallel Simulator (LAMMPS)" .

<http://demo.fiz-karlsruhe.de/matwerk/E651371> a nfdicore:Resource ;
    rdfs:label "VASP" .

<http://demo.fiz-karlsruhe.de/matwerk/E653654> a nfdicore:Resource ;
    rdfs:label "fireworks" .

<http://demo.fiz-karlsruhe.de/matwerk/E654797> a nfdicore:Resource,
        nfdicore:Software ;
    rdfs:label "custodian" ;
    mwo:hasWebsite <http://demo.fiz-karlsruhe.de/matwerk/E139076> .

<http://demo.fiz-karlsruhe.de/matwerk/E655941> a nfdicore:Resource,
        nfdicore:Software ;
    rdfs:label "atomate" ;
    nfdicore:programmingLanguage <http://demo.fiz-karlsruhe.de/matwerk/E836279> ;
    mwo:hasContributor <http://demo.fiz-karlsruhe.de/matwerk/E3776> ;
    mwo:hasRelatedResource <http://demo.fiz-karlsruhe.de/matwerk/E642279> ;
    mwo:hasWebsite <http://demo.fiz-karlsruhe.de/matwerk/E138027> .

<http://demo.fiz-karlsruhe.de/matwerk/E65621> a nfdicore:AcademicDiscipline ;
    rdfs:label "Scanning Electron Microscopy (SEM)" .

<http://demo.fiz-karlsruhe.de/matwerk/E6566> a nfdicore:Organization ;
    rdfs:label "Humboldt-Universität zu Berlin, Max Planck Computing and Data Facility (MPCDF), Fritz-Haber-Institut der Max-Planck-Gesellschaft" .

<http://demo.fiz-karlsruhe.de/matwerk/E657086> a nfdicore:Resource ;
    rdfs:label "AiiDA" .

<http://demo.fiz-karlsruhe.de/matwerk/E658232> a nfdicore:Resource,
        nfdicore:Software,
        mwo:ResearchSoftware ;
    rdfs:label "Quantum Espresso" ;
    dcterms:description "Quantum ESPRESSO Is an integrated suite of Open-Source computer codes for electronic-structure calculations and materials modeling at the nanoscale. It is based on density-functional theory, plane waves, and pseudopotentials."^^xsd:string ;
    mwo:hasContactPoint <http://demo.fiz-karlsruhe.de/matwerk/E693077> ;
    mwo:hasDiscipline <http://demo.fiz-karlsruhe.de/matwerk/E67431> ;
    mwo:hasDocumentation <http://demo.fiz-karlsruhe.de/matwerk/E249161> ;
    mwo:hasRepository <http://demo.fiz-karlsruhe.de/matwerk/E167177> ;
    mwo:hasVersion "7.1" ;
    mwo:hasWebsite <http://demo.fiz-karlsruhe.de/matwerk/E98462> ;
    mwo:usesMethod <http://demo.fiz-karlsruhe.de/matwerk/E613172> ;
    ns3:has_license <http://demo.fiz-karlsruhe.de/matwerk/E755607> ;
    schema:citation <http://demo.fiz-karlsruhe.de/matwerk/E895454> ;
    schema:operatingSystem ns3:SWO_0000022,
        ns3:SWO_0000149 .

<http://demo.fiz-karlsruhe.de/matwerk/E660527> a nfdicore:Resource ;
    rdfs:label "httk" .

<http://demo.fiz-karlsruhe.de/matwerk/E661676> a nfdicore:Resource ;
    rdfs:label "atomwork" .

<http://demo.fiz-karlsruhe.de/matwerk/E662826> a nfdicore:Resource ;
    rdfs:label "vasp" .

<http://demo.fiz-karlsruhe.de/matwerk/E663977> a nfdicore:Resource ;
    rdfs:label "Bilbao Crystallographic server" .

<http://demo.fiz-karlsruhe.de/matwerk/E6672> a nfdicore:Organization ;
    rdfs:label "Fraunhofer, BAM" .

<http://demo.fiz-karlsruhe.de/matwerk/E67796> a nfdicore:AcademicDiscipline ;
    rdfs:label "hyperelastic materials" .

<http://demo.fiz-karlsruhe.de/matwerk/E68162> a nfdicore:AcademicDiscipline ;
    rdfs:label "heat conductivity" .

<http://demo.fiz-karlsruhe.de/matwerk/E683698> a mwo:ContactPoint ;
    rdfs:label "openbis-support@id.ethz.ch" ;
    mwo:emailAddress "openbis-support@id.ethz.ch"^^xsd:string .

<http://demo.fiz-karlsruhe.de/matwerk/E688379> a mwo:ContactPoint ;
    rdfs:label "feap@berkeley.edu" ;
    mwo:emailAddress "feap@berkeley.edu"^^xsd:string .

<http://demo.fiz-karlsruhe.de/matwerk/E6887> a nfdicore:Organization ;
    rdfs:label "Cambridge Crystallographic Data Centre (CCDC)" .

<http://demo.fiz-karlsruhe.de/matwerk/E690726> a mwo:ContactPoint ;
    rdfs:label "support@vasp.at" ;
    mwo:emailAddress "support@vasp.at"^^xsd:string .

<http://demo.fiz-karlsruhe.de/matwerk/E691901> a mwo:ContactPoint ;
    rdfs:label "info@abinit.org" ;
    mwo:emailAddress "info@abinit.org"^^xsd:string .

<http://demo.fiz-karlsruhe.de/matwerk/E693077> a mwo:ContactPoint ;
    rdfs:label "info@quantum-espresso.org" ;
    mwo:emailAddress "info@quantum-espresso.org"^^xsd:string .

<http://demo.fiz-karlsruhe.de/matwerk/E695432> a mwo:ContactPoint ;
    rdfs:label "demon2k-l@mailman.ucalgary.ca" ;
    mwo:emailAddress "demon2k-l@mailman.ucalgary.ca"^^xsd:string .

<http://demo.fiz-karlsruhe.de/matwerk/E69636> a nfdicore:AcademicDiscipline ;
    rdfs:label "measurement processing" .

<http://demo.fiz-karlsruhe.de/matwerk/E696611> a mwo:ContactPoint ;
    rdfs:label "aims-coordinators@fhi-berlin.mpg.de" ;
    mwo:emailAddress "aims-coordinators@fhi-berlin.mpg.de"^^xsd:string .

<http://demo.fiz-karlsruhe.de/matwerk/E6996> a nfdicore:Organization ;
    rdfs:label "FIZ Karlsruhe" .

<http://demo.fiz-karlsruhe.de/matwerk/E700154> a mwo:ContactPoint ;
    rdfs:label "imd@itap.physik.uni-stuttgart.de" ;
    mwo:emailAddress "imd@itap.physik.uni-stuttgart.de"^^xsd:string .

<http://demo.fiz-karlsruhe.de/matwerk/E701337> a mwo:ContactPoint ;
    rdfs:label "damask@mpie.de" ;
    mwo:emailAddress "damask@mpie.de"^^xsd:string .

<http://demo.fiz-karlsruhe.de/matwerk/E704892> a mwo:ContactPoint ;
    rdfs:label "aixvipmap@icme.rwth-aachen.de" ;
    mwo:emailAddress "aixvipmap@icme.rwth-aachen.de"^^xsd:string .

<http://demo.fiz-karlsruhe.de/matwerk/E70752> a nfdicore:AcademicDiscipline ;
    rdfs:label "Quantum Chemistry" .

<http://demo.fiz-karlsruhe.de/matwerk/E708456> a mwo:ContactPoint ;
    rdfs:label "qhull@qhull.org" ;
    mwo:emailAddress "qhull@qhull.org"^^xsd:string .

<http://demo.fiz-karlsruhe.de/matwerk/E7106> a nfdicore:Organization ;
    rdfs:label "Marvel NCCR" .

<http://demo.fiz-karlsruhe.de/matwerk/E7107> a nfdicore:Organization ;
    rdfs:label "MAX (MAterials design at the eXascale)" .

<http://demo.fiz-karlsruhe.de/matwerk/E710837> a mwo:ContactPoint ;
    rdfs:label "ibc@hzdr.de" ;
    mwo:emailAddress "ibc@hzdr.de"^^xsd:string ;
    mwo:hasWebsite <http://demo.fiz-karlsruhe.de/matwerk/E1229529> .

<http://demo.fiz-karlsruhe.de/matwerk/E71126> a nfdicore:AcademicDiscipline ;
    rdfs:label "Computational Material Science" ;
    owl:sameAs <http://www.wikidata.org/entity/Q85753722> .

<http://demo.fiz-karlsruhe.de/matwerk/E712029> a mwo:ContactPoint ;
    rdfs:label "emmo@emmc.eu" ;
    mwo:emailAddress "emmo@emmc.eu"^^xsd:string .

<http://demo.fiz-karlsruhe.de/matwerk/E71501> a nfdicore:AcademicDiscipline ;
    rdfs:label "Excited States" .

<http://demo.fiz-karlsruhe.de/matwerk/E715611> a mwo:ContactPoint ;
    rdfs:label "Contact@Osf.Io" ;
    mwo:emailAddress "Contact@Osf.Io"^^xsd:string .

<http://demo.fiz-karlsruhe.de/matwerk/E716807> a mwo:ContactPoint ;
    rdfs:label "info@figshare.com" ;
    mwo:emailAddress "info@figshare.com"^^xsd:string .

<http://demo.fiz-karlsruhe.de/matwerk/E718004> a mwo:ContactPoint ;
    rdfs:label "potentials@nist.gov" ;
    mwo:emailAddress "potentials@nist.gov"^^xsd:string .

<http://demo.fiz-karlsruhe.de/matwerk/E720401> a mwo:ContactPoint ;
    rdfs:label "info@ncbi.nlm.nih.gov" ;
    mwo:emailAddress "info@ncbi.nlm.nih.gov"^^xsd:string .

<http://demo.fiz-karlsruhe.de/matwerk/E721601> a mwo:ContactPoint ;
    rdfs:label "administrador.bcs@ehu.eus" ;
    mwo:emailAddress "administrador.bcs@ehu.eus"^^xsd:string .

<http://demo.fiz-karlsruhe.de/matwerk/E724004> a mwo:ContactPoint ;
    rdfs:label "info@materialscloud.org" ;
    mwo:emailAddress "info@materialscloud.org"^^xsd:string .

<http://demo.fiz-karlsruhe.de/matwerk/E725207> a mwo:ContactPoint ;
    rdfs:label "support@nomad-lab.eu" ;
    mwo:emailAddress "support@nomad-lab.eu"^^xsd:string .

<http://demo.fiz-karlsruhe.de/matwerk/E726411> a mwo:ContactPoint ;
    rdfs:label "yury.lysogorskiy@rub.de" ;
    mwo:emailAddress "yury.lysogorskiy@rub.de"^^xsd:string .

<http://demo.fiz-karlsruhe.de/matwerk/E727616> a mwo:ContactPoint ;
    rdfs:label "contactopenmaterialsdb.se" ;
    mwo:emailAddress "contactopenmaterialsdb.se"^^xsd:string .

<http://demo.fiz-karlsruhe.de/matwerk/E728822> a mwo:ContactPoint ;
    rdfs:label "oqmd.questions@gmail.com" ;
    mwo:emailAddress "oqmd.questions@gmail.com"^^xsd:string .

<http://demo.fiz-karlsruhe.de/matwerk/E730029> a mwo:ContactPoint ;
    rdfs:label "info@matdat.com" ;
    mwo:emailAddress "info@matdat.com"^^xsd:string .

<http://demo.fiz-karlsruhe.de/matwerk/E731237> a mwo:ContactPoint ;
    rdfs:label "hybrid3project@duke.edu" ;
    mwo:emailAddress "hybrid3project@duke.edu"^^xsd:string .

<http://demo.fiz-karlsruhe.de/matwerk/E732446> a mwo:ContactPoint ;
    rdfs:label "materialsdatafacility@uchicago.edu" ;
    mwo:emailAddress "materialsdatafacility@uchicago.edu"^^xsd:string ;
    mwo:hasWebsite <http://demo.fiz-karlsruhe.de/matwerk/E334337> .

<http://demo.fiz-karlsruhe.de/matwerk/E734867> a mwo:ContactPoint ;
    rdfs:label "administrator@topologicalquantumchemistry.org" ;
    mwo:emailAddress "administrator@topologicalquantumchemistry.org"^^xsd:string .

<http://demo.fiz-karlsruhe.de/matwerk/E738506> a ns3:SWO_0000002 ;
    rdfs:label "ASL/ BSD-3" ;
    owl:sameAs <http://www.wikidata.org/entity/Q18491847> .

<http://demo.fiz-karlsruhe.de/matwerk/E743372> a <http://www.ebi.ac.uk/swo/license/SWO_1000002> ;
    rdfs:label "Propietary" .

<http://demo.fiz-karlsruhe.de/matwerk/E744591> a ns3:SWO_0000002 ;
    rdfs:label "OSI-approved BSD 3-clause License, https://github.com/Kitware/ParaView/blob/master/Copyright.txt" .

<http://demo.fiz-karlsruhe.de/matwerk/E74537> a nfdicore:City ;
    rdfs:label "Bochum" ;
    nfdicore:country <http://demo.fiz-karlsruhe.de/matwerk/E80004> ;
    owl:sameAs <http://www.wikidata.org/entity/Q2103> .

<http://demo.fiz-karlsruhe.de/matwerk/E745811> a <http://www.ebi.ac.uk/swo/license/SWO_1000061> ;
    rdfs:label "BSD license" ;
    owl:sameAs <http://www.wikidata.org/entity/Q191307> .

<http://demo.fiz-karlsruhe.de/matwerk/E748254> a ns3:SWO_0000002 ;
    rdfs:label "Proprietary license" .

<http://demo.fiz-karlsruhe.de/matwerk/E74921> a nfdicore:City ;
    rdfs:label "Paderborn" ;
    nfdicore:country <http://demo.fiz-karlsruhe.de/matwerk/E80004> ;
    owl:sameAs <http://www.wikidata.org/entity/Q2971> .

<http://demo.fiz-karlsruhe.de/matwerk/E749477> a ns3:SWO_0000002 ;
    rdfs:label "GPLv3+" ;
    owl:sameAs <http://www.wikidata.org/entity/Q27016754> .

<http://demo.fiz-karlsruhe.de/matwerk/E750701> a ns3:SWO_0000002 ;
    rdfs:label "public domain, https://github.com/imagej/ImageJ/blob/master/LICENSE.txt" .

<http://demo.fiz-karlsruhe.de/matwerk/E751926> a <http://www.ebi.ac.uk/swo/license/SWO_1000061> ;
    rdfs:label "BSD-2" ;
    owl:sameAs <http://www.wikidata.org/entity/Q18517294> .

<http://demo.fiz-karlsruhe.de/matwerk/E75306> a nfdicore:City ;
    rdfs:label "Darmstadt" ;
    nfdicore:country <http://demo.fiz-karlsruhe.de/matwerk/E80004> ;
    owl:sameAs <http://www.wikidata.org/entity/Q2973> .

<http://demo.fiz-karlsruhe.de/matwerk/E754379> a ns3:SWO_0000002 ;
    rdfs:label "CPMD Free License for NPOs" .

<http://demo.fiz-karlsruhe.de/matwerk/E756836> a ns3:SWO_0000002 ;
    rdfs:label "LBNL BSD" .

<http://demo.fiz-karlsruhe.de/matwerk/E75692> a nfdicore:City ;
    rdfs:label "Clausthal-Zellerfeld" ;
    nfdicore:country <http://demo.fiz-karlsruhe.de/matwerk/E80004> ;
    owl:sameAs <http://www.wikidata.org/entity/Q504590> .

<http://demo.fiz-karlsruhe.de/matwerk/E758066> a ns3:SWO_0000002 ;
    rdfs:label "Apache license" ;
    owl:sameAs <http://www.wikidata.org/entity/Q616526> .

<http://demo.fiz-karlsruhe.de/matwerk/E761762> a ns3:SWO_0000002 ;
    rdfs:label "https://www.fplo.de/wp-content/uploads/lic21.pdf" .

<http://demo.fiz-karlsruhe.de/matwerk/E767942> a <http://www.ebi.ac.uk/swo/license/SWO_1000043> ;
    rdfs:label "GNU Lesser General Public License v2.1" ;
    owl:sameAs <http://www.wikidata.org/entity/Q18534390> .

<http://demo.fiz-karlsruhe.de/matwerk/E76856> a nfdicore:City ;
    rdfs:label "Halle (Saale)" ;
    nfdicore:country <http://demo.fiz-karlsruhe.de/matwerk/E80004> ;
    owl:sameAs <http://www.wikidata.org/entity/Q2814> .

<http://demo.fiz-karlsruhe.de/matwerk/E769181> a <http://www.ebi.ac.uk/swo/license/SWO_1000043> ;
    rdfs:label "GNU Affero General Public License" .

<http://demo.fiz-karlsruhe.de/matwerk/E770421> a <http://www.ebi.ac.uk/swo/license/SWO_1000002> ;
    rdfs:label "Commercial license" .

<http://demo.fiz-karlsruhe.de/matwerk/E771662> a <http://www.ebi.ac.uk/swo/license/SWO_1000043> ;
    rdfs:label "GNU Lesser General Public License v2" ;
    owl:sameAs <http://www.wikidata.org/entity/Q18534390> .

<http://demo.fiz-karlsruhe.de/matwerk/E772904> a <http://www.ebi.ac.uk/swo/license/SWO_1000061> ;
    rdfs:label "MIT/GPL" .

<http://demo.fiz-karlsruhe.de/matwerk/E774147> a ns3:SWO_0000002 ;
    rdfs:label "Distribution specific, VESTA license, free for non-commercial users" .

<http://demo.fiz-karlsruhe.de/matwerk/E775391> a ns3:SWO_0000002 ;
    rdfs:label "Distribution specific, VMD Software License Agreement" .

<http://demo.fiz-karlsruhe.de/matwerk/E77637> a nfdicore:City ;
    rdfs:label "Bremen" ;
    nfdicore:country <http://demo.fiz-karlsruhe.de/matwerk/E80004> ;
    owl:sameAs <http://www.wikidata.org/entity/Q513400> .

<http://demo.fiz-karlsruhe.de/matwerk/E776636> a <http://www.ebi.ac.uk/swo/license/SWO_1000043> ;
    rdfs:label "GNU Lesser General Public License v3" ;
    owl:sameAs <http://www.wikidata.org/entity/Q18534393> .

<http://demo.fiz-karlsruhe.de/matwerk/E777882> a ns3:SWO_0000002 ;
    rdfs:label "Academic license" .

<http://demo.fiz-karlsruhe.de/matwerk/E7787> a nfdicore:Organization ;
    rdfs:label "Joanneum Research"@de .

<http://demo.fiz-karlsruhe.de/matwerk/E78029> a nfdicore:City ;
    rdfs:label "Braunschweig" ;
    nfdicore:country <http://demo.fiz-karlsruhe.de/matwerk/E80004> ;
    owl:sameAs <http://www.wikidata.org/entity/Q2773> .

<http://demo.fiz-karlsruhe.de/matwerk/E780377> a ns3:SWO_0000002 ;
    rdfs:label "LGPL-3.0 license" ;
    owl:sameAs <http://www.wikidata.org/entity/Q18534393> .

<http://demo.fiz-karlsruhe.de/matwerk/E781626> a <http://www.ebi.ac.uk/swo/license/SWO_1000043> ;
    rdfs:label "GNU Lesser General Public License v2.1+" .

<http://demo.fiz-karlsruhe.de/matwerk/E782876> a ns3:SWO_0000002 ;
    rdfs:label "GPL-3.0 license" ;
    owl:sameAs <http://www.wikidata.org/entity/Q10513445> .

<http://demo.fiz-karlsruhe.de/matwerk/E784127> a ns3:SWO_0000002 ;
    rdfs:label "GPL-2.0 license" ;
    owl:sameAs <http://www.wikidata.org/entity/Q10513450> .

<http://demo.fiz-karlsruhe.de/matwerk/E789141> a ns3:SWO_0000002 ;
    rdfs:label "Matminer license (BSD style)" .

<http://demo.fiz-karlsruhe.de/matwerk/E790397> a <http://www.ebi.ac.uk/swo/license/SWO_1000103> ;
    rdfs:label "Vendor specific license. HTMD Software Not-for-Profit License Agreement v1.1" .

<http://demo.fiz-karlsruhe.de/matwerk/E792912> a ns3:SWO_0000002 ;
    rdfs:label "GPL 3" ;
    owl:sameAs <http://www.wikidata.org/entity/Q10513445> .

<http://demo.fiz-karlsruhe.de/matwerk/E795431> a ns3:SWO_0000002 ;
    rdfs:label "Academic Software Licence (“ASL”)" ;
    owl:sameAs <http://www.wikidata.org/entity/Q616526> .

<http://demo.fiz-karlsruhe.de/matwerk/E79607> a nfdicore:City ;
    rdfs:label "Hamburg" ;
    owl:sameAs <http://www.wikidata.org/entity/Q79657> .

<http://demo.fiz-karlsruhe.de/matwerk/E796692> a ns3:SWO_0000002 ;
    rdfs:label "Lesser General Public License version 3.0" ;
    owl:sameAs <http://www.wikidata.org/entity/Q18534393> .

<http://demo.fiz-karlsruhe.de/matwerk/E797954> a ns3:SWO_0000002 ;
    rdfs:label "MpCCI License Agreement" .

<http://demo.fiz-karlsruhe.de/matwerk/E799217> a ns3:SWO_0000002 ;
    rdfs:label "Qhull license" .

<http://demo.fiz-karlsruhe.de/matwerk/E800481> a ns3:SWO_0000002 ;
    rdfs:label "Apache" ;
    owl:sameAs <http://www.wikidata.org/entity/Q616526> .

<http://demo.fiz-karlsruhe.de/matwerk/E801746> a ns3:SWO_0000002 ;
    rdfs:label "Apache-2.0 license" ;
    owl:sameAs <http://www.wikidata.org/entity/Q13785927> .

<http://demo.fiz-karlsruhe.de/matwerk/E803012> a ns3:SWO_0000002 ;
    rdfs:label "Apache License, Version 2.0" ;
    owl:sameAs <http://www.wikidata.org/entity/Q13785927> .

<http://demo.fiz-karlsruhe.de/matwerk/E804279> a <http://www.ebi.ac.uk/swo/license/SWO_1000043> ;
    rdfs:label "GNU license" ;
    owl:sameAs <http://www.wikidata.org/entity/Q7603> .

<http://demo.fiz-karlsruhe.de/matwerk/E805547> a ns3:SWO_0000002 ;
    rdfs:label "https://creativecommons.org/publicdomain/zero/1.0/" ;
    owl:sameAs <http://www.wikidata.org/entity/Q6938433> .

<http://demo.fiz-karlsruhe.de/matwerk/E80801> a nfdicore:Website ;
    rdfs:label "https://www.mib.uni-stuttgart.de/dae/"^^xsd:anyURI ;
    nfdicore:url <https://www.mib.uni-stuttgart.de/dae/> .

<http://demo.fiz-karlsruhe.de/matwerk/E809357> a <http://www.ebi.ac.uk/swo/license/SWO_1000001> ;
    rdfs:label "Creative Commons Attribution-ShareAlike 4.0 International License" ;
    owl:sameAs <http://www.wikidata.org/entity/Q18199165> .

<http://demo.fiz-karlsruhe.de/matwerk/E810629> a ns3:SWO_0000002 ;
    rdfs:label "https://creativecommons.org/licenses/by/4.0/" ;
    owl:sameAs <http://www.wikidata.org/entity/Q20007257> .

<http://demo.fiz-karlsruhe.de/matwerk/E81201> a nfdicore:Website ;
    rdfs:label "www.bam.de" .

<http://demo.fiz-karlsruhe.de/matwerk/E813176> a ns3:SWO_0000002 ;
    rdfs:label "Apache Licence, Version 2.0" ;
    owl:sameAs <http://www.wikidata.org/entity/Q616526> .

<http://demo.fiz-karlsruhe.de/matwerk/E8141> a nfdicore:Organization ;
    rdfs:label "Cyber Physical Simulation"@de .

<http://demo.fiz-karlsruhe.de/matwerk/E814451> a <http://www.ebi.ac.uk/swo/license/SWO_1000043> ;
    rdfs:label "GNU" ;
    owl:sameAs <http://www.wikidata.org/entity/Q7603> .

<http://demo.fiz-karlsruhe.de/matwerk/E815727> a <http://www.ebi.ac.uk/swo/license/SWO_1000001> ;
    rdfs:label "CC BY-NC-ND 4.0" ;
    owl:sameAs <http://www.wikidata.org/entity/Q24082749> .

<http://demo.fiz-karlsruhe.de/matwerk/E81602> a nfdicore:Website ;
    rdfs:label "https://www.tf.uni-kiel.de/matwis/instmat/de"^^xsd:anyURI ;
    nfdicore:url <https://www.tf.uni-kiel.de/matwis/instmat/de> .

<http://demo.fiz-karlsruhe.de/matwerk/E818282> a <http://www.ebi.ac.uk/swo/license/SWO_1000001> ;
    rdfs:label "CC-BY-4.0 license" ;
    owl:sameAs <http://www.wikidata.org/entity/Q20007257> .

<http://demo.fiz-karlsruhe.de/matwerk/E819561> a <http://www.ebi.ac.uk/swo/license/SWO_1000001> ;
    rdfs:label "Creative Commons Attribution 4.0 International Public License" ;
    owl:sameAs <http://www.wikidata.org/entity/Q20007257> .

<http://demo.fiz-karlsruhe.de/matwerk/E82004> a nfdicore:Website ;
    rdfs:label "https://www.rz.uni-kiel.de/de"^^xsd:anyURI ;
    nfdicore:url <https://www.rz.uni-kiel.de/de> .

<http://demo.fiz-karlsruhe.de/matwerk/E822122> a <http://www.ebi.ac.uk/swo/license/SWO_1000001> ;
    rdfs:label "CC-BY (https://creativecommons.org/licenses/by/3.0/)" ;
    owl:sameAs <http://www.wikidata.org/entity/Q14947546> .

<http://demo.fiz-karlsruhe.de/matwerk/E823404> a ns3:SWO_0000002 ;
    rdfs:label "No license" .

<http://demo.fiz-karlsruhe.de/matwerk/E82407> a nfdicore:Website ;
    rdfs:label "https://www.uni-saarland.de/fachrichtung/mwwt.html"^^xsd:anyURI ;
    nfdicore:url <https://www.uni-saarland.de/fachrichtung/mwwt.html> .

<http://demo.fiz-karlsruhe.de/matwerk/E8261> a nfdicore:Organization ;
    rdfs:label "Chalmers University of Technology"@de .

<http://demo.fiz-karlsruhe.de/matwerk/E82811> a nfdicore:Website ;
    rdfs:label "https://www.fiz-karlsruhe.de/en"^^xsd:anyURI ;
    nfdicore:url <https://www.fiz-karlsruhe.de/en> .

<http://demo.fiz-karlsruhe.de/matwerk/E83216> a nfdicore:Website ;
    rdfs:label "https://www.fz-juelich.de/de/ias/ias-9"^^xsd:anyURI ;
    nfdicore:url <https://www.fz-juelich.de/de/ias/ias-9> .

<http://demo.fiz-karlsruhe.de/matwerk/E832406> a nfdicore:ProgrammingLanguage ;
    rdfs:label "Python" ;
    owl:sameAs <http://www.wikidata.org/entity/Q28865> .

<http://demo.fiz-karlsruhe.de/matwerk/E83622> a nfdicore:Website ;
    rdfs:label "https://www.icams.de/"^^xsd:anyURI ;
    nfdicore:url <https://www.icams.de/> .

<http://demo.fiz-karlsruhe.de/matwerk/E837572> a nfdicore:ProgrammingLanguage ;
    rdfs:label "ruby" ;
    owl:sameAs <http://www.wikidata.org/entity/Q161053> .

<http://demo.fiz-karlsruhe.de/matwerk/E840161> a nfdicore:ProgrammingLanguage ;
    rdfs:label "Perl" ;
    owl:sameAs <http://www.wikidata.org/entity/Q42478> .

<http://demo.fiz-karlsruhe.de/matwerk/E84029> a nfdicore:Website ;
    rdfs:label "https://www.imm.rwth-aachen.de/index.php?id=2&L=0"^^xsd:anyURI ;
    nfdicore:url <https://www.imm.rwth-aachen.de/index.php?id=2&L=0> .

<http://demo.fiz-karlsruhe.de/matwerk/E842754> a nfdicore:ProgrammingLanguage ;
    rdfs:label "Julia" ;
    owl:sameAs <http://www.wikidata.org/entity/Q2613697> .

<http://demo.fiz-karlsruhe.de/matwerk/E84437> a nfdicore:Website ;
    rdfs:label "https://ilh.uni-paderborn.de/"^^xsd:anyURI ;
    nfdicore:url <https://ilh.uni-paderborn.de/> .

<http://demo.fiz-karlsruhe.de/matwerk/E846651> a nfdicore:ProgrammingLanguage ;
    rdfs:label "fortran" ;
    owl:sameAs <http://www.wikidata.org/entity/Q83303> .

<http://demo.fiz-karlsruhe.de/matwerk/E847952> a nfdicore:ProgrammingLanguage ;
    rdfs:label "javascript" ;
    owl:sameAs <http://www.wikidata.org/entity/Q2005> .

<http://demo.fiz-karlsruhe.de/matwerk/E84846> a nfdicore:Website ;
    rdfs:label "https://www.mawi.tu-darmstadt.de/materialwissenschaft/willkommen_mawi/index.de.jsp"^^xsd:anyURI ;
    nfdicore:url <https://www.mawi.tu-darmstadt.de/materialwissenschaft/willkommen_mawi/index.de.jsp> .

<http://demo.fiz-karlsruhe.de/matwerk/E849254> a nfdicore:ProgrammingLanguage ;
    rdfs:label "css" ;
    owl:sameAs <http://www.wikidata.org/entity/Q46441> .

<http://demo.fiz-karlsruhe.de/matwerk/E851861> a nfdicore:fundingProject ;
    rdfs:label "https://gepris.dfg.de/gepris/projekt/405621217?context=projekt&task=showDetail&id=405621217&"^^xsd:anyURI ;
    nfdicore:url <https://gepris.dfg.de/gepris/projekt/405621217?context=projekt&task=showDetail&id=405621217&> .

<http://demo.fiz-karlsruhe.de/matwerk/E85256> a nfdicore:Website ;
    rdfs:label "https://www.itm.tu-clausthal.de/en/"^^xsd:anyURI ;
    nfdicore:url <https://www.itm.tu-clausthal.de/en/> .

<http://demo.fiz-karlsruhe.de/matwerk/E853166> a nfdicore:fundingProject ;
    rdfs:label "DFG-FR2702/8" .

<http://demo.fiz-karlsruhe.de/matwerk/E854472> a nfdicore:fundingProject ;
    rdfs:label "DFG-FR2702/6" .

<http://demo.fiz-karlsruhe.de/matwerk/E855779> a nfdicore:fundingProject ;
    rdfs:label "EXC 310/2" .

<http://demo.fiz-karlsruhe.de/matwerk/E85667> a nfdicore:Website ;
    rdfs:label "http://www.bio.uni-freiburg.de/fakultaet/institute/bio2"^^xsd:anyURI ;
    nfdicore:url <http://www.bio.uni-freiburg.de/fakultaet/institute/bio2> .

<http://demo.fiz-karlsruhe.de/matwerk/E859706> a nfdicore:fundingProject ;
    rdfs:label "SFB 716" .

<http://demo.fiz-karlsruhe.de/matwerk/E86079> a nfdicore:Website ;
    rdfs:label "https://www.imtek.de/"^^xsd:anyURI ;
    nfdicore:url <https://www.imtek.de/> .

<http://demo.fiz-karlsruhe.de/matwerk/E861017> a nfdicore:Project ;
    rdfs:label "SFB1394" .

<http://demo.fiz-karlsruhe.de/matwerk/E862329> a nfdicore:Project ;
    rdfs:label "Project No. 409476157" .

<http://demo.fiz-karlsruhe.de/matwerk/E863642> a nfdicore:Project ;
    rdfs:label "EMMC-CSA (2016-2019)" .

<http://demo.fiz-karlsruhe.de/matwerk/E86492> a nfdicore:Website ;
    rdfs:label "https://www.iwm.fraunhofer.de/"^^xsd:anyURI ;
    nfdicore:url <https://www.iwm.fraunhofer.de/> .

<http://demo.fiz-karlsruhe.de/matwerk/E864956> a nfdicore:Project ;
    rdfs:label "SimDOME (2019-2023)" .

<http://demo.fiz-karlsruhe.de/matwerk/E866271> a nfdicore:Project ;
    rdfs:label "MarketPlace (2018-2022)" .

<http://demo.fiz-karlsruhe.de/matwerk/E867587> a nfdicore:Project ;
    rdfs:label "VIMMP (2018-2021)" .

<http://demo.fiz-karlsruhe.de/matwerk/E868904> a nfdicore:Project ;
    rdfs:label "OntoTrans (2020-2024)" .

<http://demo.fiz-karlsruhe.de/matwerk/E86906> a nfdicore:Website ;
    rdfs:label "https://www.itm.kit.edu/index.php"^^xsd:anyURI ;
    nfdicore:url <https://www.itm.kit.edu/index.php> .

<http://demo.fiz-karlsruhe.de/matwerk/E870222> a nfdicore:Project ;
    rdfs:label "ReaxPro (2019-2023)" .

<http://demo.fiz-karlsruhe.de/matwerk/E871541> a nfdicore:Project ;
    rdfs:label "OntoCommons (2020-2023)" .

<http://demo.fiz-karlsruhe.de/matwerk/E872861> a nfdicore:Project ;
    rdfs:label "OYSTER (2017-2021)" .

<http://demo.fiz-karlsruhe.de/matwerk/E87321> a nfdicore:Website ;
    rdfs:label "https://www.imws.fraunhofer.de/"^^xsd:anyURI ;
    nfdicore:url <https://www.imws.fraunhofer.de/> .

<http://demo.fiz-karlsruhe.de/matwerk/E874182> a nfdicore:Project ;
    rdfs:label "NanoMECommons (2021-2025)" .

<http://demo.fiz-karlsruhe.de/matwerk/E875504> a nfdicore:Project ;
    rdfs:label "OpenModel (2021-2025)" .

<http://demo.fiz-karlsruhe.de/matwerk/E876827> a nfdicore:Project ;
    rdfs:label "European Research Council through the ERC Grant Agreement No. 759419 MuDiLingo (”A Multiscale Dislocation Language for Data-Driven Materials Science”)" .

<http://demo.fiz-karlsruhe.de/matwerk/E87737> a nfdicore:Website ;
    rdfs:label "https://www.mv.uni-kl.de/en/wkk/home"^^xsd:anyURI ;
    nfdicore:url <https://www.mv.uni-kl.de/en/wkk/home> .

<http://demo.fiz-karlsruhe.de/matwerk/E878151> a nfdicore:Project ;
    rdfs:label "Open Databases Integration for Materials Design (OPTIMADE)" .

<http://demo.fiz-karlsruhe.de/matwerk/E879476> a nfdicore:Project ;
    rdfs:label "Platform Material Digital" .

<http://demo.fiz-karlsruhe.de/matwerk/E880802> a nfdicore:Publication ;
    dcterms:title "Automated free-energy calculation from atomistic simulations" ;
    mwo:hasAuthor <http://demo.fiz-karlsruhe.de/matwerk/E19529>,
        <http://demo.fiz-karlsruhe.de/matwerk/E34671>,
        <http://demo.fiz-karlsruhe.de/matwerk/E35454>,
        <http://demo.fiz-karlsruhe.de/matwerk/E8627> ;
    mwo:hasDOI "https://doi.org/10.1103/PhysRevMaterials.5.103801" ;
    schema:datePublished "10/11/2021 0:00" .

<http://demo.fiz-karlsruhe.de/matwerk/E88154> a nfdicore:Website ;
    rdfs:label "https://via.cs.uni-kl.de/"^^xsd:anyURI ;
    nfdicore:url <https://via.cs.uni-kl.de/> .

<http://demo.fiz-karlsruhe.de/matwerk/E882129> a nfdicore:Publication ;
    dcterms:title "pyscal: A python module for structural analysis of atomic environments." ;
    mwo:hasAuthor <http://demo.fiz-karlsruhe.de/matwerk/E19916>,
        <http://demo.fiz-karlsruhe.de/matwerk/E8627> ;
    mwo:hasDOI "https://doi.org/10.21105/joss.01824" ;
    schema:datePublished "11/1/2019 0:00" .

<http://demo.fiz-karlsruhe.de/matwerk/E883457> a nfdicore:Publication ;
    dcterms:title "On the generation of periodic discrete structures with identical two-point correlation" ;
    mwo:hasAuthor <http://demo.fiz-karlsruhe.de/matwerk/E16226>,
        <http://demo.fiz-karlsruhe.de/matwerk/E16577> ;
    mwo:hasDOI "https://doi.org/10.1098/rspa.2020.0568" ;
    schema:datePublished "10/21/2020 0:00" .

<http://demo.fiz-karlsruhe.de/matwerk/E88572> a nfdicore:Website ;
    rdfs:label "https://www.iwt-bremen.de/en/home"^^xsd:anyURI ;
    nfdicore:url <https://www.iwt-bremen.de/en/home> .

<http://demo.fiz-karlsruhe.de/matwerk/E886116> a nfdicore:Publication ;
    dcterms:title "Data-Driven Microstructure Property Relations" ;
    mwo:hasAuthor <http://demo.fiz-karlsruhe.de/matwerk/E16577>,
        <http://demo.fiz-karlsruhe.de/matwerk/E16754> ;
    mwo:hasDOI "https://doi.org/10.3390/mca24020057" ;
    schema:datePublished "5/31/2019 0:00" .

<http://demo.fiz-karlsruhe.de/matwerk/E887447> a nfdicore:Publication ;
    dcterms:title "Schroeder, Will; Martin, Ken; Lorensen, Bill (2006), The Visualization Toolkit (4th ed.), Kitware, ISBN 978-1-930934-19-1" .

<http://demo.fiz-karlsruhe.de/matwerk/E888779> a nfdicore:Publication ;
    dcterms:title """[1] G. Kresse and J. Hafner, Phys. Rev. B 47 , 558 (1993); ibid. 49 , 14 251 (1994).\r
[2] G. Kresse and J. FurthmÃ¼ller, Comput. Mat. Sci. 6 , 15 (1996).\r
[3] G. Kresse and J. FurthmÃ¼ller, Phys. Rev. B 54 , 11 169 (1996).""" .

<http://demo.fiz-karlsruhe.de/matwerk/E88991> a nfdicore:Website ;
    rdfs:label "https://www.ptb.de/cms/"^^xsd:anyURI ;
    nfdicore:url <https://www.ptb.de/cms/> .

<http://demo.fiz-karlsruhe.de/matwerk/E890112> a nfdicore:Publication ;
    dcterms:title "\"First principles methods using CASTEP\", Zeitschrift fuer Kristallographie 220(5-6) pp. 567-570 (2005) S. J. Clark, M. D. Segall, C. J. Pickard, P. J. Hasnip, M. J. Probert, K. Refson, M. C. Payne" .

<http://demo.fiz-karlsruhe.de/matwerk/E891446> a nfdicore:Publication ;
    dcterms:title "https://www.cpmd.org/wordpress/index.php/the-code/references/general-bibliographical-references/" .

<http://demo.fiz-karlsruhe.de/matwerk/E892781> a nfdicore:Publication ;
    dcterms:title "The Abinit project: Impact, environment and recent developments Comput. Phys. Commun. 248, 107042 (2020) URL: https://doi.org/10.1016/j.cpc.2019.107042; ABINIT: Overview, and focus on selected capabilities J. Chem. Phys. 152, 124102 (2020)" .

<http://demo.fiz-karlsruhe.de/matwerk/E89411> a nfdicore:Website ;
    rdfs:label "https://www.fz-juelich.de/de/iek/iek-2"^^xsd:anyURI ;
    nfdicore:url <https://www.fz-juelich.de/de/iek/iek-2> .

<http://demo.fiz-karlsruhe.de/matwerk/E894117> a nfdicore:Publication ;
    dcterms:title "https://doi.org/10.1063/5.0004792" .

<http://demo.fiz-karlsruhe.de/matwerk/E895454> a nfdicore:Publication ;
    dcterms:title "P. Giannozzi, S. Baroni, N. Bonini, M. Calandra, R. Car, C. Cavazzoni, D. Ceresoli, G. L. Chiarotti, M. Cococcioni, I. Dabo, A. Dal Corso, S. Fabris, G. Fratesi, S. de Gironcoli, R. Gebauer, U. Gerstmann, C. Gougoussis, A. Kokalj, M. Lazzeri, L. Martin-Samos, N. Marzari, F. Mauri, R. Mazzarello, S. Paolini, A. Pasquarello, L. Paulatto, C. Sbraccia, S. Scandolo, G. Sclauzero, A. P. Seitsonen, A. Smogunov, P. Umari, R. M. Wentzcovitch, J.Phys.: Condens.Matter 21, 395502 (2009) and P. Giannozzi, O. Andreussi, T. Brumme, O. Bunau, M. Buongiorno Nardelli, M. Calandra, R. Car, C. Cavazzoni, D. Ceresoli, M. Cococcioni, N. Colonna, I. Carnimeo, A. Dal Corso, S. de Gironcoli, P. Delugas, R. A. DiStasio Jr, A. Ferretti, A. Floris, G. Fratesi, G. Fugallo, R. Gebauer, U. Gerstmann, F. Giustino, T. Gorni, J Jia, M. Kawamura, H.-Y. Ko, A. Kokalj, E. Küçükbenli, M .Lazzeri, M. Marsili, N. Marzari, F. Mauri, N. L. Nguyen, H.-V. Nguyen, A. Otero-de-la-Roza, L. Paulatto, S. Poncé, D. Rocca, R. Sabatini, B. Santra, M. Schlipf, A. P. Seitsonen, A. Smogunov, I. Timrov, T. Thonhauser, P. Umari, N. Vast, X. Wu, S. Baroni, J.Phys.: Condens.Matter 29, 465901 (2017)" .

<http://demo.fiz-karlsruhe.de/matwerk/E896792> a nfdicore:Publication ;
    dcterms:title "R. Sundararaman, K. Letchworth-Weaver, K.A. Schwarz, D. Gunceler, Y. Ozhabes and T.A. Arias, 'JDFTx: software for joint density-functional theory', SoftwareX 6, 278 (2017)" .

<http://demo.fiz-karlsruhe.de/matwerk/E898131> a nfdicore:Publication ;
    dcterms:title "J. R. Chelikowsky, N. Troullier, and Y. Saad, Finite-difference pseudo potential method: Electronic structure calculations without a basis, Phys. Rev. Lett. 72, 1240 (1994). J. R. Chelikowsky, The pseudopotential-density functional method applied to nanostructures, J. of Phys. D 33, R33 (2000). L. Kronik, A. Makmal, M.L. Tiago, M.M.G. Alemany, M. Jain, X. Huang, Y. Saad, and J.R. Chelikowsky, PARSEC-the pseudopotential algorithm for real-space electronic structure calculations: Recent Advances and novel applications to nano-structures, physica status solidi (b) 243, 1063 (2006). Y. Saad, J.R. Chelikowsky and S.M. Shontz, Numerical methods for electronic structure calculations of materials, SIAM Rev. 52, 3 (2010)." .

<http://demo.fiz-karlsruhe.de/matwerk/E899471> a nfdicore:Publication ;
    dcterms:title "J. J. Mortensen, L. B. Hansen, and K. W. Jacobsen Real-space grid implementation of the projector augmented wave method Phys. Rev. B 71, 035109 (2005) J. Enkovaara, C. Rostgaard, J. J. Mortensen et al. Electronic structure calculations with GPAW: a real-space implementation of the projector augmented-wave method J. Phys.: Condens. Matter 22, 253202 (2010)" .

<http://demo.fiz-karlsruhe.de/matwerk/E900812> a nfdicore:Publication ;
    dcterms:title "10.21105/jcon.00069" .

<http://demo.fiz-karlsruhe.de/matwerk/E902154> a nfdicore:Publication ;
    dcterms:title "https://iopscience.iop.org/article/10.1088/0953-8984/14/11/302/meta" .

<http://demo.fiz-karlsruhe.de/matwerk/E90254> a nfdicore:Website ;
    rdfs:label "https://www.itc.rwth-aachen.de/cms/~epto/IT-Center/"^^xsd:anyURI ;
    nfdicore:url <https://www.itc.rwth-aachen.de/cms/~epto/IT-Center/> .

<http://demo.fiz-karlsruhe.de/matwerk/E903497> a nfdicore:Publication ;
    dcterms:title "https://wires.onlinelibrary.wiley.com/doi/10.1002/wcms.1360" .

<http://demo.fiz-karlsruhe.de/matwerk/E904841> a nfdicore:Publication ;
    dcterms:title """[1] K. Koepernik and H. Eschrig, Phys. Rev. B 59, 1743 (1999).\r
[2] I. Opahle, K. Koepernik, and H. Eschrig, Phys. Rev. B 60, 14035 (1999).\r
[3] H. Eschrig, M. Richter, I. Opahle, Relativistic Solid State Calculations, in: Relativistic Electronic Structure Theory, Part 2. Applications (P. Schwerdtfeger, ed.), Theoretical and Computational Chemistry, vol.13, Elsevier, 2004, pp.723–776.\r
[4] H. Eschrig, K. Koepernik, and I. Chaplygin, J. Solid State Chemistry 176, 482 (2003).\r
[5] Helmut. Eschrig: The Fundamentals of Density Functional Theory, 2nd Edition, Edition am Gutenbergplatz, Leipzig, 2003.\r
[6] K. Lejaeghere et al., Science 351, 1415-U81 (2016).""" .

<http://demo.fiz-karlsruhe.de/matwerk/E906186> a nfdicore:Publication ;
    dcterms:title "https://aip.scitation.org/doi/10.1063/1.5143061" .

<http://demo.fiz-karlsruhe.de/matwerk/E90677> a nfdicore:Website ;
    rdfs:label "https://www.dfki.de/web"^^xsd:anyURI ;
    nfdicore:url <https://www.dfki.de/web> .

<http://demo.fiz-karlsruhe.de/matwerk/E907532> a nfdicore:Publication ;
    dcterms:title """J. Roth, F. Gähler, and H.-R. Trebin,\r
A molecular dynamics run with 5.180.116.000 particles,\r
Int. J. Mod. Phys. C 11, 317-22 (2000).\r
PDF-File (184k)\r
\r
J. Stadler, R. Mikulla, and H.-R. Trebin,\r
IMD: A Software Package for Molecular Dynamics Studies on Parallel Computers,\r
Int. J. Mod. Phys. C 8, 1131-1140 (1997).\r
gzipped PostScript (690k)  PDF-File (325k)\r
\r
J. Roth\r
IMD: A Typical Massively Parallel Molecular Dynamics Code for Classical Simulations - Structure, Applications, Latest Developments\r
Sustained Simulation Performance 2013,\r
eds. M. M. Resch, W. Bez, E. Forcht, H. Kobayashi, Y. Kovalenko, Springer, Heidelberg 2013, pp. 63-76.""" .

<http://demo.fiz-karlsruhe.de/matwerk/E908879> a nfdicore:Publication ;
    dcterms:title """* GROMACS: A message-passing parallel molecular dynamics implementation\r
  H.J.C. Berendsen, D. van der Spoel and R. van Drunen\r
  Comp. Phys. Comm. 91, 43-56 (1995)\r
  DOI: https://doi.org/10.1016/0010-4655(95)00042-E\r
 \r
* GROMACS 4: Algorithms for highly efficient, load-balanced, and scalable\r
  molecular simulation\r
  B. Hess and C. Kutzner and D. van der Spoel and E. Lindahl\r
  J. Chem. Theory Comput. 4 (2008) pp. 435-447\r
  DOI: https://doi.org/10.1021/ct700301q\r
\r
* GROMACS 4.5: a high-throughput and highly parallel open source\r
  molecular simulation toolkit\r
  Sander Pronk, Szilárd Páll, Roland Schulz, Per Larsson, Pär Bjelkmar,\r
  Rossen Apostolov, Michael R. Shirts, Jeremy C. Smith, Peter M. Kasson,\r
  David van der Spoel, Berk Hess, Erik Lindahl.\r
  Bioinformatics 29 (2013) pp. 845-54\r
  DOI: https://doi.org/10.1093/bioinformatics/btt055\r
\r
* Tackling Exascale Software Challenges in Molecular Dynamics Simulations\r
  with GROMACS\r
  Szilárd Páll, Mark J. Abraham, Carsten Kutzner, Berk Hess, Erik Lindahl\r
  In S. Markidis & E. Laure (Eds.), Solving Software Challenges for Exascale,\r
  Lecture Notes for Computer Science, 8759 (2015) pp. 3–27\r
  DOI: https://doi.org/10.1007/978-3-319-15976-8_1\r
\r
* GROMACS: High performance molecular simulations through multi-level parallelism from laptops to supercomputers\r
  M. J. Abraham, T. Murtola, R. Schulz, S. Páll, J. C. Smith, B. Hess, E. Lindahl,\r
  SoftwareX, 1, (2015), 19-25\r
  DOI: https://doi.org/10.1016/j.softx.2015.06.001""" .

<http://demo.fiz-karlsruhe.de/matwerk/E910227> a nfdicore:Publication ;
    dcterms:title "https://doi.org/10.1016/j.commatsci.2018.04.030" .

<http://demo.fiz-karlsruhe.de/matwerk/E91101> a nfdicore:Website ;
    rdfs:label "https://www.scc.kit.edu/index.php"^^xsd:anyURI ;
    nfdicore:url <https://www.scc.kit.edu/index.php> .

<http://demo.fiz-karlsruhe.de/matwerk/E911576> a nfdicore:Publication ;
    dcterms:title """title = {pyiron: An integrated development environment for computational materials science},\r
  journal = {Computational Materials Science},\r
  volume = {163},\r
  pages = {24 - 36},\r
  year = {2019},\r
  issn = {0927-0256},\r
  doi = {https://doi.org/10.1016/j.commatsci.2018.07.043},\r
  url = {http://www.sciencedirect.com/science/article/pii/S0927025618304786},\r
  author = {Jan Janssen and Sudarsan Surendralal and Yury Lysogorskiy and Mira Todorova and Tilmann Hickel and Ralf Drautz and Jörg Neugebauer},\r
  keywords = {Modelling workflow, Integrated development environment, Complex simulation protocols},""" .

<http://demo.fiz-karlsruhe.de/matwerk/E912926> a nfdicore:Publication ;
    dcterms:title """https://doi.org/10.1038/s41597-020-00638-4\r
https://doi.org/10.1016/j.commatsci.2020.110086\r
http://dx.doi.org/10.1016/j.commatsci.2015.09.013""" .

<http://demo.fiz-karlsruhe.de/matwerk/E914277> a nfdicore:Publication ;
    dcterms:title "Torbjorn Bjorkman, \"CIF2Cell: Generating geometries for electronic structure programs\", Computer Physics Communications 182, 1183-1186 (2011) doi: 10.1016/j.cpc.2011.01.013" .

<http://demo.fiz-karlsruhe.de/matwerk/E91526> a nfdicore:Website ;
    rdfs:label "https://www.iws.fraunhofer.de/"^^xsd:anyURI ;
    nfdicore:url <https://www.iws.fraunhofer.de/> .

<http://demo.fiz-karlsruhe.de/matwerk/E915629> a nfdicore:Publication ;
    dcterms:title "http://www.jcheminf.com/content/4/1/17" .

<http://demo.fiz-karlsruhe.de/matwerk/E916982> a nfdicore:Publication ;
    dcterms:title "C. Schran, F. L. Thiemann, P. Rowe, E. A. Müller, O. Marsalek, A. Michaelides, \"Machine learning potentials for complex aqueous systems made simple\", PNAS 118, e2110077118 (2021), 10.1073/pnas.2110077118 C. Schran, K. Brezina, O. Marsalek, \"Committee neural network potentials control generalization errors and enable active learning\", J. Chem. Phys. 153, 104105 (2020), 10.1063/5.0016004" .

<http://demo.fiz-karlsruhe.de/matwerk/E918336> a nfdicore:Publication ;
    dcterms:title "https://doi.org/10.1002/jcc.24900 https://doi.org/10.1002/jcc.26112 " .

<http://demo.fiz-karlsruhe.de/matwerk/E919691> a nfdicore:Publication ;
    dcterms:title "David W.H. Swenson, Jan-Hendrik Prinz, Frank Noé, John D. Chodera, and Peter G. Bolhuis. “OpenPathSampling: A flexible, open framework for path sampling simulations. 1. Basics.” J. Chem. Theory Comput. 15, 813 (2019). https://doi.org/10.1021/acs.jctc.8b00626      David W.H. Swenson, Jan-Hendrik Prinz, Frank Noé, John D. Chodera, and Peter G. Bolhuis. “OpenPathSampling: A flexible, open framework for path sampling simulations. 2. Building and Customizing Path Ensembles and Sample Schemes.” J. Chem. Theory Comput. 15, 837 (2019). https://doi.org/10.1021/acs.jctc.8b00627 " .

<http://demo.fiz-karlsruhe.de/matwerk/E921047> a nfdicore:Publication ;
    dcterms:title "Ghysels, A.; Verstraelen, T.; Hemelsoet, K.; Waroquier, M.; Van Speybroeck, V. J. Chem. Inf. Model. 2010, 50, 1736-1750." .

<http://demo.fiz-karlsruhe.de/matwerk/E922404> a nfdicore:Publication ;
    dcterms:title "Hai Nguyen, David A Case, Alexander S Rose; NGLview - Interactive molecular graphics for Jupyter notebooks, Bioinformatics, , btx789, https://doi.org/10.1093/bioinformatics/btx789" .

<http://demo.fiz-karlsruhe.de/matwerk/E923762> a nfdicore:Publication ;
    dcterms:title "L. Vanduyfhuys, S. Vandenbrande, T. Verstraelen, R. Schmid, M. Waroquier, V. Van Speybroeck, J. Comput. Chem., 2015, 36, 13, 1015-1027 If you use version 2.x.x or higher, please also refer to the follow-up paper  L. Vanduyfhuys, S. Vandenbrande, J. Wieme, M. Waroquier, T. Verstraelen, V. Van Speybroeck, J. Comput. Chem., 2018, 39, 16, 999-1011" .

<http://demo.fiz-karlsruhe.de/matwerk/E925121> a nfdicore:Publication ;
    dcterms:title "J. Chang, D. Kleiven, M. Melander, J. Akola, J. M. Garcia-Lastra and T. Vegge CLEASE: A versatile and user-friendly implementation of Cluster Expansion method Journal of Physics: Condensed Matter" .

<http://demo.fiz-karlsruhe.de/matwerk/E926481> a nfdicore:Publication ;
    dcterms:title "M. Ångqvist, W. A. Muñoz, J. M. Rahm, E. Fransson, C. Durniak, P. Rozyczko, T. H. Rod, and P. Erhart ICET – A Python Library for Constructing and Sampling Alloy Cluster Expansions Adv. Theory. Sim., 1900015 (2019) doi: 10.1002/adts.201900015" .

<http://demo.fiz-karlsruhe.de/matwerk/E927842> a nfdicore:Publication ;
    dcterms:title "A. Carreras, A. Togo, I. Tanaka, DynaPhoPy: A code for extracting phonon quasiparticles from molecular dynamics simulations, Computer Physics Communications (2017). " .

<http://demo.fiz-karlsruhe.de/matwerk/E92807> a nfdicore:Website ;
    rdfs:label "http://projects.ce.berkeley.edu/feap/"^^xsd:anyURI ;
    nfdicore:url <http://projects.ce.berkeley.edu/feap/> .

<http://demo.fiz-karlsruhe.de/matwerk/E929204> a nfdicore:Publication ;
    dcterms:title "https://doi.org/10.1557/mrc.2019.59" .

<http://demo.fiz-karlsruhe.de/matwerk/E930567> a nfdicore:Publication ;
    dcterms:title "Otis, R. & Liu, Z.-K., (2017). pycalphad: CALPHAD-based Computational Thermodynamics in Python. Journal of Open Research Software. 5(1), p.1. DOI: http://doi.org/10.5334/jors.140" .

<http://demo.fiz-karlsruhe.de/matwerk/E931931> a nfdicore:Publication ;
    dcterms:title "L.B. Partay, A.P. Bartok, G. Csanyi, Efficient Sampling of Atomic Configurational Spaces, J. Phys. Chem. B (2010), 114, 10502–10512, http://pubs.acs.org/doi/abs/10.1021/jp1012973  R.J.N. Baldock, L.B. Partay, A.P. Bartok, M.C. Payne, G. Csanyi, Determining pressure-temperature phase diagrams of materials, Phys. Rev. B (2016), 93, 174108, http://journals.aps.org/prb/abstract/10.1103/PhysRevB.93.174108  R.J.N. Baldock, N. Bernstein, K. M. Salerno, L.B. Partay, G. Csanyi, Constant-pressure nested sampling with atomistic dynamics, Phys. Rev. E (2017), 96, 043311, http://link.aps.org/doi/10.1103/PhysRevE.96.043311" .

<http://demo.fiz-karlsruhe.de/matwerk/E93236> a nfdicore:Website ;
    rdfs:label "https://www.paraview.org/"^^xsd:anyURI ;
    nfdicore:url <https://www.paraview.org/> .

<http://demo.fiz-karlsruhe.de/matwerk/E933296> a nfdicore:Publication ;
    dcterms:title "doi     = {10.1016/j.cpc.2021.108218}" .

<http://demo.fiz-karlsruhe.de/matwerk/E934662> a nfdicore:Publication ;
    dcterms:title "Singraber, A.; Behler, J.; Dellago, C. Library-Based LAMMPS Implementation of High-Dimensional Neural Network Potentials. J. Chem. Theory Comput. 2019, 15 (3), 1827–1840. https://doi.org/10.1021/acs.jctc.8b00770" .

<http://demo.fiz-karlsruhe.de/matwerk/E936029> a nfdicore:Publication ;
    dcterms:title "Ward, L., Dunn, A., Faghaninia, A., Zimmermann, N. E. R., Bajaj, S., Wang, Q., Montoya, J. H., Chen, J., Bystrom, K., Dylla, M., Chard, K., Asta, M., Persson, K., Snyder, G. J., Foster, I., Jain, A., Matminer: An open source toolkit for materials data mining. Comput. Mater. Sci. 152, 60-69 (2018)." .

<http://demo.fiz-karlsruhe.de/matwerk/E93666> a nfdicore:Website ;
    rdfs:label "https://vtk.org/"^^xsd:anyURI ;
    nfdicore:url <https://vtk.org/> .

<http://demo.fiz-karlsruhe.de/matwerk/E937397> a nfdicore:Publication ;
    dcterms:title "Dunn, A., Wang, Q., Ganose, A., Dopp, D., Jain, A. Benchmarking Materials Property Prediction Methods: The Matbench Test Set and Automatminer Reference Algorithm. npj  Computational Materials 6, 138 (2020). https://doi.org/10.1038/s41524-020-00406-3" .

<http://demo.fiz-karlsruhe.de/matwerk/E938766> a nfdicore:Publication ;
    dcterms:title "A. Stukowski, E. Fransson, M. Mock, and P. Erhart, Atomicrex - a general purpose tool for the construction of atomic interaction models, Modelling Simul. Mater. Sci. Eng. 25, 055003 (2017), doi: 10.1088/1361-651X/aa6ecf" .

<http://demo.fiz-karlsruhe.de/matwerk/E940136> a nfdicore:Publication ;
    dcterms:title "Fredrik Eriksson, Erik Fransson, and Paul Erhart The Hiphive Package for the Extraction of High‐Order Force Constants by Machine Learning Adv. Theory. Sim., 1800184 (2019) doi: 10.1002/adts.201800184" .

<http://demo.fiz-karlsruhe.de/matwerk/E94097> a nfdicore:Website ;
    rdfs:label "https://www.physik.uni-wuerzburg.de/lrm/forschung/software/"^^xsd:anyURI ;
    nfdicore:url <https://www.physik.uni-wuerzburg.de/lrm/forschung/software/> .

<http://demo.fiz-karlsruhe.de/matwerk/E941507> a nfdicore:Publication ;
    dcterms:title "J. Magnus Rahm and Paul Erhart WulffPack: A Python package for Wulff constructions J. Open Source Softw. 5, 1944 (2020) doi: 10.21105/joss.01944" .

<http://demo.fiz-karlsruhe.de/matwerk/E942879> a nfdicore:Publication ;
    dcterms:title "Dynasor – A tool for extracting dynamical structure factors and current correlation functions from molecular dynamics simulations Erik Fransson, Mattias Slabanja, Paul Erhart, and Göran Wahnström Advanced Theory and Simulations 4, 2000240 (2021); DOI:10.1002/adts.202000240" .

<http://demo.fiz-karlsruhe.de/matwerk/E944252> a nfdicore:Publication ;
    dcterms:title "https://doi.org/10.1103/PhysRevB.85.184203" .

<http://demo.fiz-karlsruhe.de/matwerk/E94529> a nfdicore:Website ;
    rdfs:label "https://www.thermofisher.com/de/de/home/electron-microscopy/products/software-em-3d-vis/avizo-software.html#features"^^xsd:anyURI ;
    nfdicore:url <https://www.thermofisher.com/de/de/home/electron-microscopy/products/software-em-3d-vis/avizo-software.html#features> .

<http://demo.fiz-karlsruhe.de/matwerk/E945626> a nfdicore:Publication ;
    dcterms:title """Bochkarev, A., Lysogorskiy, Y., Menon, S., Qamar, M., Mrovec, M., & Drautz, R. (2022). Efficient parametrization of the atomic cluster expansion. Physical Review Materials, 6(1), 013804\r
Lysogorskiy, Y., Oord, C. V. D., Bochkarev, A., Menon, S., Rinaldi, M., Hammerschmidt, T., ... & Drautz, R. (2021). Performant implementation of the atomic cluster expansion (PACE) and application to copper and silicon. npj Computational Materials, 7(1), 1-12""" .

<http://demo.fiz-karlsruhe.de/matwerk/E947001> a nfdicore:Publication ;
    dcterms:title "https://link.springer.com/article/10.1007/s40192-019-00138-3" .

<http://demo.fiz-karlsruhe.de/matwerk/E948377> a nfdicore:Publication ;
    dcterms:title "B. Patzák, D. Rypl, and J. Kruis. Mupif – a distributed multi-physics integration tool. Advances in Engineering Software, 60–61(0):89 – 97, 2013 (http://www.sciencedirect.com/science/article/pii/S0965997812001329)." .

<http://demo.fiz-karlsruhe.de/matwerk/E94962> a nfdicore:Website ;
    rdfs:label "https://fiji.sc/"^^xsd:anyURI ;
    nfdicore:url <https://fiji.sc/> .

<http://demo.fiz-karlsruhe.de/matwerk/E949754> a nfdicore:Publication ;
    dcterms:title "Huber, Hadian, Grabowski, and Neugebauer, npj Computational Materials 4 (2018), 1-8" .

<http://demo.fiz-karlsruhe.de/matwerk/E951132> a nfdicore:Publication ;
    dcterms:title "Zongrui Pei, DIST: A dislocation-simulation toolkit, Computer Physics Communications 233(2018)44-50." .

<http://demo.fiz-karlsruhe.de/matwerk/E952511> a nfdicore:Publication ;
    dcterms:title "Hadian et al., (2018). GB code: A grain boundary generation code. Journal of Open Source Software, 3(29), 900, https://doi.org/10.21105/joss.00900" .

<http://demo.fiz-karlsruhe.de/matwerk/E953891> a nfdicore:Publication ;
    dcterms:title """Markus Kühbach, Priyanshu Bajaj, Andrew Breen, Eric A. Jägle, and Baptiste Gault\r
On Strong Scaling Open Source Tools for Mining Atom Probe Tomography Data\r
Microscopy and Microanalysis, Vol 25, Supplement S2, 2019\r
https://dx.doi.org/10.1017/S1431927619002228""" .

<http://demo.fiz-karlsruhe.de/matwerk/E95396> a nfdicore:Website ;
    rdfs:label "https://imagej.net/software/imagej/"^^xsd:anyURI ;
    nfdicore:url <https://imagej.net/software/imagej/> .

<http://demo.fiz-karlsruhe.de/matwerk/E955272> a nfdicore:Publication ;
    dcterms:title """\r
Wang, N., Freysoldt, C., Zhang, S., Liebscher, C., & Neugebauer, J. (2021). Segmentation of Static and Dynamic Atomic-Resolution Microscopy Data Sets with Unsupervised Machine Learning Using Local Symmetry Descriptors. Microscopy and Microanalysis, 27(6), 1454-1464. doi:10.1017/S1431927621012770""" .

<http://demo.fiz-karlsruhe.de/matwerk/E956654> a nfdicore:Publication ;
    dcterms:title "https://dx.doi.org/10.13140/RG.2.2.25845.83687/2" .

<http://demo.fiz-karlsruhe.de/matwerk/E958037> a nfdicore:Publication ;
    dcterms:title "Chris H. Rycroft, Voro++: A three-dimensional Voronoi cell library in C++, Chaos 19, 041111 (2009)." .

<http://demo.fiz-karlsruhe.de/matwerk/E95831> a nfdicore:Website ;
    rdfs:label "https://imagej.net/software/imagej2/"^^xsd:anyURI ;
    nfdicore:url <https://imagej.net/software/imagej2/> .

<http://demo.fiz-karlsruhe.de/matwerk/E959421> a nfdicore:Publication ;
    dcterms:title "Barber, C.B., Dobkin, D.P., and Huhdanpaa, H.T., \"The Quickhull algorithm for convex hulls,\" ACM Transactions on Mathematical Software, 22(4):469-483, Dec 1996 [abstract]." .

<http://demo.fiz-karlsruhe.de/matwerk/E960806> a nfdicore:Publication ;
    dcterms:title "Brandt, N., Griem, L., Herrmann, C., Schoof, E., Tosato, G., Zhao, Y., Zschumme, P. and Selzer, M., 2021. Kadi4Mat: A Research Data Infrastructure for Materials Science. Data Science Journal, 20(1), p.8. DOI: http://doi.org/10.5334/dsj-2021-008" .

<http://demo.fiz-karlsruhe.de/matwerk/E962192> a nfdicore:Publication ;
    dcterms:title "R. S. Elliott and E. B. Tadmor, \"Knowledgebase of Interatomic Models (KIM) Application Programming Interface (API)\", OpenKIM (2011). doi:10.25950/ff8f563a" .

<http://demo.fiz-karlsruhe.de/matwerk/E96267> a nfdicore:Website ;
    rdfs:label "http://www.vasp.at/"^^xsd:anyURI ;
    nfdicore:url <http://www.vasp.at/> .

<http://demo.fiz-karlsruhe.de/matwerk/E963579> a nfdicore:Publication ;
    dcterms:title "TURBOMOLE: Modular program suite for ab initio quantum-chemical and condensed-matter simulations" ;
    mwo:hasDOI "https://doi.org/10.1063/5.0004635" ;
    schema:datePublished "13.05.2020" .

<http://demo.fiz-karlsruhe.de/matwerk/E964967> a nfdicore:Publication ;
    dcterms:title "De Geest, P., Droesbeke, B., Eguinoa, I., Gaignard, A., Huber, S., Leo, S., Pireddu, L., Rodríguez-Navas, L., Sirvent, R., & Soiland-Reyes, S. (2022). ro-crate-py (Version 0.7.0) [Computer software]. https://doi.org/10.5281/zenodo.3956493" .

<http://demo.fiz-karlsruhe.de/matwerk/E966356> a nfdicore:Publication ;
    dcterms:title "Many-scale finite strain computational homogenization via Concentric Interpolation" ;
    mwo:hasAuthor <http://demo.fiz-karlsruhe.de/matwerk/E16401>,
        <http://demo.fiz-karlsruhe.de/matwerk/E16577> ;
    mwo:hasDOI "https://doi.org/10.1002/nme.6454" ;
    schema:datePublished "6/8/2020" .

<http://demo.fiz-karlsruhe.de/matwerk/E96704> a nfdicore:Website ;
    rdfs:label "http://www.castep.org/"^^xsd:anyURI ;
    nfdicore:url <http://www.castep.org/> .

<http://demo.fiz-karlsruhe.de/matwerk/E967746> a nfdicore:Publication ;
    dcterms:title """Patrick Avery and Eva Zurek. Randspg: An open-source program for generating atomistic\r
crystal structures with specific spacegroups. Computer Physics Communications, 213:208–216,\r
2017.""" .

<http://demo.fiz-karlsruhe.de/matwerk/E969137> a nfdicore:Publication ;
    rdfs:label "C.A. Becker, F. Tavazza, Z.T. Trautt, and R.A. Buarque de Macedoc (2013), \"Considerations for choosing and using force fields and interatomic potentials in materials science and engineering,\" Current Opinion in Solid State and Materials Science, 17, 277-283. DOI: 10.1016/j.cossms.2013.10.001 L.M. Hale, Z.T. Trautt, and C.A. Becker (2018), \"Evaluating variability with atomistic simulations: the effect of potential and calculation methodology on the modeling of lattice and elastic constants,\" Modelling and Simulation in Materials Science and Engineering, 26, 055003. DOI: 10.1088/1361-651X/aabc05" .

<http://demo.fiz-karlsruhe.de/matwerk/E970529> a nfdicore:Publication ;
    rdfs:label "E. B. Tadmor, R. S. Elliott, J. P. Sethna, R. E. Miller and C. A. Becker, \"The Potential of Atomistic Simulations and the Knowledgebase of Interatomic Models\" JOM, 63, 17 (2011). doi:10.1007/s11837-011-0102-6" .

<http://demo.fiz-karlsruhe.de/matwerk/E97142> a nfdicore:Website ;
    rdfs:label "http://www.cpmd.org/"^^xsd:anyURI ;
    nfdicore:url <http://www.cpmd.org/> .

<http://demo.fiz-karlsruhe.de/matwerk/E971922> a nfdicore:Publication ;
    rdfs:label "Kim S. Exploring Chemical Information in PubChem. Curr. Protoc.; 2021 Aug 9; 1(8):e217. doi: https://doi.org/10.1002/cpz1.217." .

<http://demo.fiz-karlsruhe.de/matwerk/E973316> a nfdicore:Publication ;
    rdfs:label """M. I. Aroyo, J. M. Perez-Mato, D. Orobengoa, E. Tasci, G. de la Flor, A. Kirov
"Crystallography online: Bilbao Crystallographic Server"
Bulg. Chem. Commun. 43(2) 183-197 (2011). Scopus Web of Science
M. I. Aroyo, J. M. Perez-Mato, C. Capillas, E. Kroumova, S. Ivantchev, G. Madariaga, A. Kirov & H. Wondratschek
"Bilbao Crystallographic Server I: Databases and crystallographic computing programs"
Z. Krist. 221, 1, 15-27 (2006). doi:10.1524/zkri.2006.221.1.15
M. I. Aroyo, A. Kirov, C. Capillas, J. M. Perez-Mato & H. Wondratschek
"Bilbao Crystallographic Server II: Representations of crystallographic point groups and space groups"
Acta Cryst. A62, 115-128 (2006). doi:10.1107/S0108767305040286""" .

<http://demo.fiz-karlsruhe.de/matwerk/E974711> a nfdicore:Publication ;
    rdfs:label """Gražulis, S., Daškevič, A., Merkys, A., Chateigner, D., Lutterotti, L., Quirós, M., Serebryanaya, N. R., Moeck, P., Downs, R. T. & LeBail, A. (2012). Crystallography Open Database (COD): an open-access collection of crystal structures and platform for world-wide collaboration. Nucleic Acids Research, 40, D420-D427. doi: 10.1093/nar/gkr900 (BibTeX, EndNote/Refer, plain text)

Grazulis, S., Chateigner, D., Downs, R. T., Yokochi, A. T., Quiros, M., Lutterotti, L., Manakova, E., Butkus, J., Moeck, P. & Le Bail, A. (2009). Crystallography Open Database – an open-access collection of crystal structures. Journal of Applied Crystallography, 42, 726-729. doi: 10.1107/S0021889809016690 (BibTeX, EndNote/Refer, plain text)""" .

<http://demo.fiz-karlsruhe.de/matwerk/E97581> a nfdicore:Website ;
    rdfs:label "https://www.abinit.org/"^^xsd:anyURI ;
    nfdicore:url <https://www.abinit.org/> .

<http://demo.fiz-karlsruhe.de/matwerk/E976107> a nfdicore:Publication ;
    rdfs:label """A. Jain*, S.P. Ong*, G. Hautier, W. Chen, W.D. Richards, S. Dacek, S. Cholia, D. Gunter, D. Skinner, G. Ceder, K.A. Persson (*=equal contributions)
The Materials Project: A materials genome approach to accelerating materials innovation
APL Materials, 2013, 1(1), 011002.
doi:10.1063/1.4812323""" .

<http://demo.fiz-karlsruhe.de/matwerk/E977504> a nfdicore:Publication ;
    rdfs:label "https://www.nature.com/articles/s41597-020-00637-5"^^xsd:anyURI ;
    nfdicore:url <https://www.nature.com/articles/s41597-020-00637-5> .

<http://demo.fiz-karlsruhe.de/matwerk/E978902> a nfdicore:Publication ;
    rdfs:label "https://iopscience.iop.org/article/10.1088/2515-7639/ab13bb/meta"^^xsd:anyURI ;
    nfdicore:url <https://iopscience.iop.org/article/10.1088/2515-7639/ab13bb/meta> .

<http://demo.fiz-karlsruhe.de/matwerk/E98021> a nfdicore:Website ;
    rdfs:label "http://bigdft.org/Wiki/index.php?title=BigDFT_website"^^xsd:anyURI ;
    nfdicore:url <http://bigdft.org/Wiki/index.php?title=BigDFT_website> .

<http://demo.fiz-karlsruhe.de/matwerk/E980301> a nfdicore:Publication ;
    rdfs:label "https://www.nature.com/articles/s41524-020-00440-1"^^xsd:anyURI ;
    nfdicore:url <https://www.nature.com/articles/s41524-020-00440-1> .

<http://demo.fiz-karlsruhe.de/matwerk/E981701> a nfdicore:Publication ;
    rdfs:label """1. Saal, J. E., Kirklin, S., Aykol, M., Meredig, B., and Wolverton, C. "Materials Design and Discovery with High-Throughput Density Functional Theory: The Open Quantum Materials Database (OQMD)", JOM 65, 1501-1509 (2013). doi:10.1007/s11837-013-0755-4

2. Kirklin, S., Saal, J.E., Meredig, B., Thompson, A., Doak, J.W., Aykol, M., Rühl, S. and Wolverton, C. "The Open Quantum Materials Database (OQMD): assessing the accuracy of DFT formation energies", npj Computational Materials 1, 15010 (2015). doi:10.1038/npjcompumats.2015.10 Link
(See a list of citing articles here).""" .

<http://demo.fiz-karlsruhe.de/matwerk/E983102> a nfdicore:Publication ;
    rdfs:label "Yibin Xu, Masayoshi Yamazaki, and Pierre Villars: Inorganic Materials Database for Exploring the Nature of Material: Jpn. J. Appl. Phys. 50 (2011) 11RH02." .

<http://demo.fiz-karlsruhe.de/matwerk/E984504> a nfdicore:Publication ;
    rdfs:label """"Potential new scintillators identified by electronic structure calculations",
M. Klintenberg, S. E. Derenzo and M. J. Weber.
Nucl. Inst. Meth. A486, 298-302 (2002).

“A systematic search for new scintillators using electronic structure calculations”,
M. Klintenberg, S. E. Derenzo, and M. J. Weber.
Nanotech 2002 Vol. 2, Technical Proceedings of the 2002 International Conference on Computational Nanoscience and Nanotechnology.
PDF-version

"Data mining and accelerated electronic structure theory as a tool in the search for new functional materials",
C. Ortiz, O. Eriksson and M. Klintenberg.
Comput. Mater. Sci. 44, 1042-1049 (2009).""" .

<http://demo.fiz-karlsruhe.de/matwerk/E98462> a nfdicore:Website ;
    rdfs:label "http://www.quantum-espresso.org/"^^xsd:anyURI ;
    nfdicore:url <http://www.quantum-espresso.org/> .

<http://demo.fiz-karlsruhe.de/matwerk/E985907> a nfdicore:Publication ;
    rdfs:label """Machine-learning predictions of polymer properties with Polymer Genome
H. D. Tran, C. Kim, L. Chen, A. Chandrasekaran, R. Batra, S. Venkatram, D. Kamal, J. P. Lightstone, R. Gurnani, P. Shetty, M. Ramprasad, J. Laws, M. Shelton, R. Ramprasad, J. Appl. Phys., 128, 171104 (2020).

Polymer Genome: A data-powered polymer informatics platform for property predictions
C. Kim, A. Chandrasekaran, T. D. Huan, D. Das, R. Ramprasad, J. Phys. Chem. C 122, 31, 17575-17585 (2018).

A polymer dataset for accelerated property prediction and design
T. D. Huan, A. Mannodi-Kanakkithodi, C. Kim, V. Sharma, G. Pilania, R. Ramprasad, Sci. Data, 3 160012 (2016).""" .

<http://demo.fiz-karlsruhe.de/matwerk/E987311> a nfdicore:Publication ;
    rdfs:label """Blaiszik, B., K. Chard, J. Pruyne, R. Ananthakrishnan, S. Tuecke, and I. Foster. “The Materials Data Facility: Data Services to Advance Materials Science Research.” JOM 68, no. 8 (July 6, 2016): 2045–2052. doi:10.1007/s11837-016-2001-3. (link)
Blaiszik, Ben, Logan Ward, Marcus Schwarting, Jonathon Gaff, Ryan Chard, Daniel Pike, Kyle Chard, and Ian Foster. “A Data Ecosystem to Support Machine Learning in Materials Science.” MRS Communications (October 10, 2019): 1–9. doi:10.1557/mrc.2019.118. (link)""" .

<http://demo.fiz-karlsruhe.de/matwerk/E988716> a nfdicore:Publication ;
    rdfs:label "Pepponi G, Grazulis S, Chateigner D: “MPOD: a Material Property Open Database linked to structural information”. Nuclear Instruments and Methods in Physics Research B 284, 10-14 (2012)." .

<http://demo.fiz-karlsruhe.de/matwerk/E98904> a nfdicore:Website ;
    rdfs:label "http://cmsn.lbl.gov/html/PEtot/PEtot.html"^^xsd:anyURI ;
    nfdicore:url <http://cmsn.lbl.gov/html/PEtot/PEtot.html> .

<http://demo.fiz-karlsruhe.de/matwerk/E990122> a nfdicore:Publication ;
    rdfs:label "Topological Quantum Chemistry Nature 547, 298—305 (2017) A Complete Catalogue of High-Quality Topological Materials Nature 566, 480-485 (2019) All Topological Bands of all Nonmagnetic Stoichiometric Materials Science 376, 6595 (2022)" .

<http://demo.fiz-karlsruhe.de/matwerk/E991529> a nfdicore:Publication ;
    rdfs:label """2022. Towards improved FAIRness of the ThermoML Archive (DOI:10.1002/jcc.26842) External link: J. Comput. Chem. 2022, 43( 12), 879
2021. ThermoML/Data Archive (DOI:10.18434/mds2-2422)""" .

<http://demo.fiz-karlsruhe.de/matwerk/E992937> a nfdicore:Publication ;
    rdfs:label "K.F. Garrity, J.W. Bennett, K.M. Rabe and D. Vanderbilt, Comput. Mater. Sci. 81, 446 (2014)" .

<http://demo.fiz-karlsruhe.de/matwerk/E99347> a nfdicore:Website ;
    rdfs:label "http://jdftx.sourceforge.net/"^^xsd:anyURI ;
    nfdicore:url <http://jdftx.sourceforge.net/> .

<http://demo.fiz-karlsruhe.de/matwerk/E994346> a nfdicore:Publication ;
    rdfs:label "Andersen et al, OPTIMADE, an API for exchanging materials data, Sci. Data 8, 217 (2021) 10.1038/s41597-021-00974-z" .

<http://demo.fiz-karlsruhe.de/matwerk/E995756> a nfdicore:Publication ;
    rdfs:label "https://link.springer.com/article/10.1007/s13218-020-00648-9"^^xsd:anyURI ;
    nfdicore:url <https://link.springer.com/article/10.1007/s13218-020-00648-9> .

<http://demo.fiz-karlsruhe.de/matwerk/E997167> a nfdicore:Publication ;
    rdfs:label "https://jbiomedsem.biomedcentral.com/articles/10.1186/s13326-015-0005-5"^^xsd:anyURI ;
    nfdicore:url <https://jbiomedsem.biomedcentral.com/articles/10.1186/s13326-015-0005-5> .

<http://demo.fiz-karlsruhe.de/matwerk/E99791> a nfdicore:Website ;
    rdfs:label "http://real-space.org/"^^xsd:anyURI ;
    nfdicore:url <http://real-space.org/> .

<http://demo.fiz-karlsruhe.de/matwerk/E998579> a nfdicore:Publication ;
    rdfs:label "Thomas DG, Pappu RV, Baker NA.  NanoParticle Ontology for Cancer Nanotechnology Research.  J Biomed Inform, in press.  doi:10.1016/j.jbi.2010.03.001." .

<http://demo.fiz-karlsruhe.de/matwerk/E999992> a nfdicore:Publication ;
    rdfs:label "Austin T, Over H. MATDB ONLINE—A STANDARDS-BASED SYSTEM FOR PRESERVING, MANAGING, AND EXCHANGING ENGINEERING MATERIALS TEST DATA. DATA SCIENCE JOURNAL 11; 2012. JRC75978" .

nfdicore:Collection a owl:Class ;
    rdfs:label "collection"@en ;
    nfdicore:example "RISM catalogue of musical sources"@en ;
    rdfs:comment "A tangible collection of valuables published or curated by an organisation or a person."@en ;
    rdfs:subClassOf <http://schema.org/Product> .

nfdicore:TechnologicalMeans a owl:Class ;
    rdfs:label "technological means"@en ;
    nfdicore:example "Groovy on Grails, Angular"@en ;
    rdfs:comment "A technology, e.g. a web application or a programming framework used in a resource."@en .

nfdicore:bestPracticeOf a owl:ObjectProperty ;
    rdfs:label "best practice of"@en .

nfdicore:countryOf a owl:ObjectProperty ;
    rdfs:label "country of"@en .

nfdicore:federalStateOf a owl:ObjectProperty ;
    rdfs:label "federal state of"@en .

nfdicore:fundingOrganisationOf a owl:ObjectProperty ;
    rdfs:label "funding organisation of"@en ;
    rdfs:domain [ a owl:Class ;
            owl:unionOf ( nfdicore:Project nfdicore:Resource ) ] ;
    rdfs:subPropertyOf nfdicore:funderOf .

nfdicore:fundingProjectOf a owl:ObjectProperty ;
    rdfs:label "funding project of"@en ;
    rdfs:subPropertyOf nfdicore:funderOf .

nfdicore:locationOf a owl:ObjectProperty ;
    rdfs:label "location of"@en .

nfdicore:objectTypeOf a owl:ObjectProperty ;
    rdfs:label "object type of"@en .

nfdicore:programmingLanguageOf a owl:ObjectProperty ;
    rdfs:label "programming language of"@en .

nfdicore:publisherOf a owl:ObjectProperty ;
    rdfs:label "publisher of"@en .

nfdicore:semanticExpressivityOf a owl:ObjectProperty ;
    rdfs:label "semantic expressivity of"@en .

nfdicore:standardOf a owl:ObjectProperty ;
    rdfs:label "standard of"@en .

nfdicore:subsidiaryOrganization a owl:ObjectProperty ;
    rdfs:label "subsidiary organization"@en .

nfdicore:url a owl:DatatypeProperty ;
    rdfs:label "url"@en ;
    rdfs:comment "URL of a thing."@en ;
    rdfs:domain owl:Thing ;
    rdfs:range xsd:anyURI .

ns2:IAO_0000600 a owl:AnnotationProperty .

ns2:IAO_0000602 a owl:AnnotationProperty .

dc:contributor a owl:AnnotationProperty ;
    rdfs:label "Media Type or Extent"@en-us,
        "UDC"@en-us ;
    rdfs:isDefinedBy <http://www.udcc.org/> ;
    skos:definition "A media type or extent."@en-us,
        "The set of conceptual resources specified by the Universal Decimal Classification."@en-us .

dc:format a owl:AnnotationProperty .

dc:identifier a owl:AnnotationProperty .

dcterms:MediaType a owl:Class ;
    rdfs:label "Media Type"@en-us ;
    skos:definition "A file format or physical medium."@en-us .

mwo:GroupLeader a owl:Class ;
    rdfs:label "group leader"@en ;
    ns2:IAO_0000115 "A role which inheres in a bearer and is realized when this person holds the responsibility for the operations of a group of agents."@en ;
    ns4:hasRelatedSynonym mwo:Supervisor ;
    rdfs:comment "The responsibilities of a group leader might include, among others, guiding, motivating, supporting and coordinating the group in different scopes (i.e. scientific, administrative, financial). In scientific projects (i.e. within the NFDI context) the group in this definition will be a research group, institute or department. In most cases the group leader is also the supervisor to the group"@en ;
    rdfs:subClassOf ns2:BFO_0000023 .

mwo:ParticipantProject a owl:Class ;
    rdfs:subClassOf default1:Project .

mwo:ProjectManager a owl:Class ;
    rdfs:label "project manager"@en ;
    ns2:IAO_0000115 "A role which inheres in a bearer and is realized when that person is responsible for 1) helping to define the project scope, goals and deliverables, 2) taking care of the budget, documentation and staffing, 3) reporting and documenting the progress, and 4) managing a project and meeting deadlines."@en ;
    ns4:hasDbXref <https://www.indeed.com/career-advice/finding-a-job/project-leader-vs-project-manager> ;
    rdfs:subClassOf ns2:BFO_0000023 .

mwo:ProjectMember a owl:Class ;
    rdfs:label "project member"@en ;
    ns2:IAO_0000115 "A role which inheres in a bearer and is realized when this bearer participates in the planning, operation or dissemination of a project."@en ;
    rdfs:subClassOf ns2:BFO_0000023 .

mwo:Supervisor a owl:Class ;
    rdfs:label "supervisor"@en ;
    ns2:IAO_0000115 "A role which inheres in a bearer and is realized when a person is responsible for 1) the coordination  and 2) the operations of another person, group or department."@en ;
    rdfs:comment "In a project with more than one member, the project leader might engage, motivate and support the team by establishing and maintaining productive operations. Note that a project leader is not necessarily the group leader."@en ;
    rdfs:subClassOf ns2:BFO_0000023 .

mwo:WebService a owl:Class ;
    rdfs:label "web service"@en ;
    ns2:IAO_0000115 "A service that supports interoperable machine-to-machine interaction over a network."@en ;
    rdfs:subClassOf <http://schema.org/Service> ;
    owl:equivalentClass <http://www.ebi.ac.uk/swo/interface/SWO_9000051> .

mwo:hasAuthor a owl:ObjectProperty ;
    rdfs:label "has author"@en ;
    ns2:IAO_0000115 "A relation between a resource and a person, who is the author."@en ;
    rdfs:domain nfdicore:Resource ;
    rdfs:range nfdicore:Person .

mwo:hasPostalAddress a owl:DatatypeProperty ;
    rdfs:label "has postal address"@en ;
    ns2:IAO_0000115 "A data property indicating the postal address of an entity."@en ;
    rdfs:domain [ a owl:Class ;
            owl:unionOf ( nfdicore:Organization nfdicore:Person ) ] .

mwo:isContributorOf a owl:ObjectProperty ;
    rdfs:label "is contributor of"@en ;
    ns2:IAO_0000115 "A relation between an organization or person and the resource of which it is a contributor."@en ;
    rdfs:domain [ a owl:Class ;
            owl:unionOf ( nfdicore:Organization nfdicore:Person ) ] ;
    rdfs:range nfdicore:Resource .

mwo:isLeaderOf a owl:ObjectProperty ;
    rdfs:label "is leader of"@en .

mwo:memberOf a owl:ObjectProperty ;
    rdfs:label "member of"@en .

<http://schema.org/Organization> a owl:Class ;
    rdfs:label "Organization"@en ;
    rdfs:comment "An organization such as a school, NGO, corporation, club, etc."@en .

<http://schema.org/Person> a owl:Class .

<http://schema.org/Project> a owl:Class ;
    rdfs:label "Project"@en ;
    rdfs:comment "An enterprise (potentially individual but typically collaborative), planned to achieve a particular aim. Use properties from Organization, subOrganization/parentOrganization to indicate project sub-structures."@en .

ns3:SWO_0000157 a owl:ObjectProperty ;
    rdfs:label "is software for"@en ;
    rdfs:domain ns3:SWO_0000001 ;
    rdfs:range ns3:SWO_0000001 .

ns3:has_license a owl:ObjectProperty ;
    rdfs:label "has license" ;
    ns2:IAO_0000115 "The relationship between an entity and the set of legal restrictions, i.e. license, which are applied in using or otherwise interacting with that entity. Eg. relationship between software and a software license." ;
    rdfs:domain nfdicore:Resource ;
    rdfs:range ns3:SWO_0000002 ;
    owl:inverseOf ns3:is_license_for .

<http://www.ebi.ac.uk/swo/interface/SWO_9000051> a owl:Class ;
    rdfs:label "web service" ;
    ns2:IAO_0000115 "A web service is a software interface which works as a method of communication between two electronic devices over the World Wide Web and which is provided at a particular network address. There are two major classes of Web services: REST-compliant Web services, and arbitrary (or application-specific) Web services." ;
    ns2:IAO_0000118 "Web Service" ;
    ns2:IAO_0000119 "Modified from http://www.w3.org/TR/ws-arch/, accessed 6 June 2013; Modified from http://en.wikipedia.org/wiki/Web_service, accessed 6 June 2013." ;
    dcterms:creator "Allyson Lister" ;
    rdfs:subClassOf ns3:SWO_9000050 .

ns3:is_license_for a owl:ObjectProperty ;
    rdfs:label "is license for"@en ;
    ns2:IAO_0000115 "The relationship between an entity and the set of legal restrictions, i.e. license, which are applied in using or otherwise interacting with that entity. Eg. relationship between a software license and the software which implements it." .

<http://www.ebi.ac.uk/swo/license/SWO_1000008> a owl:Class ;
    rdfs:label "Open source software license" ;
    rdfs:subClassOf ns3:SWO_0000002 .

<http://www.ebi.ac.uk/swo/license/SWO_1000103> a owl:Class ;
    rdfs:label "Vendor-specific License"@en ;
    ns2:IAO_0000115 "A vendor-specific license is a license which was, at least originally, created by a specific organization to be used just on the resources created within that organization. This is a hierarchy of convenience rather than of shared philosophy. Many of the licenses have since been taken up by other groups whose licensing requirements matched those of the originating organization." ;
    ns2:IAO_0000119 "Allyson Lister" ;
    dcterms:creator "Allyson Lister" ;
    rdfs:subClassOf ns3:SWO_0000002 .

default1:Person a owl:Class ;
    rdfs:label "person"@en ;
    rdfs:comment "A resource that represents a single person."@en ;
    default1:example "Harald Sack, Tabea Tietz, Sasha Bruns, Etienne Posthumus" .

default1:fundingOrganizationOf a owl:ObjectProperty ;
    rdfs:label "funding organization of"@en .

default1:fundingProjectOf a owl:ObjectProperty ;
    rdfs:label "funding project of"@en .

schema:dateCreated a owl:DatatypeProperty ;
    rdfs:label "dateCreated"@en ;
    rdfs:comment "The date on which the CreativeWork was created or the item was added to a DataFeed."@en ;
    rdfs:domain nfdicore:Resource ;
    rdfs:isDefinedBy schema:dateCreated .

schema:datePublished a owl:DatatypeProperty ;
    rdfs:label "datePublished"@en ;
    rdfs:comment "Date of first broadcast/publication."@en ;
    rdfs:domain nfdicore:Resource ;
    rdfs:isDefinedBy schema:datePublished .

schema:free a owl:DatatypeProperty ;
    rdfs:label "free"@en ;
    rdfs:comment "A flag to signal that the item, event, or place is accessible for free."@en ;
    rdfs:domain [ a owl:Class ;
            owl:unionOf ( nfdicore:Resource ns1:OrganisedEvent ) ] ;
    rdfs:isDefinedBy schema:free .

schema:operatingSystem a owl:ObjectProperty ;
    rdfs:label "operatingSystem"@en ;
    rdfs:comment "Operating systems supported (Windows 7, OS X 10.6, Android 1.6)."@en ;
    rdfs:domain nfdicore:Software ;
    rdfs:isDefinedBy schema:operatingSystem ;
    rdfs:range ns3:SWO_0000021 .

schema:sponsor a owl:ObjectProperty ;
    rdfs:label "sponsor"@en ;
    rdfs:comment "A person or organization that supports a thing through a pledge, promise, or financial contribution. E.g. a sponsor of a Medical Study or a corporate sponsor of an event."@en ;
    rdfs:domain ns1:OrganisedEvent ;
    rdfs:isDefinedBy schema:sponsor ;
    rdfs:range [ a owl:Class ;
            owl:unionOf ( nfdicore:Organization nfdicore:Person ) ] .

ns1:endDate a owl:DatatypeProperty ;
    rdfs:label "end date"@en ;
    rdfs:comment "end date"@en ;
    rdfs:domain ns1:OrganisedEvent .

ns1:hasPart a owl:ObjectProperty ;
    rdfs:label "has part"@en ;
    rdfs:comment "has part"@en ;
    rdfs:domain owl:Thing ;
    rdfs:range owl:Thing ;
    owl:inverseOf ns1:isPartOf .

ns1:hasSubEvent a owl:ObjectProperty ;
    rdfs:label "has sub event"@en ;
    rdfs:comment "has sub event"@en ;
    rdfs:domain ns1:OrganisedEvent ;
    rdfs:range ns1:OrganisedEvent ;
    rdfs:subPropertyOf ns1:hasPart ;
    owl:inverseOf ns1:isSubEventOf .

ns1:isSubEventOf a owl:ObjectProperty ;
    rdfs:label "is sub event of"@en ;
    rdfs:comment "is sub event of"@en ;
    rdfs:subPropertyOf ns1:isPartOf .

ns1:startDate a owl:DatatypeProperty ;
    rdfs:label "start date"@en ;
    rdfs:comment "start date"@en ;
    rdfs:domain ns1:OrganisedEvent .

<https://w3id.org/seo#InvitedSpeakers> a owl:Class ;
    rdfs:label "Invited speakers"@en ;
    rdfs:comment "Invited person to give a speech in an event."@en ;
    rdfs:subClassOf nfdicore:Person .

modsci:ModernScience a owl:Class ;
    rdfs:label "Science" ;
    rdfs:comment "Science is a systematic enterprise that builds and organizes knowledge in the form of testable explanations and predictions about the universe." .

modsci:ProgrammingLanguage a owl:Class ;
    rdfs:label "Programming Language" ;
    rdfs:comment "A programming language is a formal language, which comprises a set of instructions that produce various kinds of output. Programming languages are used in computer programming to implement algorithms." ;
    rdfs:subClassOf <http://schema.org/ComputerLanguage> .

modsci:isManufacturerOf a owl:ObjectProperty ;
    rdfs:label "is manufacturer of"@en .

<http://demo.fiz-karlsruhe.de/matwerk/E10181> a nfdicore:Person ;
    rdfs:label "Ahmad Zainul Ihsan" ;
    mwo:emailAddress "a.ihsan@fz-juelich.de"^^xsd:string ;
    mwo:hasAffiliation <http://demo.fiz-karlsruhe.de/matwerk/E1022> ;
    mwo:hasExpertiseIn <http://demo.fiz-karlsruhe.de/matwerk/E39504> ;
    mwo:hasORCID <https://orcid.org/0000-0002-1008-4530> ;
    foaf:firstName "Ahmad Zainul"^^xsd:string ;
    foaf:surname "Ihsan"^^xsd:string .

<http://demo.fiz-karlsruhe.de/matwerk/E102026> a nfdicore:Website,
        mwo:Documentation ;
    rdfs:label "https://docs.dftk.org/stable/"^^xsd:anyURI ;
    nfdicore:url <https://docs.dftk.org/stable/> .

<http://demo.fiz-karlsruhe.de/matwerk/E1056> a nfdicore:Organization ;
    rdfs:label "Institute for Lightweight Design with Hybrid Systems",
        "Institut für Leichtbau mit Hybridsystemen"@de ;
    nfdicore:location <http://demo.fiz-karlsruhe.de/matwerk/E74921> ;
    nfdicore:parentOrganisation <http://demo.fiz-karlsruhe.de/matwerk/E2831> ;
    mwo:hasAcronym "ILH"^^xsd:string ;
    mwo:hasPostalCode "33098" ;
    mwo:hasWebsite <http://demo.fiz-karlsruhe.de/matwerk/E84437> .

<http://demo.fiz-karlsruhe.de/matwerk/E1114779> a modsci:ScientificInstrumentManufacturer ;
    rdfs:label "ProCon X-ray" .

<http://demo.fiz-karlsruhe.de/matwerk/E1181417> a emmo:EMMO_4207e895_8b83_4318_996a_72cfb32acd94 ;
    rdfs:label "Al-alloy" .

<http://demo.fiz-karlsruhe.de/matwerk/E1196832> a nfdicore:ObjectType ;
    rdfs:label "Image data" .

<http://demo.fiz-karlsruhe.de/matwerk/E1210791> a nfdicore:ObjectType ;
    rdfs:label "specimens" .

<http://demo.fiz-karlsruhe.de/matwerk/E1212347> a nfdicore:ObjectType ;
    rdfs:label "equipment" .

<http://demo.fiz-karlsruhe.de/matwerk/E12176> a nfdicore:Person ;
    rdfs:label "Prof. Dr. Alexander Hartmaier" ;
    mwo:emailAddress "alexander.hartmaier@rub.de"^^xsd:string ;
    mwo:hasAffiliation <http://demo.fiz-karlsruhe.de/matwerk/E1037> ;
    mwo:hasExpertiseIn <http://demo.fiz-karlsruhe.de/matwerk/E65262>,
        <http://demo.fiz-karlsruhe.de/matwerk/E65981> ;
    mwo:hasORCID <https://orcid.org/0000-0002-3710-1169> ;
    owl:sameAs <http://www.wikidata.org/entity/Q58577033> ;
    foaf:depiction <https://ams3.digitaloceanspaces.com/externalpublic/57/b3baa1ff-f648-448b-ae25-efcf9af06eb6/conversions/7572fa20-fb72-496e-a201-1ec105cb4b58-md.jpg?X-Amz-Content-Sha256=UNSIGNED-PAYLOAD&X-Amz-Algorithm=AWS4-HMAC-SHA256&X-Amz-Credential=KVC4ZMO47JLTBHVHEFZ4%2F20230512%2Fams3%2Fs3%2Faws4_request&X-Amz-Date=20230512T150442Z&X-Amz-SignedHeaders=host&X-Amz-Expires=7200&X-Amz-Signature=83236b80e40332e8e39d451d985888a67254f88074d4ca3247ce1b55dceb3acf> ;
    foaf:firstName "Alexander"^^xsd:string ;
    foaf:surname "Hartmaier"^^xsd:string ;
    foaf:title "Prof. Dr."^^xsd:string .

<http://demo.fiz-karlsruhe.de/matwerk/E1231097> a ns3:SWO_0000001 ;
    rdfs:label "paraview" .

<http://demo.fiz-karlsruhe.de/matwerk/E1234236> a nfdicore:Resource,
        ns3:SWO_0000001 ;
    rdfs:label "Aiida" .

<http://demo.fiz-karlsruhe.de/matwerk/E1242101> a ns3:SWO_0000001 ;
    rdfs:label "Sphinx" .

<http://demo.fiz-karlsruhe.de/matwerk/E1245575> a nfdicore:Person ;
    rdfs:label "Dr.-Ing. Hanna Tsybenko" ;
    mwo:emailAddress "h.tsybenko@fz-juelich.de"^^xsd:string ;
    mwo:hasAffiliation <http://demo.fiz-karlsruhe.de/matwerk/E1022> ;
    mwo:hasExpertiseIn <http://demo.fiz-karlsruhe.de/matwerk/E1245665> ;
    mwo:hasORCID <https://orcid.org/0000-0001-7691-2856> ;
    foaf:firstName "Hanna"^^xsd:string ;
    foaf:surname "Tsybenko"^^xsd:string ;
    foaf:title "Dr.-Ing."^^xsd:string .

<http://demo.fiz-karlsruhe.de/matwerk/E1246495> a mwo:Repository ;
    rdfs:label "https://gitlab.mpcdf.mpg.de/pyiron/iuc09_demonstrator"^^xsd:anyURI ;
    nfdicore:url <https://gitlab.mpcdf.mpg.de/pyiron/iuc09_demonstrator> .

<http://demo.fiz-karlsruhe.de/matwerk/E1246837> a ns3:SWO_0000002 ;
    rdfs:label "GPL 3 License" .

<http://demo.fiz-karlsruhe.de/matwerk/E1246983> a mwo:Method ;
    rdfs:label "Modified Embedded Atom Method" .

<http://demo.fiz-karlsruhe.de/matwerk/E1247062> a nfdicore:Project,
        nfdicore:fundingProject ;
    rdfs:label "FAIRmat" .

<http://demo.fiz-karlsruhe.de/matwerk/E1247370> a nfdicore:Dataset,
        nfdicore:Resource ;
    rdfs:label "Aluminum Elastic Modulus" ;
    nfdicore:fileExtension ".eln" ;
    mwo:aboutMaterial <http://demo.fiz-karlsruhe.de/matwerk/E1247872> ;
    mwo:description "an EN AW 1050A sample is polished and indented and the load-displacement curve is recorded, which is used to calculate the Young's modulus according to the Oliver-Pharr Method. Afterwards the surface height profile is measured. " ;
    mwo:hasCreator <http://demo.fiz-karlsruhe.de/matwerk/E1245575> ;
    mwo:hasDiscipline <http://demo.fiz-karlsruhe.de/matwerk/E1245665> ;
    mwo:hasRelatedResource <http://demo.fiz-karlsruhe.de/matwerk/E1247727>,
        <http://demo.fiz-karlsruhe.de/matwerk/E1247866> ;
    mwo:hasRepository <http://demo.fiz-karlsruhe.de/matwerk/E1247673> ;
    mwo:keyword "Aluminium",
        "Elastic Constants",
        "Indentation",
        "Young's modulus" ;
    mwo:usesMethod <http://demo.fiz-karlsruhe.de/matwerk/E1247857> ;
    ns3:has_license <http://demo.fiz-karlsruhe.de/matwerk/E1247861> ;
    schema:dateCreated "20:23:00-03:00"^^xsd:time ;
    schema:datePublished "2023-04-20T00:00:00.000Z" .

<http://demo.fiz-karlsruhe.de/matwerk/E1247467> a nfdicore:Resource ;
    rdfs:label "https://doi.org/10.25910/yk0y-0217"^^xsd:anyURI ;
    nfdicore:url <https://doi.org/10.25910/yk0y-0217> .

<http://demo.fiz-karlsruhe.de/matwerk/E1247518> a nfdicore:Organization ;
    rdfs:label "https://ror.org/02nv7yv05"^^xsd:anyURI ;
    nfdicore:url <https://ror.org/02nv7yv05> .

<http://demo.fiz-karlsruhe.de/matwerk/E1247671> a nfdicore:Country ;
    rdfs:label "FZJ" .

<http://demo.fiz-karlsruhe.de/matwerk/E1247673> a mwo:Repository ;
    rdfs:label "https://git.rwth-aachen.de/nfdi-matwerk/ta-wsd/user-journey-indentation/-/tree/main/Indentation"^^xsd:anyURI ;
    nfdicore:url <https://git.rwth-aachen.de/nfdi-matwerk/ta-wsd/user-journey-indentation/-/tree/main/Indentation> .

<http://demo.fiz-karlsruhe.de/matwerk/E1247763> a nfdicore:Person ;
    mwo:emailAddress "yusra.shakeel@kit.edu"^^xsd:string ;
    mwo:hasAffiliation <http://demo.fiz-karlsruhe.de/matwerk/E1247777> ;
    foaf:firstName """
Yusra"""^^xsd:string ;
    foaf:surname "Shakeel"^^xsd:string .

<http://demo.fiz-karlsruhe.de/matwerk/E1247825> a dcterms:FileFormat ;
    rdfs:label ".json" .

<http://demo.fiz-karlsruhe.de/matwerk/E1247844> a mwo:Documentation,
        mwo:Repository ;
    rdfs:label "https://doi.org/10.5281/zenodo.7625259"^^xsd:anyURI ;
    nfdicore:url <https://doi.org/10.5281/zenodo.7625259> .

<http://demo.fiz-karlsruhe.de/matwerk/E1247857> a mwo:Method ;
    rdfs:label "Oliver-Pharr Method" .

<http://demo.fiz-karlsruhe.de/matwerk/E1247861> a <http://www.ebi.ac.uk/swo/license/SWO_1000001> ;
    rdfs:label "CC BY 4.0" .

<http://demo.fiz-karlsruhe.de/matwerk/E1247866> a nfdicore:Resource ;
    rdfs:label "PASTA ELN" .

<http://demo.fiz-karlsruhe.de/matwerk/E1247872> a emmo:EMMO_4207e895_8b83_4318_996a_72cfb32acd94 ;
    rdfs:label "Aluminium" .

<http://demo.fiz-karlsruhe.de/matwerk/E1247880> rdfs:label "Strategy Development" ;
    dcterms:isPartOf <http://demo.fiz-karlsruhe.de/matwerk/E1247022> ;
    mwo:description "This TA is responsible for managing the development of a digital strategy for our consortium and the MSE community." ;
    mwo:hasWorkPackage <http://demo.fiz-karlsruhe.de/matwerk/E1247895>,
        <http://demo.fiz-karlsruhe.de/matwerk/E1247901> .

<http://demo.fiz-karlsruhe.de/matwerk/E1247947> rdfs:label "Method development for mechanical joinability in versatile process chains" .

<http://demo.fiz-karlsruhe.de/matwerk/E1247968> rdfs:label "Bundesanstalt für Materialforschung und -prüfung (BAM)" .

<http://demo.fiz-karlsruhe.de/matwerk/E1247975> rdfs:label "Physikalisch-Technische-Bundesanstalt - Persistent Identifiers (PTB)" .

<http://demo.fiz-karlsruhe.de/matwerk/E1248137> rdfs:label "Working group modeling of oxygen-free production" .

<http://demo.fiz-karlsruhe.de/matwerk/E1248247> rdfs:label "Metadata in Nanoindentation and Micromechanics" .

<http://demo.fiz-karlsruhe.de/matwerk/E1248272> rdfs:label "Profile Area Advanced Materials Engineering TU Kaiserslautern" .

<http://demo.fiz-karlsruhe.de/matwerk/E1248325> rdfs:label "Data Science in MSE education, qualification and life-long learning" .

<http://demo.fiz-karlsruhe.de/matwerk/E1352> a nfdicore:Organization ;
    rdfs:label "German Research Center for Artificial Intelligence",
        "Deutsches Forschungszentrum für Künstliche Intelligenz"@de ;
    nfdicore:location <http://demo.fiz-karlsruhe.de/matwerk/E73391> ;
    mwo:hasAcronym "DFKI"^^xsd:string ;
    mwo:hasPostalCode "D-66123" ;
    mwo:hasWebsite <http://demo.fiz-karlsruhe.de/matwerk/E90677> .

<http://demo.fiz-karlsruhe.de/matwerk/E154182> a nfdicore:Website,
        mwo:Repository ;
    rdfs:label "https://github.com/usnistgov/MDCS"^^xsd:anyURI ;
    nfdicore:url <https://github.com/usnistgov/MDCS> .

<http://demo.fiz-karlsruhe.de/matwerk/E16754> a nfdicore:Person ;
    mwo:hasAffiliation <http://demo.fiz-karlsruhe.de/matwerk/E5852> ;
    foaf:firstName "Julian"^^xsd:string ;
    foaf:surname "Lißner"^^xsd:string .

<http://demo.fiz-karlsruhe.de/matwerk/E212576> a mwo:Repository ;
    rdfs:label "https://gitlab.com/iam-cms/kadi-apy"^^xsd:anyURI ;
    nfdicore:url <https://gitlab.com/iam-cms/kadi-apy> .

<http://demo.fiz-karlsruhe.de/matwerk/E2597> a nfdicore:Organization ;
    rdfs:label "Leibniz-Gemeinschaft" ;
    mwo:hasRORID "https://ror.org/01xc6bj88",
        "https://ror.org/0387prb75" ;
    owl:sameAs <http://www.wikidata.org/entity/Q1388737>,
        <http://www.wikidata.org/entity/Q1665037> .

<http://demo.fiz-karlsruhe.de/matwerk/E2654> a nfdicore:Organization ;
    rdfs:label "Helmholtz-Gemeinschaft" ;
    mwo:hasRORID "https://ror.org/02nv7yv05",
        "https://ror.org/04t3en479" ;
    owl:sameAs <http://www.wikidata.org/entity/Q309988>,
        <http://www.wikidata.org/entity/Q697111> .

<http://demo.fiz-karlsruhe.de/matwerk/E29921> a nfdicore:Person ;
    rdfs:label "Prof. Dr. Stefan Sandfeld" ;
    mwo:emailAddress "s.sandfeld@fz-juelich.de"^^xsd:string ;
    mwo:hasAffiliation <http://demo.fiz-karlsruhe.de/matwerk/E1022> ;
    mwo:hasExpertiseIn <http://demo.fiz-karlsruhe.de/matwerk/E39504> ;
    mwo:hasORCID <https://orcid.org/0000-0001-9560-4728> ;
    owl:sameAs <http://www.wikidata.org/entity/Q60700659> ;
    foaf:firstName "Stefan"^^xsd:string ;
    foaf:surname "Sandfeld"^^xsd:string ;
    foaf:title "Prof. Dr."^^xsd:string .

<http://demo.fiz-karlsruhe.de/matwerk/E3017> a nfdicore:Organization ;
    rdfs:label "Albert-Ludwigs-Universität Freiburg" ;
    mwo:hasAcronym "Uni-Freiburg"^^xsd:string ;
    mwo:hasRORID "https://ror.org/0245cg223" ;
    owl:sameAs <http://www.wikidata.org/entity/Q153987> .

<http://demo.fiz-karlsruhe.de/matwerk/E3146> a nfdicore:Organization ;
    rdfs:label "TU Kaiserslautern" ;
    mwo:hasRORID "https://ror.org/04zrf7b53" ;
    owl:sameAs <http://www.wikidata.org/entity/Q678965> .

<http://demo.fiz-karlsruhe.de/matwerk/E32376> a nfdicore:Person ;
    rdfs:label "Oliver Weeger" ;
    mwo:hasAffiliation <http://demo.fiz-karlsruhe.de/matwerk/E8141> ;
    foaf:firstName "Oliver"^^xsd:string ;
    foaf:surname "Weeger"^^xsd:string .

<http://demo.fiz-karlsruhe.de/matwerk/E32627> a nfdicore:Person ;
    rdfs:label "Frederik Larsson" ;
    mwo:hasAffiliation <http://demo.fiz-karlsruhe.de/matwerk/E8261> ;
    foaf:firstName "Frederik"^^xsd:string ;
    foaf:surname "Larsson"^^xsd:string .

<http://demo.fiz-karlsruhe.de/matwerk/E33132> a nfdicore:Person ;
    rdfs:label "Christian Rockenhäuser" ;
    mwo:hasAffiliation <http://demo.fiz-karlsruhe.de/matwerk/E1245619>,
        <http://demo.fiz-karlsruhe.de/matwerk/E1245640> ;
    foaf:firstName "Christian"^^xsd:string ;
    foaf:surname "Rockenhäuser"^^xsd:string .

<http://demo.fiz-karlsruhe.de/matwerk/E34671> a nfdicore:Person ;
    mwo:hasAffiliation <http://demo.fiz-karlsruhe.de/matwerk/E1037> ;
    foaf:firstName "Ralf"^^xsd:string ;
    foaf:surname "Drautz"^^xsd:string .

<http://demo.fiz-karlsruhe.de/matwerk/E3486> a nfdicore:Organization ;
    rdfs:label "Humboldt-Universität zu Berlin" ;
    nfdicore:location <http://demo.fiz-karlsruhe.de/matwerk/E72632> .

<http://demo.fiz-karlsruhe.de/matwerk/E35454> a nfdicore:Person ;
    mwo:hasAffiliation <http://demo.fiz-karlsruhe.de/matwerk/E1037> ;
    foaf:firstName "Yury"^^xsd:string ;
    foaf:surname "Lysogorskiy"^^xsd:string .

<http://demo.fiz-karlsruhe.de/matwerk/E37857> a nfdicore:AcademicDiscipline ;
    rdfs:label "Deformation processes and mechanical behavior" .

<http://demo.fiz-karlsruhe.de/matwerk/E406451> a nfdicore:Website ;
    rdfs:label "internal only" .

<http://demo.fiz-karlsruhe.de/matwerk/E422822> a nfdicore:Resource,
        nfdicore:Software,
        mwo:ProcessingSoftware,
        mwo:ResearchSoftware,
        mwo:VisualizationSoftware ;
    rdfs:label "Fiji" ;
    nfdicore:programmingLanguage <http://demo.fiz-karlsruhe.de/matwerk/E833696>,
        <http://demo.fiz-karlsruhe.de/matwerk/E834987>,
        <http://demo.fiz-karlsruhe.de/matwerk/E836279>,
        <http://demo.fiz-karlsruhe.de/matwerk/E837572>,
        <http://demo.fiz-karlsruhe.de/matwerk/E838866> ;
    dcterms:description "Fiji is an image processing package—a “batteries-included” distribution of ImageJ2, bundling a lot of plugins which facilitate scientific image analysis."^^xsd:string ;
    mwo:hasDiscipline <http://demo.fiz-karlsruhe.de/matwerk/E68897>,
        <http://demo.fiz-karlsruhe.de/matwerk/E69266>,
        <http://demo.fiz-karlsruhe.de/matwerk/E70007> ;
    mwo:hasDocumentation <http://demo.fiz-karlsruhe.de/matwerk/E245651> ;
    mwo:hasRelatedResource <http://demo.fiz-karlsruhe.de/matwerk/E636629>,
        <http://demo.fiz-karlsruhe.de/matwerk/E637757> ;
    mwo:hasRepository <http://demo.fiz-karlsruhe.de/matwerk/E164307> ;
    mwo:hasVersion "2.5.0" ;
    mwo:hasWebsite <http://demo.fiz-karlsruhe.de/matwerk/E94962> ;
    ns3:has_license <http://demo.fiz-karlsruhe.de/matwerk/E749477> ;
    owl:sameAs <http://www.wikidata.org/entity/Q5425748> .

<http://demo.fiz-karlsruhe.de/matwerk/E4571> a nfdicore:Country ;
    rdfs:label "BAM" .

<http://demo.fiz-karlsruhe.de/matwerk/E49206> a nfdicore:AcademicDiscipline ;
    rdfs:label "Lightweight systems" .

<http://demo.fiz-karlsruhe.de/matwerk/E5852> a nfdicore:Organization .

<http://demo.fiz-karlsruhe.de/matwerk/E5951> a nfdicore:Organization .

<http://demo.fiz-karlsruhe.de/matwerk/E61379> a nfdicore:AcademicDiscipline ;
    rdfs:label "Molecular Dynamics (MD)" .

<http://demo.fiz-karlsruhe.de/matwerk/E622056> a nfdicore:AcademicDiscipline,
        mwo:Method ;
    rdfs:label "crystal plasticity" .

<http://demo.fiz-karlsruhe.de/matwerk/E62426> a nfdicore:AcademicDiscipline,
        modsci:Technology ;
    rdfs:label "X-ray computed tomography" ;
    owl:sameAs <http://www.wikidata.org/entity/Q32566> .

<http://demo.fiz-karlsruhe.de/matwerk/E625404> a mwo:Method ;
    rdfs:label "Transmission electron microscopy" .

<http://demo.fiz-karlsruhe.de/matwerk/E636629> a nfdicore:Resource,
        nfdicore:Software,
        mwo:ProcessingSoftware,
        mwo:ResearchSoftware,
        mwo:VisualizationSoftware ;
    rdfs:label "ImageJ2" ;
    nfdicore:programmingLanguage <http://demo.fiz-karlsruhe.de/matwerk/E833696>,
        <http://demo.fiz-karlsruhe.de/matwerk/E834987>,
        <http://demo.fiz-karlsruhe.de/matwerk/E840161> ;
    dcterms:description "ImageJ2 is a new version of ImageJ for multidimensional image data, with a focus on scientific imaging. It includes some additional features not available in the original ImageJ."^^xsd:string ;
    mwo:hasDiscipline <http://demo.fiz-karlsruhe.de/matwerk/E68897>,
        <http://demo.fiz-karlsruhe.de/matwerk/E69266>,
        <http://demo.fiz-karlsruhe.de/matwerk/E70007> ;
    mwo:hasDocumentation <http://demo.fiz-karlsruhe.de/matwerk/E245651> ;
    mwo:hasRelatedResource <http://demo.fiz-karlsruhe.de/matwerk/E422822>,
        <http://demo.fiz-karlsruhe.de/matwerk/E637757> ;
    mwo:hasRepository <http://demo.fiz-karlsruhe.de/matwerk/E165452> ;
    mwo:hasVersion "2.5.0" ;
    mwo:hasWebsite <http://demo.fiz-karlsruhe.de/matwerk/E95831> ;
    ns3:has_license <http://demo.fiz-karlsruhe.de/matwerk/E751926> .

<http://demo.fiz-karlsruhe.de/matwerk/E637757> a nfdicore:Resource,
        nfdicore:Software,
        mwo:ProcessingSoftware,
        mwo:ResearchSoftware,
        mwo:VisualizationSoftware ;
    rdfs:label "ImageJ" ;
    nfdicore:programmingLanguage <http://demo.fiz-karlsruhe.de/matwerk/E833696> ;
    dcterms:description "ImageJ is public domain software for processing and analyzing scientific images."^^xsd:string ;
    mwo:hasDiscipline <http://demo.fiz-karlsruhe.de/matwerk/E68897>,
        <http://demo.fiz-karlsruhe.de/matwerk/E69266>,
        <http://demo.fiz-karlsruhe.de/matwerk/E70007> ;
    mwo:hasDocumentation <http://demo.fiz-karlsruhe.de/matwerk/E245651> ;
    mwo:hasRelatedResource <http://demo.fiz-karlsruhe.de/matwerk/E422822>,
        <http://demo.fiz-karlsruhe.de/matwerk/E636629> ;
    mwo:hasRepository <http://demo.fiz-karlsruhe.de/matwerk/E164879> ;
    mwo:hasVersion "1.53s" ;
    mwo:hasWebsite <http://demo.fiz-karlsruhe.de/matwerk/E95396> ;
    ns3:has_license <http://demo.fiz-karlsruhe.de/matwerk/E750701> ;
    owl:sameAs <http://www.wikidata.org/entity/Q1659584> .

<http://demo.fiz-karlsruhe.de/matwerk/E652512> a nfdicore:Resource ;
    rdfs:label "pymatgen" .

<http://demo.fiz-karlsruhe.de/matwerk/E66342> a nfdicore:AcademicDiscipline ;
    rdfs:label "Research data infrastructure" ;
    owl:sameAs <http://www.wikidata.org/entity/Q96678462> .

<http://demo.fiz-karlsruhe.de/matwerk/E67067> a nfdicore:AcademicDiscipline ;
    rdfs:label "Computational mathematics" ;
    owl:sameAs <http://www.wikidata.org/entity/Q1122491> .

<http://demo.fiz-karlsruhe.de/matwerk/E689552> a mwo:ContactPoint ;
    rdfs:label "support@kitware.com" ;
    mwo:emailAddress "support@kitware.com"^^xsd:string ;
    mwo:hasWebsite <http://demo.fiz-karlsruhe.de/matwerk/E231861> .

<http://demo.fiz-karlsruhe.de/matwerk/E71877> a nfdicore:City ;
    rdfs:label "Dusseldorf" ;
    nfdicore:country <http://demo.fiz-karlsruhe.de/matwerk/E80004> ;
    owl:sameAs <http://www.wikidata.org/entity/Q1718> .

<http://demo.fiz-karlsruhe.de/matwerk/E72254> a nfdicore:City,
        nfdicore:Organization ;
    rdfs:label "Stuttgart" ;
    nfdicore:country <http://demo.fiz-karlsruhe.de/matwerk/E80004> ;
    owl:sameAs <http://www.wikidata.org/entity/Q79844> .

<http://demo.fiz-karlsruhe.de/matwerk/E722802> a mwo:ContactPoint ;
    rdfs:label "cod-bugs@ibt.lt" ;
    mwo:emailAddress "cod-bugs@ibt.lt"^^xsd:string .

<http://demo.fiz-karlsruhe.de/matwerk/E73391> a nfdicore:City ;
    rdfs:label "Saarbrücken" ;
    nfdicore:country <http://demo.fiz-karlsruhe.de/matwerk/E80004> ;
    owl:sameAs <http://www.wikidata.org/entity/Q1724> .

<http://demo.fiz-karlsruhe.de/matwerk/E73772> a nfdicore:City ;
    rdfs:label "Eggenstein-Leopoldshafen" ;
    nfdicore:country <http://demo.fiz-karlsruhe.de/matwerk/E80004> ;
    owl:sameAs <http://www.wikidata.org/entity/Q31984149> .

<http://demo.fiz-karlsruhe.de/matwerk/E747032> a <http://www.ebi.ac.uk/swo/license/SWO_1000061> ;
    rdfs:label "BSD" ;
    owl:sameAs <http://www.wikidata.org/entity/Q191307> .

<http://demo.fiz-karlsruhe.de/matwerk/E753152> a <http://www.ebi.ac.uk/swo/license/SWO_1000002> ;
    rdfs:label "Propietary academic license" .

<http://demo.fiz-karlsruhe.de/matwerk/E7556> a nfdicore:Organization ;
    rdfs:label "Institute of Mechanics"@de .

<http://demo.fiz-karlsruhe.de/matwerk/E76467> a nfdicore:City ;
    rdfs:label "Karlsruhe" ;
    nfdicore:country <http://demo.fiz-karlsruhe.de/matwerk/E80004> ;
    owl:sameAs <http://www.wikidata.org/entity/Q1026577> .

<http://demo.fiz-karlsruhe.de/matwerk/E77246> a nfdicore:City ;
    rdfs:label "Kaiserslautern" ;
    nfdicore:country <http://demo.fiz-karlsruhe.de/matwerk/E80004> ;
    owl:sameAs <http://www.wikidata.org/entity/Q3758> .

<http://demo.fiz-karlsruhe.de/matwerk/E779129> a <http://www.ebi.ac.uk/swo/license/SWO_1000043> ;
    rdfs:label "GNU General Public License version 3.0 (GPLv3)" ;
    owl:sameAs <http://www.wikidata.org/entity/Q10513445> .

<http://demo.fiz-karlsruhe.de/matwerk/E78422> a nfdicore:City ;
    rdfs:label "Jülich" ;
    nfdicore:country <http://demo.fiz-karlsruhe.de/matwerk/E80004> ;
    owl:sameAs <http://www.wikidata.org/entity/Q16045> .

<http://demo.fiz-karlsruhe.de/matwerk/E787886> a ns3:SWO_0000002 ;
    rdfs:label "LGPL-2.1 license" ;
    owl:sameAs <http://www.wikidata.org/entity/Q18534390> .

<http://demo.fiz-karlsruhe.de/matwerk/E7904> a nfdicore:Organization ;
    rdfs:label "Access GmbH"@de .

<http://demo.fiz-karlsruhe.de/matwerk/E79211> a nfdicore:City ;
    rdfs:label "Dresden" ;
    nfdicore:country <http://demo.fiz-karlsruhe.de/matwerk/E80004> ;
    owl:sameAs <http://www.wikidata.org/entity/Q737444> .

<http://demo.fiz-karlsruhe.de/matwerk/E794171> a ns3:SWO_0000002 ;
    rdfs:label "no license file" .

<http://demo.fiz-karlsruhe.de/matwerk/E8022> a nfdicore:Organization ;
    rdfs:label "Data Analytics in Engineering"@de .

<http://demo.fiz-karlsruhe.de/matwerk/E80402> a nfdicore:Website ;
    rdfs:label "https://www.mpie.de"^^xsd:anyURI ;
    nfdicore:url <https://www.mpie.de> .

<http://demo.fiz-karlsruhe.de/matwerk/E811902> a <http://www.ebi.ac.uk/swo/license/SWO_1000001> ;
    rdfs:label "Creative Commons Attribution 4.0 International License" ;
    owl:sameAs <http://www.wikidata.org/entity/Q20007257> .

<http://demo.fiz-karlsruhe.de/matwerk/E834987> a nfdicore:ProgrammingLanguage ;
    rdfs:label "Shell" ;
    owl:sameAs <http://www.wikidata.org/entity/Q14663> .

<http://demo.fiz-karlsruhe.de/matwerk/E838866> a nfdicore:ProgrammingLanguage ;
    rdfs:label "MATLAB" ;
    owl:sameAs <http://www.wikidata.org/entity/Q37805571> .

<http://demo.fiz-karlsruhe.de/matwerk/E845351> a nfdicore:ProgrammingLanguage ;
    rdfs:label "cython" ;
    owl:sameAs <http://www.wikidata.org/entity/Q975594> .

<http://demo.fiz-karlsruhe.de/matwerk/E857087> a nfdicore:fundingProject ;
    rdfs:label "SimTech EXC 2075" .

<http://demo.fiz-karlsruhe.de/matwerk/E858396> a nfdicore:fundingProject ;
    rdfs:label "NOMAD" .

<http://demo.fiz-karlsruhe.de/matwerk/E884786> a nfdicore:Publication ;
    dcterms:title "Generation of energy-minimizing point sets on spheres and their application in mesh-free interpolation and differentiation" ;
    mwo:hasAuthor <http://demo.fiz-karlsruhe.de/matwerk/E16401>,
        <http://demo.fiz-karlsruhe.de/matwerk/E16577> ;
    mwo:hasDOI "https://doi.org/10.1007/s10444-019-09726-5" ;
    schema:datePublished "12/10/2019 0:00" .

<http://demo.fiz-karlsruhe.de/matwerk/E91952> a nfdicore:Website,
        mwo:Documentation ;
    rdfs:label "https://calphy.org"^^xsd:anyURI ;
    nfdicore:url <https://calphy.org> .

<http://demo.fiz-karlsruhe.de/matwerk/E92379> a nfdicore:Website,
        mwo:Documentation ;
    rdfs:label "https://pyscal.org"^^xsd:anyURI ;
    nfdicore:url <https://pyscal.org> .

<http://demo.fiz-karlsruhe.de/matwerk/E9647> a nfdicore:Person ;
    rdfs:label "M.Sc Jonas Fell" ;
    mwo:emailAddress "jonas.fell@izfp-extern.fraunhofer.de"^^xsd:string ;
    mwo:hasExpertiseIn <http://demo.fiz-karlsruhe.de/matwerk/E62426>,
        <http://demo.fiz-karlsruhe.de/matwerk/E62777> ;
    mwo:hasORCID <https://orcid.org/0000-0002-5798-8895> ;
    foaf:firstName "Jonas"^^xsd:string ;
    foaf:surname "Fell"^^xsd:string ;
    foaf:title "M.Sc"^^xsd:string .

nfdicore:FederalState a owl:Class ;
    rdfs:label "federal state"@en ;
    nfdicore:example "Sachsen, Berlin"@de ;
    rdfs:comment "A federal state where the thing is located."@en ;
    rdfs:subClassOf nfdicore:Place .

nfdicore:Standard a owl:Class ;
    rdfs:label "standard"@en ;
    nfdicore:example "ISO 15511, DINI-Zertifikat" ;
    rdfs:comment "An international standard and norm that can be used to evaluate or create services."@en ;
    rdfs:subClassOf nfdicore:Specification .

nfdicore:funder a owl:ObjectProperty ;
    rdfs:label "funder"@en ;
    rdfs:comment "The property relates a thing to an organisation or a project that provided funding for it. The sub-properties are used to specify more specific funding relationships. "@en ;
    rdfs:domain owl:Thing ;
    rdfs:range [ a owl:Class ;
            owl:unionOf ( nfdicore:Organization nfdicore:Project ) ] ;
    owl:inverseOf nfdicore:funderOf .

mwo:ResearchTopic a owl:Class ;
    rdfs:label "research topic"@en ;
    ns2:IAO_0000115 "A research topic is a specific field of study within a broader academic discipline."@en ;
    ns4:hasBroadSynonym "Research area"@en ;
    ns4:hasExactSynonym "Research field"@en,
        "Research subject"@en ;
    rdfs:subClassOf nfdicore:AcademicDiscipline .

mwo:SparqlEndpoint a owl:Class ;
    rdfs:label "SPARQL endpoint"@en ;
    ns2:IAO_0000115 "A SPARQL endpoint is a web service that provides an access point for receiving and processing SPARQL protocol requests"@en ;
    rdfs:subClassOf mwo:WebService .

mwo:Workflow a owl:Class ;
    rdfs:label "workflow"@en ;
    ns2:IAO_0000115 "A workflow is a specification which describes a repeatable sequence of steps needed to create or produce a work."@en ;
    rdfs:subClassOf nfdicore:Specification .

<http://schema.org/ComputerLanguage> a owl:Class ;
    rdfs:label "ComputerLanguage"@en ;
    rdfs:comment "This type covers computer programming languages such as Scheme and Lisp, as well as other language-like computer representations. Natural languages are best represented with the <a class=\"localLink\" href=\"https://schema.org/Language\">Language</a> type."@en ;
    rdfs:isDefinedBy <http://schema.org/ComputerLanguage> ;
    rdfs:subClassOf <http://schema.org/Intangible> .

skos:altLabel a owl:AnnotationProperty .

default1:Consortium a owl:Class ;
    rdfs:label "consortium"@en ;
    rdfs:comment "NFDI consortia grouped by a discipline based in a science-led process managed by the German Research Foundation (DFG)."@en ;
    rdfs:subClassOf default1:Organization ;
    default1:example "NFDI4Culture, NFDI-MatWerk, DataPLANT." .

schema:citation a owl:ObjectProperty ;
    rdfs:label "citation"@en ;
    rdfs:comment "A citation or reference to another creative work, such as another publication, web page, scholarly article, etc."@en ;
    rdfs:domain nfdicore:Resource ;
    rdfs:isDefinedBy schema:citation ;
    rdfs:range nfdicore:Resource .

ns1:isPartOf a owl:ObjectProperty ;
    rdfs:label "is part of"@en ;
    rdfs:comment "is part of"@en .

modsci:ScientificInstrument a owl:Class ;
    rdfs:label "Scientific Instrument" ;
    rdfs:comment "A scientific instrument is, broadly speaking, a device or tool used for scientific purposes, including the study of both natural phenomena and theoretical research."@en ;
    rdfs:subClassOf modsci:Instrument ;
    skos:prefLabel "Instrument"@en .

<http://demo.fiz-karlsruhe.de/matwerk/E1002> a nfdicore:Organization ;
    rdfs:label "Institute of Applied Mechanics",
        "Institut für Mechanik"@de,
        "Institut für Technische Mechanik"@de ;
    nfdicore:location <http://demo.fiz-karlsruhe.de/matwerk/E72254>,
        <http://demo.fiz-karlsruhe.de/matwerk/E75692> ;
    nfdicore:parentOrganisation <http://demo.fiz-karlsruhe.de/matwerk/E2432>,
        <http://demo.fiz-karlsruhe.de/matwerk/E2954> ;
    mwo:hasAcronym "ITM"^^xsd:string,
        "MIB"^^xsd:string ;
    mwo:hasPostalCode "70569",
        "D-38678" ;
    mwo:hasWebsite <http://demo.fiz-karlsruhe.de/matwerk/E80801>,
        <http://demo.fiz-karlsruhe.de/matwerk/E85256> .

<http://demo.fiz-karlsruhe.de/matwerk/E1011> a nfdicore:Organization ;
    rdfs:label "Institute of Materials Science",
        "Institut für Materialwissenschaft"@de ;
    nfdicore:location <http://demo.fiz-karlsruhe.de/matwerk/E73011>,
        <http://demo.fiz-karlsruhe.de/matwerk/E75306> ;
    nfdicore:parentOrganisation <http://demo.fiz-karlsruhe.de/matwerk/E2486>,
        <http://demo.fiz-karlsruhe.de/matwerk/E2892> ;
    mwo:hasPostalCode "24143",
        "64287" ;
    mwo:hasWebsite <http://demo.fiz-karlsruhe.de/matwerk/E81602>,
        <http://demo.fiz-karlsruhe.de/matwerk/E84846> .

<http://demo.fiz-karlsruhe.de/matwerk/E1106> a nfdicore:Organization ;
    rdfs:label "Fraunhofer Institute for Mechanics of Materials",
        "Fraunhofer-Institut für Werkstoffmechanik"@de ;
    nfdicore:location <http://demo.fiz-karlsruhe.de/matwerk/E76079> ;
    nfdicore:parentOrganisation <http://demo.fiz-karlsruhe.de/matwerk/E3081> ;
    mwo:hasAcronym "IWM"^^xsd:string ;
    mwo:hasPostalCode "79108" ;
    mwo:hasWebsite <http://demo.fiz-karlsruhe.de/matwerk/E86492> .

<http://demo.fiz-karlsruhe.de/matwerk/E1154> a nfdicore:Organization ;
    rdfs:label "Materialwissenschaft und Werkstofftechnik an der Universität des Saarlandes" ;
    nfdicore:location <http://demo.fiz-karlsruhe.de/matwerk/E73391> ;
    nfdicore:parentOrganisation <http://demo.fiz-karlsruhe.de/matwerk/E2541>,
        <http://demo.fiz-karlsruhe.de/matwerk/E3212> ;
    mwo:hasAcronym "MWWT"^^xsd:string ;
    mwo:hasPostalCode "66123" ;
    mwo:hasWebsite <http://demo.fiz-karlsruhe.de/matwerk/E82407> .

<http://demo.fiz-karlsruhe.de/matwerk/E1221704> a dcterms:FileFormat ;
    rdfs:label "csv" .

<http://demo.fiz-karlsruhe.de/matwerk/E1245258> a nfdicore:AcademicDiscipline,
        mwo:EducationalResource ;
    rdfs:label "Information Service Engineering" ;
    dcterms:format "Academic teaching materials" ;
    mwo:description "This lecture provides an introduction into natural language processing (NLP), followed by knowledge representation basics with a focus on knowledge graphs and Semantic Web technologies. Moreover, a brief sketch of machine learning and deep learning technologies complement the lecture to provide some insights on state-of-the-art ISE applications, in particular on semantic and exploratory search." ;
    mwo:hasLecturer <http://demo.fiz-karlsruhe.de/matwerk/E14862> ;
    mwo:hasWebsite <http://demo.fiz-karlsruhe.de/matwerk/E395717>,
        <http://demo.fiz-karlsruhe.de/matwerk/E407352> ;
    mwo:isOnline true ;
    mwo:requiredTool <http://demo.fiz-karlsruhe.de/matwerk/E836279> ;
    rdfs:comment "2021" ;
    ns1:duration "90 min / week plus exercises"^^xsd:time .

<http://demo.fiz-karlsruhe.de/matwerk/E1246242> a nfdicore:Organization ;
    rdfs:label "MPIE" .

<http://demo.fiz-karlsruhe.de/matwerk/E1246803> a <http://www.ebi.ac.uk/swo/license/SWO_1000061> ;
    rdfs:label "BSD-3-Clause license" .

<http://demo.fiz-karlsruhe.de/matwerk/E1246872> a mwo:Method ;
    rdfs:label "Atom Probe Tomography" .

<http://demo.fiz-karlsruhe.de/matwerk/E1247517> a nfdicore:ProgrammingLanguage ;
    rdfs:label "python3.9" .

<http://demo.fiz-karlsruhe.de/matwerk/E1248002> rdfs:label "Defect phases in structural materials" .

<http://demo.fiz-karlsruhe.de/matwerk/E1248067> rdfs:label "Magnetoelectric sensors: from composite materials to biomagnetic diagnostics" .

<http://demo.fiz-karlsruhe.de/matwerk/E1248083> rdfs:label "Cluster of Excellence Living, Adaptive and Energy-autonomous Materials Systems – livMatS" .

<http://demo.fiz-karlsruhe.de/matwerk/E1248100> rdfs:label "DiWan - The Digital Transformation in Materials Testing: Necessary Actions for the Paradigm Change in Enterprises" .

<http://demo.fiz-karlsruhe.de/matwerk/E1248200> rdfs:label "ICAMS – Micromechanical modelling" .

<http://demo.fiz-karlsruhe.de/matwerk/E1248298> rdfs:label "Mat-o-Lab – Materials-open-Laboratory" .

<http://demo.fiz-karlsruhe.de/matwerk/E2379> a nfdicore:Organization ;
    rdfs:label "Max-Planck-Gesellschaft" ;
    mwo:hasRORID "https://ror.org/01ngpvg12" ;
    owl:sameAs <http://www.wikidata.org/entity/Q881977> .

<http://demo.fiz-karlsruhe.de/matwerk/E245651> a mwo:Documentation ;
    rdfs:label "https://imagej.net/learn/"^^xsd:anyURI ;
    nfdicore:url <https://imagej.net/learn/> .

<http://demo.fiz-karlsruhe.de/matwerk/E2486> a nfdicore:Organization ;
    rdfs:label "Christian-Albrechts-Universität zu Kiel" ;
    mwo:hasAcronym "CAU"^^xsd:string ;
    mwo:hasPostalAddress "Hermann-Rodewald-Straße 3" ;
    mwo:hasPostalCode "24118" ;
    mwo:hasRORID "https://ror.org/04v76ef78" ;
    owl:sameAs <http://www.wikidata.org/entity/Q156737> .

<http://demo.fiz-karlsruhe.de/matwerk/E3081> a nfdicore:Organization ;
    rdfs:label "Fraunhofer-Gesellschaft" ;
    mwo:hasRORID "https://ror.org/04hm8eb66",
        "https://ror.org/050mbz718",
        "https://ror.org/05h8wjh50" ;
    owl:sameAs <http://www.wikidata.org/entity/Q1452043>,
        <http://www.wikidata.org/entity/Q1452044>,
        <http://www.wikidata.org/entity/Q21997375> .

<http://demo.fiz-karlsruhe.de/matwerk/E3212> a nfdicore:Organization ;
    rdfs:label "Saarland University" ;
    mwo:hasRORID "https://ror.org/01jdpyv68" ;
    owl:sameAs <http://www.wikidata.org/entity/Q700758> .

<http://demo.fiz-karlsruhe.de/matwerk/E35717> a nfdicore:Person ;
    mwo:emailAddress "pyiron@mpie.de"^^xsd:string ;
    foaf:firstName "Jan"^^xsd:string ;
    foaf:surname "Janssen"^^xsd:string ;
    foaf:title "Dr."^^xsd:string .

<http://demo.fiz-karlsruhe.de/matwerk/E38402> a nfdicore:AcademicDiscipline ;
    rdfs:label "Research Data Management" ;
    owl:sameAs <http://www.wikidata.org/entity/Q30089794> .

<http://demo.fiz-karlsruhe.de/matwerk/E39504> a nfdicore:AcademicDiscipline ;
    rdfs:label "Materials Data Science and Informatics" .

<http://demo.fiz-karlsruhe.de/matwerk/E4404> a nfdicore:Organization ;
    rdfs:label "Linköping University"@de .

<http://demo.fiz-karlsruhe.de/matwerk/E4656> a nfdicore:Organization ;
    rdfs:label "Ruhr-Universität Bochum" ;
    mwo:hasAcronym "RUB"^^xsd:string ;
    mwo:hasRORID "https://ror.org/04tsk2644" ;
    owl:sameAs <http://www.wikidata.org/entity/Q309948> .

<http://demo.fiz-karlsruhe.de/matwerk/E49517> a nfdicore:AcademicDiscipline ;
    rdfs:label "Computational materials science" ;
    owl:sameAs <http://www.wikidata.org/entity/Q85753722> .

<http://demo.fiz-karlsruhe.de/matwerk/E641147> a nfdicore:Resource ;
    rdfs:label "ASE" .

<http://demo.fiz-karlsruhe.de/matwerk/E72632> a nfdicore:City ;
    rdfs:label "Berlin" ;
    nfdicore:country <http://demo.fiz-karlsruhe.de/matwerk/E80004> ;
    owl:sameAs <http://www.wikidata.org/entity/Q821229> .

<http://demo.fiz-karlsruhe.de/matwerk/E73011> a nfdicore:City ;
    rdfs:label "Kiel" ;
    nfdicore:country <http://demo.fiz-karlsruhe.de/matwerk/E80004> ;
    owl:sameAs <http://www.wikidata.org/entity/Q1707> .

<http://demo.fiz-karlsruhe.de/matwerk/E74154> a nfdicore:City ;
    rdfs:label "Aachen" ;
    nfdicore:country <http://demo.fiz-karlsruhe.de/matwerk/E80004> ;
    owl:sameAs <http://www.wikidata.org/entity/Q1017> .

<http://demo.fiz-karlsruhe.de/matwerk/E760529> a <http://www.ebi.ac.uk/swo/license/SWO_1000002> ;
    rdfs:label "Academic and commercial license" .

<http://demo.fiz-karlsruhe.de/matwerk/E76079> a nfdicore:City ;
    rdfs:label "Freiburg" ;
    nfdicore:country <http://demo.fiz-karlsruhe.de/matwerk/E80004> ;
    owl:sameAs <http://www.wikidata.org/entity/Q387449> .

<http://demo.fiz-karlsruhe.de/matwerk/E764231> a <http://www.ebi.ac.uk/swo/license/SWO_1000043> ;
    rdfs:label "GNU Lesser General Public License" ;
    owl:sameAs <http://www.wikidata.org/entity/Q192897> .

<http://demo.fiz-karlsruhe.de/matwerk/E765467> a <http://www.ebi.ac.uk/swo/license/SWO_1000043> ;
    rdfs:label "GNU General Public License v2" ;
    owl:sameAs <http://www.wikidata.org/entity/Q10513450> .

<http://demo.fiz-karlsruhe.de/matwerk/E766704> a <http://www.ebi.ac.uk/swo/license/SWO_1000002> ;
    rdfs:label "Propietary commercial license" .

<http://demo.fiz-karlsruhe.de/matwerk/E785379> a ns3:SWO_0000002 ;
    rdfs:label "GPL license version 3" ;
    owl:sameAs <http://www.wikidata.org/entity/Q10513445> .

<http://demo.fiz-karlsruhe.de/matwerk/E786632> a <http://www.ebi.ac.uk/swo/license/SWO_1000061> ;
    rdfs:label "Mozilla Public License Version 2.0" ;
    owl:sameAs <http://www.wikidata.org/entity/Q25428413> .

<http://demo.fiz-karlsruhe.de/matwerk/E791654> a <http://www.ebi.ac.uk/swo/license/SWO_1000043> ;
    rdfs:label "GNU AFFERO GENERAL PUBLIC LICENSE Version 3" ;
    owl:sameAs <http://www.wikidata.org/entity/Q1131681> .

<http://demo.fiz-karlsruhe.de/matwerk/E808086> a ns3:SWO_0000002 ;
    rdfs:label "partly propietary" .

<http://demo.fiz-karlsruhe.de/matwerk/E833696> a nfdicore:ProgrammingLanguage ;
    rdfs:label "Java" ;
    owl:sameAs <http://www.wikidata.org/entity/Q251> .

nfdicore:TaskArea a owl:Class .

nfdicore:funderOf a owl:ObjectProperty ;
    rdfs:label "funder of"@en .

mwo:Database a owl:Class ;
    rdfs:label "database"@en ;
    rdfs:comment "A structured collection of logically related data usually stored and retrieved using computer-based means."@en ;
    rdfs:subClassOf <http://schema.org/Product> .

mwo:ResearchGroup a owl:Class ;
    rdfs:label "research group"@en ;
    ns2:IAO_0000115 "A group of people who work in a university or research institute and carry research on one or more topics."@en .

mwo:UseCase a owl:Class .

mwo:WorkflowEnvironment a owl:Class ;
    rdfs:label "workflow environment"@en ;
    ns2:IAO_0000115 "A workflow environment is a software that manages and allows the user to create and interact with computational workflows."@en ;
    rdfs:subClassOf ns3:SWO_0000001 .

<http://schema.org/CreativeWork> a owl:Class .

<http://schema.org/Intangible> a owl:Class .

<http://schema.org/Service> a owl:Class ;
    rdfs:label "Service"@en ;
    rdfs:comment "A service provided by an organization, e.g. delivery service, print services, etc."@en ;
    rdfs:isDefinedBy <http://schema.org/Service> ;
    rdfs:subClassOf <http://schema.org/Intangible> .

ns3:SWO_9000050 a owl:Class ;
    rdfs:label "software interface" ;
    ns2:IAO_0000115 "The mode of interaction with a piece of software." .

default1:Project a owl:Class ;
    rdfs:label "project"@en ;
    rdfs:comment "A scientific or business endeavor that aims to conclude an investigation or to answer a research question."@en ;
    default1:example "Freischütz digital, Corpus Vitrearum Medii Aevi" .

<http://demo.fiz-karlsruhe.de/matwerk/E1240526> a ns3:SWO_0000001 ;
    rdfs:label "LAMMPS" .

<http://demo.fiz-karlsruhe.de/matwerk/E1246252> a dcterms:FileFormat ;
    rdfs:label ".ipynb" .

<http://demo.fiz-karlsruhe.de/matwerk/E1246362> rdfs:label "Jupyter lab" .

<http://demo.fiz-karlsruhe.de/matwerk/E1247962> rdfs:label "From atoms to turbine blades" .

<http://demo.fiz-karlsruhe.de/matwerk/E1247983> rdfs:label "Processing uncertain microstructural data" .

<http://demo.fiz-karlsruhe.de/matwerk/E1248013> rdfs:label "HoMMage - Hysteresis design of magnetic materials for efficient energy conversion" .

<http://demo.fiz-karlsruhe.de/matwerk/E1248157> rdfs:label "ERC Starting Grant MuDiLingo: Ontology Design for Dislocations" .

<http://demo.fiz-karlsruhe.de/matwerk/E1248178> rdfs:label "Tomography and Microstructure-based Modelling (Tomography)" .

<http://demo.fiz-karlsruhe.de/matwerk/E1248223> rdfs:label "Leibniz-Institut für Werkstofforientierte Technologien" .

<http://demo.fiz-karlsruhe.de/matwerk/E16226> a nfdicore:Person ;
    mwo:hasAffiliation <http://demo.fiz-karlsruhe.de/matwerk/E5951>,
        <http://demo.fiz-karlsruhe.de/matwerk/E7904>,
        <http://demo.fiz-karlsruhe.de/matwerk/E8022> ;
    foaf:firstName "Mauricio"^^xsd:string ;
    foaf:surname "Fernández"^^xsd:string .

<http://demo.fiz-karlsruhe.de/matwerk/E16401> a nfdicore:Person ;
    mwo:hasAffiliation <http://demo.fiz-karlsruhe.de/matwerk/E5852> ;
    foaf:firstName "Oliver"^^xsd:string ;
    foaf:surname "Kunc"^^xsd:string .

<http://demo.fiz-karlsruhe.de/matwerk/E3279> a nfdicore:Organization ;
    rdfs:label "RWTH Aachen University" ;
    mwo:hasRORID "https://ror.org/04xfq0f34" ;
    owl:sameAs <http://www.wikidata.org/entity/Q273263> .

<http://demo.fiz-karlsruhe.de/matwerk/E610961> a mwo:Method ;
    rdfs:label "Finite Element Method" .

<http://demo.fiz-karlsruhe.de/matwerk/E63836> a nfdicore:AcademicDiscipline ;
    rdfs:label "Density Functional Theory (DFT)" .

<http://demo.fiz-karlsruhe.de/matwerk/E65262> a nfdicore:AcademicDiscipline ;
    rdfs:label "Finite Element Method (FEM)" .

<http://demo.fiz-karlsruhe.de/matwerk/E65981> a nfdicore:AcademicDiscipline ;
    rdfs:label "multiscale modelling" .

<http://demo.fiz-karlsruhe.de/matwerk/E70379> a nfdicore:AcademicDiscipline ;
    rdfs:label "thermodynamics" ;
    owl:sameAs <http://www.wikidata.org/entity/Q11473> .

<http://demo.fiz-karlsruhe.de/matwerk/E739721> a <http://www.ebi.ac.uk/swo/license/SWO_1000061> ;
    rdfs:label "BSD-3" ;
    owl:sameAs <http://www.wikidata.org/entity/Q18491847> .

<http://demo.fiz-karlsruhe.de/matwerk/E740937> a <http://www.ebi.ac.uk/swo/license/SWO_1000061> ;
    rdfs:label "BSD 3-Clause License" ;
    owl:sameAs <http://www.wikidata.org/entity/Q18491847> .

<http://demo.fiz-karlsruhe.de/matwerk/E820841> a <http://www.ebi.ac.uk/swo/license/SWO_1000061> ;
    rdfs:label "MIT License" ;
    owl:sameAs <http://www.wikidata.org/entity/Q334661> .

<http://demo.fiz-karlsruhe.de/matwerk/E9002> a nfdicore:Person ;
    rdfs:label "Prof. Birgit Skrotzki" ;
    mwo:emailAddress "birgit.skrotzki@bam.de"^^xsd:string ;
    mwo:hasAffiliation <http://demo.fiz-karlsruhe.de/matwerk/E1245619>,
        <http://demo.fiz-karlsruhe.de/matwerk/E1245640> ;
    mwo:hasExpertiseIn <http://demo.fiz-karlsruhe.de/matwerk/E1245665>,
        <http://demo.fiz-karlsruhe.de/matwerk/E1245784>,
        <http://demo.fiz-karlsruhe.de/matwerk/E37857> ;
    mwo:hasORCID <https://orcid.org/0000-0003-0727-5499> ;
    owl:sameAs <http://www.wikidata.org/entity/Q21255757> ;
    foaf:firstName "Birgit"^^xsd:string ;
    foaf:surname "Skrotzki"^^xsd:string ;
    foaf:title "Prof."^^xsd:string .

nfdicore:Country a owl:Class ;
    rdfs:label "country"@en ;
    rdfs:comment "A country where the thing is located."@en ;
    rdfs:subClassOf nfdicore:Place .

nfdicore:Place a owl:Class ;
    rdfs:label "place"@en ;
    nfdicore:example "Hessen, Berlin, Schweiz" ;
    rdfs:comment "A spatial region, e.g. country, city or district."@en .

mwo:hasPersonalInformation a owl:DatatypeProperty ;
    rdfs:label "has personal information"@en ;
    ns2:IAO_0000115 "A data property linking a person with information about that person."@en ;
    rdfs:domain nfdicore:Person .

ns4:hasSynonym a owl:AnnotationProperty ;
    rdfs:label "has_synonym"@en ;
    ns4:hasDbXref [ ] ;
    ns4:hasDefinition [ ] ;
    rdfs:comment "Note that this should be a super-property of hasRelatedSynonym, hasExactSynonym etc; however, we cannot state this and remain in OWL-DL"^^xsd:string .

ns1:AcademicEvent a owl:Class ;
    rdfs:label "Academic event"@en ;
    rdfs:comment "Academic events are e.g. conferences and conference-like events, and all the sub-events of those which are about the topic or theme of the conference, such as talks or panels."@en ;
    rdfs:subClassOf ns1:OrganisedEvent .

<http://demo.fiz-karlsruhe.de/matwerk/E1001> a nfdicore:Organization ;
    rdfs:label "Max Planck Institute for Iron Research",
        "Max-Planck-Institut für Eisenforschung"@de ;
    nfdicore:location <http://demo.fiz-karlsruhe.de/matwerk/E71877> ;
    nfdicore:parentOrganisation <http://demo.fiz-karlsruhe.de/matwerk/E2379> ;
    mwo:hasAcronym "MPIE"^^xsd:string ;
    mwo:hasPostalCode "40237" ;
    mwo:hasWebsite <http://demo.fiz-karlsruhe.de/matwerk/E80402> .

<http://demo.fiz-karlsruhe.de/matwerk/E1016> a nfdicore:Organization ;
    rdfs:label "FIZ Karlsruhe - Leibniz Institute for Information Infrastructure",
        "FIZ Karlsruhe - Leibniz-Institut für Informationsinfrastruktur"@de ;
    nfdicore:location <http://demo.fiz-karlsruhe.de/matwerk/E73772> ;
    nfdicore:parentOrganisation <http://demo.fiz-karlsruhe.de/matwerk/E2597> ;
    mwo:hasAcronym "FIZ Karlsruhe"^^xsd:string ;
    mwo:hasPostalCode "76344" ;
    mwo:hasWebsite <http://demo.fiz-karlsruhe.de/matwerk/E82811> .

<http://demo.fiz-karlsruhe.de/matwerk/E1121> a nfdicore:Organization ;
    rdfs:label "Karlsruhe Institute of Technology",
        "Karlsruher Institut für Technologie"@de ;
    nfdicore:location <http://demo.fiz-karlsruhe.de/matwerk/E73772>,
        <http://demo.fiz-karlsruhe.de/matwerk/E76467> ;
    nfdicore:parentOrganisation <http://demo.fiz-karlsruhe.de/matwerk/E1862>,
        <http://demo.fiz-karlsruhe.de/matwerk/E2654> ;
    mwo:hasAcronym "KIT"^^xsd:string,
        "SCC"^^xsd:string ;
    mwo:hasPostalAddress "Steinbuch Centre for Computing" ;
    mwo:hasPostalCode "76131",
        "76344",
        "D-76128" ;
    mwo:hasWebsite <http://demo.fiz-karlsruhe.de/matwerk/E86906>,
        <http://demo.fiz-karlsruhe.de/matwerk/E91101> .

<http://demo.fiz-karlsruhe.de/matwerk/E1248118> rdfs:label "Integrated engineering of continuous-discontinuous long fiber reinforced polymer structures" .

<http://demo.fiz-karlsruhe.de/matwerk/E14862> a nfdicore:Person ;
    rdfs:label "Prof. Dr. Harald Sack" ;
    mwo:emailAddress "harald.sack@fiz-karlsruhe.de"^^xsd:string ;
    mwo:hasAffiliation <http://demo.fiz-karlsruhe.de/matwerk/E1016> ;
    mwo:hasExpertiseIn <http://demo.fiz-karlsruhe.de/matwerk/E1245258>,
        <http://demo.fiz-karlsruhe.de/matwerk/E59654> ;
    mwo:hasORCID <https://orcid.org/0000-0001-7069-9804> ;
    owl:sameAs <http://www.wikidata.org/entity/Q30078997>,
        <https://nfdi4culture.de/id/E1925> ;
    foaf:depiction <https://www.fiz-karlsruhe.de/sites/default/files/styles/contact_image/public/FIZ/Bilder/Personen/Harald-Sack.png?itok=GejB9r5c> ;
    foaf:firstName "Harald"^^xsd:string ;
    foaf:surname "Sack"^^xsd:string ;
    foaf:title "Prof. Dr."^^xsd:string .

<http://demo.fiz-karlsruhe.de/matwerk/E59654> a nfdicore:AcademicDiscipline ;
    rdfs:label "Computer Science" ;
    owl:sameAs <http://www.wikidata.org/entity/Q21198> .

<http://demo.fiz-karlsruhe.de/matwerk/E68897> a nfdicore:AcademicDiscipline ;
    rdfs:label "data analysis" .

<http://demo.fiz-karlsruhe.de/matwerk/E69266> a nfdicore:AcademicDiscipline ;
    rdfs:label "imaging data processing" .

<http://demo.fiz-karlsruhe.de/matwerk/E817004> a <http://www.ebi.ac.uk/swo/license/SWO_1000001> ;
    rdfs:label "Creative Commons Attribution 4.0 International" ;
    owl:sameAs <http://www.wikidata.org/entity/Q20007257> .

<http://demo.fiz-karlsruhe.de/matwerk/E844052> a nfdicore:ProgrammingLanguage ;
    rdfs:label "C" ;
    owl:sameAs <http://www.wikidata.org/entity/Q15777> .

dcterms:identifier a owl:AnnotationProperty ;
    rdfs:label "Identifier"@en-us ;
    rdfs:comment "Recommended best practice is to identify the resource by means of a string conforming to a formal identification system."@en-us ;
    rdfs:range rdfs:Literal ;
    rdfs:subPropertyOf dc:identifier ;
    skos:definition "An unambiguous reference to the resource within a given context."@en-us .

mwo:ComputationalWorkflow a owl:Class ;
    rdfs:label "computational workflow"@en ;
    ns2:IAO_0000115 "A computational workflow is a workflow which describes the complex multi-step methods that are used for data collection, data preparation, analytics, predictive modelling, and simulation that lead to new data products."@en ;
    ns4:hasDbXref <https://doi.org/10.1162/dint_a_00033> ;
    rdfs:subClassOf mwo:Workflow,
        ns3:SWO_0000001 .

<http://www.ebi.ac.uk/swo/license/SWO_1000002> a owl:Class ;
    rdfs:label "Proprietary commercial software license" ;
    rdfs:subClassOf ns3:SWO_0000002 .

<http://demo.fiz-karlsruhe.de/matwerk/E1247886> rdfs:label "Community Interaction" ;
    dcterms:isPartOf <http://demo.fiz-karlsruhe.de/matwerk/E1247022> ;
    mwo:description "This TA is responsible to stimulate the acceptance and vivid participation of the overall MSE community through communication, counselling, education / training and steady increase of the outreach." ;
    mwo:hasWorkPackage <http://demo.fiz-karlsruhe.de/matwerk/E1247935> .

<http://demo.fiz-karlsruhe.de/matwerk/E70007> a nfdicore:AcademicDiscipline ;
    rdfs:label "scientific visualization" .

nfdicore:SemanticExpressivity a owl:Class ;
    rdfs:label "semantic expressivity"@en ;
    nfdicore:example "controlled vocabulary, ontology, taxonomy"@en ;
    rdfs:comment "An entity that identifies the level of the semantic expressivity of a resource. Five instances are now included in nfdicore."@en .

mwo:EducationalEvent a owl:Class ;
    rdfs:label "educational event" ;
    ns2:IAO_0000115 "An organized event with the purpose of teaching knowledge to others by displaying educational materials."@en ;
    rdfs:subClassOf ns1:OrganisedEvent .

mwo:LargeScaleFacility a owl:Class ;
    rdfs:label "large-scale facility"@en ;
    ns2:IAO_0000115 "A facility that provides access to large-scale scientific equipment and allows scientists to carry out state-of-the-art research."@en .

modsci:ScientificInstrumentManufacturer a owl:Class ;
    rdfs:label "Scientific Instrument Manufacturer" ;
    rdfs:comment "Companies manufacturing equipment for scientific sstudies." .

<http://demo.fiz-karlsruhe.de/matwerk/E1247881> rdfs:label "Materials Data Infrastructure" ;
    dcterms:isPartOf <http://demo.fiz-karlsruhe.de/matwerk/E1247022> ;
    mwo:description "This TA is responsible for developing the Digital Materials Environment (DME) and for providing services to easily store, share, search, and analyze data and metadata while ensuring data integrity, provenance, and authorship." ;
    mwo:hasWorkPackage <http://demo.fiz-karlsruhe.de/matwerk/E1247908>,
        <http://demo.fiz-karlsruhe.de/matwerk/E1247916> .

ns3:SWO_0000020 a owl:Class ;
    rdfs:label "Unix" ;
    rdfs:subClassOf ns3:SWO_0000021 .

modsci:Technology a owl:Class ;
    rdfs:label "Technology" ;
    rdfs:comment "Technology is the collection of techniques, skills, methods, and processes used in the production of goods or services or in the accomplishment of objectives, such as scientific investigation." .

<http://demo.fiz-karlsruhe.de/matwerk/E1245619> a nfdicore:Organization ;
    rdfs:label "Federal Institute for Materials Research and Testing  Bundesanstalt für Materialforschung und -prüfung" ;
    nfdicore:location <http://demo.fiz-karlsruhe.de/matwerk/E72632> ;
    mwo:hasAcronym "BAM"^^xsd:string ;
    mwo:hasPostalCode "12200" ;
    mwo:hasWebsite <http://demo.fiz-karlsruhe.de/matwerk/E1245595> .

<http://demo.fiz-karlsruhe.de/matwerk/E616496> a mwo:Method ;
    rdfs:label "molecular dynamics" .

<http://demo.fiz-karlsruhe.de/matwerk/E762996> a <http://www.ebi.ac.uk/swo/license/SWO_1000043> ;
    rdfs:label "GNU General Public License v3" ;
    owl:sameAs <http://www.wikidata.org/entity/Q10513445> .

<http://demo.fiz-karlsruhe.de/matwerk/E841457> a nfdicore:ProgrammingLanguage ;
    rdfs:label "Fortran" ;
    owl:sameAs <http://www.wikidata.org/entity/Q83303> .

mwo:MetadataSchema a owl:Class ;
    rdfs:label "metadata schema"@en ;
    ns2:IAO_0000115 "A metadata schema is a specification which establishes the elements needed to describe a data resource in a formalized and concise manner."@en ;
    rdfs:subClassOf nfdicore:Specification .

mwo:ProcessingSoftware a owl:Class ;
    rdfs:label "processing software"@en ;
    ns2:IAO_0000115 "Software which carries out a (planned) process on digital data,"@en ;
    rdfs:comment "Depending on the temporal relation of the carried out process to an analysis process, the process might either be termed \"pre-processing\" (e.g. converting file formats) or \"post-processing\" (e.g. spatial filtering of images)."@en ;
    rdfs:subClassOf ns3:SWO_0000001 .

mwo:VisualizationSoftware a owl:Class ;
    rdfs:label "visualization software"@en ;
    ns2:IAO_0000115 "Software which creates graphical representations of data, features of data or data sets."@en ;
    ns4:hasBroadSynonym "Graphics software"@en ;
    rdfs:subClassOf ns3:SWO_0000001 .

<http://www.ebi.ac.uk/swo/license/SWO_1000001> a owl:Class ;
    rdfs:label "Creative Commons" ;
    ns2:IAO_0000118 "CC" ;
    rdfs:subClassOf ns3:SWO_0000002 .

default1:Organization a owl:Class ;
    rdfs:label "organization"@en ;
    rdfs:comment "An organization of some kind, e.g. research organization or business organization"@en ;
    default1:example "Univerity Library in Leipzig, Museums of City Cologne" .

<http://demo.fiz-karlsruhe.de/matwerk/E1125251> a nfdicore:Specification ;
    rdfs:label "OPTIMADE" ;
    mwo:description "The Open Databases Integration for Materials Design (OPTIMADE) consortium aims to make materials databases interoperable by developing a specification for a common REST API." ;
    mwo:hasDOI "10.5281/zenodo.4195050"^^xsd:anyURI ;
    mwo:hasDocumentation <http://demo.fiz-karlsruhe.de/matwerk/E320601> ;
    mwo:hasRepository <http://demo.fiz-karlsruhe.de/matwerk/E304811> ;
    mwo:hasVersion "1.1.0" ;
    ns3:has_license <http://demo.fiz-karlsruhe.de/matwerk/E818282> ;
    schema:citation <http://demo.fiz-karlsruhe.de/matwerk/E994346> ;
    schema:datePublished "7/8/2021" .

<http://demo.fiz-karlsruhe.de/matwerk/E42042> a nfdicore:AcademicDiscipline ;
    rdfs:label "Computational Materials Science" ;
    owl:sameAs <http://www.wikidata.org/entity/Q85753722> .

<http://demo.fiz-karlsruhe.de/matwerk/E457491> a nfdicore:Resource,
        nfdicore:Software,
        mwo:ResearchSoftware,
        mwo:WorkflowEnvironment,
        ns3:SWO_0000001 ;
    rdfs:label "Pyiron" ;
    nfdicore:programmingLanguage <http://demo.fiz-karlsruhe.de/matwerk/E836279> ;
    dcterms:description "pyiron is an integrated development environment for implementing, testing, and running simulations in computational materials science."^^xsd:string ;
    mwo:hasContributor <http://demo.fiz-karlsruhe.de/matwerk/E3416> ;
    mwo:hasDiscipline <http://demo.fiz-karlsruhe.de/matwerk/E67431> ;
    mwo:hasDocumentation <http://demo.fiz-karlsruhe.de/matwerk/E260561> ;
    mwo:hasRepository <http://demo.fiz-karlsruhe.de/matwerk/E177122> ;
    mwo:hasVersion "0.4.6" ;
    mwo:hasWebsite <http://demo.fiz-karlsruhe.de/matwerk/E111686> ;
    ns3:has_license <http://demo.fiz-karlsruhe.de/matwerk/E739721> ;
    schema:citation <http://demo.fiz-karlsruhe.de/matwerk/E911576> .

<http://demo.fiz-karlsruhe.de/matwerk/E6779> a nfdicore:Organization ;
    rdfs:label "National Institute for Materials Science (NIMS), Japan" .

emmo:EMMO_4207e895_8b83_4318_996a_72cfb32acd94 a owl:Class ;
    rdfs:label "Material" ;
    emmo:EMMO_967080e5_2f42_4eb2_a3a9_c58143e835f9 "A matter individual that stands for a real world object representing an amount of a physical substance (or mixture of substances) in different states of matter or phases."@en ;
    rdfs:comment "An instance of a material (e.g. nitrogen) can represent different states of matter. The fact that the individual also belongs to other classes (e.g. Gas) would reveal the actual form in which the material is found."@en,
        "Material usually means some definite kind, quality, or quantity of matter, especially as intended for use."@en ;
    skos:prefLabel "Material"@en .

nfdicore:fundingProject a owl:ObjectProperty ;
    rdfs:label "funding project"@en ;
    rdfs:comment "The property relateds a resource to the project that provided funding for it."@en ;
    rdfs:domain nfdicore:Resource ;
    rdfs:range nfdicore:Project ;
    rdfs:subPropertyOf nfdicore:funder ;
    owl:inverseOf nfdicore:fundingProjectOf .

<http://demo.fiz-karlsruhe.de/matwerk/E1022> a nfdicore:Organization ;
    rdfs:label "Forschungszentrum Jülich",
        "Forschungszentrum Jülich"@de ;
    nfdicore:location <http://demo.fiz-karlsruhe.de/matwerk/E74154>,
        <http://demo.fiz-karlsruhe.de/matwerk/E78422> ;
    nfdicore:parentOrganisation <http://demo.fiz-karlsruhe.de/matwerk/E2654> ;
    mwo:hasAcronym "FZJ"^^xsd:string ;
    mwo:hasPostalAddress "Wilhelm-Johnen-Straße" ;
    mwo:hasPostalCode "52068",
        "52428" ;
    mwo:hasWebsite <http://demo.fiz-karlsruhe.de/matwerk/E83216>,
        <http://demo.fiz-karlsruhe.de/matwerk/E89411> .

<http://demo.fiz-karlsruhe.de/matwerk/E1037> a nfdicore:Organization ;
    rdfs:label "Interdisciplinary Centre for Advanced Materials Simulation" ;
    nfdicore:location <http://demo.fiz-karlsruhe.de/matwerk/E74537> ;
    nfdicore:parentOrganisation <http://demo.fiz-karlsruhe.de/matwerk/E4656> ;
    mwo:hasAcronym "ICAMS"^^xsd:string ;
    mwo:hasPostalCode "44801" ;
    mwo:hasWebsite <http://demo.fiz-karlsruhe.de/matwerk/E83622> .

<http://demo.fiz-karlsruhe.de/matwerk/E1245640> a nfdicore:Organization ;
    rdfs:label "Federal Institute For Materials Research and Testing",
        "Bundesanstalt für Materialforschung und -prüfung"@de ;
    nfdicore:location <http://demo.fiz-karlsruhe.de/matwerk/E72632> ;
    nfdicore:parentOrganisation <http://demo.fiz-karlsruhe.de/matwerk/E2379> ;
    mwo:hasAcronym " BAM"^^xsd:string,
        "BAM"^^xsd:string ;
    mwo:hasPostalCode " 12205",
        "12205" ;
    mwo:hasWebsite <http://demo.fiz-karlsruhe.de/matwerk/E81201> .

nfdicore:Dataset a owl:Class ;
    rdfs:label "dataset"@en ;
    rdfs:comment "A dataset is associated with a structured information about a resource."@en ;
    rdfs:subClassOf <http://schema.org/CreativeWork> .

ns2:BFO_0000023 a owl:Class ;
    rdfs:label "role"@en ;
    ns2:BFO_0000179 "role" ;
    ns2:BFO_0000180 "Role" ;
    ns2:IAO_0000112 "John’s role of husband to Mary is dependent on Mary’s role of wife to John, and both are dependent on the object aggregate comprising John and Mary as member parts joined together through the relational quality of being married."@en,
        "the priest role"@en,
        "the role of a boundary to demarcate two neighboring administrative territories"@en,
        "the role of a building in serving as a military target"@en,
        "the role of a stone in marking a property boundary"@en,
        "the role of subject in a clinical trial"@en,
        "the student role"@en ;
    ns2:IAO_0000116 "BFO 2 Reference: One major family of examples of non-rigid universals involves roles, and ontologies developed for corresponding administrative purposes may consist entirely of representatives of entities of this sort. Thus ‘professor’, defined as follows,b instance_of professor at t =Def. there is some c, c instance_of professor role & c inheres_in b at t.denotes a non-rigid universal and so also do ‘nurse’, ‘student’, ‘colonel’, ‘taxpayer’, and so forth. (These terms are all, in the jargon of philosophy, phase sortals.) By using role terms in definitions, we can create a BFO conformant treatment of such entities drawing on the fact that, while an instance of professor may be simultaneously an instance of trade union member, no instance of the type professor role is also (at any time) an instance of the type trade union member role (any more than any instance of the type color is at any time an instance of the type length). If an ontology of employment positions should be defined in terms of roles following the above pattern, this enables the ontology to do justice to the fact that individuals instantiate the corresponding universals –  professor, sergeant, nurse – only during certain phases in their lives."@en ;
    ns2:IAO_0000600 "b is a role means: b is a realizable entity & b exists because there is some single bearer that is in some special physical, social, or institutional set of circumstances in which this bearer does not have to be& b is not such that, if it ceases to exist, then the physical make-up of the bearer is thereby changed. (axiom label in BFO2 Reference: [061-001])"@en ;
    ns2:IAO_0000602 "(forall (x) (if (Role x) (RealizableEntity x))) // axiom label in BFO2 CLIF: [061-001] " ;
    rdfs:isDefinedBy ns2:bfo.owl .

dcterms:FileFormat a owl:Class ;
    rdfs:label "File Format"@en-us ;
    rdfs:comment "Examples include the formats defined by the list of Internet Media Types."@en-us ;
    rdfs:subClassOf dcterms:MediaType ;
    skos:definition "A digital resource format."@en-us .

<http://schema.org/Product> a owl:Class .

<http://www.ebi.ac.uk/swo/license/SWO_1000061> a owl:Class ;
    rdfs:label "free to use license"@en ;
    ns2:IAO_0000115 "A license which allows any form of usage of the artifact." ;
    rdfs:subClassOf ns3:SWO_0000002 .

<http://demo.fiz-karlsruhe.de/matwerk/E1245665> a nfdicore:AcademicDiscipline ;
    rdfs:label "Materials Science" .

<http://demo.fiz-karlsruhe.de/matwerk/E16577> a nfdicore:Person ;
    rdfs:label "Prof. Felix Fritzen" ;
    mwo:emailAddress "fritzen@simtech.uni-stuttgart.de"^^xsd:string ;
    mwo:hasAffiliation <http://demo.fiz-karlsruhe.de/matwerk/E1002>,
        <http://demo.fiz-karlsruhe.de/matwerk/E5951>,
        <http://demo.fiz-karlsruhe.de/matwerk/E72254>,
        <http://demo.fiz-karlsruhe.de/matwerk/E7904>,
        <http://demo.fiz-karlsruhe.de/matwerk/E8022> ;
    mwo:hasExpertiseIn <http://demo.fiz-karlsruhe.de/matwerk/E36512>,
        <http://demo.fiz-karlsruhe.de/matwerk/E62076> ;
    mwo:hasORCID <https://orcid.org/0000-0003-4926-0068> ;
    owl:sameAs <http://www.wikidata.org/entity/Q59867527> ;
    foaf:depiction <https://ams3.digitaloceanspaces.com/externalpublic/57/0bcbb4ae-e059-4932-a7c4-aee43951861e/conversions/b5f442a4-2cd5-4c7f-96b0-510908256b96-md.jpg?X-Amz-Content-Sha256=UNSIGNED-PAYLOAD&X-Amz-Algorithm=AWS4-HMAC-SHA256&X-Amz-Credential=KVC4ZMO47JLTBHVHEFZ4%2F20230512%2Fams3%2Fs3%2Faws4_request&X-Amz-Date=20230512T150442Z&X-Amz-SignedHeaders=host&X-Amz-Expires=7200&X-Amz-Signature=8e28db6da36cde184da55273f8380adef20a250483682f7c754f3792c80490e0> ;
    foaf:firstName "Felix"^^xsd:string ;
    foaf:surname "Fritzen"^^xsd:string ;
    foaf:title "Prof."^^xsd:string .

<http://demo.fiz-karlsruhe.de/matwerk/E755607> a <http://www.ebi.ac.uk/swo/license/SWO_1000043> ;
    rdfs:label "GNU General Public License" ;
    owl:sameAs <http://www.wikidata.org/entity/Q7603> .

<http://demo.fiz-karlsruhe.de/matwerk/E8627> a nfdicore:Person ;
    rdfs:label "Dr Sarath Menon" ;
    mwo:emailAddress "s.menon@mpie.de"^^xsd:string ;
    mwo:hasAffiliation <http://demo.fiz-karlsruhe.de/matwerk/E1001>,
        <http://demo.fiz-karlsruhe.de/matwerk/E1037>,
        <http://demo.fiz-karlsruhe.de/matwerk/E1247851> ;
    mwo:hasExpertiseIn <http://demo.fiz-karlsruhe.de/matwerk/E36246>,
        <http://demo.fiz-karlsruhe.de/matwerk/E61379>,
        <http://demo.fiz-karlsruhe.de/matwerk/E63482>,
        <http://demo.fiz-karlsruhe.de/matwerk/E67431> ;
    mwo:hasORCID <https://orcid.org/0000-0002-6776-1213> ;
    owl:sameAs <http://www.wikidata.org/entity/Q99549690> ;
    foaf:firstName "Sarath"^^xsd:string ;
    foaf:surname "Menon"^^xsd:string ;
    foaf:title "Dr"^^xsd:string .

ns3:SWO_0000021 a owl:Class ;
    rdfs:label "operating system" ;
    ns2:IAO_0000115 "An operating system is a piece of software which is responsible for managing software that runs on a computer and the interactions of that software with the hardware and system resources." ;
    rdfs:subClassOf ns3:SWO_0000001 .

ns1:OrganisedEvent a owl:Class ;
    rdfs:label "Organised event"@en ;
    rdfs:comment "Any kind of organised event having a start and an end date."@en ;
    rdfs:subClassOf [ a owl:Restriction ;
            owl:allValuesFrom ns1:OrganisedEvent ;
            owl:onProperty ns1:hasSubEvent ],
        [ a owl:Restriction ;
            owl:onProperty ns1:endDate ;
            owl:someValuesFrom xsd:dateTime ],
        [ a owl:Restriction ;
            owl:onProperty ns1:startDate ;
            owl:someValuesFrom xsd:dateTime ] .

<http://demo.fiz-karlsruhe.de/matwerk/E3416> a nfdicore:Organization ;
    rdfs:label "Max-Planck-Institut für Eisenforschung GmbH" .

<http://demo.fiz-karlsruhe.de/matwerk/E63482> a nfdicore:AcademicDiscipline,
        mwo:Method ;
    rdfs:label "atomistic simulations" .

<http://www.ebi.ac.uk/swo/license/SWO_1000043> a owl:Class ;
    rdfs:label "GNU Project Free License Type" ;
    ns2:IAO_0000115 """A licensed is a free license according to GNU if the users have the four essential freedoms:

    The freedom to run the program, for any purpose (freedom 0).
    The freedom to study how the program works, and change it so it does your computing as you wish (freedom 1). Access to the source code is a precondition for this.
    The freedom to redistribute copies so you can help your neighbor (freedom 2).
    The freedom to distribute copies of your modified versions to others (freedom 3). By doing this you can give the whole community a chance to benefit from your changes. Access to the source code is a precondition for this.

A program is free software if users have all of these freedoms. Thus, you should be free to redistribute copies, either with or without modifications, either gratis or charging a fee for distribution, to anyone anywhere. Being free to do these things means (among other things) that you do not have to ask or pay for permission to do so.

“Free software” does not mean “noncommercial”. A free program must be available for commercial use, commercial development, and commercial distribution. Commercial development of free software is no longer unusual; such free commercial software is very important. You may have paid money to get copies of free software, or you may have obtained copies at no charge. But regardless of how you got your copies, you always have the freedom to copy and change the software, even to sell copies. """ ;
    ns2:IAO_0000119 "http://www.gnu.org/philosophy/free-sw.html, accessed 12 June 2013." ;
    dcterms:creator "Allyson Lister" ;
    rdfs:comment "Allyson Lister: This class defines those licenses which are free licenses, but which may or may not be compatible with any version of the GNU GPL." ;
    rdfs:subClassOf <http://www.ebi.ac.uk/swo/license/SWO_1000008> .

<http://demo.fiz-karlsruhe.de/matwerk/E1247022> a nfdicore:Project,
        nfdicore:fundingProject,
        default1:Consortium ;
    rdfs:label "NFDI-MatWerk" .

<http://demo.fiz-karlsruhe.de/matwerk/E1247883> rdfs:label "Ontologies for Materials Science" ;
    dcterms:isPartOf <http://demo.fiz-karlsruhe.de/matwerk/E1247022> ;
    mwo:description "This TA develops Ontologies and metadata schemes in close cooperation with the stakeholders, tailored to their respective needs." ;
    mwo:hasWorkPackage <http://demo.fiz-karlsruhe.de/matwerk/E1247925> .

<http://demo.fiz-karlsruhe.de/matwerk/E828542> a nfdicore:ProgrammingLanguage ;
    rdfs:label "C++" ;
    owl:sameAs <http://www.wikidata.org/entity/Q2407> .

nfdicore:ObjectType a owl:Class ;
    rdfs:label "object type"@en ;
    nfdicore:example "book, photograph, music sheet"@en ;
    rdfs:comment "A resource that identifies the type of object in a data collection."@en .

nfdicore:Ontology a nfdicore:SemanticExpressivity .

modsci:Instrument a owl:Class ;
    rdfs:label "Instrument"@en ;
    rdfs:comment "A tool or implement, especially one for precision work."@en ;
    rdfs:subClassOf <http://schema.org/Product> .

<http://demo.fiz-karlsruhe.de/matwerk/E1247890> rdfs:label "Workflows and Software Development" ;
    dcterms:isPartOf <http://demo.fiz-karlsruhe.de/matwerk/E1247022> ;
    mwo:description "This TA is responsible for advancing the research in MSE by providing solutions for workflow management and software foundations that will improve both productivity and quality of the data processing and simulation aspects." ;
    mwo:hasWorkPackage <http://demo.fiz-karlsruhe.de/matwerk/E1247946> .

mwo:EducationalResource a owl:Class ;
    rdfs:label "educational resource"@en ;
    ns2:IAO_0000115 "A resource or material that can be used for teaching and learning puposes."@en ;
    rdfs:subClassOf nfdicore:Resource .

nfdicore:ProgrammingLanguage a owl:Class ;
    rdfs:label "programming language"@en ;
    nfdicore:example "Java, Ruby, C++, Perl, PHP" ;
    rdfs:comment "A formal language used for implementing a software."@en ;
    rdfs:subClassOf nfdicore:TechnologicalMeans ;
    owl:equivalentClass modsci:ProgrammingLanguage .

mwo:SemanticResource a owl:Class ;
    rdfs:label "semantic resource" ;
    ns2:IAO_0000115 "A machine-actionable controlled vocabularies to describe the meaning of the content and express relations among them."@en ;
    rdfs:subClassOf nfdicore:Resource .

nfdicore:Specification a owl:Class ;
    rdfs:label "specification"@en ;
    nfdicore:example "RDF, SPARQL, Federation" ;
    rdfs:comment "A set of requirements, guidelines, standards contributed by an organisation or a person."@en ;
    rdfs:subClassOf <http://schema.org/Product> .

ns3:SWO_9000072 a owl:Class ;
    rdfs:label "Microsoft Windows" ;
    rdfs:comment "The Windows Operating System" ;
    rdfs:subClassOf ns3:SWO_0000021 .

ns3:SWO_0000149 a owl:Class ;
    rdfs:label "Mac OS"@en ;
    ns2:IAO_0000115 "Mac OS is software which is used as the operating system for the Macintosh personal computer created by Apple Inc." ;
    ns2:IAO_0000119 "http://en.wikipedia.org/wiki/History_of_Mac_OS, accessed 25 March 2015." ;
    dcterms:creator "Allyson Lister" ;
    rdfs:subClassOf ns3:SWO_0000021 .

<http://demo.fiz-karlsruhe.de/matwerk/E759297> a <http://www.ebi.ac.uk/swo/license/SWO_1000061> ;
    rdfs:label "MIT" ;
    owl:sameAs <http://www.wikidata.org/entity/Q334661> .

nfdicore:City a owl:Class ;
    rdfs:label "city"@en ;
    nfdicore:example "Berlin, Hannover, Kyiv"@en ;
    rdfs:comment "A city or a town where the thing is located."@en ;
    rdfs:subClassOf nfdicore:Place .

mwo:Method a owl:Class ;
    rdfs:label "method"@en ;
    ns2:IAO_0000115 "A method is a systematic procedure, technique, or mode of inquiry employed by or proper to a particular discipline or art."@en ;
    ns4:hasDbXref <https://www.merriam-webster.com/dictionary/method#:~:text=a(1),the%20lecture%20method> ;
    ns4:hasExactSynonym "Approach"@en,
        "Procedure"@en,
        "Technique"@en .

<http://demo.fiz-karlsruhe.de/matwerk/E613172> a mwo:Method ;
    rdfs:label "Density functional theory" .

<http://demo.fiz-karlsruhe.de/matwerk/E80004> a nfdicore:Country ;
    rdfs:label "Germany" ;
    owl:sameAs <http://www.wikidata.org/entity/Q183> .

ns3:SWO_0000022 a owl:Class ;
    rdfs:label "Linux" ;
    rdfs:subClassOf ns3:SWO_0000021 .

ns3:SWO_0000001 a owl:Class ;
    rdfs:label "software" ;
    ns2:IAO_0000115 "Computer software, or generally just software, is any set of machine-readable instructions (most often in the form of a computer program) that conform to a given syntax (sometimes referred to as a language) that is interpretable by a given processor and that directs a computer's processor to perform specific operations." ;
    ns2:IAO_0000119 "James Malone",
        "Modified in parts from https://en.wikipedia.org/wiki/Software",
        "Robert Stevens" ;
    rdfs:comment "AL 7.9.22: There are some reasoning oddities associated with marking IAO and SWO software as equivalent; once these are sorted out, the equivalence statement will take the place of this current parent-child relationship." .

mwo:ContactPoint a owl:Class ;
    rdfs:label "contact point"@en ;
    ns2:IAO_0000115 "A contact point is a person, website or e-mail which provides information concerning a resource."@en ;
    ns4:hasExactSynonym "Point of contact"@en .

nfdicore:Project a owl:Class ;
    rdfs:label "project"@en ;
    nfdicore:example "Freisch\\u00fctz digital, Corpus Vitrearum Medii Aevi" ;
    rdfs:comment "A scientific or business endeavour that aims to conclude an investigation or to answer a research question."@en ;
    owl:equivalentClass <http://schema.org/Project> .

<http://demo.fiz-karlsruhe.de/matwerk/E67431> a nfdicore:AcademicDiscipline ;
    rdfs:label "computational materials science" ;
    owl:sameAs <http://www.wikidata.org/entity/Q85753722> .

ns3:SWO_0000002 a owl:Class ;
    rdfs:label "software license",
        "licence"@en ;
    ns2:IAO_0000115 "A licence is a legal instrument (usually by way of contract law, with or without printed material) governing the use or redistribution of the resource containing the licence." ;
    ns2:IAO_0000119 "Modified from http://en.wikipedia.org/wiki/Software_license" ;
    dcterms:creator "James Malone" ;
    rdfs:subClassOf [ a owl:Restriction ;
            owl:onProperty [ owl:inverseOf ns3:has_license ] ;
            owl:someValuesFrom ns3:SWO_0000001 ] .

mwo:ResearchSoftware a owl:Class ;
    rdfs:label "research software"@en ;
    ns2:IAO_0000115 "Software which was created for a research purpose."@en ;
    ns4:hasDbXref <https://doi.org/10.5281/zenodo.5504016> ;
    ns4:hasExactSynonym "Scientific software"@en ;
    rdfs:comment """Software components (e.g., operating systems, libraries, dependencies, packages, scripts, etc.) that are used for research but were not created during or with a clear research intent should be considered software in research and not Research Software. This differentiation may vary between disciplines.
Research software might be source code files, algorithms, scripts, computational workflows and executables"""@en ;
    rdfs:subClassOf ns3:SWO_0000001 .

<http://demo.fiz-karlsruhe.de/matwerk/E836279> a nfdicore:ProgrammingLanguage,
        ns3:SWO_0000001 ;
    rdfs:label "python" ;
    owl:sameAs <http://www.wikidata.org/entity/Q28865> .

nfdicore:DataPortal a owl:Class ;
    rdfs:label "data portal"@en ;
    nfdicore:example "Bach digital, KultSam, MusiXplora"@en ;
    rdfs:comment "An online platform that provides access to data collections and datasets."@en ;
    rdfs:subClassOf <http://schema.org/Service> .

nfdicore:Resource a owl:Class ;
    rdfs:label "resource"@en ;
    rdfs:comment "The most generic kind of a resource and may be associated with any kind of creative work, e.g. datasets, books, movies, photographs; offered products and services, e.g. data portals, data curation, data digitization; and intangible things, e.g. subjects of creative works, topics of events, offers, a list of enumerations."@en ;
    rdfs:subClassOf [ a owl:Class ;
            owl:unionOf ( <http://schema.org/CreativeWork> <http://schema.org/Intangible> <http://schema.org/Product> ) ] .

nfdicore:Organization a owl:Class ;
    rdfs:label "organization"@en ;
    nfdicore:example "Universit\\u00e4tsbibliothek Leipzig, S\\u00e4chsisches Wirtschaftsarchiv, Museen der Stadt K\\u00f6ln" ;
    rdfs:comment "An organisation of some kind, e.g. research organisation or business organisation"@en ;
    owl:equivalentClass <http://schema.org/Organization> .

nfdicore:Publication a owl:Class ;
    rdfs:label "publication"@en ;
    nfdicore:example "MusiXplora: Visual analysis of a musicological encyclopedia, Textkategorien in kompositorischen Werkstattdokumenten" ;
    rdfs:comment "A published scholarly work that reports on ongoing activity about or within a resource, e.g. a dataset."@en ;
    rdfs:subClassOf <http://schema.org/CreativeWork> .

mwo:Documentation a owl:Class ;
    rdfs:label "documentation"@en ;
    ns2:IAO_0000115 "Documentation is any communicable material that is used to describe, explain or instruct regarding some attributes of an object, system or procedure, such as its parts, assembly, installation, maintenance and use"@en ;
    rdfs:subClassOf <http://schema.org/Product> .

nfdicore:Person a owl:Class ;
    rdfs:label "person"@en ;
    nfdicore:example "Harald Sack, Tabea Tietz, Sasha Bruns, Etienne Posthumus" ;
    rdfs:comment "A resource that represents a single person."@en ;
    owl:equivalentClass <http://schema.org/Person> .

nfdicore:AcademicDiscipline a owl:Class ;
    rdfs:label "academic discipline"@en ;
    nfdicore:example <https://www.wikidata.org/entity/Q12271>,
        "Architecture, Art History, Musicology, Media Studies, Performing Arts"@en ;
    rdfs:comment "An academic discipline, a research field or domain of a resource, e.g. a data portal or a field of study of a person."@en ;
    rdfs:subClassOf modsci:ModernScience .

mwo:Repository a owl:Class ;
    rdfs:label "repository"@en ;
    rdfs:comment "A central location in which data is stored and managed."@en ;
    rdfs:subClassOf <http://schema.org/Product> .

nfdicore:Software a owl:Class ;
    rdfs:label "software"@en ;
    nfdicore:example "Edirom, Muscat" ;
    rdfs:comment "A computer software provided by an organisation or a person."@en ;
    rdfs:subClassOf <http://schema.org/Product> ;
    owl:equivalentClass ns3:SWO_0000001 .

nfdicore:Website a owl:Class ;
    rdfs:label "website"@en ;
    nfdicore:example "https:\\/\\/opac.rism.info" ;
    rdfs:comment "A collection of webpages contributed by an organisation or a person."@en ;
    rdfs:subClassOf <http://schema.org/Product> .

[] a owl:Axiom ;
    ns2:IAO_0010000 <http://purl.obolibrary.org/obo/bfo/axiom/061-001> ;
    owl:annotatedProperty ns2:IAO_0000600 ;
    owl:annotatedSource ns2:BFO_0000023 ;
    owl:annotatedTarget "b is a role means: b is a realizable entity & b exists because there is some single bearer that is in some special physical, social, or institutional set of circumstances in which this bearer does not have to be& b is not such that, if it ceases to exist, then the physical make-up of the bearer is thereby changed. (axiom label in BFO2 Reference: [061-001])"@en .

[] a owl:Axiom ;
    ns2:IAO_0010000 <http://purl.obolibrary.org/obo/bfo/axiom/061-001> ;
    owl:annotatedProperty ns2:IAO_0000602 ;
    owl:annotatedSource ns2:BFO_0000023 ;
    owl:annotatedTarget "(forall (x) (if (Role x) (RealizableEntity x))) // axiom label in BFO2 CLIF: [061-001] " .

